@prefix agg: <http://jena.apache.org/ARQ/function/aggregate#> .
@prefix : <http://127.0.0.1:3333/> .
@prefix sail: <http://www.openrdf.org/config/sail#> .
@prefix owl: <http://www.w3.org/2002/07/owl#> .
@prefix geof: <http://www.opengis.net/def/function/geosparql/> .
@prefix xsd: <http://www.w3.org/2001/XMLSchema#> .
@prefix fn: <http://www.w3.org/2005/xpath-functions> .
@prefix rdfs: <http://www.w3.org/2000/01/rdf-schema#> .
@prefix spif: <http://spinrdf.org/spif#> .
@prefix geo: <http://www.opengis.net/ont/geosparql#> .
@prefix path: <http://www.ontotext.com/path#> .
@prefix array: <http://www.w3.org/2005/xpath-functions/array> .
@prefix apf: <http://jena.apache.org/ARQ/property#> .
@prefix xml: <http://www.w3.org/XML/1998/namespace> .
@prefix sem: <http://semanticweb.cs.vu.nl/2009/11/sem/> .
@prefix rep: <http://www.openrdf.org/config/repository#> .
@prefix map: <http://www.w3.org/2005/xpath-functions/map> .
@prefix foaf: <http://xmlns.com/foaf/0.1/> .
@prefix sr: <http://www.openrdf.org/config/repository/sail#> .
@prefix wgs: <http://www.w3.org/2003/01/geo/wgs84_pos#> .
@prefix gn: <http://www.geonames.org/ontology#> .
@prefix afn: <http://jena.apache.org/ARQ/function#> .
@prefix vcard: <http://www.w3.org/2006/vcard/ns#> .
@prefix list: <http://jena.apache.org/ARQ/list#> .
@prefix rdf: <http://www.w3.org/1999/02/22-rdf-syntax-ns#> .
@prefix ofn: <http://www.ontotext.com/sparql/functions/> .
@prefix geoext: <http://rdf.useekm.com/ext#> .
@prefix graphdb: <http://www.ontotext.com/config/graphdb#> .
@prefix math: <http://www.w3.org/2005/xpath-functions/math> .
@prefix time: <http://www.w3.org/2006/time#> .
@prefix omgeo: <http://www.ontotext.com/owlim/geo#> .
@prefix dc: <http://purl.org/dc/elements/1.1/> .

rdf:type a owl:ObjectProperty .

rdfs:subClassOf a owl:ObjectProperty .

rdfs:Container a owl:Class .

rdfs:seeAlso a owl:ObjectProperty .

geo:asWKT a owl:DatatypeProperty .

geo:asGML a owl:DatatypeProperty .

geo:hasDefaultGeometry a owl:ObjectProperty .

geo:sfEquals a owl:ObjectProperty .

geo:sfDisjoint a owl:ObjectProperty .

geo:sfIntersects a owl:ObjectProperty .

geo:sfTouches a owl:ObjectProperty .

geo:sfWithin a owl:ObjectProperty .

geo:sfContains a owl:ObjectProperty .

geo:sfOverlaps a owl:ObjectProperty .

geo:sfCrosses a owl:ObjectProperty .

geo:ehEquals a owl:ObjectProperty .

geo:ehDisjoint a owl:ObjectProperty .

geo:ehMeet a owl:ObjectProperty .

geo:ehOverlap a owl:ObjectProperty .

geo:ehCovers a owl:ObjectProperty .

geo:ehCoveredBy a owl:ObjectProperty .

geo:ehInside a owl:ObjectProperty .

geo:ehContains a owl:ObjectProperty .

geo:rcc8eq a owl:ObjectProperty .

geo:rcc8dc a owl:ObjectProperty .

geo:rcc8ec a owl:ObjectProperty .

geo:rcc8po a owl:ObjectProperty .

geo:rcc8tppi a owl:ObjectProperty .

geo:rcc8tpp a owl:ObjectProperty .

geo:rcc8ntpp a owl:ObjectProperty .

geo:rcc8ntppi a owl:ObjectProperty .

<http://127.0.0.1:3333/> a owl:Ontology .

<http://purl.org/dc/terms/contributor> a owl:AnnotationProperty .

<http://purl.org/dc/terms/created> a owl:AnnotationProperty .

<http://purl.org/dc/terms/creator> a owl:AnnotationProperty .

<http://purl.org/dc/terms/description> a owl:AnnotationProperty .

<http://purl.org/dc/terms/license> a owl:AnnotationProperty .

<http://purl.org/dc/terms/modified> a owl:AnnotationProperty .

<http://purl.org/dc/terms/publisher> a owl:AnnotationProperty .

<http://purl.org/dc/terms/replaces> a owl:AnnotationProperty .

<http://purl.org/dc/terms/rights> a owl:AnnotationProperty .

<http://purl.org/dc/terms/source> a owl:AnnotationProperty .

<http://purl.org/dc/terms/title> a owl:AnnotationProperty .

<http://purl.org/vocab/vann/preferredNamespacePrefix> a owl:AnnotationProperty .

<http://purl.org/vocab/vann/preferredNamespaceUri> a owl:AnnotationProperty .

:image a owl:AnnotationProperty .

:wikiurl a owl:AnnotationProperty .

<http://www.w3.org/2004/02/skos/core#broadMatch> a owl:AnnotationProperty .

<http://www.w3.org/2004/02/skos/core#closeMatch> a owl:AnnotationProperty .

<http://www.w3.org/2004/02/skos/core#definition> a owl:AnnotationProperty .

<http://www.w3.org/2004/02/skos/core#exactMatch> a owl:AnnotationProperty .

<http://www.w3.org/2004/02/skos/core#example> a owl:AnnotationProperty .

<http://www.w3.org/2004/02/skos/core#narrowMatch> a owl:AnnotationProperty .

<http://www.w3.org/2004/02/skos/core#note> a owl:AnnotationProperty .

<http://www.w3.org/2004/02/skos/core#prefLabel> a owl:AnnotationProperty .

<http://www.w3.org/2004/02/skos/core#relatedMatch> a owl:AnnotationProperty .

<http://www.w3.org/2004/02/skos/core#scopeNote> a owl:AnnotationProperty .

<https://schema.org/affiliation> a owl:AnnotationProperty .

<https://schema.org/email> a owl:AnnotationProperty .

<https://schema.org/name> a owl:AnnotationProperty .

<https://schema.org/url> a owl:AnnotationProperty .

geo:dggsLiteral a rdfs:Datatype .

geo:geoJSONLiteral a rdfs:Datatype .

geo:gmlLiteral a rdfs:Datatype .

geo:kmlLiteral a rdfs:Datatype .

geo:wktLiteral a rdfs:Datatype .

time:generalDay a rdfs:Datatype .

time:generalMonth a rdfs:Datatype .

time:generalYear a rdfs:Datatype .

:hasChild a owl:ObjectProperty .

:hasParent a owl:ObjectProperty .

sem:Actor a owl:Class .

:hasLocation a owl:ObjectProperty .

:isLocationOf a owl:ObjectProperty .

sem:Event a owl:Class .

geo:Feature a owl:Class .

foaf:Person a owl:Class .

:hasRelative a owl:SymmetricProperty, owl:ObjectProperty .

:isActorOf a owl:ObjectProperty .

sem:hasActor a owl:ObjectProperty .

:rootEvent a owl:ObjectProperty .

sem:View a owl:Class .

sem:accordingTo a owl:ObjectProperty .

sem:Authority a owl:Class .

sem:actorType a owl:ObjectProperty .

sem:type a owl:ObjectProperty .

sem:ActorType a owl:Class .

sem:eventProperty a owl:ObjectProperty .

sem:eventType a owl:ObjectProperty .

sem:EventType a owl:Class .

sem:hasPlace a owl:ObjectProperty .

sem:Place a owl:Class .

sem:hasSubEvent a owl:ObjectProperty .

sem:subEventOf a owl:ObjectProperty .

sem:hasSubType a owl:ObjectProperty .

sem:subTypeOf a owl:ObjectProperty .

sem:Type a owl:Class .

sem:hasTime a owl:ObjectProperty .

sem:Time a owl:Class .

time:TemporalEntity a owl:Class .

sem:placeType a owl:ObjectProperty .

sem:PlaceType a owl:Class .

sem:roleType a owl:ObjectProperty .

sem:Role a owl:Class .

sem:RoleType a owl:Class .

sem:timeType a owl:ObjectProperty .

sem:TimeType a owl:Class .

geo:defaultGeometry a owl:ObjectProperty .

geo:hasGeometry a owl:ObjectProperty .

geo:Geometry a owl:Class .

geo:SpatialObject a owl:Class .

geo:hasArea a owl:ObjectProperty .

geo:hasSize a owl:ObjectProperty .

geo:hasBoundingBox a owl:ObjectProperty .

geo:hasCentroid a owl:ObjectProperty .

geo:hasLength a owl:ObjectProperty .

geo:hasPerimeterLength a owl:ObjectProperty .

geo:hasSpatialAccuracy a owl:ObjectProperty .

geo:hasSpatialResolution a owl:ObjectProperty .

geo:hasVolume a owl:ObjectProperty .

rdfs:member a owl:ObjectProperty .

time:after a owl:ObjectProperty .

time:before a owl:TransitiveProperty, owl:ObjectProperty .

time:dayOfWeek a owl:ObjectProperty .

time:GeneralDateTimeDescription a owl:Class .

time:DayOfWeek a owl:Class .

time:hasBeginning a owl:ObjectProperty .

time:hasTime a owl:ObjectProperty .

time:Instant a owl:Class .

time:hasDateTimeDescription a owl:ObjectProperty .

time:DateTimeInterval a owl:Class .

time:hasDuration a owl:ObjectProperty .

time:hasTemporalDuration a owl:ObjectProperty .

time:Duration a owl:Class .

time:hasDurationDescription a owl:ObjectProperty .

time:GeneralDurationDescription a owl:Class .

time:hasEnd a owl:ObjectProperty .

time:hasTRS a owl:ObjectProperty, owl:FunctionalProperty .

_:node10 a owl:Class .

time:TemporalPosition a owl:Class .

time:TRS a owl:Class .

time:TemporalDuration a owl:Class .

time:inDateTime a owl:ObjectProperty .

time:inTemporalPosition a owl:ObjectProperty .

time:inTimePosition a owl:ObjectProperty .

time:TimePosition a owl:Class .

time:inside a owl:ObjectProperty .

time:Interval a owl:Class .

time:intervalAfter a owl:ObjectProperty .

time:intervalDisjoint a owl:ObjectProperty .

time:intervalBefore a owl:ObjectProperty .

time:ProperInterval a owl:Class .

time:intervalContains a owl:ObjectProperty .

time:intervalDuring a owl:ObjectProperty .

time:intervalIn a owl:ObjectProperty .

time:intervalEquals a owl:ObjectProperty .

time:intervalFinishedBy a owl:ObjectProperty .

time:intervalFinishes a owl:ObjectProperty .

time:intervalMeets a owl:ObjectProperty .

time:intervalMetBy a owl:ObjectProperty .

time:intervalOverlappedBy a owl:ObjectProperty .

time:intervalOverlaps a owl:ObjectProperty .

time:intervalStartedBy a owl:ObjectProperty .

time:intervalStarts a owl:ObjectProperty .

time:monthOfYear a owl:ObjectProperty .

time:MonthOfYear a owl:Class .

time:timeZone a owl:ObjectProperty .

time:TimeZone a owl:Class .

time:unitType a owl:ObjectProperty .

_:node13 a owl:Class .

time:TemporalUnit a owl:Class .

:deathCause a owl:DatatypeProperty .

:latitude a owl:DatatypeProperty .

:longitude a owl:DatatypeProperty .

sem:hasBeginTimeStamp a owl:DatatypeProperty .

sem:hasTimeStamp a owl:DatatypeProperty .

sem:hasEarliestBeginTimeStamp a owl:DatatypeProperty .

sem:hasEarliestEndTimeStamp a owl:DatatypeProperty .

sem:hasEndTimeStamp a owl:DatatypeProperty .

sem:hasLatestBeginTimeStamp a owl:DatatypeProperty .

sem:hasLatestEndTimeStamp a owl:DatatypeProperty .

geo:asDGGS a owl:DatatypeProperty .

geo:hasSerialization a owl:DatatypeProperty .

geo:asGeoJSON a owl:DatatypeProperty .

geo:asKML a owl:DatatypeProperty .

geo:coordinateDimension a owl:DatatypeProperty .

geo:dimension a owl:DatatypeProperty .

geo:hasMetricArea a owl:DatatypeProperty .

geo:hasMetricSize a owl:DatatypeProperty .

geo:hasMetricLength a owl:DatatypeProperty .

geo:hasMetricPerimeterLength a owl:DatatypeProperty .

geo:hasMetricSpatialAccuracy a owl:DatatypeProperty .

geo:hasMetricSpatialResolution a owl:DatatypeProperty .

geo:hasMetricVolume a owl:DatatypeProperty .

geo:isEmpty a owl:DatatypeProperty .

geo:isSimple a owl:DatatypeProperty .

geo:spatialDimension a owl:DatatypeProperty .

time:day a owl:DatatypeProperty .

time:dayOfYear a owl:DatatypeProperty .

time:days a owl:DatatypeProperty .

time:hasXSDDuration a owl:DatatypeProperty .

time:hour a owl:DatatypeProperty .

time:hours a owl:DatatypeProperty .

time:inXSDDate a owl:DatatypeProperty .

time:inXSDDateTime a owl:DatatypeProperty .

time:inXSDDateTimeStamp a owl:DatatypeProperty .

time:inXSDgYear a owl:DatatypeProperty .

time:inXSDgYearMonth a owl:DatatypeProperty .

time:minute a owl:DatatypeProperty .

time:minutes a owl:DatatypeProperty .

time:month a owl:DatatypeProperty .

time:months a owl:DatatypeProperty .

time:nominalPosition a owl:DatatypeProperty .

time:numericDuration a owl:DatatypeProperty .

time:numericPosition a owl:DatatypeProperty .

time:second a owl:DatatypeProperty .

time:seconds a owl:DatatypeProperty .

time:week a owl:DatatypeProperty .

time:weeks a owl:DatatypeProperty .

time:xsdDateTime a owl:DatatypeProperty .

time:year a owl:DatatypeProperty .

time:years a owl:DatatypeProperty .

sem:Core a owl:Class .

sem:Constraint a owl:Class .

sem:Object a owl:Class .

sem:Temporary a owl:Class .

geo:FeatureCollection a owl:Class .

geo:SpatialObjectCollection a owl:Class .

_:node16 a owl:Restriction .

geo:GeometryCollection a owl:Class .

_:node17 a owl:Restriction .

_:node18 a owl:Restriction .

time:DateTimeDescription a owl:Class .

_:node19 a owl:Restriction .

_:node20 a owl:Restriction .

_:node21 a owl:Restriction .

_:node22 a owl:Restriction .

_:node23 a owl:Restriction .

_:node24 a owl:Restriction .

time:DurationDescription a owl:Class .

_:node25 a owl:Restriction .

_:node26 a owl:Restriction .

_:node27 a owl:Restriction .

_:node28 a owl:Restriction .

_:node29 a owl:Restriction .

_:node30 a owl:Restriction .

_:node31 a owl:Restriction .

_:node32 a owl:Restriction .

_:node33 a owl:Restriction .

_:node34 a owl:Restriction .

_:node35 a owl:Restriction .

_:node36 a owl:Restriction .

_:node37 a owl:Restriction .

_:node38 a owl:Restriction .

_:node39 a owl:Restriction .

_:node40 a owl:Restriction .

_:node41 a owl:Restriction .

_:node42 a owl:Restriction .

_:node43 a owl:Restriction .

_:node44 a owl:Restriction .

_:node45 a owl:Restriction .

_:node46 a owl:Restriction .

_:node47 a owl:Restriction .

_:node48 a owl:Restriction .

_:node49 a owl:Restriction .

_:node50 a owl:Restriction .

_:node51 a owl:Restriction .

_:node52 a owl:Restriction .

time:January a owl:Class .

_:node53 a owl:Restriction .

time:unitMonth a time:TemporalUnit .

_:node54 a owl:Restriction .

_:node55 a owl:Restriction .

_:node56 a owl:Restriction .

_:node57 a owl:Restriction .

_:node58 a owl:Restriction .

_:node59 a owl:Restriction .

_:node60 a owl:Restriction .

_:node61 a owl:Restriction .

_:node62 a owl:Restriction .

_:node63 a owl:Class .

_:node66 a owl:Restriction .

_:node67 a owl:Class .

_:node69 a owl:Restriction .

_:node71 a owl:Restriction .

time:Year a owl:Class .

_:node72 a owl:Restriction .

_:node73 a owl:Restriction .

_:node74 a owl:Restriction .

_:node75 a owl:Restriction .

_:node76 a owl:Restriction .

_:node77 a owl:Restriction .

_:node78 a owl:Restriction .

time:Friday a time:DayOfWeek .

time:Monday a time:DayOfWeek .

time:Saturday a time:DayOfWeek .

time:Sunday a time:DayOfWeek .

time:Thursday a time:DayOfWeek .

time:Tuesday a time:DayOfWeek .

time:Wednesday a time:DayOfWeek .

time:unitCentury a time:TemporalUnit, owl:NamedIndividual .

time:unitDay a time:TemporalUnit .

time:unitDecade a time:TemporalUnit, owl:NamedIndividual .

time:unitHour a time:TemporalUnit .

time:unitMillenium a time:TemporalUnit, owl:NamedIndividual .

time:unitMinute a time:TemporalUnit .

time:unitSecond a time:TemporalUnit .

time:unitWeek a time:TemporalUnit .

time:unitYear a time:TemporalUnit .

:wikipediaBandungLautanApi a sem:View .

_:node100 a time:temporanEntity .

_:node101 a time:Instant .

_:node102 a <http://www.w3.org/2006/time#(General)DateTimeDescription> .

_:node103 a time:Instant .

_:node104 a <http://www.w3.org/2006/time#(General)DateTimeDescription> .

:wikipedia a sem:Authority, <https://semanticweb.cs.vu.nl/2009/11/sem/Authority> .

:RevolusiNasionalIndonesia a sem:Event .

_:node105 a time:temporanEntity .

_:node106 a time:Instant .

_:node107 a <http://www.w3.org/2006/time#(General)DateTimeDescription> .

_:node108 a time:Instant .

_:node109 a <http://www.w3.org/2006/time#(General)DateTimeDescription> .

_:node110 a time:temporanEntity .

_:node111 a time:Instant .

_:node112 a <http://www.w3.org/2006/time#(General)DateTimeDescription> .

_:node113 a time:Instant .

_:node114 a <http://www.w3.org/2006/time#(General)DateTimeDescription> .

:wikipediaPemberontakanDITIIdiAceh a sem:View .

_:node115 a time:temporanEntity .

_:node116 a time:Instant .

_:node117 a <http://www.w3.org/2006/time#(General)DateTimeDescription> .

_:node118 a time:Instant .

_:node119 a <http://www.w3.org/2006/time#(General)DateTimeDescription> .

:wikipediaKampanyeKalimantan1945 a sem:View .

_:node120 a time:temporanEntity .

_:node121 a time:Instant .

_:node122 a <http://www.w3.org/2006/time#(General)DateTimeDescription> .

_:node123 a time:Instant .

_:node124 a <http://www.w3.org/2006/time#(General)DateTimeDescription> .

_:node125 a time:temporanEntity .

_:node126 a time:Instant .

_:node127 a <http://www.w3.org/2006/time#(General)DateTimeDescription> .

_:node128 a time:Instant .

_:node129 a <http://www.w3.org/2006/time#(General)DateTimeDescription> .

:wikipediaPertempuranBojongKokosan a sem:View .

_:node130 a time:temporanEntity .

_:node131 a time:Instant .

_:node132 a <http://www.w3.org/2006/time#(General)DateTimeDescription> .

_:node133 a time:Instant .

_:node134 a <http://www.w3.org/2006/time#(General)DateTimeDescription> .

:KampanyeHindiaBelanda a sem:Event .

:wikipediaRevolusiNasionalIndonesia a sem:View .

_:node135 a time:temporanEntity .

_:node136 a time:Instant .

_:node137 a <http://www.w3.org/2006/time#(General)DateTimeDescription> .

_:node138 a time:Instant .

_:node139 a <http://www.w3.org/2006/time#(General)DateTimeDescription> .

:PertempuranBojongKokosan a sem:Event .

:DelapanJamPertempurandiMangkang a sem:Event .

_:node140 a time:temporanEntity .

_:node141 a time:Instant .

_:node142 a <http://www.w3.org/2006/time#(General)DateTimeDescription> .

_:node143 a time:Instant .

_:node144 a <http://www.w3.org/2006/time#(General)DateTimeDescription> .

_:node145 a time:temporanEntity .

_:node146 a time:Instant .

_:node147 a <http://www.w3.org/2006/time#(General)DateTimeDescription> .

_:node148 a time:Instant .

_:node149 a <http://www.w3.org/2006/time#(General)DateTimeDescription> .

_:node150 a time:temporanEntity .

_:node151 a time:Instant .

_:node152 a <http://www.w3.org/2006/time#(General)DateTimeDescription> .

_:node153 a time:Instant .

_:node154 a <http://www.w3.org/2006/time#(General)DateTimeDescription> .

:PeristiwaTigaMaret a sem:Event .

:Operasi17Agustus a sem:Event .

_:node155 a time:temporanEntity .

_:node156 a time:Instant .

_:node157 a <http://www.w3.org/2006/time#(General)DateTimeDescription> .

_:node158 a time:Instant .

_:node159 a <http://www.w3.org/2006/time#(General)DateTimeDescription> .

:BandungLautanApi a sem:Event .

:Gerakan30September a sem:Event .

_:node160 a time:temporanEntity .

_:node161 a time:Instant .

_:node162 a <http://www.w3.org/2006/time#(General)DateTimeDescription> .

_:node163 a time:Instant .

_:node164 a <http://www.w3.org/2006/time#(General)DateTimeDescription> .

_:node165 a time:temporanEntity .

_:node166 a time:Instant .

_:node167 a <http://www.w3.org/2006/time#(General)DateTimeDescription> .

_:node168 a time:Instant .

_:node169 a <http://www.w3.org/2006/time#(General)DateTimeDescription> .

:wikipediaPerangCumbok a sem:View .

_:node170 a time:temporanEntity .

_:node171 a time:Instant .

_:node172 a <http://www.w3.org/2006/time#(General)DateTimeDescription> .

_:node173 a time:Instant .

_:node174 a <http://www.w3.org/2006/time#(General)DateTimeDescription> .

_:node175 a time:temporanEntity .

_:node176 a time:Instant .

_:node177 a <http://www.w3.org/2006/time#(General)DateTimeDescription> .

_:node178 a time:Instant .

_:node179 a <http://www.w3.org/2006/time#(General)DateTimeDescription> .

_:node180 a time:temporanEntity .

_:node181 a time:Instant .

_:node182 a <http://www.w3.org/2006/time#(General)DateTimeDescription> .

_:node183 a time:Instant .

_:node184 a <http://www.w3.org/2006/time#(General)DateTimeDescription> .

:wikipediaSeranganUmum1Maret1949 a sem:View .

_:node185 a time:temporanEntity .

_:node186 a time:Instant .

_:node187 a <http://www.w3.org/2006/time#(General)DateTimeDescription> .

_:node188 a time:Instant .

_:node189 a <http://www.w3.org/2006/time#(General)DateTimeDescription> .

:KonflikPapua a sem:Event .

_:node190 a time:temporanEntity .

_:node191 a time:Instant .

_:node192 a <http://www.w3.org/2006/time#(General)DateTimeDescription> .

_:node193 a time:Instant .

_:node194 a <http://www.w3.org/2006/time#(General)DateTimeDescription> .

_:node195 a time:temporanEntity .

_:node196 a time:Instant .

_:node197 a <http://www.w3.org/2006/time#(General)DateTimeDescription> .

_:node198 a time:Instant .

_:node199 a <http://www.w3.org/2006/time#(General)DateTimeDescription> .

:PerangDayakDesa a sem:Event .

:wikipediaKonflikPapua a sem:View .

_:node200 a time:temporanEntity .

_:node201 a time:Instant .

_:node202 a <http://www.w3.org/2006/time#(General)DateTimeDescription> .

_:node203 a time:Instant .

_:node204 a <http://www.w3.org/2006/time#(General)DateTimeDescription> .

:wikipediaPeristiwaTigaMaret a sem:View .

_:node205 a time:temporanEntity .

_:node206 a time:Instant .

_:node207 a <http://www.w3.org/2006/time#(General)DateTimeDescription> .

_:node208 a time:Instant .

_:node209 a <http://www.w3.org/2006/time#(General)DateTimeDescription> .

:wikipediaPenyerbuanKotabaruYogyakarta a sem:View .

_:node210 a time:temporanEntity .

_:node211 a time:Instant .

_:node212 a <http://www.w3.org/2006/time#(General)DateTimeDescription> .

_:node213 a time:Instant .

_:node214 a <http://www.w3.org/2006/time#(General)DateTimeDescription> .

_:node215 a time:temporanEntity .

_:node216 a time:Instant .

_:node217 a <http://www.w3.org/2006/time#(General)DateTimeDescription> .

_:node218 a time:Instant .

_:node219 a <http://www.w3.org/2006/time#(General)DateTimeDescription> .

_:node220 a time:temporanEntity .

_:node221 a time:Instant .

_:node222 a <http://www.w3.org/2006/time#(General)DateTimeDescription> .

_:node223 a time:Instant .

_:node224 a <http://www.w3.org/2006/time#(General)DateTimeDescription> .

_:node225 a time:temporanEntity .

_:node226 a time:Instant .

_:node227 a <http://www.w3.org/2006/time#(General)DateTimeDescription> .

_:node228 a time:Instant .

_:node229 a <http://www.w3.org/2006/time#(General)DateTimeDescription> .

:wikipediaPerangDayakDesa a sem:View .

_:node230 a time:temporanEntity .

_:node231 a time:Instant .

_:node232 a <http://www.w3.org/2006/time#(General)DateTimeDescription> .

_:node233 a time:Instant .

_:node234 a <http://www.w3.org/2006/time#(General)DateTimeDescription> .

:KampanyeKalimantan1945 a sem:Event .

:SeranganUmum1Maret1949 a sem:Event .

:PertempuranLengkong a sem:Event .

:wikipediaGerakan30September a sem:View .

_:node235 a time:temporanEntity .

_:node236 a time:Instant .

_:node237 a <http://www.w3.org/2006/time#(General)DateTimeDescription> .

_:node238 a time:Instant .

_:node239 a <http://www.w3.org/2006/time#(General)DateTimeDescription> .

:wikipediaKampanyeHindiaBelanda a sem:View .

_:node240 a time:temporanEntity .

_:node241 a time:Instant .

_:node242 a <http://www.w3.org/2006/time#(General)DateTimeDescription> .

_:node243 a time:Instant .

_:node244 a <http://www.w3.org/2006/time#(General)DateTimeDescription> .

_:node245 a time:temporanEntity .

_:node246 a time:Instant .

_:node247 a <http://www.w3.org/2006/time#(General)DateTimeDescription> .

_:node248 a time:Instant .

_:node249 a <http://www.w3.org/2006/time#(General)DateTimeDescription> .

:Peristiwa19November a sem:Event .

:wikipediaPertempuranLengkong a sem:View .

_:node250 a time:temporanEntity .

_:node251 a time:Instant .

_:node252 a <http://www.w3.org/2006/time#(General)DateTimeDescription> .

_:node253 a time:Instant .

_:node254 a <http://www.w3.org/2006/time#(General)DateTimeDescription> .

_:node255 a time:temporanEntity .

_:node256 a time:Instant .

_:node257 a <http://www.w3.org/2006/time#(General)DateTimeDescription> .

_:node258 a time:Instant .

_:node259 a <http://www.w3.org/2006/time#(General)DateTimeDescription> .

:wikipediaPertempuranMedanArea a sem:View .

_:node260 a time:temporanEntity .

_:node261 a time:Instant .

_:node262 a <http://www.w3.org/2006/time#(General)DateTimeDescription> .

_:node263 a time:Instant .

_:node264 a <http://www.w3.org/2006/time#(General)DateTimeDescription> .

:wikipediaPertempuranKumai a sem:View .

_:node265 a time:temporanEntity .

_:node266 a time:Instant .

_:node267 a <http://www.w3.org/2006/time#(General)DateTimeDescription> .

_:node268 a time:Instant .

_:node269 a <http://www.w3.org/2006/time#(General)DateTimeDescription> .

:wikipediaSeranganUmumSurakarta a sem:View .

_:node270 a time:temporanEntity .

_:node271 a time:Instant .

_:node272 a <http://www.w3.org/2006/time#(General)DateTimeDescription> .

_:node273 a time:Instant .

_:node274 a <http://www.w3.org/2006/time#(General)DateTimeDescription> .

:PertempuranLimaHari a sem:Event .

_:node275 a time:temporanEntity .

_:node276 a time:Instant .

_:node277 a <http://www.w3.org/2006/time#(General)DateTimeDescription> .

_:node278 a time:Instant .

_:node279 a <http://www.w3.org/2006/time#(General)DateTimeDescription> .

:wikipediaPuputanMargarana a sem:View .

_:node280 a time:temporanEntity .

_:node281 a time:Instant .

_:node282 a <http://www.w3.org/2006/time#(General)DateTimeDescription> .

_:node283 a time:Instant .

_:node284 a <http://www.w3.org/2006/time#(General)DateTimeDescription> .

:wikipediaPertempuranLimaHari a sem:View .

_:node285 a time:temporanEntity .

_:node286 a time:Instant .

_:node287 a <http://www.w3.org/2006/time#(General)DateTimeDescription> .

_:node288 a time:Instant .

_:node289 a <http://www.w3.org/2006/time#(General)DateTimeDescription> .

_:node290 a time:temporanEntity .

_:node291 a time:Instant .

_:node292 a <http://www.w3.org/2006/time#(General)DateTimeDescription> .

_:node293 a time:Instant .

_:node294 a <http://www.w3.org/2006/time#(General)DateTimeDescription> .

:PertempuranSurabaya a sem:Event .

_:node295 a time:temporanEntity .

_:node296 a time:Instant .

_:node297 a <http://www.w3.org/2006/time#(General)DateTimeDescription> .

_:node298 a time:Instant .

_:node299 a <http://www.w3.org/2006/time#(General)DateTimeDescription> .

:PertempuranMedanArea a sem:Event .

:wikipediaPertempuranSurabaya a sem:View .

_:node300 a time:temporanEntity .

_:node301 a time:Instant .

_:node302 a <http://www.w3.org/2006/time#(General)DateTimeDescription> .

_:node303 a time:Instant .

_:node304 a <http://www.w3.org/2006/time#(General)DateTimeDescription> .

_:node305 a time:temporanEntity .

_:node306 a time:Instant .

_:node307 a <http://www.w3.org/2006/time#(General)DateTimeDescription> .

_:node308 a time:Instant .

_:node309 a <http://www.w3.org/2006/time#(General)DateTimeDescription> .

_:node310 a time:temporanEntity .

_:node311 a time:Instant .

_:node312 a <http://www.w3.org/2006/time#(General)DateTimeDescription> .

_:node313 a time:Instant .

_:node314 a <http://www.w3.org/2006/time#(General)DateTimeDescription> .

_:node315 a time:temporanEntity .

_:node316 a time:Instant .

_:node317 a <http://www.w3.org/2006/time#(General)DateTimeDescription> .

_:node318 a time:Instant .

_:node319 a <http://www.w3.org/2006/time#(General)DateTimeDescription> .

_:node320 a time:temporanEntity .

_:node321 a time:Instant .

_:node322 a <http://www.w3.org/2006/time#(General)DateTimeDescription> .

_:node323 a time:Instant .

_:node324 a <http://www.w3.org/2006/time#(General)DateTimeDescription> .

:wikipediaDelapanJamPertempurandiMangkang a sem:View .

_:node325 a time:temporanEntity .

_:node326 a time:Instant .

_:node327 a <http://www.w3.org/2006/time#(General)DateTimeDescription> .

_:node328 a time:Instant .

_:node329 a <http://www.w3.org/2006/time#(General)DateTimeDescription> .

_:node330 a time:temporanEntity .

_:node331 a time:Instant .

_:node332 a <http://www.w3.org/2006/time#(General)DateTimeDescription> .

_:node333 a time:Instant .

_:node334 a <http://www.w3.org/2006/time#(General)DateTimeDescription> .

:wikipediaPeristiwa19November a sem:View .

_:node335 a time:temporanEntity .

_:node336 a time:Instant .

_:node337 a <http://www.w3.org/2006/time#(General)DateTimeDescription> .

_:node338 a time:Instant .

_:node339 a <http://www.w3.org/2006/time#(General)DateTimeDescription> .

:PemberontakanDITIIdiAceh a sem:Event .

_:node340 a time:temporanEntity .

_:node341 a time:Instant .

_:node342 a <http://www.w3.org/2006/time#(General)DateTimeDescription> .

_:node343 a time:Instant .

_:node344 a <http://www.w3.org/2006/time#(General)DateTimeDescription> .

:PertempuranKumai a sem:Event .

:PenyerbuanKotabaruYogyakarta a sem:Event .

:PuputanMargarana a sem:Event .

:PerangCumbok a sem:Event .

_:node345 a time:temporanEntity .

_:node346 a time:Instant .

_:node347 a <http://www.w3.org/2006/time#(General)DateTimeDescription> .

_:node348 a time:Instant .

_:node349 a <http://www.w3.org/2006/time#(General)DateTimeDescription> .

:wikipediaOperasi17Agustus a sem:View .

_:node350 a time:temporanEntity .

_:node351 a time:Instant .

_:node352 a <http://www.w3.org/2006/time#(General)DateTimeDescription> .

_:node353 a time:Instant .

_:node354 a <http://www.w3.org/2006/time#(General)DateTimeDescription> .

:SeranganUmumSurakarta a sem:Event .

:JisaburoOzawa a sem:Actor .

:MuhammadMangundiprojo a sem:Actor .

:Soengkono a sem:Actor .

:HarioJonosewojo a sem:Actor .

:MoehammadJasin a sem:Actor .

:Moestopo a sem:Actor .

:RobertMansergh a sem:Actor .

:AubertinMallaby a sem:Actor .

:Sutomo a sem:Actor .

:GoliathTabuni a sem:Actor .

:Soekarno a sem:Actor .

:KiyotakeKawaguchi a sem:Actor .

:RaymondWesterling a sem:Actor .

:MathiasWenda a sem:Actor .

:JuliusTahija a sem:Actor .

:InfanteriBelanda a sem:Actor .

:Moekijat a sem:Actor .

:MohammadHatta a sem:Actor .

:DouglasMacArthur a sem:Actor .

:ListyoSigitPrabowo a sem:Actor .

:REMartadinata a sem:Actor .

:TeukuKeumanganUmar a sem:Actor .

:NobutakeKond a sem:Actor .

:SutanSjahrir a sem:Actor .

:SlametRijadi a sem:Actor .

:TEDKelly a sem:Actor .

:AgusSubiyanto a sem:Actor .

:Assaat a sem:Actor .

:PangRati a sem:Actor .

:MacDonald a sem:Actor .

:MuhammadToha a sem:Actor .

:AbdulHarisNasution a sem:Actor .

:KidoShinichir a sem:Actor .

:PrabowoSubianto a sem:Actor .

:EgianusKogoya a sem:Actor .

:BudiGunawan a sem:Actor .

:JaminGinting a sem:Actor .

:AbdulKarimMS a sem:Actor .

:AchmadTahir a sem:Actor .

:HubertusJohannesvanMook a sem:Actor .

:TeungkuHasanKruengKalee a sem:Actor .

:TeukuDaudCumbok a sem:Actor .

:TeukuNyakArif a sem:Actor .

:TeungkuAhmadHasballah a sem:Actor .

:SyamaunGaharu a sem:Actor .

:DaudBeureueh a sem:Actor .

:MichiakiKamada a sem:Actor .

:ThomasKinkaid a sem:Actor .

:HeinterPoorten a sem:Actor .

:JBTKnig a sem:Actor .

:FMollinger a sem:Actor .

:IGustiNgurahRai a sem:Actor .

:SimonSpoor a sem:Actor .

:BabaMasao a sem:Actor .

:SyafruddinPrawiranegara a sem:Actor .

:MaludinSimbolon a sem:Actor .

:AhmadYani a sem:Actor .

:AhmadHusein a sem:Actor .

:HitoshiImamura a sem:Actor .

:AJFDoulton a sem:Actor .

:EdiSukardi a sem:Actor .

:Musso a sem:Actor .

:TanMalaka a sem:Actor .

:HisaichiTerauchi a sem:Actor .

:Meyer a sem:Actor .

:JoniBotak a sem:Actor .

:LouisMountbatten a sem:Actor .

:Djampi a sem:Actor .

:PangIyo a sem:Actor .

:PangSuma a sem:Actor .

:Nagatani a sem:Actor .

:DirkCornelisBuurmanvanVreeden a sem:Actor .

:SebbySambom a sem:Actor .

:Mollinger a sem:Actor .

:AlidiusTjardavanStarkenborghStachouwer a sem:Actor .

:DaanMogot a sem:Actor .

:IbTakahashi a sem:Actor .

:LudolphHendrikvanOyen a sem:Actor .

:TjokordaGdeRakaSoekawati a sem:Actor .

:Wongsonegoro a sem:Actor .

:Kariadi a sem:Actor .

:GatotSoebroto a sem:Actor .

:KellyKwalik a sem:Actor .

:BJHabibie a sem:Actor .

:VanVreeden a sem:Actor .

:ThomasCHart a sem:Actor .

:ShojiNishimura a sem:Actor .

:Soedirman a sem:Actor .

:TakeoTakagi a sem:Actor .

:DirkReinhardAdelbertvanLangen a sem:Actor .

:BambangSoegeng a sem:Actor .

:OeripSoemohardjo a sem:Actor .

:AndikaPerkasa a sem:Actor .

:ConradHelfrich a sem:Actor .

:ArchibaldWavell1stEarlWavell a sem:Actor .

:RichardPeirse a sem:Actor .

:KarelDoorman a sem:Actor .

:HamengkubuwanaIX a sem:Actor .

:VentjeSumual a sem:Actor .

:JMvdBerge a sem:Actor .

:Soeharto a sem:Actor .

:Otzuka a sem:Actor .

:LeslieMorshead a sem:Actor .

:SusiloBambangYudhoyono a sem:Actor .

:SaalahYusufSutanMangkuto a sem:Actor .

:WilhelminadariBelanda a sem:Actor .

:LeonardusBenyaminMoerdani a sem:Actor .

:MarufAmin a sem:Actor .

:MegawatiSoekarnoputri a sem:Actor .

:TBSimatupang a sem:Actor .

:AdamBB a sem:Actor .

:Wiranto a sem:Actor .

:LoaSekHie a sem:Actor .

:SyarifHamidIIdariPontianak a sem:Actor .

:PhilipChristison a sem:Actor .

:BennyWenda a sem:Actor .

:AbdulkadirWidjojoatmodjo a sem:Actor .

:JacobPrai a sem:Actor .

:AbdulKaharMuzakkar a sem:Actor .

:IsmaelLengah a sem:Actor .

:TrySutrisno a sem:Actor .

:PakubuwanaXII a sem:Actor .

:MangkunegaraVIII a sem:Actor .

:AchmadiHadisoemarto a sem:Actor .

:JokoWidodo a sem:Actor .

:JacobRumbiak a sem:Actor .

:SekarmadjiMaridjanKartosoewirjo a sem:Actor .

:AmirSjarifoeddin a sem:Actor .

:AgustinusAdisoetjipto a sem:Actor .

:AbdurrahmanWahid a sem:Actor .

:JulianadariBelanda a sem:Actor .

_:node355 a time:temporanEntity .

_:node356 a time:Instant .

_:node357 a <http://www.w3.org/2006/time#(General)DateTimeDescription> .

_:node358 a time:Instant .

_:node359 a <http://www.w3.org/2006/time#(General)DateTimeDescription> .

_:node360 a time:temporanEntity .

_:node361 a time:Instant .

_:node362 a <http://www.w3.org/2006/time#(General)DateTimeDescription> .

_:node363 a time:Instant .

_:node364 a <http://www.w3.org/2006/time#(General)DateTimeDescription> .

_:node365 a time:temporanEntity .

_:node366 a time:Instant .

_:node367 a <http://www.w3.org/2006/time#(General)DateTimeDescription> .

_:node368 a time:Instant .

_:node369 a <http://www.w3.org/2006/time#(General)DateTimeDescription> .

_:node370 a time:temporanEntity .

_:node371 a time:Instant .

_:node372 a <http://www.w3.org/2006/time#(General)DateTimeDescription> .

_:node373 a time:Instant .

_:node374 a <http://www.w3.org/2006/time#(General)DateTimeDescription> .

_:node375 a time:temporanEntity .

_:node376 a time:Instant .

_:node377 a <http://www.w3.org/2006/time#(General)DateTimeDescription> .

_:node378 a time:Instant .

_:node379 a <http://www.w3.org/2006/time#(General)DateTimeDescription> .

_:node380 a time:temporanEntity .

_:node381 a time:Instant .

_:node382 a <http://www.w3.org/2006/time#(General)DateTimeDescription> .

_:node383 a time:Instant .

_:node384 a <http://www.w3.org/2006/time#(General)DateTimeDescription> .

_:node385 a time:temporanEntity .

_:node386 a time:Instant .

_:node387 a <http://www.w3.org/2006/time#(General)DateTimeDescription> .

_:node388 a time:Instant .

_:node389 a <http://www.w3.org/2006/time#(General)DateTimeDescription> .

_:node390 a time:temporanEntity .

_:node391 a time:Instant .

_:node392 a <http://www.w3.org/2006/time#(General)DateTimeDescription> .

_:node393 a time:Instant .

_:node394 a <http://www.w3.org/2006/time#(General)DateTimeDescription> .

_:node395 a time:temporanEntity .

_:node396 a time:Instant .

_:node397 a <http://www.w3.org/2006/time#(General)DateTimeDescription> .

_:node398 a time:Instant .

_:node399 a <http://www.w3.org/2006/time#(General)DateTimeDescription> .

_:node400 a time:temporanEntity .

_:node401 a time:Instant .

_:node402 a <http://www.w3.org/2006/time#(General)DateTimeDescription> .

_:node403 a time:Instant .

_:node404 a <http://www.w3.org/2006/time#(General)DateTimeDescription> .

_:node405 a time:temporanEntity .

_:node406 a time:Instant .

_:node407 a <http://www.w3.org/2006/time#(General)DateTimeDescription> .

_:node408 a time:Instant .

_:node409 a <http://www.w3.org/2006/time#(General)DateTimeDescription> .

_:node410 a time:temporanEntity .

_:node411 a time:Instant .

_:node412 a <http://www.w3.org/2006/time#(General)DateTimeDescription> .

_:node413 a time:Instant .

_:node414 a <http://www.w3.org/2006/time#(General)DateTimeDescription> .

_:node415 a time:temporanEntity .

_:node416 a time:Instant .

_:node417 a <http://www.w3.org/2006/time#(General)DateTimeDescription> .

_:node418 a time:Instant .

_:node419 a <http://www.w3.org/2006/time#(General)DateTimeDescription> .

_:node420 a time:temporanEntity .

_:node421 a time:Instant .

_:node422 a <http://www.w3.org/2006/time#(General)DateTimeDescription> .

_:node423 a time:Instant .

_:node424 a <http://www.w3.org/2006/time#(General)DateTimeDescription> .

_:node425 a time:temporanEntity .

_:node426 a time:Instant .

_:node427 a <http://www.w3.org/2006/time#(General)DateTimeDescription> .

_:node428 a time:Instant .

_:node429 a <http://www.w3.org/2006/time#(General)DateTimeDescription> .

_:node430 a time:temporanEntity .

_:node431 a time:Instant .

_:node432 a <http://www.w3.org/2006/time#(General)DateTimeDescription> .

_:node433 a time:Instant .

_:node434 a <http://www.w3.org/2006/time#(General)DateTimeDescription> .

_:node435 a time:temporanEntity .

_:node436 a time:Instant .

_:node437 a <http://www.w3.org/2006/time#(General)DateTimeDescription> .

_:node438 a time:Instant .

_:node439 a <http://www.w3.org/2006/time#(General)DateTimeDescription> .

_:node440 a time:temporanEntity .

_:node441 a time:Instant .

_:node442 a <http://www.w3.org/2006/time#(General)DateTimeDescription> .

_:node443 a time:Instant .

_:node444 a <http://www.w3.org/2006/time#(General)DateTimeDescription> .

_:node445 a time:temporanEntity .

_:node446 a time:Instant .

_:node447 a <http://www.w3.org/2006/time#(General)DateTimeDescription> .

_:node448 a time:Instant .

_:node449 a <http://www.w3.org/2006/time#(General)DateTimeDescription> .

_:node450 a time:temporanEntity .

_:node451 a time:Instant .

_:node452 a <http://www.w3.org/2006/time#(General)DateTimeDescription> .

_:node453 a time:Instant .

_:node454 a <http://www.w3.org/2006/time#(General)DateTimeDescription> .

_:node455 a time:temporanEntity .

_:node456 a time:Instant .

_:node457 a <http://www.w3.org/2006/time#(General)DateTimeDescription> .

_:node458 a time:Instant .

_:node459 a <http://www.w3.org/2006/time#(General)DateTimeDescription> .

_:node460 a time:temporanEntity .

_:node461 a time:Instant .

_:node462 a <http://www.w3.org/2006/time#(General)DateTimeDescription> .

_:node463 a time:Instant .

_:node464 a <http://www.w3.org/2006/time#(General)DateTimeDescription> .

_:node465 a time:temporanEntity .

_:node466 a time:Instant .

_:node467 a <http://www.w3.org/2006/time#(General)DateTimeDescription> .

_:node468 a time:Instant .

_:node469 a <http://www.w3.org/2006/time#(General)DateTimeDescription> .

_:node470 a time:temporanEntity .

_:node471 a time:Instant .

_:node472 a <http://www.w3.org/2006/time#(General)DateTimeDescription> .

_:node473 a time:Instant .

_:node474 a <http://www.w3.org/2006/time#(General)DateTimeDescription> .

_:node475 a time:temporanEntity .

_:node476 a time:Instant .

_:node477 a <http://www.w3.org/2006/time#(General)DateTimeDescription> .

_:node478 a time:Instant .

_:node479 a <http://www.w3.org/2006/time#(General)DateTimeDescription> .

_:node480 a time:temporanEntity .

_:node481 a time:Instant .

_:node482 a <http://www.w3.org/2006/time#(General)DateTimeDescription> .

_:node483 a time:Instant .

_:node484 a <http://www.w3.org/2006/time#(General)DateTimeDescription> .

_:node485 a time:temporanEntity .

_:node486 a time:Instant .

_:node487 a <http://www.w3.org/2006/time#(General)DateTimeDescription> .

_:node488 a time:Instant .

_:node489 a <http://www.w3.org/2006/time#(General)DateTimeDescription> .

_:node490 a time:temporanEntity .

_:node491 a time:Instant .

_:node492 a <http://www.w3.org/2006/time#(General)DateTimeDescription> .

_:node493 a time:Instant .

_:node494 a <http://www.w3.org/2006/time#(General)DateTimeDescription> .

_:node495 a time:temporanEntity .

_:node496 a time:Instant .

_:node497 a <http://www.w3.org/2006/time#(General)DateTimeDescription> .

_:node498 a time:Instant .

_:node499 a <http://www.w3.org/2006/time#(General)DateTimeDescription> .

_:node500 a time:temporanEntity .

_:node501 a time:Instant .

_:node502 a <http://www.w3.org/2006/time#(General)DateTimeDescription> .

_:node503 a time:Instant .

_:node504 a <http://www.w3.org/2006/time#(General)DateTimeDescription> .

_:node505 a time:temporanEntity .

_:node506 a time:Instant .

_:node507 a <http://www.w3.org/2006/time#(General)DateTimeDescription> .

_:node508 a time:Instant .

_:node509 a <http://www.w3.org/2006/time#(General)DateTimeDescription> .

_:node510 a time:temporanEntity .

_:node511 a time:Instant .

_:node512 a <http://www.w3.org/2006/time#(General)DateTimeDescription> .

_:node513 a time:Instant .

_:node514 a <http://www.w3.org/2006/time#(General)DateTimeDescription> .

_:node515 a time:temporanEntity .

_:node516 a time:Instant .

_:node517 a <http://www.w3.org/2006/time#(General)DateTimeDescription> .

_:node518 a time:Instant .

_:node519 a <http://www.w3.org/2006/time#(General)DateTimeDescription> .

_:node520 a time:temporanEntity .

_:node521 a time:Instant .

_:node522 a <http://www.w3.org/2006/time#(General)DateTimeDescription> .

_:node523 a time:Instant .

_:node524 a <http://www.w3.org/2006/time#(General)DateTimeDescription> .

_:node525 a time:temporanEntity .

_:node526 a time:Instant .

_:node527 a <http://www.w3.org/2006/time#(General)DateTimeDescription> .

_:node528 a time:Instant .

_:node529 a <http://www.w3.org/2006/time#(General)DateTimeDescription> .

_:node530 a time:temporanEntity .

_:node531 a time:Instant .

_:node532 a <http://www.w3.org/2006/time#(General)DateTimeDescription> .

_:node533 a time:Instant .

_:node534 a <http://www.w3.org/2006/time#(General)DateTimeDescription> .

_:node535 a time:temporanEntity .

_:node536 a time:Instant .

_:node537 a <http://www.w3.org/2006/time#(General)DateTimeDescription> .

_:node538 a time:Instant .

_:node539 a <http://www.w3.org/2006/time#(General)DateTimeDescription> .

_:node540 a time:temporanEntity .

_:node541 a time:Instant .

_:node542 a <http://www.w3.org/2006/time#(General)DateTimeDescription> .

_:node543 a time:Instant .

_:node544 a <http://www.w3.org/2006/time#(General)DateTimeDescription> .

_:node545 a time:temporanEntity .

_:node546 a time:Instant .

_:node547 a <http://www.w3.org/2006/time#(General)DateTimeDescription> .

_:node548 a time:Instant .

_:node549 a <http://www.w3.org/2006/time#(General)DateTimeDescription> .

_:node550 a time:temporanEntity .

_:node551 a time:Instant .

_:node552 a <http://www.w3.org/2006/time#(General)DateTimeDescription> .

_:node553 a time:Instant .

_:node554 a <http://www.w3.org/2006/time#(General)DateTimeDescription> .

_:node555 a time:temporanEntity .

_:node556 a time:Instant .

_:node557 a <http://www.w3.org/2006/time#(General)DateTimeDescription> .

_:node558 a time:Instant .

_:node559 a <http://www.w3.org/2006/time#(General)DateTimeDescription> .

_:node560 a time:temporanEntity .

_:node561 a time:Instant .

_:node562 a <http://www.w3.org/2006/time#(General)DateTimeDescription> .

_:node563 a time:Instant .

_:node564 a <http://www.w3.org/2006/time#(General)DateTimeDescription> .

_:node565 a time:temporanEntity .

_:node566 a time:Instant .

_:node567 a <http://www.w3.org/2006/time#(General)DateTimeDescription> .

_:node568 a time:Instant .

_:node569 a <http://www.w3.org/2006/time#(General)DateTimeDescription> .

_:node570 a time:temporanEntity .

_:node571 a time:Instant .

_:node572 a <http://www.w3.org/2006/time#(General)DateTimeDescription> .

_:node573 a time:Instant .

_:node574 a <http://www.w3.org/2006/time#(General)DateTimeDescription> .

_:node575 a time:temporanEntity .

_:node576 a time:Instant .

_:node577 a <http://www.w3.org/2006/time#(General)DateTimeDescription> .

_:node578 a time:Instant .

_:node579 a <http://www.w3.org/2006/time#(General)DateTimeDescription> .

_:node580 a time:temporanEntity .

_:node581 a time:Instant .

_:node582 a <http://www.w3.org/2006/time#(General)DateTimeDescription> .

_:node583 a time:Instant .

_:node584 a <http://www.w3.org/2006/time#(General)DateTimeDescription> .

_:node585 a time:temporanEntity .

_:node586 a time:Instant .

_:node587 a <http://www.w3.org/2006/time#(General)DateTimeDescription> .

_:node588 a time:Instant .

_:node589 a <http://www.w3.org/2006/time#(General)DateTimeDescription> .

_:node590 a time:temporanEntity .

_:node591 a time:Instant .

_:node592 a <http://www.w3.org/2006/time#(General)DateTimeDescription> .

_:node593 a time:Instant .

_:node594 a <http://www.w3.org/2006/time#(General)DateTimeDescription> .

_:node595 a time:temporanEntity .

_:node596 a time:Instant .

_:node597 a <http://www.w3.org/2006/time#(General)DateTimeDescription> .

_:node598 a time:Instant .

_:node599 a <http://www.w3.org/2006/time#(General)DateTimeDescription> .

_:node600 a time:temporanEntity .

_:node601 a time:Instant .

_:node602 a <http://www.w3.org/2006/time#(General)DateTimeDescription> .

_:node603 a time:Instant .

_:node604 a <http://www.w3.org/2006/time#(General)DateTimeDescription> .

_:node605 a time:temporanEntity .

_:node606 a time:Instant .

_:node607 a <http://www.w3.org/2006/time#(General)DateTimeDescription> .

_:node608 a time:Instant .

_:node609 a <http://www.w3.org/2006/time#(General)DateTimeDescription> .

_:node610 a time:temporanEntity .

_:node611 a time:Instant .

_:node612 a <http://www.w3.org/2006/time#(General)DateTimeDescription> .

_:node613 a time:Instant .

_:node614 a <http://www.w3.org/2006/time#(General)DateTimeDescription> .

_:node615 a time:temporanEntity .

_:node616 a time:Instant .

_:node617 a <http://www.w3.org/2006/time#(General)DateTimeDescription> .

_:node618 a time:Instant .

_:node619 a <http://www.w3.org/2006/time#(General)DateTimeDescription> .

_:node620 a time:temporanEntity .

_:node621 a time:Instant .

_:node622 a <http://www.w3.org/2006/time#(General)DateTimeDescription> .

_:node623 a time:Instant .

_:node624 a <http://www.w3.org/2006/time#(General)DateTimeDescription> .

_:node625 a time:temporanEntity .

_:node626 a time:Instant .

_:node627 a <http://www.w3.org/2006/time#(General)DateTimeDescription> .

_:node628 a time:Instant .

_:node629 a <http://www.w3.org/2006/time#(General)DateTimeDescription> .

_:node630 a time:temporanEntity .

_:node631 a time:Instant .

_:node632 a <http://www.w3.org/2006/time#(General)DateTimeDescription> .

_:node633 a time:Instant .

_:node634 a <http://www.w3.org/2006/time#(General)DateTimeDescription> .

_:node635 a time:temporanEntity .

_:node636 a time:Instant .

_:node637 a <http://www.w3.org/2006/time#(General)DateTimeDescription> .

_:node638 a time:Instant .

_:node639 a <http://www.w3.org/2006/time#(General)DateTimeDescription> .

_:node640 a time:temporanEntity .

_:node641 a time:Instant .

_:node642 a <http://www.w3.org/2006/time#(General)DateTimeDescription> .

_:node643 a time:Instant .

_:node644 a <http://www.w3.org/2006/time#(General)DateTimeDescription> .

_:node645 a time:temporanEntity .

_:node646 a time:Instant .

_:node647 a <http://www.w3.org/2006/time#(General)DateTimeDescription> .

_:node648 a time:Instant .

_:node649 a <http://www.w3.org/2006/time#(General)DateTimeDescription> .

_:node650 a time:temporanEntity .

_:node651 a time:Instant .

_:node652 a <http://www.w3.org/2006/time#(General)DateTimeDescription> .

_:node653 a time:Instant .

_:node654 a <http://www.w3.org/2006/time#(General)DateTimeDescription> .

_:node655 a time:temporanEntity .

_:node656 a time:Instant .

_:node657 a <http://www.w3.org/2006/time#(General)DateTimeDescription> .

_:node658 a time:Instant .

_:node659 a <http://www.w3.org/2006/time#(General)DateTimeDescription> .

_:node660 a time:temporanEntity .

_:node661 a time:Instant .

_:node662 a <http://www.w3.org/2006/time#(General)DateTimeDescription> .

_:node663 a time:Instant .

_:node664 a <http://www.w3.org/2006/time#(General)DateTimeDescription> .

_:node665 a time:temporanEntity .

_:node666 a time:Instant .

_:node667 a <http://www.w3.org/2006/time#(General)DateTimeDescription> .

_:node668 a time:Instant .

_:node669 a <http://www.w3.org/2006/time#(General)DateTimeDescription> .

_:node670 a time:temporanEntity .

_:node671 a time:Instant .

_:node672 a <http://www.w3.org/2006/time#(General)DateTimeDescription> .

_:node673 a time:Instant .

_:node674 a <http://www.w3.org/2006/time#(General)DateTimeDescription> .

_:node675 a time:temporanEntity .

_:node676 a time:Instant .

_:node677 a <http://www.w3.org/2006/time#(General)DateTimeDescription> .

_:node678 a time:Instant .

_:node679 a <http://www.w3.org/2006/time#(General)DateTimeDescription> .

_:node680 a time:temporanEntity .

_:node681 a time:Instant .

_:node682 a <http://www.w3.org/2006/time#(General)DateTimeDescription> .

_:node683 a time:Instant .

_:node684 a <http://www.w3.org/2006/time#(General)DateTimeDescription> .

_:node685 a time:temporanEntity .

_:node686 a time:Instant .

_:node687 a <http://www.w3.org/2006/time#(General)DateTimeDescription> .

_:node688 a time:Instant .

_:node689 a <http://www.w3.org/2006/time#(General)DateTimeDescription> .

_:node690 a time:temporanEntity .

_:node691 a time:Instant .

_:node692 a <http://www.w3.org/2006/time#(General)DateTimeDescription> .

_:node693 a time:Instant .

_:node694 a <http://www.w3.org/2006/time#(General)DateTimeDescription> .

_:node695 a time:temporanEntity .

_:node696 a time:Instant .

_:node697 a <http://www.w3.org/2006/time#(General)DateTimeDescription> .

_:node698 a time:Instant .

_:node699 a <http://www.w3.org/2006/time#(General)DateTimeDescription> .

_:node700 a time:temporanEntity .

_:node701 a time:Instant .

_:node702 a <http://www.w3.org/2006/time#(General)DateTimeDescription> .

_:node703 a time:Instant .

_:node704 a <http://www.w3.org/2006/time#(General)DateTimeDescription> .

_:node705 a time:temporanEntity .

_:node706 a time:Instant .

_:node707 a <http://www.w3.org/2006/time#(General)DateTimeDescription> .

_:node708 a time:Instant .

_:node709 a <http://www.w3.org/2006/time#(General)DateTimeDescription> .

_:node710 a time:temporanEntity .

_:node711 a time:Instant .

_:node712 a <http://www.w3.org/2006/time#(General)DateTimeDescription> .

_:node713 a time:Instant .

_:node714 a <http://www.w3.org/2006/time#(General)DateTimeDescription> .

_:node715 a time:temporanEntity .

_:node716 a time:Instant .

_:node717 a <http://www.w3.org/2006/time#(General)DateTimeDescription> .

_:node718 a time:Instant .

_:node719 a <http://www.w3.org/2006/time#(General)DateTimeDescription> .

_:node720 a time:temporanEntity .

_:node721 a time:Instant .

_:node722 a <http://www.w3.org/2006/time#(General)DateTimeDescription> .

_:node723 a time:Instant .

_:node724 a <http://www.w3.org/2006/time#(General)DateTimeDescription> .

_:node725 a time:temporanEntity .

_:node726 a time:Instant .

_:node727 a <http://www.w3.org/2006/time#(General)DateTimeDescription> .

_:node728 a time:Instant .

_:node729 a <http://www.w3.org/2006/time#(General)DateTimeDescription> .

_:node730 a time:temporanEntity .

_:node731 a time:Instant .

_:node732 a <http://www.w3.org/2006/time#(General)DateTimeDescription> .

_:node733 a time:Instant .

_:node734 a <http://www.w3.org/2006/time#(General)DateTimeDescription> .

_:node735 a time:temporanEntity .

_:node736 a time:Instant .

_:node737 a <http://www.w3.org/2006/time#(General)DateTimeDescription> .

_:node738 a time:Instant .

_:node739 a <http://www.w3.org/2006/time#(General)DateTimeDescription> .

_:node740 a time:temporanEntity .

_:node741 a time:Instant .

_:node742 a <http://www.w3.org/2006/time#(General)DateTimeDescription> .

_:node743 a time:Instant .

_:node744 a <http://www.w3.org/2006/time#(General)DateTimeDescription> .

_:node745 a time:temporanEntity .

_:node746 a time:Instant .

_:node747 a <http://www.w3.org/2006/time#(General)DateTimeDescription> .

_:node748 a time:Instant .

_:node749 a <http://www.w3.org/2006/time#(General)DateTimeDescription> .

_:node750 a time:temporanEntity .

_:node751 a time:Instant .

_:node752 a <http://www.w3.org/2006/time#(General)DateTimeDescription> .

_:node753 a time:Instant .

_:node754 a <http://www.w3.org/2006/time#(General)DateTimeDescription> .

_:node755 a time:temporanEntity .

_:node756 a time:Instant .

_:node757 a <http://www.w3.org/2006/time#(General)DateTimeDescription> .

_:node758 a time:Instant .

_:node759 a <http://www.w3.org/2006/time#(General)DateTimeDescription> .

_:node760 a time:temporanEntity .

_:node761 a time:Instant .

_:node762 a <http://www.w3.org/2006/time#(General)DateTimeDescription> .

_:node763 a time:Instant .

_:node764 a <http://www.w3.org/2006/time#(General)DateTimeDescription> .

_:node765 a time:temporanEntity .

_:node766 a time:Instant .

_:node767 a <http://www.w3.org/2006/time#(General)DateTimeDescription> .

_:node768 a time:Instant .

_:node769 a <http://www.w3.org/2006/time#(General)DateTimeDescription> .

_:node770 a time:temporanEntity .

_:node771 a time:Instant .

_:node772 a <http://www.w3.org/2006/time#(General)DateTimeDescription> .

_:node773 a time:Instant .

_:node774 a <http://www.w3.org/2006/time#(General)DateTimeDescription> .

_:node775 a time:temporanEntity .

_:node776 a time:Instant .

_:node777 a <http://www.w3.org/2006/time#(General)DateTimeDescription> .

_:node778 a time:Instant .

_:node779 a <http://www.w3.org/2006/time#(General)DateTimeDescription> .

_:node780 a time:temporanEntity .

_:node781 a time:Instant .

_:node782 a <http://www.w3.org/2006/time#(General)DateTimeDescription> .

_:node783 a time:Instant .

_:node784 a <http://www.w3.org/2006/time#(General)DateTimeDescription> .

_:node785 a time:temporanEntity .

_:node786 a time:Instant .

_:node787 a <http://www.w3.org/2006/time#(General)DateTimeDescription> .

_:node788 a time:Instant .

_:node789 a <http://www.w3.org/2006/time#(General)DateTimeDescription> .

_:node790 a time:temporanEntity .

_:node791 a time:Instant .

_:node792 a <http://www.w3.org/2006/time#(General)DateTimeDescription> .

_:node793 a time:Instant .

_:node794 a <http://www.w3.org/2006/time#(General)DateTimeDescription> .

_:node795 a time:temporanEntity .

_:node796 a time:Instant .

_:node797 a <http://www.w3.org/2006/time#(General)DateTimeDescription> .

_:node798 a time:Instant .

_:node799 a <http://www.w3.org/2006/time#(General)DateTimeDescription> .

_:node800 a time:temporanEntity .

_:node801 a time:Instant .

_:node802 a <http://www.w3.org/2006/time#(General)DateTimeDescription> .

_:node803 a time:Instant .

_:node804 a <http://www.w3.org/2006/time#(General)DateTimeDescription> .

_:node805 a time:temporanEntity .

_:node806 a time:Instant .

_:node807 a <http://www.w3.org/2006/time#(General)DateTimeDescription> .

_:node808 a time:Instant .

_:node809 a <http://www.w3.org/2006/time#(General)DateTimeDescription> .

_:node810 a time:temporanEntity .

_:node811 a time:Instant .

_:node812 a <http://www.w3.org/2006/time#(General)DateTimeDescription> .

_:node813 a time:Instant .

_:node814 a <http://www.w3.org/2006/time#(General)DateTimeDescription> .

_:node815 a time:temporanEntity .

_:node816 a time:Instant .

_:node817 a <http://www.w3.org/2006/time#(General)DateTimeDescription> .

_:node818 a time:Instant .

_:node819 a <http://www.w3.org/2006/time#(General)DateTimeDescription> .

_:node820 a time:temporanEntity .

_:node821 a time:Instant .

_:node822 a <http://www.w3.org/2006/time#(General)DateTimeDescription> .

_:node823 a time:Instant .

_:node824 a <http://www.w3.org/2006/time#(General)DateTimeDescription> .

_:node825 a time:temporanEntity .

_:node826 a time:Instant .

_:node827 a <http://www.w3.org/2006/time#(General)DateTimeDescription> .

_:node828 a time:Instant .

_:node829 a <http://www.w3.org/2006/time#(General)DateTimeDescription> .

_:node830 a time:temporanEntity .

_:node831 a time:Instant .

_:node832 a <http://www.w3.org/2006/time#(General)DateTimeDescription> .

_:node833 a time:Instant .

_:node834 a <http://www.w3.org/2006/time#(General)DateTimeDescription> .

_:node835 a time:temporanEntity .

_:node836 a time:Instant .

_:node837 a <http://www.w3.org/2006/time#(General)DateTimeDescription> .

_:node838 a time:Instant .

_:node839 a <http://www.w3.org/2006/time#(General)DateTimeDescription> .

_:node840 a time:temporanEntity .

_:node841 a time:Instant .

_:node842 a <http://www.w3.org/2006/time#(General)DateTimeDescription> .

_:node843 a time:Instant .

_:node844 a <http://www.w3.org/2006/time#(General)DateTimeDescription> .

_:node845 a time:temporanEntity .

_:node846 a time:Instant .

_:node847 a <http://www.w3.org/2006/time#(General)DateTimeDescription> .

_:node848 a time:Instant .

_:node849 a <http://www.w3.org/2006/time#(General)DateTimeDescription> .

_:node850 a time:temporanEntity .

_:node851 a time:Instant .

_:node852 a <http://www.w3.org/2006/time#(General)DateTimeDescription> .

_:node853 a time:Instant .

_:node854 a <http://www.w3.org/2006/time#(General)DateTimeDescription> .

_:node855 a time:temporanEntity .

_:node856 a time:Instant .

_:node857 a <http://www.w3.org/2006/time#(General)DateTimeDescription> .

_:node858 a time:Instant .

_:node859 a <http://www.w3.org/2006/time#(General)DateTimeDescription> .

_:node860 a time:temporanEntity .

_:node861 a time:Instant .

_:node862 a <http://www.w3.org/2006/time#(General)DateTimeDescription> .

_:node863 a time:Instant .

_:node864 a <http://www.w3.org/2006/time#(General)DateTimeDescription> .

_:node865 a time:temporanEntity .

_:node866 a time:Instant .

_:node867 a <http://www.w3.org/2006/time#(General)DateTimeDescription> .

_:node868 a time:Instant .

_:node869 a <http://www.w3.org/2006/time#(General)DateTimeDescription> .

_:node870 a time:temporanEntity .

_:node871 a time:Instant .

_:node872 a <http://www.w3.org/2006/time#(General)DateTimeDescription> .

_:node873 a time:Instant .

_:node874 a <http://www.w3.org/2006/time#(General)DateTimeDescription> .

_:node875 a time:temporanEntity .

_:node876 a time:Instant .

_:node877 a <http://www.w3.org/2006/time#(General)DateTimeDescription> .

_:node878 a time:Instant .

_:node879 a <http://www.w3.org/2006/time#(General)DateTimeDescription> .

_:node880 a time:temporanEntity .

_:node881 a time:Instant .

_:node882 a <http://www.w3.org/2006/time#(General)DateTimeDescription> .

_:node883 a time:Instant .

_:node884 a <http://www.w3.org/2006/time#(General)DateTimeDescription> .

_:node885 a time:temporanEntity .

_:node886 a time:Instant .

_:node887 a <http://www.w3.org/2006/time#(General)DateTimeDescription> .

_:node888 a time:Instant .

_:node889 a <http://www.w3.org/2006/time#(General)DateTimeDescription> .

_:node890 a time:temporanEntity .

_:node891 a time:Instant .

_:node892 a <http://www.w3.org/2006/time#(General)DateTimeDescription> .

_:node893 a time:Instant .

_:node894 a <http://www.w3.org/2006/time#(General)DateTimeDescription> .

_:node895 a time:temporanEntity .

_:node896 a time:Instant .

_:node897 a <http://www.w3.org/2006/time#(General)DateTimeDescription> .

_:node898 a time:Instant .

_:node899 a <http://www.w3.org/2006/time#(General)DateTimeDescription> .

_:node900 a time:temporanEntity .

_:node901 a time:Instant .

_:node902 a <http://www.w3.org/2006/time#(General)DateTimeDescription> .

_:node903 a time:Instant .

_:node904 a <http://www.w3.org/2006/time#(General)DateTimeDescription> .

_:node905 a time:temporanEntity .

_:node906 a time:Instant .

_:node907 a <http://www.w3.org/2006/time#(General)DateTimeDescription> .

_:node908 a time:Instant .

_:node909 a <http://www.w3.org/2006/time#(General)DateTimeDescription> .

_:node910 a time:temporanEntity .

_:node911 a time:Instant .

_:node912 a <http://www.w3.org/2006/time#(General)DateTimeDescription> .

_:node913 a time:Instant .

_:node914 a <http://www.w3.org/2006/time#(General)DateTimeDescription> .

_:node915 a time:temporanEntity .

_:node916 a time:Instant .

_:node917 a <http://www.w3.org/2006/time#(General)DateTimeDescription> .

_:node918 a time:Instant .

_:node919 a <http://www.w3.org/2006/time#(General)DateTimeDescription> .

_:node920 a time:temporanEntity .

_:node921 a time:Instant .

_:node922 a <http://www.w3.org/2006/time#(General)DateTimeDescription> .

_:node923 a time:Instant .

_:node924 a <http://www.w3.org/2006/time#(General)DateTimeDescription> .

_:node925 a time:temporanEntity .

_:node926 a time:Instant .

_:node927 a <http://www.w3.org/2006/time#(General)DateTimeDescription> .

_:node928 a time:Instant .

_:node929 a <http://www.w3.org/2006/time#(General)DateTimeDescription> .

_:node930 a time:temporanEntity .

_:node931 a time:Instant .

_:node932 a <http://www.w3.org/2006/time#(General)DateTimeDescription> .

_:node933 a time:Instant .

_:node934 a <http://www.w3.org/2006/time#(General)DateTimeDescription> .

_:node935 a time:temporanEntity .

_:node936 a time:Instant .

_:node937 a <http://www.w3.org/2006/time#(General)DateTimeDescription> .

_:node938 a time:Instant .

_:node939 a <http://www.w3.org/2006/time#(General)DateTimeDescription> .

_:node940 a time:temporanEntity .

_:node941 a time:Instant .

_:node942 a <http://www.w3.org/2006/time#(General)DateTimeDescription> .

_:node943 a time:Instant .

_:node944 a <http://www.w3.org/2006/time#(General)DateTimeDescription> .

_:node945 a time:temporanEntity .

_:node946 a time:Instant .

_:node947 a <http://www.w3.org/2006/time#(General)DateTimeDescription> .

_:node948 a time:Instant .

_:node949 a <http://www.w3.org/2006/time#(General)DateTimeDescription> .

_:node950 a time:temporanEntity .

_:node951 a time:Instant .

_:node952 a <http://www.w3.org/2006/time#(General)DateTimeDescription> .

_:node953 a time:Instant .

_:node954 a <http://www.w3.org/2006/time#(General)DateTimeDescription> .

_:node955 a time:temporanEntity .

_:node956 a time:Instant .

_:node957 a <http://www.w3.org/2006/time#(General)DateTimeDescription> .

_:node958 a time:Instant .

_:node959 a <http://www.w3.org/2006/time#(General)DateTimeDescription> .

_:node960 a time:temporanEntity .

_:node961 a time:Instant .

_:node962 a <http://www.w3.org/2006/time#(General)DateTimeDescription> .

_:node963 a time:Instant .

_:node964 a <http://www.w3.org/2006/time#(General)DateTimeDescription> .

_:node965 a time:temporanEntity .

_:node966 a time:Instant .

_:node967 a <http://www.w3.org/2006/time#(General)DateTimeDescription> .

_:node968 a time:Instant .

_:node969 a <http://www.w3.org/2006/time#(General)DateTimeDescription> .

_:node970 a time:temporanEntity .

_:node971 a time:Instant .

_:node972 a <http://www.w3.org/2006/time#(General)DateTimeDescription> .

_:node973 a time:Instant .

_:node974 a <http://www.w3.org/2006/time#(General)DateTimeDescription> .

_:node975 a time:temporanEntity .

_:node976 a time:Instant .

_:node977 a <http://www.w3.org/2006/time#(General)DateTimeDescription> .

_:node978 a time:Instant .

_:node979 a <http://www.w3.org/2006/time#(General)DateTimeDescription> .

_:node980 a time:temporanEntity .

_:node981 a time:Instant .

_:node982 a <http://www.w3.org/2006/time#(General)DateTimeDescription> .

_:node983 a time:Instant .

_:node984 a <http://www.w3.org/2006/time#(General)DateTimeDescription> .

_:node985 a time:temporanEntity .

_:node986 a time:Instant .

_:node987 a <http://www.w3.org/2006/time#(General)DateTimeDescription> .

_:node988 a time:Instant .

_:node989 a <http://www.w3.org/2006/time#(General)DateTimeDescription> .

_:node990 a time:temporanEntity .

_:node991 a time:Instant .

_:node992 a <http://www.w3.org/2006/time#(General)DateTimeDescription> .

_:node993 a time:Instant .

_:node994 a <http://www.w3.org/2006/time#(General)DateTimeDescription> .

_:node995 a time:temporanEntity .

_:node996 a time:Instant .

_:node997 a <http://www.w3.org/2006/time#(General)DateTimeDescription> .

_:node998 a time:Instant .

_:node999 a <http://www.w3.org/2006/time#(General)DateTimeDescription> .

_:node1000 a time:temporanEntity .

_:node1001 a time:Instant .

_:node1002 a <http://www.w3.org/2006/time#(General)DateTimeDescription> .

_:node1003 a time:Instant .

_:node1004 a <http://www.w3.org/2006/time#(General)DateTimeDescription> .

_:node1005 a time:temporanEntity .

_:node1006 a time:Instant .

_:node1007 a <http://www.w3.org/2006/time#(General)DateTimeDescription> .

_:node1008 a time:Instant .

_:node1009 a <http://www.w3.org/2006/time#(General)DateTimeDescription> .

:wikipediaPendudukanJepangdiKalimantanBarat a sem:View .

:wikipediaPersengketaanNuginiBaratdanDekolonisasiOseania a sem:View .

:wikipediaPemberontakanDITII a sem:View .

:wikipediaPerangKemerdekaanIndonesia a sem:View .

:wikipediaPerangPasifikdariPerangDuniaII a sem:View .

:PerangPasifikdariPerangDuniaII a sem:Event .

:PascaPerangDuniaKedua a sem:Event .

:wikipediaPascaPerangDuniaKedua a sem:View .

:wikipediaPerangDuniaII a sem:View .

:PemberontakanDITII a sem:Event .

:PerangDuniaII a sem:Event .

:PerangKemerdekaanIndonesia a sem:Event .

:PersengketaanNuginiBaratdanDekolonisasiOseania a sem:Event .

:PendudukanJepangdiKalimantanBarat a sem:Event .

:Indonesia a sem:Actor .

:Tuvalu a sem:Actor .

:Jepang a sem:Actor .

:KerajaanBelanda a sem:Actor .

:KNIL a sem:Actor .

:Belanda a sem:Actor .

:KekaisaranJepang a sem:Actor .

:SelandiaBaru a sem:Actor .

:TNI a sem:Actor .

:RepublikIndonesia a sem:Actor .

:India a sem:Actor .

:BritaniaRaya a sem:Actor .

:DesertirTentaraIndia a sem:Actor .

:SukuDayakDesa a sem:Actor .

:AmerikaSerikat a sem:Actor .

:Samoa a sem:Actor .

:PapuaNugini a sem:Actor .

:Tonga a sem:Actor .

:OrganisasiPapuaMerdeka a sem:Actor .

:KepulauanSolomon a sem:Actor .

:Vanuatu a sem:Actor .

:Nauru a sem:Actor .

:Fiji a sem:Actor .

:Australia a sem:Actor .

:UniSoviet a sem:Actor .

:Libya a sem:Actor .

:Palau a sem:Actor .

:NegaraIslamIndonesia a sem:Actor .

:KorpsBrigadeMobil a sem:Actor .

:BKR a sem:Actor .

:PUSA a sem:Actor .

:Kaumuleebalang a sem:Actor .

:TRI a sem:Actor .

:PDRI a sem:Actor .

:KemaharajaanBritania a sem:Actor .

:AngkatanPerangRatuAdil a sem:Actor .

:BarisanUlama a sem:Actor .

:PaoAnTui a sem:Actor .

:ABDACommand a sem:Actor .

:HindiaBelanda a sem:Actor .

:KesultananPontianak a sem:Actor .

:ImperiumBelanda a sem:Actor .

:PemerintahanSipilHindiaBelanda a sem:Actor .

:KekaisaranBritania a sem:Actor .

:NICA a sem:Actor .

:RelawanTentaraKekaisaranJepang a sem:Actor .

:PRRI a sem:Actor .

:LaskarKalimantan a sem:Actor .

:TKR a sem:Actor .

:MilitanIslam a sem:Actor .

:TentaraKeamananRakyat a sem:Actor .

rdfs:seeAlso rdfs:subPropertyOf owl:topObjectProperty;
  rdfs:domain sem:Event;
  rdfs:range sem:View .

geo:asWKT rdfs:subPropertyOf geo:hasSerialization;
  rdfs:domain geo:Geometry;
  rdfs:range geo:wktLiteral .

geo:asGML rdfs:subPropertyOf geo:hasSerialization;
  rdfs:domain geo:Geometry;
  rdfs:range geo:gmlLiteral .

geo:hasDefaultGeometry rdfs:subPropertyOf geo:hasGeometry;
  rdfs:domain geo:Feature;
  rdfs:range geo:Geometry .

:hasLocation rdfs:subPropertyOf owl:topObjectProperty;
  rdfs:domain sem:Event;
  rdfs:range geo:Feature;
  owl:inverseOf :isLocationOf .

:rootEvent rdfs:subPropertyOf owl:topObjectProperty;
  rdfs:domain sem:View;
  rdfs:range sem:Event;
  owl:inverseOf rdfs:seeAlso .

sem:actorType rdfs:subPropertyOf sem:type;
  rdfs:domain sem:Actor;
  rdfs:range sem:ActorType;
  rdfs:comment "Has actor type is used to assign a type to an actor." .

sem:type rdfs:subPropertyOf rdf:type;
  rdfs:range sem:Type;
  rdfs:comment "Type is the super property of the properties that are used to indicate the type of a Core instance, eventType, actorType, placeType, timeType; and of roleType. Types can be both classes and individuals, cf. OWL 2 punning." .

sem:eventType rdfs:subPropertyOf sem:type;
  rdfs:domain sem:Event;
  rdfs:range sem:EventType;
  rdfs:comment "Has event type is used to assign a type to an event." .

sem:hasSubEvent rdfs:subPropertyOf sem:eventProperty;
  rdfs:domain sem:Event;
  rdfs:range sem:Event;
  owl:inverseOf sem:subEventOf;
  rdfs:comment "Has subevent connects an Event to other Events that belong to it. This is a very generic property that does not mean the subevents fully define the superconcept or that there is any causal relationship." .

sem:subTypeOf rdfs:subPropertyOf rdfs:subClassOf;
  rdfs:comment "The inverse property of hasSubType." .

sem:placeType rdfs:subPropertyOf sem:type;
  rdfs:domain sem:Place;
  rdfs:range sem:PlaceType;
  rdfs:comment "Has place type is used to assign a type to a place." .

sem:roleType rdfs:subPropertyOf sem:type;
  rdfs:domain sem:Role;
  rdfs:range sem:RoleType;
  rdfs:comment "Has role type is used to assign a role type to a Role property constraint. This role is a subspecification of the eventProperty which it constrains. For example, if an Event hasActor an Actor and this property is given a Role Constraint, then roleType can be used to assign a role to the participation of the Actor in the Event indicated by hasActor." .

sem:timeType rdfs:subPropertyOf sem:type;
  rdfs:domain sem:Time;
  rdfs:range sem:TimeType;
  rdfs:comment "Has time type is used to assign a type to a time individual." .

geo:defaultGeometry rdfs:subPropertyOf geo:hasGeometry;
  rdfs:domain geo:Feature;
  rdfs:range geo:Geometry;
  owl:equivalentProperty geo:hasDefaultGeometry .

geo:hasArea rdfs:subPropertyOf geo:hasSize;
  rdfs:domain geo:SpatialObject .

geo:hasBoundingBox rdfs:subPropertyOf geo:hasGeometry;
  rdfs:domain geo:Feature;
  rdfs:range geo:Geometry .

geo:hasCentroid rdfs:subPropertyOf geo:hasGeometry;
  rdfs:domain geo:Feature;
  rdfs:range geo:Geometry .

geo:hasLength rdfs:subPropertyOf geo:hasSize;
  rdfs:domain geo:SpatialObject .

geo:hasPerimeterLength rdfs:subPropertyOf geo:hasSize;
  rdfs:domain geo:SpatialObject .

geo:hasVolume rdfs:subPropertyOf geo:hasSize;
  rdfs:domain geo:SpatialObject .

time:hasBeginning rdfs:subPropertyOf time:hasTime;
  rdfs:domain time:TemporalEntity;
  rdfs:range time:Instant;
  rdfs:comment "Beginning of a temporal entity"@en, "Comienzo de una entidad temporal."@es .

time:hasDuration rdfs:subPropertyOf time:hasTemporalDuration;
  rdfs:range time:Duration;
  rdfs:comment "Duracin de una entidad temporal, expresada como un valor escalado o un valor nominal."@es,
    "Duration of a temporal entity, expressed as a scaled value or nominal value"@en .

time:hasDurationDescription rdfs:subPropertyOf time:hasTemporalDuration;
  rdfs:range time:GeneralDurationDescription;
  rdfs:comment "Duracin de una entidad temporal, expresada utilizando una descripcin estructurada."@es,
    "Duration of a temporal entity, expressed using a structured description"@en .

time:hasEnd rdfs:subPropertyOf time:hasTime;
  rdfs:domain time:TemporalEntity;
  rdfs:range time:Instant;
  rdfs:comment "End of a temporal entity."@en, "Final de una entidad temporal."@es .

time:inDateTime rdfs:subPropertyOf time:inTemporalPosition;
  rdfs:domain time:Instant;
  rdfs:range time:GeneralDateTimeDescription;
  rdfs:comment "Posicin de un instante, expresada utilizando una descripcin estructurada."@es,
    "Position of an instant, expressed using a structured description"@en .

time:inTimePosition rdfs:subPropertyOf time:inTemporalPosition;
  rdfs:domain time:Instant;
  rdfs:range time:TimePosition;
  rdfs:comment "Posicin de un instante, expresada como una coordenada temporal o un valor nominal."@es,
    "Position of an instant, expressed as a temporal coordinate or nominal value"@en .

time:intervalAfter rdfs:subPropertyOf time:after, time:intervalDisjoint;
  rdfs:domain time:ProperInterval;
  rdfs:range time:ProperInterval;
  owl:inverseOf time:intervalBefore;
  rdfs:comment "If a proper interval T1 is intervalAfter another proper interval T2, then the beginning of T1 is after the end of T2."@en,
    "Si un intervalo propio T1 es posterior a otro intervalo propio T2, entonces el principio de T1 est despus que el final de T2." .

time:intervalBefore rdfs:subPropertyOf time:before, time:intervalDisjoint;
  rdfs:domain time:ProperInterval;
  rdfs:range time:ProperInterval;
  rdfs:comment "If a proper interval T1 is intervalBefore another proper interval T2, then the end of T1 is before the beginning of T2."@en,
    "Si un intervalo propio T1 est antes que otro intervalo propio T2, entonces el final de T1 est antes que el principio de T2."@es .

time:intervalDuring rdfs:subPropertyOf time:intervalIn;
  rdfs:domain time:ProperInterval;
  rdfs:range time:ProperInterval .

time:intervalFinishes rdfs:subPropertyOf time:intervalIn;
  rdfs:domain time:ProperInterval;
  rdfs:range time:ProperInterval .

time:intervalStarts rdfs:subPropertyOf time:intervalIn;
  rdfs:domain time:ProperInterval;
  rdfs:range time:ProperInterval .

sem:hasBeginTimeStamp rdfs:subPropertyOf sem:hasTimeStamp .

sem:hasEarliestBeginTimeStamp rdfs:subPropertyOf sem:hasBeginTimeStamp .

sem:hasEarliestEndTimeStamp rdfs:subPropertyOf sem:hasEndTimeStamp .

sem:hasEndTimeStamp rdfs:subPropertyOf sem:hasTimeStamp .

sem:hasLatestBeginTimeStamp rdfs:subPropertyOf sem:hasBeginTimeStamp .

sem:hasLatestEndTimeStamp rdfs:subPropertyOf sem:hasEndTimeStamp .

geo:asDGGS rdfs:subPropertyOf geo:hasSerialization;
  rdfs:domain geo:Geometry;
  rdfs:range geo:dggsLiteral .

geo:asGeoJSON rdfs:subPropertyOf geo:hasSerialization;
  rdfs:domain geo:Geometry;
  rdfs:range geo:geoJSONLiteral .

geo:asKML rdfs:subPropertyOf geo:hasSerialization;
  rdfs:domain geo:Geometry;
  rdfs:range geo:kmlLiteral .

geo:hasMetricArea rdfs:subPropertyOf geo:hasMetricSize;
  rdfs:domain geo:SpatialObject;
  rdfs:range xsd:double .

geo:hasMetricLength rdfs:subPropertyOf geo:hasMetricSize;
  rdfs:domain geo:SpatialObject;
  rdfs:range xsd:double .

geo:hasMetricPerimeterLength rdfs:subPropertyOf geo:hasMetricSize;
  rdfs:domain geo:SpatialObject;
  rdfs:range xsd:double .

geo:hasMetricVolume rdfs:subPropertyOf geo:hasMetricSize;
  rdfs:domain geo:SpatialObject;
  rdfs:range xsd:double .

sem:Actor rdfs:subClassOf sem:Authority, sem:Core;
  rdfs:comment """Actors are entities that take part in an Event, either actively or passively. Actors do not necessarily have to be sentient. They can also be objects. Actors are a thing, animate or inanimate, physical or non-physical.
""" .

sem:Event rdfs:subClassOf sem:Core;
  rdfs:comment "Events are things that happen. This comprises everything from historical events to web site sessions and mythical journeys. Event is the central class of SEM." .

geo:Feature rdfs:subClassOf geo:SpatialObject .

foaf:Person rdfs:subClassOf sem:Actor .

sem:View rdfs:subClassOf sem:Constraint;
  rdfs:comment "Views are properties that only hold according to a certain Authority." .

sem:ActorType rdfs:subClassOf sem:Type;
  rdfs:comment "EventType contains all resources that are used to classify Actors, e.g. person" .

sem:EventType rdfs:subClassOf sem:Type;
  rdfs:comment "EventType contains all resources that are used to classify Events, e.g. meeting." .

sem:Place rdfs:subClassOf sem:Core;
  rdfs:comment "Places are locations where an Event happens. They do not need to be physical places and hence do not necessarily need coordinates. Neither do they need to have any significance apart from them being the location of an Event." .

sem:Time rdfs:subClassOf sem:Core;
  rdfs:comment "Time contains symbolic representations of when an Event took place. Time instances do not necessarily need to have a timestamp associated with them. The Time class exists to represent semantics of time, e.g. that one thing happens before another, even though the exact timestamps are unknown." .

time:TemporalEntity rdfs:subClassOf owl:Thing;
  owl:equivalentClass _:node63;
  rdfs:comment "A temporal interval or instant."@en, "Un intervalo temporal o un instante."@es .

sem:PlaceType rdfs:subClassOf sem:Type;
  rdfs:comment "EventType contains all resources that are used to classify Places, e.g. river." .

sem:Role rdfs:subClassOf sem:Constraint;
  rdfs:comment "Roles are properties with a subspecified function or position indicated by a RoleType in the scope of an Event. For example, the sem:hasActor property can be subspecified with the RoleType attacker, to denote that the type of participation of the Actor in the scope of the Event is \"attacker\". The sem:hasPlace property can be subspecified with the RoleType origin, to denote that within the scope of the Event it is the origin." .

sem:RoleType rdfs:subClassOf sem:Type;
  rdfs:comment "EventType contains all resources that are used to classify Roles, e.g. receiver." .

sem:TimeType rdfs:subClassOf sem:Type;
  rdfs:comment "EventType contains all resources that are used to classify Time, e.g. century." .

geo:Geometry rdfs:subClassOf geo:SpatialObject .

time:GeneralDateTimeDescription rdfs:subClassOf time:TemporalPosition, _:node33, _:node34,
    _:node35, _:node36, _:node37, _:node38, _:node39, _:node40, _:node41, _:node42, _:node43,
    _:node44;
  rdfs:comment "Descripcin de fecha y hora estructurada con valores separados para los distintos elementos de un sistema calendario-reloj."@es,
    "Description of date and time structured with separate values for the various elements of a calendar-clock system"@en .

time:DayOfWeek rdfs:subClassOf owl:Thing;
  rdfs:comment "El da de la semana"@es, "The day of week"@en .

time:Instant rdfs:subClassOf time:TemporalEntity;
  rdfs:comment "A temporal entity with zero extent or duration"@en, "Una entidad temporal con una extensin o duracin cero."@es .

time:DateTimeInterval rdfs:subClassOf time:ProperInterval;
  rdfs:comment "'intervalo de fecha-hora' es una subclase de 'intervalo propio', definida utilizando el multi-elemento 'descripcin de fecha-hora'."@es,
    "DateTimeInterval is a subclass of ProperInterval, defined using the multi-element DateTimeDescription."@en .

time:Duration rdfs:subClassOf time:TemporalDuration, _:node23, _:node24;
  rdfs:comment "Duracin de una extensin temporal expresada como un nmero escalado por una unidad temporal."@es,
    "Duration of a temporal extent expressed as a number scaled by a temporal unit"@en .

time:GeneralDurationDescription rdfs:subClassOf time:TemporalDuration, _:node45, _:node46,
    _:node47, _:node48, _:node49, _:node50, _:node51, _:node52;
  rdfs:comment "Descripcin de extensin temporal estructurada con valores separados para los distintos elementos de un sistema de horario-calendario."@es,
    "Description of temporal extent structured with separate values for the various elements of a calendar-clock system."@en .

time:TemporalPosition rdfs:subClassOf _:node66;
  rdfs:comment "A position on a time-line"@en, "Una posicin sobre una lnea de tiempo."@es .

time:TimePosition rdfs:subClassOf time:TemporalPosition, _:node67;
  rdfs:comment "A temporal position described using either a (nominal) value from an ordinal reference system, or a (numeric) value in a temporal coordinate system. "@en,
    "Una posicin temporal descrita utilizando bien un valor (nominal) de un sistema de referencia ordinal, o un valor (numrico) en un sistema de coordenadas temporales."@es .

time:Interval rdfs:subClassOf time:TemporalEntity;
  rdfs:comment "A temporal entity with an extent or duration"@en, "Una entidad temporal con una extensin o duracin."@es .

time:ProperInterval rdfs:subClassOf time:Interval;
  rdfs:comment "A temporal entity with non-zero extent or duration, i.e. for which the value of the beginning and end are different"@en .

time:MonthOfYear rdfs:subClassOf time:DateTimeDescription, _:node55, _:node56, _:node57,
    _:node58, _:node59, _:node60, _:node61, _:node62 .

time:TemporalUnit rdfs:subClassOf time:TemporalDuration .

sem:Object rdfs:subClassOf sem:Actor .

sem:Temporary rdfs:subClassOf sem:Constraint .

geo:FeatureCollection rdfs:subClassOf geo:SpatialObjectCollection, _:node16 .

geo:SpatialObjectCollection rdfs:subClassOf rdfs:Container, _:node18 .

geo:GeometryCollection rdfs:subClassOf geo:SpatialObjectCollection, _:node17 .

time:DateTimeDescription rdfs:subClassOf time:GeneralDateTimeDescription, _:node19,
    _:node20, _:node21, _:node22 .

time:DurationDescription rdfs:subClassOf time:GeneralDurationDescription, _:node25,
    _:node26, _:node27, _:node28, _:node29, _:node30, _:node31, _:node32 .

time:January rdfs:subClassOf time:DateTimeDescription, _:node53, _:node54 .

time:Year rdfs:subClassOf time:DurationDescription, _:node72, _:node73, _:node74,
    _:node75, _:node76, _:node77, _:node78 .

geo:sfEquals rdfs:domain geo:SpatialObject;
  rdfs:range geo:SpatialObject .

geo:sfDisjoint rdfs:domain geo:SpatialObject;
  rdfs:range geo:SpatialObject .

geo:sfIntersects rdfs:domain geo:SpatialObject;
  rdfs:range geo:SpatialObject .

geo:sfTouches rdfs:domain geo:SpatialObject;
  rdfs:range geo:SpatialObject .

geo:sfWithin rdfs:domain geo:SpatialObject;
  rdfs:range geo:SpatialObject .

geo:sfContains rdfs:domain geo:SpatialObject;
  rdfs:range geo:SpatialObject .

geo:sfOverlaps rdfs:domain geo:SpatialObject;
  rdfs:range geo:SpatialObject .

geo:sfCrosses rdfs:domain geo:SpatialObject;
  rdfs:range geo:SpatialObject .

geo:ehEquals rdfs:domain geo:SpatialObject;
  rdfs:range geo:SpatialObject;
  owl:equivalentProperty geo:sfEquals .

geo:ehDisjoint rdfs:domain geo:SpatialObject;
  rdfs:range geo:SpatialObject;
  owl:equivalentProperty geo:sfDisjoint .

geo:ehMeet rdfs:domain geo:SpatialObject;
  rdfs:range geo:SpatialObject;
  owl:equivalentProperty geo:sfTouches .

geo:ehOverlap rdfs:domain geo:SpatialObject;
  rdfs:range geo:SpatialObject .

geo:ehCovers rdfs:domain geo:SpatialObject;
  rdfs:range geo:SpatialObject .

geo:ehCoveredBy rdfs:domain geo:SpatialObject;
  rdfs:range geo:SpatialObject .

geo:ehInside rdfs:domain geo:SpatialObject;
  rdfs:range geo:SpatialObject .

geo:ehContains rdfs:domain geo:SpatialObject;
  rdfs:range geo:SpatialObject .

geo:rcc8eq rdfs:domain geo:SpatialObject;
  rdfs:range geo:SpatialObject .

geo:rcc8dc rdfs:domain geo:SpatialObject;
  rdfs:range geo:SpatialObject .

geo:rcc8ec rdfs:domain geo:SpatialObject;
  rdfs:range geo:SpatialObject .

geo:rcc8po rdfs:domain geo:SpatialObject;
  rdfs:range geo:SpatialObject .

geo:rcc8tppi rdfs:domain geo:SpatialObject;
  rdfs:range geo:SpatialObject .

geo:rcc8tpp rdfs:domain geo:SpatialObject;
  rdfs:range geo:SpatialObject .

geo:rcc8ntpp rdfs:domain geo:SpatialObject;
  rdfs:range geo:SpatialObject .

geo:rcc8ntppi rdfs:domain geo:SpatialObject;
  rdfs:range geo:SpatialObject .

:hasChild rdfs:domain sem:Actor;
  rdfs:range sem:Actor;
  owl:inverseOf :hasParent .

:hasParent rdfs:domain foaf:Person;
  rdfs:range foaf:Person .

:isLocationOf rdfs:domain geo:Feature;
  rdfs:range sem:Event .

:hasRelative rdfs:domain foaf:Person;
  rdfs:range foaf:Person .

:isActorOf rdfs:domain sem:Actor;
  rdfs:range sem:Event;
  owl:inverseOf sem:hasActor .

sem:hasActor rdfs:domain sem:View;
  rdfs:range sem:Actor;
  rdfs:comment "Has actor is used to state which Actors or Objects participate in an Event." .

sem:accordingTo rdfs:domain sem:View;
  rdfs:range sem:Authority;
  rdfs:comment "According to is used to state which Authority sais that a property constrained by the View Constraint is true." .

sem:eventProperty rdfs:domain sem:Event;
  rdfs:comment "Event properties connect Events to other SEM Core entities." .

sem:hasPlace rdfs:domain sem:View;
  rdfs:range geo:Feature, sem:Place;
  rdfs:comment "Has place is used to state in which Place(s) an Event happened. Coordinates can be attached to the Place with the W3C Geospatial Vocabulary (http://www.w3.org/2005/Incubator/geo/XGR-geo-20071023/)." .

sem:subEventOf rdfs:domain sem:Event;
  rdfs:range sem:Event;
  rdfs:comment "Inverse property of hasSubEvent" .

sem:hasSubType rdfs:domain sem:Type;
  rdfs:range sem:Type;
  owl:inverseOf sem:subTypeOf;
  rdfs:comment "Has sub type is used to state that a type falls under another type. This is a generic aggregation relation that is used to generalize over various hierarchical relations that can exist between types." .

sem:hasTime rdfs:domain sem:View;
  rdfs:range sem:Time, time:TemporalEntity;
  rdfs:comment "Has time is used to indicate at which time an Event took place or when a property under the Temporary Constraint is valid. Has time points to a symbolic representation of time, which allows semantic relations between time resources. (see http://www.w3.org/TR/owl-time/)" .

geo:hasGeometry rdfs:domain geo:Feature;
  rdfs:range geo:Geometry .

geo:hasSize rdfs:domain geo:SpatialObject .

geo:hasSpatialAccuracy rdfs:domain geo:Geometry .

geo:hasSpatialResolution rdfs:domain geo:Geometry .

time:after rdfs:domain time:TemporalEntity;
  rdfs:range time:TemporalEntity;
  owl:inverseOf time:before;
  rdfs:comment "Asume una direccin en el tiempo. Si una entidad temporal T1 est despus de otra entidad temporal T2, entonces el principio de T1 est despus del final de T2."@es,
    "The subject is a temporal entity that occurs after the object. If a temporal entity T1 is after another temporal entity T2, then the beginning of T1 is after the end of T2."@en .

time:before rdfs:domain time:TemporalEntity;
  rdfs:range time:TemporalEntity;
  rdfs:comment "Asume una direccin en el tiempo. Si una entidad temporal T1 est antes que otra entidad temporal T2, entonces el final de T1 est antes que el principio de T2. As, \"antes\" se puede considerar bsica para instantes y derivada para intervalos."@es,
    "The subject is a temporal entity that occurs before the object. If a temporal entity T1 is before another temporal entity T2, then the end of T1 is before the beginning of T2. Thus, \"before\" can be considered to be basic to instants and derived for intervals."@en .

time:dayOfWeek rdfs:domain time:GeneralDateTimeDescription;
  rdfs:range time:DayOfWeek;
  rdfs:comment "The day of week, whose value is a member of the class time:DayOfWeek"@en,
    "El da de la semana, cuyo valor es un miembro de la clase 'da de la semana'." .

time:hasDateTimeDescription rdfs:domain time:DateTimeInterval;
  rdfs:range time:GeneralDateTimeDescription;
  rdfs:comment "Valor de intervalo de fecha-hora expresado como un valor estructurado. El principio y el final del intervalo coincide con los lmites del elemento ms corto en la descripcin."@es,
    "Value of DateTimeInterval expressed as a structured value. The beginning and end of the interval coincide with the limits of the shortest element in the description."@en .

time:hasTemporalDuration rdfs:domain time:TemporalEntity;
  rdfs:range time:TemporalDuration;
  rdfs:comment "Duracin de una entidad temporal."@es, "Duration of a temporal entity."@en .

time:hasTRS rdfs:domain _:node10;
  rdfs:range time:TRS;
  rdfs:comment "El sistema de referencia temporal utilizado por una posicin temporal o descripcin de extensin."@es,
    "The temporal reference system used by a temporal position or extent description. "@en .

time:inTemporalPosition rdfs:domain time:Instant;
  rdfs:range time:TemporalPosition;
  rdfs:comment "Posicin de un instante de tiempo."@es, "Position of a time instant"@en .

time:inside rdfs:domain time:Interval;
  rdfs:range time:Instant;
  rdfs:comment "An instant that falls inside the interval. It is not intended to include beginnings and ends of intervals."@en,
    "Un instante que cae dentro del intervalo. Se asume que no es ni el principio ni el final de ningn intervalo."@es .

time:intervalDisjoint rdfs:domain time:ProperInterval;
  rdfs:range time:ProperInterval;
  rdfs:comment "If a proper interval T1 is intervalDisjoint another proper interval T2, then the beginning of T1 is after the end of T2, or the end of T1 is before the beginning of T2, i.e. the intervals do not overlap in any way, but their ordering relationship is not known."@en,
    "Si un intervalo propio T1 es disjunto con otro intervalo propio T2, entonces el principio de T1 est despus del final de T2, o el final de T1 est antes que el principio de T2, es decir, los intervalos no se solapan de ninguna forma, aunque su relacin de orden no se conozca."@es .

time:intervalContains rdfs:domain time:ProperInterval;
  rdfs:range time:ProperInterval;
  owl:inverseOf time:intervalDuring .

time:intervalIn rdfs:domain time:ProperInterval;
  rdfs:range time:ProperInterval .

time:intervalEquals rdfs:domain time:ProperInterval;
  rdfs:range time:ProperInterval .

time:intervalFinishedBy rdfs:domain time:ProperInterval;
  rdfs:range time:ProperInterval;
  owl:inverseOf time:intervalFinishes .

time:intervalMeets rdfs:domain time:ProperInterval;
  rdfs:range time:ProperInterval;
  owl:inverseOf time:intervalMetBy .

time:intervalMetBy rdfs:domain time:ProperInterval;
  rdfs:range time:ProperInterval .

time:intervalOverlappedBy rdfs:domain time:ProperInterval;
  rdfs:range time:ProperInterval;
  owl:inverseOf time:intervalOverlaps .

time:intervalOverlaps rdfs:domain time:ProperInterval;
  rdfs:range time:ProperInterval .

time:intervalStartedBy rdfs:domain time:ProperInterval;
  rdfs:range time:ProperInterval;
  owl:inverseOf time:intervalStarts .

time:monthOfYear rdfs:domain time:GeneralDateTimeDescription;
  rdfs:range time:MonthOfYear .

time:timeZone rdfs:domain time:GeneralDateTimeDescription;
  rdfs:range time:TimeZone .

time:unitType rdfs:domain _:node13;
  rdfs:range time:TemporalUnit .

:deathCause rdfs:domain foaf:Person;
  rdfs:range xsd:string .

:latitude rdfs:domain geo:Geometry;
  rdfs:range xsd:double .

:longitude rdfs:domain geo:Geometry;
  rdfs:range xsd:double .

geo:hasSerialization rdfs:domain geo:Geometry;
  rdfs:range rdfs:Literal .

geo:coordinateDimension rdfs:domain geo:Geometry;
  rdfs:range xsd:integer .

geo:dimension rdfs:domain geo:Geometry;
  rdfs:range xsd:integer .

geo:hasMetricSize rdfs:domain geo:SpatialObject;
  rdfs:range xsd:double .

geo:hasMetricSpatialAccuracy rdfs:domain geo:Geometry;
  rdfs:range xsd:double .

geo:hasMetricSpatialResolution rdfs:domain geo:Geometry;
  rdfs:range xsd:double .

geo:isEmpty rdfs:domain geo:Geometry;
  rdfs:range xsd:boolean .

geo:isSimple rdfs:domain geo:Geometry;
  rdfs:range xsd:boolean .

geo:spatialDimension rdfs:domain geo:Geometry;
  rdfs:range xsd:integer .

time:day rdfs:domain time:GeneralDateTimeDescription .

time:dayOfYear rdfs:domain time:GeneralDateTimeDescription;
  rdfs:range xsd:nonNegativeInteger .

time:days rdfs:domain time:GeneralDurationDescription;
  rdfs:range xsd:decimal .

time:hasXSDDuration rdfs:domain time:TemporalEntity;
  rdfs:range xsd:duration .

time:hour rdfs:domain time:GeneralDateTimeDescription;
  rdfs:range xsd:nonNegativeInteger .

time:hours rdfs:domain time:GeneralDurationDescription;
  rdfs:range xsd:decimal .

time:inXSDDate rdfs:domain time:Instant;
  rdfs:range xsd:date .

time:inXSDDateTime rdfs:domain time:Instant;
  rdfs:range xsd:dateTime .

time:inXSDDateTimeStamp rdfs:domain time:Instant;
  rdfs:range xsd:dateTimeStamp .

time:inXSDgYear rdfs:domain time:Instant;
  rdfs:range xsd:gYear .

time:inXSDgYearMonth rdfs:domain time:Instant;
  rdfs:range xsd:gYearMonth .

time:minute rdfs:domain time:GeneralDateTimeDescription;
  rdfs:range xsd:nonNegativeInteger .

time:minutes rdfs:domain time:GeneralDurationDescription;
  rdfs:range xsd:decimal .

time:month rdfs:domain time:GeneralDateTimeDescription .

time:months rdfs:domain time:GeneralDurationDescription;
  rdfs:range xsd:decimal .

time:nominalPosition rdfs:domain time:TimePosition;
  rdfs:range xsd:string .

time:numericDuration rdfs:domain time:Duration;
  rdfs:range xsd:decimal .

time:numericPosition rdfs:domain time:TimePosition;
  rdfs:range xsd:decimal .

time:second rdfs:domain time:GeneralDateTimeDescription;
  rdfs:range xsd:decimal .

time:seconds rdfs:domain time:GeneralDurationDescription;
  rdfs:range xsd:decimal .

time:week rdfs:domain time:GeneralDateTimeDescription;
  rdfs:range xsd:nonNegativeInteger .

time:weeks rdfs:domain time:GeneralDurationDescription;
  rdfs:range xsd:decimal .

time:xsdDateTime rdfs:domain time:DateTimeInterval;
  rdfs:range xsd:dateTime .

time:year rdfs:domain time:GeneralDateTimeDescription .

time:years rdfs:domain time:GeneralDurationDescription;
  rdfs:range xsd:decimal .

:image rdfs:range xsd:string .

:wikiurl rdfs:range xsd:string .

time:hasTime rdfs:range time:TemporalEntity;
  rdfs:comment "Proporciona soporte a la asociacin de una entidad temporal (instante o intervalo) a cualquier cosa."@es,
    "Supports the association of a temporal entity (instant or interval) to any thing"@en .

_:node11 rdf:first time:GeneralDurationDescription;
  rdf:rest _:node12 .

_:node12 rdf:first time:TemporalPosition;
  rdf:rest rdf:nil .

_:node14 rdf:first time:Duration;
  rdf:rest _:node15 .

_:node15 rdf:first time:GeneralDateTimeDescription;
  rdf:rest rdf:nil .

_:node64 rdf:first time:Instant;
  rdf:rest _:node65 .

_:node65 rdf:first time:Interval;
  rdf:rest rdf:nil .

_:node68 rdf:first _:node69;
  rdf:rest _:node70 .

_:node70 rdf:first _:node71;
  rdf:rest rdf:nil .

time:generalDay rdfs:comment """Day of month - formulated as a text string with a pattern constraint to reproduce the same lexical form as gDay, except that values up to 99 are permitted, in order to support calendars with more than 31 days in a month. 
Note that the value-space is not defined, so a generic OWL2 processor cannot compute ordering relationships of values of this type."""@en,
    """Da del mes - formulado como una cadena de texto con una restriccin patrn para reproducir la misma forma lxica que gDay, excepto que se permiten valores hasta el 99, con el propsito de proporcionar soporte a calendarios con meses con ms de 31 das.
            Ntese que el espacio de valores no est definido, por tanto, un procesador genrico de OWL2 no puede computar relaciones de orden de valores de este tipo."""@es .

time:generalMonth rdfs:comment """Mes del ao - formulado como una cadena de texto con una restriccin patrn para reproducir la misma forma lxica que gMonth, excepto que se permiten valores hasta el 20, con el propsito de proporcionar soporte a calendarios con aos con ms de 12 meses.
            Ntese que el espacio de valores no est definido, por tanto, un procesador genrico de OWL2 no puede computar relaciones de orden de valores de este tipo."""@es,
    """Month of year - formulated as a text string with a pattern constraint to reproduce the same lexical form as gMonth, except that values up to 20 are permitted, in order to support calendars with more than 12 months in the year. 
Note that the value-space is not defined, so a generic OWL2 processor cannot compute ordering relationships of values of this type."""@en .

time:generalYear rdfs:comment """Nmero de ao - formulado como una cadena de texto con una restriccin patrn para reproducir la misma forma lxica que gYear, aunque no est restringido a valores del calendario gregoriano.
            Ntese que el espacio de valores no est definido, por tanto, un procesador genrico de OWL2 no puede computar relaciones de orden de valores de este tipo."""@es,
    """Year number - formulated as a text string with a pattern constraint to reproduce the same lexical form as gYear, but not restricted to values from the Gregorian calendar. 
Note that the value-space is not defined, so a generic OWL2 processor cannot compute ordering relationships of values of this type."""@en .

sem:Authority rdfs:comment "Authorities are entities that state SEM properties. Their nature is not specified. They can symbolize people, organizations, sources of information, etc." .

sem:Type rdfs:comment "The SEM Type class contains all types of Core instances. These can be either individuals of classes themselves. This class is meant to be extended for each application domain." .

time:TRS rdfs:comment """A temporal reference system, such as a temporal coordinate system (with an origin, direction, and scale), a calendar-clock combination, or a (possibly hierarchical) ordinal system. 

This is a stub class, representing the set of all temporal reference systems."""@en,
    """Un sistema de referencia temporal, tal como un sistema de coordenadas temporales (con un origen, una direccin y una escala), una combinacin calendario-reloj, o un sistema ordinal (posiblemente jerrquico).
        Esta clase comodn representa el conjunto de todos los sistemas de referencia temporal."""@es .

time:TemporalDuration rdfs:comment "Extensin de tiempo; duracin de un intervalo de tiempo independiente de su posicin de inicio particular."@es,
    "Time extent; duration of a time interval separate from its particular start position"@en .

time:ProperInterval rdfs:comment "Una entidad temporal con extensin o duracin distinta de cero, es decir, para la cual los valores de principio y fin del intervalo son diferentes."@es;
  rdfs:label "Proper interval"@en, "intervalo propio"@es .

time:intervalContains rdfs:comment "If a proper interval T1 is intervalContains another proper interval T2, then the beginning of T1 is before the beginning of T2, and the end of T1 is after the end of T2."@en,
    "Si un intervalo propio T1 contiene otro intervalo propio T2, entonces el principio de T1 est antes que el principio de T2, y el final de T1 est despus del final de T2."@es;
  rdfs:label "interval contains"@en, "intervalo contiene"@es .

time:intervalDuring rdfs:comment "If a proper interval T1 is intervalDuring another proper interval T2, then the beginning of T1 is after the beginning of T2, and the end of T1 is before the end of T2."@en,
    "Si un intervalo propio T1 est durante otro intervalo propio T2, entonces del principio de T1 est despus del principio de T2, y el final de T1 est antes que el final de T2."@es;
  rdfs:label "interval during"@en, "intervalo durante"@es .

time:intervalIn rdfs:comment "If a proper interval T1 is intervalIn another proper interval T2, then the beginning of T1 is after the beginning of T2 or is coincident with the beginning of T2, and the end of T1 is before the end of T2, or is coincident with the end of T2, except that end of T1 may not be coincident with the end of T2 if the beginning of T1 is coincident with the beginning of T2."@en,
    "Si un intervalo propio T1 es un intervalo interior a otro intervalo propio T2, entonces el principio de T1 est despus del principio de T2 o coincide con el principio de T2, y el final de T1 est antes que el final de T2, o coincide con el final de T2, excepto que el final de T1 puede no coincidir con el final de T2 si el principio de T1 coincide con el principio de T2."@es;
  rdfs:label "interval in"@en, "intervalo interior"@es .

time:intervalEquals rdfs:comment "If a proper interval T1 is intervalEquals another proper interval T2, then the beginning of T1 is coincident with the beginning of T2, and the end of T1 is coincident with the end of T2."@en,
    "Si un intervalo propio T1 es igual a otro intervalo propio T2, entonces el principio de T1 coincide con el principio de T2, y el final de T1 coincide con el final de T2."@es;
  rdfs:label "interval equals"@en, "intervalo igual"@es .

time:intervalFinishedBy rdfs:comment "If a proper interval T1 is intervalFinishedBy another proper interval T2, then the beginning of T1 is before the beginning of T2, and the end of T1 is coincident with the end of T2."@en,
    "Si un intervalo propio T1 est terminado por otro intervalo propio T2, entonces el principio de T1 est antes que el principio de T2, y el final de T1 coincide con el final de T2."@es;
  rdfs:label "interval finished by"@en, "intervalo terminado por"@es .

time:intervalFinishes rdfs:comment "If a proper interval T1 is intervalFinishes another proper interval T2, then the beginning of T1 is after the beginning of T2, and the end of T1 is coincident with the end of T2."@en,
    "Si un intervalo propio T1 termina otro intervalo propio T2, entonces del principio de T1 est despus del principio de T2, y el final de T1 coincide con el final de T2."@es;
  rdfs:label "interval finishes"@en, "intervalo termina"@es .

time:intervalMeets rdfs:comment "If a proper interval T1 is intervalMeets another proper interval T2, then the end of T1 is coincident with the beginning of T2."@en,
    "Si un intervalo propio T1 se encuentra con otro intervalo propio T2, entonces el final de T1 coincide con el principio de T2."@es;
  rdfs:label "interval meets"@en, "intervalo se encuentra"@es .

time:intervalMetBy rdfs:comment "If a proper interval T1 is intervalMetBy another proper interval T2, then the beginning of T1 is coincident with the end of T2."@en,
    "Si un intervalo propio T1 es 'intervalo encontrado por' otro intervalo propio T2, entonces el principio de T1 coincide con el final de T2."@es;
  rdfs:label "interval met by"@en, "intervalo encontrado por"@es .

time:intervalOverlappedBy rdfs:comment "If a proper interval T1 is intervalOverlappedBy another proper interval T2, then the beginning of T1 is after the beginning of T2, the beginning of T1 is before the end of T2, and the end of T1 is after the end of T2."@en,
    "Si un intervalo propio T1 es 'intervalo solapado por' otro intervalo propio T2, entonces el principio de T1 es posterior al principio de T2, y el principio de T1 es anterior al final de T2, y el final de T1 es posterior al final de T2."@es;
  rdfs:label "interval overlapped by"@en, "intervalo solapado por"@es .

time:intervalOverlaps rdfs:comment "Asume una direccin en el tiempo. Si una entidad temporal T1 est despus de otra entidad temporal T2, entonces el principio de T1 est despus del final de T2."@es,
    "If a proper interval T1 is intervalOverlaps another proper interval T2, then the beginning of T1 is before the beginning of T2, the end of T1 is after the beginning of T2, and the end of T1 is before the end of T2."@en,
    "Si un intervalo propio T1 se solapa con otro intervalo propio T2, entonces el principio de T1 es anterior al principio de T2, el final de T1 es posterior al principio de T2, y el final de T1 es anterior al final de T2."@es;
  rdfs:label "interval overlaps"@en, "intervalo se solapa"@es .

time:intervalStartedBy rdfs:comment "If a proper interval T1 is intervalStarted another proper interval T2, then the beginning of T1 is coincident with the beginning of T2, and the end of T1 is after the end of T2."@en,
    "Si un intervalo propio T1 es empezado por otro intervalo propio T2, entonces el principio de T1 coincide con el principio de T2, y el final de T1 es posterior al final de T2."@es;
  rdfs:label "interval started by"@en .

time:intervalStarts rdfs:comment "If a proper interval T1 is intervalStarts another proper interval T2, then the beginning of T1 is coincident with the beginning of T2, and the end of T1 is before the end of T2."@en,
    "Si un intervalo propio T1 empieza otro intervalo propio T2, entonces del principio de T1 con el principio de T2, y el final de T1 es anterior al final de T2."@es;
  rdfs:label "interval starts"@en, "intervalo empieza"@es .

time:monthOfYear rdfs:comment "El mes del ao, cuyo valor es un miembro de la clase 'mes del ao'."@es,
    "The month of the year, whose value is a member of the class time:MonthOfYear"@en;
  rdfs:label "mes del ao"@es, "month of year"@en .

time:MonthOfYear rdfs:comment "El mes del ao."@es, "The month of the year"@en;
  rdfs:label "mes del ao"@es, "Month of year"@en .

time:timeZone rdfs:comment "The time zone for clock elements in the temporal position"@en;
  rdfs:label "en huso horario"@es, "in time zone"@en;
  <http://www.w3.org/2004/02/skos/core#historyNote> """En la versin original de OWL-Time de 2006, el rango de 'en huso horario' se defini en un espacio de nombres diferente \"http://www.w3.org/2006/timezone#\".
            Un axioma de alineacin permite que los datos codificados de acuerdo con la versin anterior sean consistentes con la ontologa actualizada."""@es,
    """In the original 2006 version of OWL-Time, the range of time:timeZone was a TimeZone class in a separate namespace \"http://www.w3.org/2006/timezone#\". 
An alignment axiom 
	tzont:TimeZone rdfs:subClassOf time:TimeZone . 
allows data encoded according to the previous version to be consistent with the updated ontology. """ .

time:TimeZone rdfs:comment """A Time Zone specifies the amount by which the local time is offset from UTC. 
	A time zone is usually denoted geographically (e.g. Australian Eastern Daylight Time), with a constant value in a given region. 
The region where it applies and the offset from UTC are specified by a locally recognised governing authority."""@en,
    """Un huso horario especifica la cantidad en que la hora local est desplazada con respecto a UTC.
        Un huso horario normalmente se denota geogrficamente (p.ej. el horario de verano del este de Australia), con un valor constante en una regin dada.
        La regin donde aplica y el desplazamiento desde UTC las especifica una autoridad gubernamental localmente reconocida."""@es;
  rdfs:label "Time Zone"@en, "huso horario"@es;
  <http://www.w3.org/2004/02/skos/core#historyNote> """En la versin original de OWL-Time de 2006, se defini, en un espacio de nombres diferente \"http://www.w3.org/2006/timezone#\", la clase 'huso horario', con varias propiedades especficas correspondientes a un modelo especfico de huso horario.
    En la versin actual hay una clase con el mismo nombre local en el espacio de nombres de OWL-Time, eliminando la dependencia del espacio de nombres externo.
    Un axioma de alineacin permite que los datos codificados de acuerdo con la versin anterior sean consistentes con la ontologa actualizada."""@es,
    """In the original 2006 version of OWL-Time, the TimeZone class, with several properties corresponding to a specific model of time-zones, was defined in a separate namespace \"http://www.w3.org/2006/timezone#\". 

In the current version a class with same local name is put into the main OWL-Time namespace, removing the dependency on the external namespace. 

An alignment axiom 
	tzont:TimeZone rdfs:subClassOf time:TimeZone . 
allows data encoded according to the previous version to be consistent with the updated ontology. """ .

time:unitType rdfs:comment "La unidad de tiempo que proporciona la precisin de un valor fecha-hora o la escala de una extensin temporal."@es,
    "The temporal unit which provides the precision of a date-time value or scale of a temporal extent"@en;
  rdfs:label "temporal unit type"@en, "tipo de unidad temporal"@es .

time:TemporalUnit rdfs:comment "A standard duration, which provides a scale factor for a time extent, or the granularity or precision for a time position."@en,
    "Una duracin estndar, que proporciona un factor de escala para una extensin de tiempo, o la granularidad o precisin para una posicin de tiempo."@es;
  rdfs:label "Temporal unit"@en, "unidad de tiempo"@es;
  <http://www.w3.org/2004/02/skos/core#changeNote> """Remove enumeration from definition, in order to allow other units to be used when required in other coordinate systems. 
NOTE: existing units are still present as members of the class, but the class membership is now open. 

In the original OWL-Time the following constraint appeared: 
  owl:oneOf (
      time:unitSecond
      time:unitMinute
      time:unitHour
      time:unitDay
      time:unitWeek
      time:unitMonth
      time:unitYear
    ) ;"""@en .

sem:hasBeginTimeStamp rdfs:comment "Has begin timestamp is used to indicate the beginning of a time interval. Omitting the hasBeginTimeStamp while stating a hasEndTimeStamp is interpreted as an open ended interval.";
  rdfs:label "has begin timestamp" .

sem:hasTimeStamp rdfs:comment "Has timestamp is used to put time indicators on any individual. It is the most common way to state when an Event took place. There are subproperties of hasTimeStamp to represent time intervals and uncertain time intervals. If the exact moment is not known, but it is necessary to specify a certain time, use hasTime instead. All of these properties are also used to indicate the time at which a property under the Temporary Constraint is valid.";
  rdfs:label "has timestamp" .

sem:hasEarliestBeginTimeStamp rdfs:comment "Has earliest begin timestamp is used to indicate the earliest possible starting time of an uncertain time interval.";
  rdfs:label "has earliest begin timestamp" .

sem:hasEarliestEndTimeStamp rdfs:comment "Has earliest end timestamp is used to indicate the earliest possible ending time of an uncertain time interval.";
  rdfs:label "has earliest end timestamp" .

sem:hasEndTimeStamp rdfs:comment "Has end timestamp is used to indicate the end of a time interval. Omitting the hasEndTimeStamp while stating a hasBeginTimeStamp is interpreted as an open ended interval.";
  rdfs:label "has end timestamp" .

sem:hasLatestBeginTimeStamp rdfs:comment "Has latest begin timestamp is used to indicate the latest possible starting time of an uncertain time interval.";
  rdfs:label "has latest begin timestamp" .

sem:hasLatestEndTimeStamp rdfs:comment "Has latest end timestamp is used to indicate the latest possible ending time of an uncertain time interval.";
  rdfs:label "has latest end timestamp" .

time:day rdfs:comment """Day position in a calendar-clock system.

The range of this property is not specified, so can be replaced by any specific representation of a calendar day from any calendar. """@en,
    "Posicin de da en un sistema calendario-reloj."@es;
  rdfs:label "day"@en, "da"@es .

time:dayOfYear rdfs:comment "El nmero de da en el ao."@es, "The number of the day within the year"@en;
  rdfs:label "day of year"@en, "da del ao"@es .

time:days rdfs:comment "Longitud de, o elemento de la longitud de, una extensin temporal expresada en das."@es,
    "length of, or element of the length of, a temporal extent expressed in days"@en;
  rdfs:label "days duration"@en, "duracin en das"@es .

time:hasXSDDuration rdfs:comment "Extensin de una entidad temporal, expresada utilizando xsd:duration."@es,
    "Extent of a temporal entity, expressed using xsd:duration"@en;
  rdfs:label "has XSD duration"@en, "tiene duracin XSD"@es .

time:hour rdfs:comment "Hour position in a calendar-clock system."@en, "Posicin de hora en un sistema calendario-reloj."@es;
  rdfs:label "hora"@es, "hour"@en .

time:hours rdfs:comment "Longitud de, o elemento de la longitud de, una extensin temporal expresada en horas."@es,
    "length of, or element of the length of, a temporal extent expressed in hours"@en;
  rdfs:label "duracin en horas"@es, "hours duration"@en .

time:inXSDDate rdfs:comment "Posicin de un instante, expresado utilizando xsd:date."@es,
    "Position of an instant, expressed using xsd:date"@en;
  rdfs:label "en fecha XSD"@es, "in XSD date"@en .

time:inXSDDateTime rdfs:comment "Posicin de un instante, expresado utilizando xsd:dateTime."@es,
    "Position of an instant, expressed using xsd:dateTime"@en;
  rdfs:label "en fecha-tiempo XSD"@es, "in XSD Date-Time"@en .

time:inXSDDateTimeStamp rdfs:comment "Posicin de un instante, expresado utilizando xsd:dateTimeStamp."@es,
    "Position of an instant, expressed using xsd:dateTimeStamp"@en;
  rdfs:label "en fecha-sello de tiempo XSD"@es, "in XSD Date-Time-Stamp"@en .

time:inXSDgYear rdfs:comment "Posicin de un instante, expresado utilizando xsd:gYear."@es,
    "Position of an instant, expressed using xsd:gYear"@en;
  rdfs:label "en ao gregoriano XSD"@es, "in XSD g-Year"@en .

time:inXSDgYearMonth rdfs:comment "Posicin de un instante, expresado utilizando xsd:gYearMonth."@es,
    "Position of an instant, expressed using xsd:gYearMonth"@en;
  rdfs:label "en ao-mes gregoriano XSD"@es, "in XSD g-YearMonth"@en .

time:minute rdfs:comment "Minute position in a calendar-clock system."@en, "Posicin de minuto en un sistema calendario-reloj."@es;
  rdfs:label "minute"@en, "minuto"@es .

time:minutes rdfs:comment "Longitud de, o elemento de la longitud de, una extensin temporal expresada en minutos."@es,
    "length, or element of, a temporal extent expressed in minutes"@en;
  rdfs:label "minutes"@en, "minutos"@es .

time:month rdfs:comment """Month position in a calendar-clock system.

The range of this property is not specified, so can be replaced by any specific representation of a calendar month from any calendar. """@en,
    """Posicin de mes en un sistema calendario-reloj.
    El rango de esta propiedad no est especificado, por tanto, se puede reemplazar por cualquier representacin especfica de un mes de calendario de un calendario cualquiera."""@es;
  rdfs:label "mes"@es, "month"@en .

time:months rdfs:comment "Longitud de, o elemento de la longitud de, una extensin temporal expresada en meses."@es,
    "length of, or element of the length of, a temporal extent expressed in months"@en;
  rdfs:label "duracin en meses"@es, "months duration"@en .

time:nominalPosition rdfs:comment "El valor (nominal) que indica posicin temporal en un sistema de referencia ordinal."@es,
    "The (nominal) value indicating temporal position in an ordinal reference system "@en;
  rdfs:label "Name of temporal position"@en, "nombre de posicin temporal"@es .

time:numericDuration rdfs:comment "Valor de una extensin temporal expresada como un nmero decimal escalado por una unidad de tiempo."@es,
    "Value of a temporal extent expressed as a decimal number scaled by a temporal unit"@en;
  rdfs:label "Numeric value of temporal duration"@en, "valor numrico de duracin temporal"@es .

time:numericPosition rdfs:comment "El valor (numrico) que indica posicin temporal en un sistema de referencia ordinal."@es,
    "The (numeric) value indicating position within a temporal coordinate system "@en;
  rdfs:label "Numeric value of temporal position"@en, "valor numrico de posicin temporal"@es .

time:second rdfs:comment "Posicin de segundo en un sistema calendario-reloj."@es,
    "Second position in a calendar-clock system."@en;
  rdfs:label "second"@en, "segundo"@es .

time:seconds rdfs:comment "Longitud de, o elemento de la longitud de, una extensin temporal expresada en segundos."@es,
    "length of, or element of the length of, a temporal extent expressed in seconds"@en;
  rdfs:label "duracin en segundos"@es, "seconds duration"@en;
  rdfs:seeAlso <http://www.bipm.org/en/publications/si-brochure/second.html> .

time:week rdfs:comment "Nmero de semana en el ao."@es, "Week number within the year."@en;
  rdfs:label "semana"@es, "week"@en .

time:weeks rdfs:comment "Longitud de, o elemento de la longitud de, una extensin temporal expresada en semanas."@es,
    "length of, or element of the length of, a temporal extent expressed in weeks"@en;
  rdfs:label "duracin en semanas"@es, "weeks duration"@en .

time:xsdDateTime rdfs:comment "Valor de 'intervalo de fecha-hora' expresado como un valor compacto."@es,
    "Value of DateTimeInterval expressed as a compact value."@en;
  rdfs:label "has XSD date-time"@en, "tiene fecha-hora XSD"@es .

time:year rdfs:comment """Posicin de ao en un sistema calendario-reloj.

l rango de esta propiedad no est especificado, por tanto, se puede reemplazar por cualquier representacin especfica de un ao de calendario de un calendario cualquiera."""@es,
    """Year position in a calendar-clock system.

The range of this property is not specified, so can be replaced by any specific representation of a calendar year from any calendar. """@en;
  rdfs:label "year"@en .

time:years rdfs:comment "Longitud de, o elemento de la longitud de, una extensin temporal expresada en aos."@es,
    "length of, or element of the length of, a temporal extent expressed in years"@en;
  rdfs:label "duracin en aos"@es, "years duration"@en .

sem:Core rdfs:comment "The SEM Core class contains all entities that make up the context of an event: Events, Actors, Places, Times. This class is meant to be extended for each application domain.";
  rdfs:label "Core" .

sem:Constraint rdfs:comment "The SEM Constraint class contains instances of properties that have a constrained (i.e. not universal) validity. This includes time dependent validity (Temporary), validity in the guise of a specific role (Role), or validity according to a given Authority (View).";
  rdfs:label "Constraint" .

sem:Object rdfs:comment "Objects are passive, inanimate Actors.";
  rdfs:label "Object" .

sem:Temporary rdfs:comment "Temporaries are properties that only hold during a certain Time, which is either indicated with the sem:hasTime property to an instance of sem:Time, or with the sem:hasTimeStamp property to some timestamp(s).";
  rdfs:label "Temporary" .

time:DateTimeDescription rdfs:comment "Descripcin de fecha y tiempo estructurada con valores separados para los diferentes elementos de un sistema calendario-reloj. El sistema de referencia temporal est fijado al calendario gregoriano, y el rango de las propiedades ao, mes, da restringidas a los correspondientes tipos del XML Schema xsd:gYear, xsd:gMonth y xsd:gDay respectivamente."@es,
    "Description of date and time structured with separate values for the various elements of a calendar-clock system. The temporal reference system is fixed to Gregorian Calendar, and the range of year, month, day properties restricted to corresponding XML Schema types xsd:gYear, xsd:gMonth and xsd:gDay, respectively."@en;
  rdfs:label "Date-Time description"@en, "descripcin de fecha-tiempo"@es .

time:DurationDescription rdfs:comment "Descripcin de extensin temporal estructurada con valores separados para los distintos elementos de un sistema de horario-calendario. El sistema de referencia temporal se fija al calendario gregoriano, y el intervalo de cada una de las propiedades numricas se restringe a xsd:decimal."@es,
    "Description of temporal extent structured with separate values for the various elements of a calendar-clock system. The temporal reference system is fixed to Gregorian Calendar, and the range of each of the numeric properties is restricted to xsd:decimal"@en;
  rdfs:label "Duration description"@en, "descripcin de duracin"@es .

time:Year rdfs:comment "Year duration";
  rdfs:label "Year"@en;
  <http://www.w3.org/2004/02/skos/core#historyNote> """Year was proposed in the 2006 version of OWL-Time as an example of how DurationDescription could be specialized to allow for a duration to be restricted to a number of years. 

It is deprecated in this edition of OWL-Time. """ .

rdfs:seeAlso rdfs:label "other version of event" .

<http://127.0.0.1:3333/> rdfs:label "OWL-Time"@en, "Tiempo en OWL"@es;
  rdfs:seeAlso <http://www.w3.org/TR/owl-time>, <http://www.opengis.net/doc/IS/geosparql/1.1>,
    <http://dx.doi.org/10.3233/SW-150187>, <http://www.semantic-web-journal.net/content/time-ontology-extended-non-gregorian-calendar-applications>;
  owl:versionIRI :1.0.0;
  owl:imports <http://www.opengis.net/ont/geosparql/1.1>, time:2016;
  <http://purl.org/dc/terms/contributor> <https://orcid.org/0000-0001-8269-8171>, <mailto:chris.little@metoffice.gov.uk>,
    _:node1, _:node2, _:node3, _:node4, _:node5, _:node6, _:node7, _:node8;
  <http://purl.org/dc/terms/created> "2020-09-09"^^xsd:date;
  <http://purl.org/dc/terms/creator> <http://orcid.org/0000-0002-3884-3420>, <https://en.wikipedia.org/wiki/Jerry_Hobbs>,
    <mailto:panfeng66@gmail.com>, "OGC GeoSPARQL Standards Working Group";
  <http://purl.org/dc/terms/description> "An RDF/OWL vocabulary for representing spatial information"@en;
  <http://purl.org/dc/terms/isVersionOf> <http://www.w3.org/TR/owl-time>;
  <http://purl.org/dc/terms/license> <https://creativecommons.org/licenses/by/4.0/>,
    "https://www.ogc.org/license"^^xsd:anyURI;
  <http://purl.org/dc/terms/modified> "2021-10-27"^^xsd:date, "2024-02-29"^^xsd:date;
  <http://purl.org/dc/terms/publisher> _:node9;
  <http://purl.org/dc/terms/replaces> <http://www.opengis.net/ont/geosparql/1.0>;
  <http://purl.org/dc/terms/rights> "Copyright  2006-2021 W3C, OGC. W3C and OGC liability, trademark and document use rules apply."@en,
    "(c) 2021 Open Geospatial Consortium";
  <http://purl.org/dc/terms/source> <http://www.opengis.net/doc/IS/geosparql/1.1>, "OGC GeoSPARQL - A Geographic Query Language for RDF Data OGC 11-052r5"@en;
  <http://purl.org/dc/terms/title> "GeoSPARQL Ontology";
  <http://purl.org/vocab/vann/preferredNamespacePrefix> "geo";
  <http://purl.org/vocab/vann/preferredNamespaceUri> "http://www.opengis.net/ont/geosparql#"^^xsd:anyURI;
  owl:priorVersion time:2006;
  owl:versionInfo "OGC GeoSPARQL 1.1";
  <http://www.w3.org/2004/02/skos/core#changeNote> "2016-06-15 - initial update of OWL-Time - modified to support arbitrary temporal reference systems. ",
    "2016-12-20 - adjust range of time:timeZone to time:TimeZone, moved up from the tzont ontology.  ",
    "2016-12-20 - restore time:Year and time:January which were present in the 2006 version of the ontology, but now marked \"deprecated\". ",
    "2017-02 - intervalIn, intervalDisjoint, monthOfYear added; TemporalUnit subclass of TemporalDuration",
    "2017-04-06 - hasTime, hasXSDDuration added; Number removed; all duration elements changed to xsd:decimal",
    "2021-01-27 - clarified definition and label for time:after and time:before", "2024-02-29 - Fixed datatype on all cardinality restrictions";
  <http://www.w3.org/2004/02/skos/core#historyNote> """Update of OWL-Time ontology, extended to support general temporal reference systems. 

Ontology engineering by Simon J D Cox"""@en .

xsd:dateTimeStamp rdfs:label "sello de tiempo"@es .

time:generalDay rdfs:label "Da generalizado"@es, "Generalized day"@en .

time:generalMonth rdfs:label "Generalized month"@en, "Mes generalizado"@es .

time:generalYear rdfs:label "Ao generalizado"@es, "Generalized year"@en .

:hasChild rdfs:label "child" .

:hasParent rdfs:label "parent" .

sem:Actor rdfs:label "Actor" .

:hasLocation rdfs:label "location" .

:isLocationOf rdfs:label "is location of" .

sem:Event rdfs:label "Event" .

geo:Feature rdfs:label "Feature";
  rdfs:isDefinedBy <http://www.opengis.net/ont/geosparql#>, <http://www.opengis.net/spec/geosparql/1.0/req/core/feature-class>,
    <http://www.opengis.net/spec/geosparql/1.1/req/core/feature-class> .

foaf:Person rdfs:label "Person" .

:hasRelative rdfs:label "relative" .

:isActorOf rdfs:label "is actor of" .

sem:hasActor rdfs:label "has Actor" .

:rootEvent rdfs:label "mainstream view of event" .

sem:View rdfs:label "View" .

sem:accordingTo rdfs:label "according to" .

sem:Authority rdfs:label "Authority" .

sem:actorType rdfs:label "has actor type" .

sem:type rdfs:label "type property" .

sem:ActorType rdfs:label "Actor type" .

sem:eventProperty rdfs:label "event property" .

sem:eventType rdfs:label "has event type" .

sem:EventType rdfs:label "Event type" .

sem:hasPlace rdfs:label "has Place" .

sem:Place rdfs:label "Place" .

sem:hasSubEvent rdfs:label "has subevent" .

sem:subEventOf rdfs:label "subevent of" .

sem:hasSubType rdfs:label "has subtype" .

sem:subTypeOf rdfs:label "subtype of" .

sem:Type rdfs:label "Type" .

sem:hasTime rdfs:label "has Time" .

sem:Time rdfs:label "Time" .

time:TemporalEntity rdfs:label "Temporal entity"@en, "entidad temporal"@es .

sem:placeType rdfs:label "has place type" .

sem:PlaceType rdfs:label "Place type" .

sem:roleType rdfs:label "has role type" .

sem:Role rdfs:label "Role" .

sem:RoleType rdfs:label "Role type" .

sem:timeType rdfs:label "has time type" .

sem:TimeType rdfs:label "Time type" .

time:after rdfs:label "despus"@es, "is after"@en .

time:before rdfs:label "antes"@es, "is before"@en .

time:dayOfWeek rdfs:label "day of week"@en, "da de la semana"@es .

time:GeneralDateTimeDescription rdfs:label "Generalized date-time description"@en,
    "descripcin de fecha-hora generalizada"@es .

time:DayOfWeek rdfs:label "da de la semana"@es, "Day of week"@en;
  <http://www.w3.org/2004/02/skos/core#changeNote> """Remove enumeration from definition, in order to allow other days to be used when required in other calendars. 
NOTE: existing days are still present as members of the class, but the class membership is now open. 

In the original OWL-Time the following constraint appeared: 
  owl:oneOf (
      time:Monday
      time:Tuesday
      time:Wednesday
      time:Thursday
      time:Friday
      time:Saturday
      time:Sunday
    ) ;"""@en .

time:hasBeginning rdfs:label "has beginning"@en, "tiene principio"@es .

time:hasTime rdfs:label "has time"@en, "tiene tiempo"@es .

time:Instant rdfs:label "Time instant"@en, "instante de tiempo."@es .

time:hasDateTimeDescription rdfs:label "has Date-Time description"@en, "tiene descripcin fecha-hora"@es .

time:DateTimeInterval rdfs:label "Date-time interval"@en, "intervalo de fecha-hora"@es .

time:hasDuration rdfs:label "has duration"@en, "tiene duracin"@es .

time:hasTemporalDuration rdfs:label "has temporal duration"@en, "tiene duracin temporal"@es .

time:Duration rdfs:label "Time duration"@en, "duracin de tiempo" .

time:hasDurationDescription rdfs:label "has duration description"@en, "tiene descripcin de duracin"@es .

time:GeneralDurationDescription rdfs:label "Generalized duration description"@en,
    "descripcin de duracin generalizada"@es .

time:hasEnd rdfs:label "has end"@en, "tiene fin"@es .

time:hasTRS rdfs:label "Temporal reference system used"@en, "sistema de referencia temporal utilizado"@es .

time:TemporalPosition rdfs:label "Temporal position"@en, "posicin temporal"@es .

time:TRS rdfs:label "Temporal Reference System"@en, "sistema de referencia temporal"@es .

time:TemporalDuration rdfs:label "Temporal duration"@en, "duracin temporal"@es .

time:inDateTime rdfs:label "en descripcin de fecha-hora"@es, "in date-time description"@en .

time:inTemporalPosition rdfs:label "Temporal position"@en, "posicin temporal"@es .

time:inTimePosition rdfs:label "Time position"@en, "posicin de tiempo"@es .

time:TimePosition rdfs:label "Time position"@en, "posicin de tiempo"@es .

time:inside rdfs:label "has time instant inside"@en, "tiene instante de tiempo dentro"@es .

time:Interval rdfs:label "Time interval"@en, "intervalo de tiempo"@es .

time:intervalAfter rdfs:label "interval after"@en, "intervalo posterior"@es .

time:intervalDisjoint rdfs:label "interval disjoint"@en, "intervalo disjunto"@es .

time:intervalBefore rdfs:label "interval before"@en, "intervalo anterior"@es .

time:January rdfs:label "January";
  <http://www.w3.org/2004/02/skos/core#historyNote> "This class was present in the 2006 version of OWL-Time. It was presented as an example of how DateTimeDescription could be specialized, but does not belong in the revised ontology. " .

time:unitMonth rdfs:label "Month (unit of temporal duration)"@en .

time:Friday rdfs:label "Friday"@en .

time:Monday rdfs:label "Monday"@en .

time:Saturday rdfs:label "Saturday"@en .

time:Sunday rdfs:label "Sunday"@en .

time:Thursday rdfs:label "Thursday"@en .

time:Tuesday rdfs:label "Tuesday"@en .

time:Wednesday rdfs:label "Wednesday"@en .

time:unitCentury rdfs:label "Century (unit of temporal duration)"@en .

time:unitDay rdfs:label "Day (unit of temporal duration)"@en .

time:unitDecade rdfs:label "Decade (unit of temporal duration)"@en .

time:unitHour rdfs:label "Hour (unit of temporal duration)"@en .

time:unitMillenium rdfs:label "Century (unit of temporal duration)"@en .

time:unitMinute rdfs:label "Minute (unit of temporal duration)"@en .

time:unitSecond rdfs:label "Second (unit of temporal duration)"@en .

time:unitWeek rdfs:label "Week (unit of temporal duration)"@en .

time:unitYear rdfs:label "Year (unit of temporal duration)"@en .

:PerangTakhtaJawaKedua rdfs:label "Perang Takhta Jawa Kedua";
  rdfs:seeAlso "wikipediaPerangTakhtaJawaKedua" .

:wikipediaBandungLautanApi rdfs:label "wikipedia Bandung Lautan Api";
  :image "File:Bandung Lautan Api.jpg" .

:RevolusiNasionalIndonesia rdfs:label "Revolusi Nasional Indonesia";
  rdfs:seeAlso "wikipediaRevolusiNasionalIndonesia", :wikipediaRevolusiNasionalIndonesia .

:PerangDiponegoro rdfs:label "Perang Diponegoro";
  rdfs:seeAlso "wikipediaPerangDiponegoro" .

:wikipediaPerangBelandaPortugal rdfs:label "wikipedia Perang Belanda-Portugal" .

:PerangJawa17411743 rdfs:label "Perang Jawa (17411743)";
  rdfs:seeAlso "wikipediaPerangJawa17411743" .

:PerangTakhtaJawaPertama rdfs:label "Perang Takhta Jawa Pertama";
  rdfs:seeAlso "wikipediaPerangTakhtaJawaPertama" .

:wikipediaPeperanganeraNapoleon rdfs:label "wikipedia Peperangan era Napoleon" .

:PerangBubat rdfs:label "Perang Bubat";
  rdfs:seeAlso "wikipediaPerangBubat" .

:wikipediaPemberontakanDITIIdiAceh rdfs:label "wikipedia Pemberontakan DI/TII di Aceh" .

:wikipediaKampanyeKalimantan1945 rdfs:label "wikipedia Kampanye Kalimantan (1945)" .

:wikipediaPerangPasifik rdfs:label "wikipedia Perang Pasifik" .

:wikipediaPertempuranBojongKokosan rdfs:label "wikipedia Pertempuran Bojong Kokosan" .

:PerangRegreg rdfs:label "Perang Regreg";
  rdfs:seeAlso "wikipediaPerangRegreg" .

:KampanyeHindiaBelanda rdfs:label "Kampanye Hindia Belanda";
  rdfs:seeAlso "wikipediaKampanyeHindiaBelanda", :wikipediaKampanyeHindiaBelanda .

:wikipediaRevolusiNasionalIndonesia rdfs:label "wikipedia Revolusi Nasional Indonesia" .

:PertempuranBojongKokosan rdfs:label "Pertempuran Bojong Kokosan";
  rdfs:seeAlso :wikipediaPertempuranBojongKokosan, "wikipediaPertempuranBojongKokosan" .

:DelapanJamPertempurandiMangkang rdfs:label "Delapan Jam Pertempuran di Mangkang";
  rdfs:seeAlso "wikipediaDelapanJamPertempurandiMangkang", :wikipediaDelapanJamPertempurandiMangkang .

:wikipediaPerangAceh rdfs:label "wikipedia Perang Aceh" .

:wikipediaInvasiCholakeSriwijaya rdfs:label "wikipedia Invasi Chola ke Sriwijaya" .

:PerangBayu rdfs:label "Perang Bayu";
  rdfs:seeAlso "wikipediaPerangBayu" .

:PerangBelasting rdfs:label "Perang Belasting";
  rdfs:seeAlso "wikipediaPerangBelasting" .

:PeristiwaTigaMaret rdfs:label "Peristiwa Tiga Maret";
  rdfs:seeAlso "wikipediaPeristiwaTigaMaret", :wikipediaPeristiwaTigaMaret .

:IntervensiBelandadiBali1858 rdfs:label "Intervensi Belanda di Bali (1858)";
  rdfs:seeAlso "wikipediaIntervensiBelandadiBali1858" .

:Operasi17Agustus rdfs:label "Operasi 17 Agustus";
  rdfs:seeAlso "wikipediaOperasi17Agustus", :wikipediaOperasi17Agustus .

:wikipediaPerangBelasting rdfs:label "wikipedia Perang Belasting" .

:BandungLautanApi rdfs:label "Bandung Lautan Api";
  rdfs:seeAlso :wikipediaBandungLautanApi, "wikipediaBandungLautanApi" .

:Gerakan30September rdfs:label "Gerakan 30 September";
  rdfs:seeAlso "wikipediaGerakan30September", :wikipediaGerakan30September .

:wikipediaPerangKuning rdfs:label "wikipedia Perang Kuning" .

:wikipediaPerangPadri rdfs:label "wikipedia Perang Padri" .

:wikipediaPerangCumbok rdfs:label "wikipedia Perang Cumbok" .

:wikipediaPerangJawa17411743 rdfs:label "wikipedia Perang Jawa (17411743)" .

:wikipediaPerangTakhtaJawaKetiga rdfs:label "wikipedia Perang Takhta Jawa Ketiga" .

:wikipediaSeranganUmum1Maret1949 rdfs:label "wikipedia Serangan Umum 1 Maret 1949" .

:KonflikPapua rdfs:label "Konflik Papua";
  rdfs:seeAlso "wikipediaKonflikPapua", :wikipediaKonflikPapua .

:InvasiMaluku rdfs:label "Invasi Maluku";
  rdfs:seeAlso "wikipediaInvasiMaluku" .

:wikipediaPerangTakhtaJawaKedua rdfs:label "wikipedia Perang Takhta Jawa Kedua" .

:wikipediaIntervensiBelandadiBali1858 rdfs:label "wikipedia Intervensi Belanda di Bali (1858)" .

:GegerSepehi rdfs:label "Geger Sepehi";
  rdfs:seeAlso "wikipediaGegerSepehi" .

:PerangDayakDesa rdfs:label "Perang Dayak Desa";
  rdfs:seeAlso "wikipediaPerangDayakDesa", :wikipediaPerangDayakDesa .

:wikipediaKonflikPapua rdfs:label "wikipedia Konflik Papua" .

:wikipediaPeristiwaTigaMaret rdfs:label "wikipedia Peristiwa Tiga Maret" .

:wikipediaPenyerbuanKotabaruYogyakarta rdfs:label "wikipedia Penyerbuan Kotabaru Yogyakarta" .

:IntervensiBelandadiBali1908 rdfs:label "Intervensi Belanda di Bali (1908)";
  rdfs:seeAlso "wikipediaIntervensiBelandadiBali1908" .

:wikipediaPerangBayu rdfs:label "wikipedia Perang Bayu" .

:wikipediaPerangRegreg rdfs:label "wikipedia Perang Regreg" .

:wikipediaPerangBubat rdfs:label "wikipedia Perang Bubat" .

:wikipediaPerangDayakDesa rdfs:label "wikipedia Perang Dayak Desa" .

:KampanyeKalimantan1945 rdfs:label "Kampanye Kalimantan (1945)";
  rdfs:seeAlso :wikipediaKampanyeKalimantan1945, "wikipediaKampanyeKalimantan1945" .

:PenyerbuanMeesterCornelis rdfs:label "Penyerbuan Meester Cornelis";
  rdfs:seeAlso "wikipediaPenyerbuanMeesterCornelis" .

:SeranganUmum1Maret1949 rdfs:label "Serangan Umum 1 Maret 1949";
  rdfs:seeAlso :wikipediaSeranganUmum1Maret1949, "wikipediaSeranganUmum1Maret1949" .

:PertempuranLengkong rdfs:label "Pertempuran Lengkong";
  rdfs:seeAlso "wikipediaPertempuranLengkong", :wikipediaPertempuranLengkong .

:wikipediaGerakan30September rdfs:label "wikipedia Gerakan 30 September" .

:wikipediaKampanyeHindiaBelanda rdfs:label "wikipedia Kampanye Hindia Belanda" .

:Peristiwa19November rdfs:label "Peristiwa 19 November";
  rdfs:seeAlso "wikipediaPeristiwa19November", :wikipediaPeristiwa19November .

:wikipediaPertempuranLengkong rdfs:label "wikipedia Pertempuran Lengkong" .

:InvasiCholakeSriwijaya rdfs:label "Invasi Chola ke Sriwijaya";
  rdfs:seeAlso "wikipediaInvasiCholakeSriwijaya" .

:wikipediaPertempuranMelaka1641 rdfs:label "wikipedia Pertempuran Melaka (1641)" .

:wikipediaPertempuranMedanArea rdfs:label "wikipedia Pertempuran Medan Area" .

:PerangPadri rdfs:label "Perang Padri";
  rdfs:seeAlso "wikipediaPerangPadri" .

:PerangBelandaPortugal rdfs:label "Perang Belanda-Portugal";
  rdfs:seeAlso "wikipediaPerangBelandaPortugal" .

:wikipediaPertempuranKumai rdfs:label "wikipedia Pertempuran Kumai" .

:PeperanganeraNapoleon rdfs:label "Peperangan era Napoleon";
  rdfs:seeAlso "wikipediaPeperanganeraNapoleon" .

:wikipediaSeranganUmumSurakarta rdfs:label "wikipedia Serangan Umum Surakarta" .

:PertempuranLimaHari rdfs:label "Pertempuran Lima Hari";
  rdfs:seeAlso "wikipediaPertempuranLimaHari", :wikipediaPertempuranLimaHari .

:wikipediaPenyerbuanMeesterCornelis rdfs:label "wikipedia Penyerbuan Meester Cornelis" .

:wikipediaPuputanMargarana rdfs:label "wikipedia Puputan Margarana" .

:wikipediaPertempuranLimaHari rdfs:label "wikipedia Pertempuran Lima Hari" .

:PertempuranSurabaya rdfs:label "Pertempuran Surabaya";
  rdfs:seeAlso "wikipediaPertempuranSurabaya", :wikipediaPertempuranSurabaya .

:wikipediaIntervensiBelandadiBali1908 rdfs:label "wikipedia Intervensi Belanda di Bali (1908)" .

:PertempuranMedanArea rdfs:label "Pertempuran Medan Area";
  rdfs:seeAlso :wikipediaPertempuranMedanArea, "wikipediaPertempuranMedanArea" .

:wikipediaPertempuranSurabaya rdfs:label "wikipedia Pertempuran Surabaya" .

:wikipediaInvasiMaluku rdfs:label "wikipedia Invasi Maluku" .

:wikipediaPerangDiponegoro rdfs:label "wikipedia Perang Diponegoro" .

:PerangTakhtaJawaKetiga rdfs:label "Perang Takhta Jawa Ketiga";
  rdfs:seeAlso "wikipediaPerangTakhtaJawaKetiga" .

:wikipediaEkspedisiPalembangII rdfs:label "wikipedia Ekspedisi Palembang II" .

:wikipediaSerbuanYuanMongolkeJawa rdfs:label "wikipedia Serbuan Yuan-Mongol ke Jawa" .

:wikipediaDelapanJamPertempurandiMangkang rdfs:label "wikipedia Delapan Jam Pertempuran di Mangkang" .

:wikipediaPemberontakanRadenRonggo rdfs:label "wikipedia Pemberontakan Raden Ronggo" .

:wikipediaPeristiwa19November rdfs:label "wikipedia Peristiwa 19 November" .

:SerbuanYuanMongolkeJawa rdfs:label "Serbuan Yuan-Mongol ke Jawa";
  rdfs:seeAlso "wikipediaSerbuanYuanMongolkeJawa" .

:PemberontakanRadenRonggo rdfs:label "Pemberontakan Raden Ronggo";
  rdfs:seeAlso "wikipediaPemberontakanRadenRonggo" .

:PemberontakanDITIIdiAceh rdfs:label "Pemberontakan DI/TII di Aceh";
  rdfs:seeAlso :wikipediaPemberontakanDITIIdiAceh, "wikipediaPemberontakanDITIIdiAceh" .

:EkspedisiPalembangII rdfs:label "Ekspedisi Palembang II";
  rdfs:seeAlso "wikipediaEkspedisiPalembangII" .

:PerangAceh rdfs:label "Perang Aceh";
  rdfs:seeAlso "wikipediaPerangAceh" .

:wikipediaGegerSepehi rdfs:label "wikipedia Geger Sepehi" .

:PertempuranKumai rdfs:label "Pertempuran Kumai";
  rdfs:seeAlso :wikipediaPertempuranKumai, "wikipediaPertempuranKumai" .

:PerangPasifik rdfs:label "Perang Pasifik";
  rdfs:seeAlso "wikipediaPerangPasifik" .

:PerangKuning rdfs:label "Perang Kuning";
  rdfs:seeAlso "wikipediaPerangKuning" .

:PenyerbuanKotabaruYogyakarta rdfs:label "Penyerbuan Kotabaru Yogyakarta";
  rdfs:seeAlso :wikipediaPenyerbuanKotabaruYogyakarta, "wikipediaPenyerbuanKotabaruYogyakarta" .

:PuputanMargarana rdfs:label "Puputan Margarana";
  rdfs:seeAlso :wikipediaPuputanMargarana, "wikipediaPuputanMargarana" .

:PertempuranMelaka1641 rdfs:label "Pertempuran Melaka (1641)";
  rdfs:seeAlso "wikipediaPertempuranMelaka1641" .

:PerangCumbok rdfs:label "Perang Cumbok";
  rdfs:seeAlso :wikipediaPerangCumbok, "wikipediaPerangCumbok" .

:wikipediaPerangTakhtaJawaPertama rdfs:label "wikipedia Perang Takhta Jawa Pertama" .

:wikipediaOperasi17Agustus rdfs:label "wikipedia Operasi 17 Agustus" .

:SeranganUmumSurakarta rdfs:label "Serangan Umum Surakarta";
  rdfs:seeAlso :wikipediaSeranganUmumSurakarta, "wikipediaSeranganUmumSurakarta" .

:JisaburoOzawa rdfs:label "Jisaburo Ozawa" .

:MuhammadMangundiprojo rdfs:label "Muhammad Mangundiprojo" .

:Soengkono rdfs:label "Soengkono" .

:HarioJonosewojo rdfs:label "Hario Jonosewojo" .

:MoehammadJasin rdfs:label "Moehammad Jasin" .

:Moestopo rdfs:label "Moestopo" .

:RobertMansergh rdfs:label "Robert Mansergh" .

:AubertinMallaby rdfs:label "Aubertin Mallaby" .

:Sutomo rdfs:label "Sutomo" .

:GoliathTabuni rdfs:label "Goliath Tabuni" .

:Soekarno rdfs:label "Soekarno" .

:KiyotakeKawaguchi rdfs:label "Kiyotake Kawaguchi" .

:RaymondWesterling rdfs:label "Raymond Westerling" .

:MathiasWenda rdfs:label "Mathias Wenda" .

:JuliusTahija rdfs:label "Julius Tahija" .

:InfanteriBelanda rdfs:label "Infanteri Belanda" .

:Moekijat rdfs:label "Moekijat" .

:MohammadHatta rdfs:label "Mohammad Hatta" .

:DouglasMacArthur rdfs:label "Douglas MacArthur" .

:ListyoSigitPrabowo rdfs:label "Listyo Sigit Prabowo" .

:REMartadinata rdfs:label "R. E. Martadinata" .

:TeukuKeumanganUmar rdfs:label "Teuku Keumangan Umar" .

:NobutakeKond rdfs:label "Nobutake Kond" .

:SutanSjahrir rdfs:label "Sutan Sjahrir" .

:SlametRijadi rdfs:label "Slamet Rijadi" .

:TEDKelly rdfs:label "T.E.D. Kelly" .

:AgusSubiyanto rdfs:label "Agus Subiyanto" .

:Assaat rdfs:label "Assaat" .

:PangRati rdfs:label "Pang Rati" .

:MacDonald rdfs:label "MacDonald" .

:MuhammadToha rdfs:label "Muhammad Toha" .

:AbdulHarisNasution rdfs:label "Abdul Haris Nasution" .

:KidoShinichir rdfs:label "Kido Shinichir" .

:PrabowoSubianto rdfs:label "Prabowo Subianto" .

:EgianusKogoya rdfs:label "Egianus Kogoya" .

:BudiGunawan rdfs:label "Budi Gunawan" .

:JaminGinting rdfs:label "Jamin Ginting" .

:AbdulKarimMS rdfs:label "Abdul Karim M.S" .

:AchmadTahir rdfs:label "Achmad Tahir" .

:HubertusJohannesvanMook rdfs:label "Hubertus Johannes van Mook" .

:TeungkuHasanKruengKalee rdfs:label "Teungku Hasan Krueng Kalee" .

:TeukuDaudCumbok rdfs:label "Teuku Daud Cumbok" .

:TeukuNyakArif rdfs:label "Teuku Nyak Arif" .

:TeungkuAhmadHasballah rdfs:label "Teungku Ahmad Hasballah" .

:SyamaunGaharu rdfs:label "Syamaun Gaharu" .

:DaudBeureueh rdfs:label "Daud Beureu'eh" .

:MichiakiKamada rdfs:label "Michiaki Kamada" .

:ThomasKinkaid rdfs:label "Thomas Kinkaid" .

:HeinterPoorten rdfs:label "Hein ter Poorten" .

:JBTKnig rdfs:label "J.B.T Knig" .

:FMollinger rdfs:label "F. Mollinger" .

:IGustiNgurahRai rdfs:label "I Gusti Ngurah Rai" .

:SimonSpoor rdfs:label "Simon Spoor" .

:BabaMasao rdfs:label "Baba Masao" .

:SyafruddinPrawiranegara rdfs:label "Syafruddin Prawiranegara" .

:MaludinSimbolon rdfs:label "Maludin Simbolon" .

:AhmadYani rdfs:label "Ahmad Yani" .

:AhmadHusein rdfs:label "Ahmad Husein" .

:HitoshiImamura rdfs:label "Hitoshi Imamura" .

:AJFDoulton rdfs:label "AJF Doulton" .

:EdiSukardi rdfs:label "Edi Sukardi" .

:Musso rdfs:label "Musso" .

:TanMalaka rdfs:label "Tan Malaka" .

:HisaichiTerauchi rdfs:label "Hisaichi Terauchi" .

:Meyer rdfs:label "Meyer" .

:JoniBotak rdfs:label "Joni Botak" .

:LouisMountbatten rdfs:label "Louis Mountbatten" .

:Djampi rdfs:label "Djampi" .

:PangIyo rdfs:label "Pang Iyo" .

:PangSuma rdfs:label "Pang Suma" .

:Nagatani rdfs:label "Nagatani" .

:DirkCornelisBuurmanvanVreeden rdfs:label "Dirk Cornelis Buurman van Vreeden" .

:SebbySambom rdfs:label "Sebby Sambom" .

:Mollinger rdfs:label "Mollinger" .

:AlidiusTjardavanStarkenborghStachouwer rdfs:label "Alidius Tjarda van Starkenborgh Stachouwer" .

:DaanMogot rdfs:label "Daan Mogot" .

:IbTakahashi rdfs:label "Ib Takahashi" .

:LudolphHendrikvanOyen rdfs:label "Ludolph Hendrik van Oyen" .

:TjokordaGdeRakaSoekawati rdfs:label "Tjokorda Gde Raka Soekawati" .

:Wongsonegoro rdfs:label "Wongsonegoro" .

:Kariadi rdfs:label "Kariadi" .

:GatotSoebroto rdfs:label "Gatot Soebroto" .

:KellyKwalik rdfs:label "Kelly Kwalik" .

:BJHabibie rdfs:label "B. J. Habibie" .

:VanVreeden rdfs:label "Van Vreeden" .

:ThomasCHart rdfs:label "Thomas C. Hart" .

:ShojiNishimura rdfs:label "Shoji Nishimura" .

:Soedirman rdfs:label "Soedirman" .

:TakeoTakagi rdfs:label "Takeo Takagi" .

:DirkReinhardAdelbertvanLangen rdfs:label "Dirk Reinhard Adelbert van Langen" .

:BambangSoegeng rdfs:label "Bambang Soegeng" .

:OeripSoemohardjo rdfs:label "Oerip Soemohardjo" .

:AndikaPerkasa rdfs:label "Andika Perkasa" .

:ConradHelfrich rdfs:label "Conrad Helfrich" .

:ArchibaldWavell1stEarlWavell rdfs:label "Archibald Wavell, 1st Earl Wavell" .

:RichardPeirse rdfs:label "Richard Peirse" .

:KarelDoorman rdfs:label "Karel Doorman" .

:HamengkubuwanaIX rdfs:label "Hamengkubuwana IX" .

:VentjeSumual rdfs:label "Ventje Sumual" .

:JMvdBerge rdfs:label "J.M. v/d Berge" .

:Soeharto rdfs:label "Soeharto" .

:Otzuka rdfs:label "Otzuka" .

:LeslieMorshead rdfs:label "Leslie Morshead" .

:SusiloBambangYudhoyono rdfs:label "Susilo Bambang Yudhoyono" .

:SaalahYusufSutanMangkuto rdfs:label "Saalah Yusuf Sutan Mangkuto" .

:WilhelminadariBelanda rdfs:label "Wilhelmina dari Belanda" .

:LeonardusBenyaminMoerdani rdfs:label "Leonardus Benyamin Moerdani" .

:MarufAmin rdfs:label "Ma'ruf Amin" .

:MegawatiSoekarnoputri rdfs:label "Megawati Soekarnoputri" .

:TBSimatupang rdfs:label "T.B. Simatupang" .

:AdamBB rdfs:label "Adam B.B." .

:Wiranto rdfs:label "Wiranto" .

:LoaSekHie rdfs:label "Loa Sek Hie" .

:SyarifHamidIIdariPontianak rdfs:label "Syarif Hamid II dari Pontianak" .

:PhilipChristison rdfs:label "Philip Christison" .

:BennyWenda rdfs:label "Benny Wenda" .

:AbdulkadirWidjojoatmodjo rdfs:label "Abdulkadir Widjojoatmodjo" .

:JacobPrai rdfs:label "Jacob Prai" .

:AbdulKaharMuzakkar rdfs:label "Abdul Kahar Muzakkar" .

:IsmaelLengah rdfs:label "Ismael Lengah" .

:TrySutrisno rdfs:label "Try Sutrisno" .

:PakubuwanaXII rdfs:label "Pakubuwana XII" .

:MangkunegaraVIII rdfs:label "Mangkunegara VIII" .

:AchmadiHadisoemarto rdfs:label "Achmadi Hadisoemarto" .

:JokoWidodo rdfs:label "Joko Widodo" .

:JacobRumbiak rdfs:label "Jacob Rumbiak" .

:SekarmadjiMaridjanKartosoewirjo rdfs:label "Sekarmadji Maridjan Kartosoewirjo" .

:AmirSjarifoeddin rdfs:label "Amir Sjarifoeddin" .

:AgustinusAdisoetjipto rdfs:label "Agustinus Adisoetjipto" .

:AbdurrahmanWahid rdfs:label "Abdurrahman Wahid" .

:JulianadariBelanda rdfs:label "Juliana dari Belanda" .

:wikipediaPendudukanJepangdiKalimantanBarat rdfs:label "wikipedia Pendudukan Jepang di Kalimantan Barat" .

:wikipediaPersengketaanNuginiBaratdanDekolonisasiOseania rdfs:label "wikipedia Persengketaan Nugini Barat dan Dekolonisasi Oseania" .

:wikipediaPemberontakanDITII rdfs:label "wikipedia Pemberontakan DI/TII" .

:wikipediaPerangKemerdekaanIndonesia rdfs:label "wikipedia Perang Kemerdekaan Indonesia" .

:wikipediaPerangPasifikdariPerangDuniaII rdfs:label "wikipedia Perang Pasifik dari Perang Dunia II" .

:PerangPasifikdariPerangDuniaII rdfs:label "Perang Pasifik dari Perang Dunia II";
  rdfs:seeAlso :wikipediaPerangPasifikdariPerangDuniaII .

:PascaPerangDuniaKedua rdfs:label "Pasca Perang Dunia Kedua";
  rdfs:seeAlso :wikipediaPascaPerangDuniaKedua .

:wikipediaPascaPerangDuniaKedua rdfs:label "wikipedia Pasca Perang Dunia Kedua" .

:wikipediaPerangDuniaII rdfs:label "wikipedia Perang Dunia II" .

:PemberontakanDITII rdfs:label "Pemberontakan DI/TII";
  rdfs:seeAlso :wikipediaPemberontakanDITII .

:PerangDuniaII rdfs:label "Perang Dunia II";
  rdfs:seeAlso :wikipediaPerangDuniaII .

:PerangKemerdekaanIndonesia rdfs:label "Perang Kemerdekaan Indonesia";
  rdfs:seeAlso :wikipediaPerangKemerdekaanIndonesia .

:PersengketaanNuginiBaratdanDekolonisasiOseania rdfs:label "Persengketaan Nugini Barat dan Dekolonisasi Oseania";
  rdfs:seeAlso :wikipediaPersengketaanNuginiBaratdanDekolonisasiOseania .

:PendudukanJepangdiKalimantanBarat rdfs:label "Pendudukan Jepang di Kalimantan Barat";
  rdfs:seeAlso :wikipediaPendudukanJepangdiKalimantanBarat .

:Indonesia rdfs:label "Indonesia" .

:Tuvalu rdfs:label "Tuvalu" .

:Jepang rdfs:label "Jepang" .

:KerajaanBelanda rdfs:label "Kerajaan Belanda" .

:KNIL rdfs:label "KNIL" .

:Belanda rdfs:label "Belanda" .

:KekaisaranJepang rdfs:label "Kekaisaran Jepang" .

:SelandiaBaru rdfs:label "Selandia Baru" .

:TNI rdfs:label "TNI" .

:RepublikIndonesia rdfs:label "Republik Indonesia" .

:India rdfs:label "India" .

:BritaniaRaya rdfs:label "Britania Raya" .

:DesertirTentaraIndia rdfs:label "Desertir Tentara India" .

:SukuDayakDesa rdfs:label "Suku Dayak Desa" .

:AmerikaSerikat rdfs:label "Amerika Serikat" .

:Samoa rdfs:label "Samoa" .

:PapuaNugini rdfs:label "Papua Nugini" .

:Tonga rdfs:label "Tonga" .

:OrganisasiPapuaMerdeka rdfs:label "Organisasi Papua Merdeka" .

:KepulauanSolomon rdfs:label "Kepulauan Solomon" .

:Vanuatu rdfs:label "Vanuatu" .

:Nauru rdfs:label "Nauru" .

:Fiji rdfs:label "Fiji" .

:Australia rdfs:label "Australia" .

:UniSoviet rdfs:label "Uni Soviet" .

:Libya rdfs:label "Libya" .

:Palau rdfs:label "Palau" .

:NegaraIslamIndonesia rdfs:label "Negara Islam Indonesia" .

:KorpsBrigadeMobil rdfs:label "Korps Brigade Mobil" .

:BKR rdfs:label "BKR" .

:PUSA rdfs:label "PUSA" .

:Kaumuleebalang rdfs:label "Kaum uleebalang" .

:TRI rdfs:label "TRI" .

:PDRI rdfs:label "PDRI" .

:KemaharajaanBritania rdfs:label "Kemaharajaan Britania" .

:AngkatanPerangRatuAdil rdfs:label "Angkatan Perang Ratu Adil" .

:BarisanUlama rdfs:label "Barisan Ulama" .

:PaoAnTui rdfs:label "Pao An Tui" .

:ABDACommand rdfs:label "ABDA Command" .

:HindiaBelanda rdfs:label "Hindia Belanda" .

:KesultananPontianak rdfs:label "Kesultanan Pontianak" .

:ImperiumBelanda rdfs:label "Imperium Belanda" .

:PemerintahanSipilHindiaBelanda rdfs:label "Pemerintahan Sipil Hindia Belanda" .

:KekaisaranBritania rdfs:label "Kekaisaran Britania" .

:NICA rdfs:label "NICA" .

:RelawanTentaraKekaisaranJepang rdfs:label "Relawan Tentara Kekaisaran Jepang" .

:PRRI rdfs:label "PRRI" .

:LaskarKalimantan rdfs:label "Laskar Kalimantan" .

:TKR rdfs:label "TKR" .

:MilitanIslam rdfs:label "Militan Islam" .

:TentaraKeamananRakyat rdfs:label "Tentara Keamanan Rakyat" .

geo:asWKT rdfs:isDefinedBy <http://www.opengis.net/ont/geosparql#>, <http://www.opengis.net/spec/geosparql/1.0/req/geometry-extension/geometry-as-wkt-literal>,
    <http://www.opengis.net/spec/geosparql/1.1/req/geometry-extension/geometry-as-wkt-literal> .

geo:asGML rdfs:isDefinedBy <http://www.opengis.net/ont/geosparql#>, <http://www.opengis.net/spec/geosparql/1.0/req/geometry-extension/geometry-as-gml-literal>,
    <http://www.opengis.net/spec/geosparql/1.1/req/geometry-extension/geometry-as-gml-literal> .

geo:hasDefaultGeometry rdfs:isDefinedBy <http://www.opengis.net/ont/geosparql#>, <http://www.opengis.net/spec/geosparql/1.1/req/geometry-extension/feature-properties>,
    <http://www.opengis.net/spec/geosparql/1.0/req/geometry-extension/feature-properties> .

geo:sfEquals rdfs:isDefinedBy <http://www.opengis.net/ont/geosparql#>, <http://www.opengis.net/spec/geosparql/1.0/req/topology-vocab-extension/sf-spatial-relations>,
    <http://www.opengis.net/spec/geosparql/1.1/req/topology-vocab-extension/sf-spatial-relations>;
  rdfs:seeAlso <http://dbpedia.org/resource/DE-9IM> .

geo:sfDisjoint rdfs:isDefinedBy <http://www.opengis.net/ont/geosparql#>, <http://www.opengis.net/spec/geosparql/1.0/req/topology-vocab-extension/sf-spatial-relations>,
    <http://www.opengis.net/spec/geosparql/1.1/req/topology-vocab-extension/sf-spatial-relations>;
  rdfs:seeAlso <http://dbpedia.org/resource/DE-9IM> .

geo:sfIntersects rdfs:isDefinedBy <http://www.opengis.net/ont/geosparql#>, <http://www.opengis.net/spec/geosparql/1.0/req/topology-vocab-extension/sf-spatial-relations>,
    <http://www.opengis.net/spec/geosparql/1.1/req/topology-vocab-extension/sf-spatial-relations>;
  rdfs:seeAlso <http://dbpedia.org/resource/DE-9IM> .

geo:sfTouches rdfs:isDefinedBy <http://www.opengis.net/ont/geosparql#>, <http://www.opengis.net/spec/geosparql/1.0/req/topology-vocab-extension/sf-spatial-relations>,
    <http://www.opengis.net/spec/geosparql/1.1/req/topology-vocab-extension/sf-spatial-relations>;
  rdfs:seeAlso <http://dbpedia.org/resource/DE-9IM> .

geo:sfWithin rdfs:isDefinedBy <http://www.opengis.net/ont/geosparql#>, <http://www.opengis.net/spec/geosparql/1.0/req/topology-vocab-extension/sf-spatial-relations>,
    <http://www.opengis.net/spec/geosparql/1.1/req/topology-vocab-extension/sf-spatial-relations>;
  rdfs:seeAlso <http://dbpedia.org/resource/DE-9IM> .

geo:sfContains rdfs:isDefinedBy <http://www.opengis.net/ont/geosparql#>, <http://www.opengis.net/spec/geosparql/1.0/req/topology-vocab-extension/rcc8-spatial-relations>,
    <http://www.opengis.net/spec/geosparql/1.1/req/topology-vocab-extension/rcc8-spatial-relations>;
  rdfs:seeAlso <http://dbpedia.org/resource/DE-9IM> .

geo:sfOverlaps rdfs:isDefinedBy <http://www.opengis.net/ont/geosparql#>, <http://www.opengis.net/spec/geosparql/1.0/req/topology-vocab-extension/sf-spatial-relations>,
    <http://www.opengis.net/spec/geosparql/1.1/req/topology-vocab-extension/sf-spatial-relations>;
  rdfs:seeAlso <http://dbpedia.org/resource/DE-9IM> .

geo:sfCrosses rdfs:isDefinedBy <http://www.opengis.net/ont/geosparql#>, <http://www.opengis.net/spec/geosparql/1.0/req/topology-vocab-extension/sf-spatial-relations>,
    <http://www.opengis.net/spec/geosparql/1.1/req/topology-vocab-extension/sf-spatial-relations>;
  rdfs:seeAlso <http://dbpedia.org/resource/DE-9IM> .

geo:ehEquals rdfs:isDefinedBy <http://www.opengis.net/ont/geosparql#>, <http://www.opengis.net/spec/geosparql/1.0/req/geometry-extension/eh-spatial-relations>,
    <http://www.opengis.net/spec/geosparql/1.1/req/geometry-extension/eh-spatial-relations>;
  rdfs:seeAlso <http://dbpedia.org/resource/DE-9IM> .

geo:ehDisjoint rdfs:isDefinedBy <http://www.opengis.net/ont/geosparql#>, <http://www.opengis.net/spec/geosparql/1.0/req/geometry-extension/eh-spatial-relations>,
    <http://www.opengis.net/spec/geosparql/1.1/req/geometry-extension/eh-spatial-relations>;
  rdfs:seeAlso <http://dbpedia.org/resource/DE-9IM> .

geo:ehMeet rdfs:isDefinedBy <http://www.opengis.net/ont/geosparql#>, <http://www.opengis.net/spec/geosparql/1.0/req/geometry-extension/eh-spatial-relations>,
    <http://www.opengis.net/spec/geosparql/1.1/req/geometry-extension/eh-spatial-relations>;
  rdfs:seeAlso <http://dbpedia.org/resource/DE-9IM> .

geo:ehOverlap rdfs:isDefinedBy <http://www.opengis.net/ont/geosparql#>, <http://www.opengis.net/spec/geosparql/1.0/req/geometry-extension/eh-spatial-relations>,
    <http://www.opengis.net/spec/geosparql/1.1/req/geometry-extension/eh-spatial-relations>;
  rdfs:seeAlso <http://dbpedia.org/resource/DE-9IM> .

geo:ehCovers rdfs:isDefinedBy <http://www.opengis.net/ont/geosparql#>, <http://www.opengis.net/spec/geosparql/1.0/req/geometry-extension/eh-spatial-relations>,
    <http://www.opengis.net/spec/geosparql/1.1/req/geometry-extension/eh-spatial-relations>;
  rdfs:seeAlso <http://dbpedia.org/resource/DE-9IM> .

geo:ehCoveredBy rdfs:isDefinedBy <http://www.opengis.net/ont/geosparql#>, <http://www.opengis.net/spec/geosparql/1.0/req/geometry-extension/eh-spatial-relations>,
    <http://www.opengis.net/spec/geosparql/1.1/req/geometry-extension/eh-spatial-relations>;
  rdfs:seeAlso <http://dbpedia.org/resource/DE-9IM> .

geo:ehInside rdfs:isDefinedBy <http://www.opengis.net/ont/geosparql#>, <http://www.opengis.net/spec/geosparql/1.0/req/geometry-extension/eh-spatial-relations>,
    <http://www.opengis.net/spec/geosparql/1.1/req/geometry-extension/eh-spatial-relations>;
  rdfs:seeAlso <http://dbpedia.org/resource/DE-9IM> .

geo:ehContains rdfs:isDefinedBy <http://www.opengis.net/ont/geosparql#>, <http://www.opengis.net/spec/geosparql/1.0/req/geometry-extension/eh-spatial-relations>,
    <http://www.opengis.net/spec/geosparql/1.1/req/geometry-extension/eh-spatial-relations>;
  rdfs:seeAlso <http://dbpedia.org/resource/DE-9IM> .

geo:rcc8eq rdfs:isDefinedBy <http://www.opengis.net/ont/geosparql#>, <http://www.opengis.net/spec/geosparql/1.0/req/topology-vocab-extension/rcc8-spatial-relations>,
    <http://www.opengis.net/spec/geosparql/1.1/req/topology-vocab-extension/rcc8-spatial-relations>;
  rdfs:seeAlso <http://dbpedia.org/resource/DE-9IM> .

geo:rcc8dc rdfs:isDefinedBy <http://www.opengis.net/ont/geosparql#>, <http://www.opengis.net/spec/geosparql/1.0/req/topology-vocab-extension/rcc8-spatial-relations>,
    <http://www.opengis.net/spec/geosparql/1.1/req/topology-vocab-extension/rcc8-spatial-relations>;
  rdfs:seeAlso <http://dbpedia.org/resource/DE-9IM> .

geo:rcc8ec rdfs:isDefinedBy <http://www.opengis.net/ont/geosparql#>, <http://www.opengis.net/spec/geosparql/1.0/req/topology-vocab-extension/rcc8-spatial-relations>,
    <http://www.opengis.net/spec/geosparql/1.1/req/topology-vocab-extension/rcc8-spatial-relations>;
  rdfs:seeAlso <http://dbpedia.org/resource/DE-9IM> .

geo:rcc8po rdfs:isDefinedBy <http://www.opengis.net/ont/geosparql#>, <http://www.opengis.net/spec/geosparql/1.0/req/topology-vocab-extension/rcc8-spatial-relations>,
    <http://www.opengis.net/spec/geosparql/1.1/req/topology-vocab-extension/rcc8-spatial-relations>;
  rdfs:seeAlso <http://dbpedia.org/resource/DE-9IM> .

geo:rcc8tppi rdfs:isDefinedBy <http://www.opengis.net/ont/geosparql#>, <http://www.opengis.net/spec/geosparql/1.0/req/topology-vocab-extension/rcc8-spatial-relations>,
    <http://www.opengis.net/spec/geosparql/1.1/req/topology-vocab-extension/rcc8-spatial-relations>;
  rdfs:seeAlso <http://dbpedia.org/resource/DE-9IM> .

geo:rcc8tpp rdfs:isDefinedBy <http://www.opengis.net/ont/geosparql#>, <http://www.opengis.net/spec/geosparql/1.0/req/topology-vocab-extension/rcc8-spatial-relations>,
    <http://www.opengis.net/spec/geosparql/1.1/req/topology-vocab-extension/rcc8-spatial-relations>;
  rdfs:seeAlso <http://dbpedia.org/resource/DE-9IM> .

geo:rcc8ntpp rdfs:isDefinedBy <http://www.opengis.net/ont/geosparql#>, <http://www.opengis.net/spec/geosparql/1.0/req/topology-vocab-extension/rcc8-spatial-relations>,
    <http://www.opengis.net/spec/geosparql/1.1/req/topology-vocab-extension/rcc8-spatial-relations>;
  rdfs:seeAlso <http://dbpedia.org/resource/DE-9IM> .

geo:rcc8ntppi rdfs:isDefinedBy <http://www.opengis.net/ont/geosparql#>, <http://www.opengis.net/spec/geosparql/1.0/req/topology-vocab-extension/rcc8-spatial-relations>,
    <http://www.opengis.net/spec/geosparql/1.1/req/topology-vocab-extension/rcc8-spatial-relations>;
  rdfs:seeAlso <http://dbpedia.org/resource/DE-9IM> .

geo:dggsLiteral rdfs:isDefinedBy <http://www.opengis.net/ont/geosparql#>, <http://www.opengis.net/spec/geosparql/1.1/req/geometry-extension/dggs-literal>;
  rdfs:seeAlso <http://www.opengis.net/doc/AS/dggs/2.0> .

geo:geoJSONLiteral rdfs:isDefinedBy <http://www.opengis.net/ont/geosparql#>, <http://www.opengis.net/spec/geosparql/1.1/req/geometry-extension/geojson-literal>;
  rdfs:seeAlso <https://tools.ietf.org/html/rfc7946> .

geo:gmlLiteral rdfs:isDefinedBy <http://www.opengis.net/ont/geosparql#>, <http://www.opengis.net/spec/geosparql/1.0/req/geometry-extension/gml-literal>,
    <http://www.opengis.net/spec/geosparql/1.1/req/geometry-extension/gml-literal>;
  rdfs:seeAlso <https://portal.ogc.org/files/?artifact_id=20509> .

geo:kmlLiteral rdfs:isDefinedBy <http://www.opengis.net/ont/geosparql#>, <http://www.opengis.net/spec/geosparql/1.1/req/geometry-extension/kml-literal>;
  rdfs:seeAlso <https://www.ogc.org/standards/kml/> .

geo:wktLiteral rdfs:isDefinedBy <http://www.opengis.net/ont/geosparql#>, <http://www.opengis.net/spec/geosparql/1.0/req/geometry-extension/wkt-literal>,
    <http://www.opengis.net/spec/geosparql/1.1/req/geometry-extension/wkt-literal>;
  rdfs:seeAlso <https://portal.ogc.org/files/?artifact_id=25355> .

<http://linkedevents.org/ontology/involved> rdfs:isDefinedBy <http://linkedevents.org/ontology/> .

<http://www.kulttuurisampo.fi/ebkr/agent> rdfs:isDefinedBy <http://www.kulttuurisampo.fi/ebkr/> .

<http://www.kulttuurisampo.fi/ebkr/place> rdfs:isDefinedBy <http://www.kulttuurisampo.fi/ebkr/> .

<http://linkedevents.org/ontology/inSpace> rdfs:isDefinedBy <http://linkedevents.org/ontology/> .

<http://purl.org/NET/c4dm/event.owl#sub_event> rdfs:isDefinedBy <http://purl.org/NET/c4dm/event.owl#> .

<http://linkedevents.org/ontology/atTime> rdfs:isDefinedBy <http://linkedevents.org/ontology/> .

dc:type rdfs:isDefinedBy <http://purl.org/dc/elements/1.1/> .

<http://www.kulttuurisampo.fi/ebkr/quality> rdfs:isDefinedBy <http://www.kulttuurisampo.fi/ebkr/> .

geo:defaultGeometry rdfs:isDefinedBy <http://www.opengis.net/ont/geosparql#>, <http://www.opengis.net/spec/geosparql/1.1/req/geometry-extension/feature-properties> .

geo:hasGeometry rdfs:isDefinedBy <http://www.opengis.net/ont/geosparql#>, <http://www.opengis.net/spec/geosparql/1.1/req/geometry-extension/feature-properties>,
    <http://www.opengis.net/spec/geosparql/1.0/req/geometry-extension/feature-properties> .

geo:Geometry rdfs:isDefinedBy <http://www.opengis.net/ont/geosparql#>, <http://www.opengis.net/spec/geosparql/1.0/req/geometry-extension/geometry-class>,
    <http://www.opengis.net/spec/geosparql/1.1/req/geometry-extension/geometry-class> .

geo:SpatialObject rdfs:isDefinedBy <http://www.opengis.net/ont/geosparql#>, <http://www.opengis.net/spec/geosparql/1.0/req/core/spatial-object-class>,
    <http://www.opengis.net/spec/geosparql/1.1/req/core/spatial-object-class> .

geo:hasArea rdfs:isDefinedBy <http://www.opengis.net/ont/geosparql#>, <http://www.opengis.net/spec/geosparql/1.1/req/geometry-extension/spatial-object-properties> .

geo:hasSize rdfs:isDefinedBy <http://www.opengis.net/ont/geosparql#>, <http://www.opengis.net/spec/geosparql/1.0/req/topology-vocab-extension/spatial-object-properties>,
    <http://www.opengis.net/spec/geosparql/1.1/req/topology-vocab-extension/spatial-object-properties> .

geo:hasBoundingBox rdfs:isDefinedBy <http://www.opengis.net/ont/geosparql#>, <http://www.opengis.net/spec/geosparql/1.1/req/geometry-extension/feature-properties> .

geo:hasCentroid rdfs:isDefinedBy <http://www.opengis.net/ont/geosparql#>, <http://www.opengis.net/spec/geosparql/1.1/req/geometry-extension/feature-properties> .

geo:hasLength rdfs:isDefinedBy <http://www.opengis.net/ont/geosparql#>, <http://www.opengis.net/spec/geosparql/1.1/req/geometry-extension/spatial-object-properties> .

geo:hasPerimeterLength rdfs:isDefinedBy <http://www.opengis.net/ont/geosparql#>, <http://www.opengis.net/spec/geosparql/1.1/req/geometry-extension/spatial-object-properties> .

geo:hasSpatialAccuracy rdfs:isDefinedBy <http://www.opengis.net/ont/geosparql#>, <http://www.opengis.net/spec/geosparql/1.1/req/geometry-extension/geometry-properties> .

geo:hasSpatialResolution rdfs:isDefinedBy <http://www.opengis.net/ont/geosparql#>,
    <http://www.opengis.net/spec/geosparql/1.1/req/geometry-extension/feature-properties> .

geo:hasVolume rdfs:isDefinedBy <http://www.opengis.net/ont/geosparql#>, <http://www.opengis.net/spec/geosparql/1.1/req/geometry-extension/spatial-object-properties> .

<http://www.kulttuurisampo.fi/ebkr/time> rdfs:isDefinedBy <http://www.kulttuurisampo.fi/ebkr/> .

geo:asDGGS rdfs:isDefinedBy <http://www.opengis.net/ont/geosparql#>, <http://www.opengis.net/spec/geosparql/1.1/req/geometry-extension/geometry-as-dggs-literal> .

geo:hasSerialization rdfs:isDefinedBy <http://www.opengis.net/ont/geosparql#>, <http://www.opengis.net/spec/geosparql/1.1/req/geometry-extension/geometry-properties>,
    <http://www.opengis.net/spec/geosparql/1.0/req/geometry-extension/geometry-properties> .

geo:asGeoJSON rdfs:isDefinedBy <http://www.opengis.net/ont/geosparql#>, <http://www.opengis.net/spec/geosparql/1.1/req/geometry-extension/geometry-as-geojson-literal>;
  rdfs:seeAlso <https://tools.ietf.org/html/rfc7946> .

geo:asKML rdfs:isDefinedBy <http://www.opengis.net/ont/geosparql#>, <http://www.opengis.net/spec/geosparql/1.1/req/geometry-extension/geometry-as-kml-literal>;
  rdfs:seeAlso <https://www.ogc.org/standards/kml> .

geo:coordinateDimension rdfs:isDefinedBy <http://www.opengis.net/ont/geosparql#>,
    <http://www.opengis.net/spec/geosparql/1.1/req/geometry-extension/geometry-properties> .

geo:dimension rdfs:isDefinedBy <http://www.opengis.net/ont/geosparql#>, <http://www.opengis.net/spec/geosparql/1.1/req/geometry-extension/geometry-properties> .

geo:hasMetricArea rdfs:isDefinedBy <http://www.opengis.net/ont/geosparql#>, <http://www.opengis.net/spec/geosparql/1.1/req/geometry-extension/spatial-object-properties> .

geo:hasMetricSize rdfs:isDefinedBy <http://www.opengis.net/ont/geosparql#>, <http://www.opengis.net/spec/geosparql/1.1/req/geometry-extension/spatial-object-properties> .

geo:hasMetricLength rdfs:isDefinedBy <http://www.opengis.net/ont/geosparql#>, <http://www.opengis.net/spec/geosparql/1.1/req/geometry-extension/spatial-object-properties> .

geo:hasMetricPerimeterLength rdfs:isDefinedBy <http://www.opengis.net/ont/geosparql#>,
    <http://www.opengis.net/spec/geosparql/1.1/req/geometry-extension/spatial-object-properties> .

geo:hasMetricSpatialAccuracy rdfs:isDefinedBy <http://www.opengis.net/ont/geosparql#>,
    <http://www.opengis.net/spec/geosparql/1.1/req/geometry-extension/geometry-properties> .

geo:hasMetricSpatialResolution rdfs:isDefinedBy <http://www.opengis.net/ont/geosparql#>,
    <http://www.opengis.net/spec/geosparql/1.1/req/geometry-extension/geometry-properties> .

geo:hasMetricVolume rdfs:isDefinedBy <http://www.opengis.net/ont/geosparql#>, <http://www.opengis.net/spec/geosparql/1.1/req/geometry-extension/spatial-object-properties> .

geo:isEmpty rdfs:isDefinedBy <http://www.opengis.net/ont/geosparql#>, <http://www.opengis.net/spec/geosparql/1.1/req/geometry-extension/geometry-properties>,
    <http://www.opengis.net/spec/geosparql/1.0/req/geometry-extension/geometry-properties> .

geo:isSimple rdfs:isDefinedBy <http://www.opengis.net/ont/geosparql#>, <http://www.opengis.net/spec/geosparql/1.1/req/geometry-extension/geometry-properties>,
    <http://www.opengis.net/spec/geosparql/1.0/req/geometry-extension/geometry-properties>;
  rdfs:seeAlso <https://portal.ogc.org/files/?artifact_id=25355> .

geo:spatialDimension rdfs:isDefinedBy <http://www.opengis.net/ont/geosparql#>, <http://www.opengis.net/spec/geosparql/1.1/req/geometry-extension/geometry-properties>,
    <http://www.opengis.net/spec/geosparql/1.0/req/geometry-extension/geometry-properties> .

<http://sw.opencyc.org/2009/04/07/concept/en/SomethingExisting> rdfs:isDefinedBy <http://sw.opencyc.org/2009/04/07/concept/en/> .

<http://www.loa-cnr.it/ontologies/DOLCE-Lite.owl#endurant> rdfs:isDefinedBy <http://www.loa-cnr.it/ontologies/DOLCE-Lite.owl#> .

<http://purl.org/dc/terms/Agent> rdfs:isDefinedBy <http://purl.org/dc/terms/> .

<http://purl.org/dc/terms/AgentClass> rdfs:isDefinedBy <http://purl.org/dc/terms/> .

<http://sw.opencyc.org/2009/04/07/concept/en/Agent-Generic> rdfs:isDefinedBy <http://sw.opencyc.org/2009/04/07/concept/en/> .

<http://www.ontologyportal.org/translations/SUMO.owl.txt#Agent> rdfs:isDefinedBy <http://www.ontologyportal.org/translations/SUMO.owl.txt#> .

<http://www8.informatik.uni-erlangen.de/IMMD8/Services/cidoc-crm/erlangen-crm_090330_5_0_1.owl#E39.Actor>
  rdfs:isDefinedBy <http://www8.informatik.uni-erlangen.de/IMMD8/Services/cidoc-crm/erlangen-crm_090330_5_0_1.owl#> .

foaf:Agent rdfs:isDefinedBy <http://xmlns.com/foaf/0.1/> .

<http://linkedevents.org/ontology/Event> rdfs:isDefinedBy <http://linkedevents.org/ontology/> .

<http://purl.org/NET/c4dm/event.owl#Event> rdfs:isDefinedBy <http://purl.org/NET/c4dm/event.owl#> .

<http://purl.org/dc/dcmitype/Event> rdfs:isDefinedBy <http://purl.org/dc/dcmitype/> .

<http://sw.opencyc.org/2009/04/07/concept/en/Situation> rdfs:isDefinedBy <http://sw.opencyc.org/2009/04/07/concept/en/> .

<http://www.loa-cnr.it/ontologies/DOLCE-Lite.owl#perdurant> rdfs:isDefinedBy <http://www.loa-cnr.it/ontologies/DOLCE-Lite.owl#> .

<http://www.ontologyportal.org/translations/SUMO.owl.txt#Process> rdfs:isDefinedBy
    <http://www.ontologyportal.org/translations/SUMO.owl.txt#> .

<http://www8.informatik.uni-erlangen.de/IMMD8/Services/cidoc-crm/erlangen-crm_090330_5_0_1.owl#E5.Event>
  rdfs:isDefinedBy <http://www8.informatik.uni-erlangen.de/IMMD8/Services/cidoc-crm/erlangen-crm_090330_5_0_1.owl#> .

<http://www.ontologyportal.org/translations/SUMO.owl.txt#Object> rdfs:isDefinedBy
    <http://www.ontologyportal.org/translations/SUMO.owl.txt#> .

<http://www8.informatik.uni-erlangen.de/IMMD8/Services/cidoc-crm/erlangen-crm_090330_5_0_1.owl#E19.Physical_Object>
  rdfs:isDefinedBy <http://www8.informatik.uni-erlangen.de/IMMD8/Services/cidoc-crm/erlangen-crm_090330_5_0_1.owl#> .

<http://www8.informatik.uni-erlangen.de/IMMD8/Services/cidoc-crm/erlangen-crm_090330_5_0_1.owl#E21.Person>
  rdfs:isDefinedBy <http://www8.informatik.uni-erlangen.de/IMMD8/Services/cidoc-crm/erlangen-crm_090330_5_0_1.owl#> .

<http://purl.org/NET/c4dm/event.owl#Factor> rdfs:isDefinedBy <http://purl.org/NET/c4dm/event.owl#> .

<http://purl.org/NET/c4dm/event.owl#Product> rdfs:isDefinedBy <http://purl.org/NET/c4dm/event.owl#> .

<http://purl.org/dc/dcmitype/PhysicalObject> rdfs:isDefinedBy <http://purl.org/dc/dcmitype/> .

<http://purl.org/dc/terms/PhysicalResource> rdfs:isDefinedBy <http://purl.org/dc/terms/> .

<http://purl.org/dc/terms/Location> rdfs:isDefinedBy <http://purl.org/dc/terms/> .

<http://sw.opencyc.org/2009/04/07/concept/en/EnduringThing-Localized> rdfs:isDefinedBy
    <http://sw.opencyc.org/2009/04/07/concept/en/> .

<http://www.ontologyportal.org/translations/SUMO.owl.txt#GeographicArea> rdfs:isDefinedBy
    <http://www.ontologyportal.org/translations/SUMO.owl.txt#> .

<http://www8.informatik.uni-erlangen.de/IMMD8/Services/cidoc-crm/erlangen-crm_090330_5_0_1.owl#E53.Place>
  rdfs:isDefinedBy <http://www8.informatik.uni-erlangen.de/IMMD8/Services/cidoc-crm/erlangen-crm_090330_5_0_1.owl#> .

<http://www.loa-cnr.it/ontologies/DOLCE-Lite.owl#PhysicalRegion> rdfs:isDefinedBy
    <http://www.loa-cnr.it/ontologies/DOLCE-Lite.owl#> .

wgs:SpatialThing rdfs:isDefinedBy <http://www.w3.org/2003/01/geo/wgs84_pos#> .

<http://sw.opencyc.org/2009/04/07/concept/en/Role> rdfs:isDefinedBy <http://sw.opencyc.org/2009/04/07/concept/en/> .

<http://www.loa-cnr.it/ontologies/DOLCE-Lite.owl#region> rdfs:isDefinedBy <http://www.loa-cnr.it/ontologies/DOLCE-Lite.owl#> .

<http://www.ontologyportal.org/translations/SUMO.owl.txt#IntentionalProcess> rdfs:isDefinedBy
    <http://www.ontologyportal.org/translations/SUMO.owl.txt#> .

<http://www.w3.org/2006/timeTemporalEntity> rdfs:isDefinedBy <http://www.w3.org/2006/time> .

<http://www.loa-cnr.it/ontologies/DOLCE-Lite.owl#AbstractRegion> rdfs:isDefinedBy
    <http://www.loa-cnr.it/ontologies/DOLCE-Lite.owl#> .

<http://www8.informatik.uni-erlangen.de/IMMD8/Services/cidoc-crm/erlangen-crm_090330_5_0_1.owl#E55.Type>
  rdfs:isDefinedBy <http://www8.informatik.uni-erlangen.de/IMMD8/Services/cidoc-crm/erlangen-crm_090330_5_0_1.owl#> .

geo:FeatureCollection rdfs:isDefinedBy <http://www.opengis.net/ont/geosparql#>, <http://www.opengis.net/spec/geosparql/1.1/req/core/feature-collection-class> .

geo:SpatialObjectCollection rdfs:isDefinedBy <http://www.opengis.net/ont/geosparql#>,
    <http://www.opengis.net/spec/geosparql/1.1/req/core/spatial-object-collection-class> .

geo:GeometryCollection rdfs:isDefinedBy <http://www.opengis.net/ont/geosparql#>, <http://www.opengis.net/spec/geosparql/1.1/req/core/geometry-collection-class> .

:wikipediaKampanyeKalimantan1945 :image "Borneo_Campaign_CMH.jpg";
  :wikiurl "https://id.wikipedia.org/wiki/Kampanye_Kalimantan_(1945)" .

:wikipediaPertempuranBojongKokosan :image "https://aartreya.com/images/berita/konten_bojongkokoksan%20foto%20jokam.jpg";
  :wikiurl "https://id.wikipedia.org/wiki/Pertempuran_Bojong_Kokosan" .

:wikipediaRevolusiNasionalIndonesia :image "Indonesia flag raising witnesses 17 August 1945.jpg";
  :wikiurl "https://id.wikipedia.org/wiki/Revolusi_Nasional_Indonesia" .

:wikipediaPerangCumbok :image "https://asset.kompas.com/crops/DJM_P8kIygNnZPCmB5ZULPCpq64=/0x54:698x520/750x500/data/photo/2021/11/05/6184a0902d731.jpeg";
  :wikiurl "https://id.wikipedia.org/wiki/Perang_Cumbok" .

:wikipediaSeranganUmum1Maret1949 :image "Munumen Serangan Umum 1 Maret 1949.jpg";
  :wikiurl "https://id.wikipedia.org/wiki/Serangan_Umum_1_Maret_1949" .

:wikipediaKonflikPapua :image "https://ichef.bbci.co.uk/ace/ws/800/cpsprodpb/524A/production/_118566012_a3b9d61f-12ff-4266-910c-22bbd3bcfb84.jpg";
  :wikiurl "https://id.wikipedia.org/wiki/Konflik_Papua" .

:wikipediaPeristiwaTigaMaret :image "https://koropak.co.id/storage/cover/sejarah-sumatra-barat-peristiwa-pemberontakan-tiga-maret_1709380377.jpg";
  :wikiurl "https://id.wikipedia.org/wiki/Peristiwa_Tiga_Maret" .

:wikipediaPenyerbuanKotabaruYogyakarta :image "https://asset.kompas.com/crops/ZCeNV4OThSPOlTUz36NGVVy-Bmg=/177x0:2475x1532/750x500/data/photo/2021/12/22/61c2fb04e3e5c.jpg";
  :wikiurl "https://id.wikipedia.org/wiki/Penyerbuan_Kotabaru_Yogyakarta" .

:wikipediaPerangDayakDesa :image "SultanPontianak.jpg";
  :wikiurl "https://id.wikipedia.org/wiki/Perang_Dayak_Desa" .

:wikipediaGerakan30September :image "potret gestapu.jpg";
  :wikiurl "https://id.wikipedia.org/wiki/Gerakan_30_September" .

:wikipediaKampanyeHindiaBelanda :image "COLLECTIE TROPENMUSEUM Japanse invasie op Java TMnr 10001990.jpg";
  :wikiurl "https://id.wikipedia.org/wiki/Kampanye_Hindia_Belanda" .

:wikipediaPertempuranLengkong :image "https://d220hvstrn183r.cloudfront.net/attachment/30585619145983802199";
  :wikiurl "https://id.wikipedia.org/wiki/Pertempuran_Lengkong" .

:wikipediaPertempuranMedanArea :image "Medan Area Memorial.jpg";
  :wikiurl "https://id.wikipedia.org/wiki/Pertempuran_Medan_Area" .

:wikipediaPertempuranKumai :image "https://koranmakassar.com/wp-content/uploads/2022/01/c20b11ce5265054a5d4a3cf888edd9e1-e1642090647236.jpg";
  :wikiurl "https://id.wikipedia.org/wiki/Pertempuran_Kumai" .

:wikipediaSeranganUmumSurakarta :image "Monumen_Serangan_Umum_4_Hari_Surakarta.jpg";
  :wikiurl "https://id.wikipedia.org/wiki/Serangan_Umum_Surakarta" .

:wikipediaPuputanMargarana :image "https://wiki.edunitas.com/_sepakbola/_baca_image.php?td=9&kodegb=Puputan2.jpg";
  :wikiurl "https://id.wikipedia.org/wiki/Puputan_Margarana" .

:wikipediaPertempuranLimaHari :image "File:Becak_Tugu_Muda_Semarang_Central_Java.jpg";
  :wikiurl "https://id.wikipedia.org/wiki/Pertempuran_Lima_Hari" .

:wikipediaPertempuranSurabaya :image "Collectie_NMvWereldculturen,_7082-nf-1167,_Ansichtkaart-_Oranje_Hotel_in_Surabaya,_1937.jpg";
  :wikiurl "https://id.wikipedia.org/wiki/Pertempuran_Surabaya" .

:wikipediaOperasi17Agustus :image "Navy military operations against PRRI (crop), Jalesveva Jayamahe, p241.jpg";
  :wikiurl "https://id.wikipedia.org/wiki/Operasi_17_Agustus" .

:JisaburoOzawa :image "Ozawa11.jpg";
  :wikiurl "https://id.wikipedia.org/wiki/Jisaburo_Ozawa" .

:MuhammadMangundiprojo :image "Muhammadmangundiprojo.png";
  :wikiurl "https://id.wikipedia.org/wiki/Muhammad_Mangundiprojo" .

:Soengkono :image "Col_Sungkono,_Kenang-Kenangan_Pada_Panglima_Besar_Letnan_Djenderal_Soedirman,_p27.jpg";
  :wikiurl "https://id.wikipedia.org/wiki/Soengkono" .

:HarioJonosewojo :image "https://d220hvstrn183r.cloudfront.net/attachment/55089736130230161617.large";
  :wikiurl "https://id.wikipedia.org/wiki/Hario_Jonosewojo" .

:MoehammadJasin :image "Moehammad_Jasin.jpg";
  :wikiurl "https://id.wikipedia.org/wiki/Moehammad_Jasin" .

:Moestopo :image "Prof-Dr-Moestopo1.jpg";
  :wikiurl "https://id.wikipedia.org/wiki/Moestopo" .

:RobertMansergh :image "Robertmansergh.jpg";
  :wikiurl "https://id.wikipedia.org/wiki/Robert_Mansergh" .

:AubertinMallaby :image "Indonesian_delegate_speaking_to_Mallaby,_Impressions_of_the_Fight_..._in_Indonesia,_p16.jpg";
  :wikiurl "https://id.wikipedia.org/wiki/Aubertin_Mallaby" .

:Sutomo :image "Bung_Tomo.jpg";
  :wikiurl "https://id.wikipedia.org/wiki/Sutomo" .

:GoliathTabuni :image "Jenderal._Goliath_Tabuni.JPG";
  :wikiurl "https://id.wikipedia.org/wiki/Goliath_Tabuni" .

:Soekarno :image "Presiden_Sukarno.jpg";
  :wikiurl "https://id.wikipedia.org/wiki/Soekarno" .

:KiyotakeKawaguchi :image "Kawaguchi_Kiyotake.jpg";
  :wikiurl "https://id.wikipedia.org/wiki/Kiyotake_Kawaguchi" .

:RaymondWesterling :image "Raymond_Westerling.jpg";
  :wikiurl "https://id.wikipedia.org/wiki/Raymond_Westerling" .

:JuliusTahija :image "Julius_Tahija,_Minister_of_Social_Affairs.jpg";
  :wikiurl "https://id.wikipedia.org/wiki/Julius_Tahija" .

:Moekijat :image "Moekijat.jpg";
  :wikiurl "https://id.wikipedia.org/wiki/Moekijat" .

:MohammadHatta :image "Mohammad_Hatta,_Pekan_Buku_Indonesia_1954,_p242.jpg";
  :wikiurl "https://id.wikipedia.org/wiki/Mohammad_Hatta" .

:DouglasMacArthur :image "MacArthur_Manila.jpg";
  :wikiurl "https://id.wikipedia.org/wiki/Douglas_MacArthur" .

:ListyoSigitPrabowo :image "KAPOLRI,Jenderal_POL_Listyo_Sigit_Prabowo.jpg";
  :wikiurl "https://id.wikipedia.org/wiki/Listyo_Sigit_Prabowo" .

:REMartadinata :image "R.E_Martadinata_colorized_by_colorbykevin.jpg";
  :wikiurl "https://id.wikipedia.org/wiki/R._E._Martadinata" .

:NobutakeKond :image "Vizeadmiral_Nobutake_Kondo.jpg";
  :wikiurl "https://id.wikipedia.org/wiki/Nobutake_Kond%C5%8D" .

:SutanSjahrir :image "Soetan_Sjahrir_1948.jpg";
  :wikiurl "https://id.wikipedia.org/wiki/Sutan_Sjahrir" .

:SlametRijadi :image "Zaterdag,_12_november_werd_in_het_stadion_te_Solo_een_grote_massabijeenkomst_geh,_Bestanddeelnr_924_(Slamet_Rijadi,_cropped).jpg";
  :wikiurl "https://id.wikipedia.org/wiki/Slamet_Rijadi" .

:AgusSubiyanto :image "Panglima_TNI_Jenderal_TNI_Agus_Subiyanto.jpg";
  :wikiurl "https://id.wikipedia.org/wiki/Agus_Subiyanto" .

:Assaat :image "Assaat,_Mr._Gelar_Datuk_Mudo,_Kami_Perkenalkan_(1954)_p76.jpg";
  :wikiurl "https://id.wikipedia.org/wiki/Assaat" .

:MuhammadToha :image "Muhammad Toha.jpg";
  :wikiurl "https://id.wikipedia.org/wiki/Muhammad_Toha" .

:AbdulHarisNasution :image "Abdul Haris Nasution.jpg";
  :wikiurl "https://id.wikipedia.org/wiki/Abdul_Haris_Nasution" .

:PrabowoSubianto :image "Prabowo Subianto, Candidate for Indonesia's President in 2024.jpg";
  :wikiurl "https://id.wikipedia.org/wiki/Prabowo_Subianto" .

:EgianusKogoya :image "https://img.inews.co.id/media/822/files/inews_new/2023/03/18/egianus_kogoya.jpg";
  :wikiurl "https://id.wikipedia.org/wiki/Egianus_Kogoya" .

:BudiGunawan :image "Budi_Gunawan.jpg";
  :wikiurl "https://id.wikipedia.org/wiki/Budi_Gunawan" .

:JaminGinting :image "Djamin_Ginting.jpg";
  :wikiurl "https://id.wikipedia.org/wiki/Jamin_Ginting" .

:AchmadTahir :image "Achmad Tahir - Fourth Development Cabinet.jpg";
  :wikiurl "https://id.wikipedia.org/wiki/Achmad_Tahir" .

:HubertusJohannesvanMook :image "Hubertus_J._van_Mook,_minister_van_kolonin,_NG-1992-3-3-9.jpg";
  :wikiurl "https://id.wikipedia.org/wiki/Hubertus_Johannes_van_Mook" .

:TeukuNyakArif :image "Tnarief.jpg";
  :wikiurl "https://id.wikipedia.org/wiki/Teuku_Nyak_Arif" .

:SyamaunGaharu :image "Letnan_Kolonel_Sjamaun_Gaharu.jpg";
  :wikiurl "https://id.wikipedia.org/wiki/Syamaun_Gaharu" .

:DaudBeureueh :image "Teuku Daud Beureueh.jpg";
  :wikiurl "https://id.wikipedia.org/wiki/Daud_Beureu%27eh" .

:HeinterPoorten :image "Hein_ter_Poorten.jpg";
  :wikiurl "https://id.wikipedia.org/wiki/Hein_ter_Poorten" .

:IGustiNgurahRai :image "Lukisan_I_Gusti_Ngurah.jpg";
  :wikiurl "https://id.wikipedia.org/wiki/I_Gusti_Ngurah_Rai" .

:SimonSpoor :image "Simon_Spoor_(1948).jpg";
  :wikiurl "https://id.wikipedia.org/wiki/Simon_Spoor" .

:SyafruddinPrawiranegara :image "Sjafruddin_Prawiranegara.jpg";
  :wikiurl "https://id.wikipedia.org/wiki/Syafruddin_Prawiranegara" .

:MaludinSimbolon :image "Kolonel_Maludin_SIMBOLON.jpg";
  :wikiurl "https://id.wikipedia.org/wiki/Maludin_Simbolon" .

:AhmadYani :image "Ahmad_Yani.jpg";
  :wikiurl "https://id.wikipedia.org/wiki/Ahmad_Yani" .

:AhmadHusein :image "Let._Kol._Ahmad_Husein.jpg";
  :wikiurl "https://id.wikipedia.org/wiki/Ahmad_Husein" .

:HitoshiImamura :image "Hitoshi_Imamura.jpg";
  :wikiurl "https://id.wikipedia.org/wiki/Hitoshi_Imamura" .

:EdiSukardi :image "https://asset.kompas.com/crops/2smuVP-LEEDoc5vLkCgfE03gmtA=/777x584:2053x1435/750x500/data/photo/2021/12/31/61ce9776188f8.png";
  :wikiurl "https://id.wikipedia.org/wiki/Edi_Sukardi" .

:Musso :image "Musso.jpg";
  :wikiurl "https://id.wikipedia.org/wiki/Musso" .

:TanMalaka :image "TanMalaka_DariPendjara_ed3.jpg";
  :wikiurl "https://id.wikipedia.org/wiki/Tan_Malaka" .

:HisaichiTerauchi :image "Hisaichi_Terauchi_2.jpg";
  :wikiurl "https://id.wikipedia.org/wiki/Hisaichi_Terauchi" .

:LouisMountbatten :image "Lord_Mountbatten_Naval_in_colour_Allan_Warren.jpg";
  :wikiurl "https://id.wikipedia.org/wiki/Louis_Mountbatten" .

:DirkCornelisBuurmanvanVreeden :image "Dirk_Cornelis_Buurman_van_Vreeden_(1946).jpg";
  :wikiurl "https://id.wikipedia.org/wiki/Dirk_Cornelis_Buurman_van_Vreeden" .

:SebbySambom :image "https://static.promediateknologi.id/crop/0x0:0x0/750x500/webp/photo/p1/698/2023/11/29/Jubir-Sebby-Sambom-3846253716.png";
  :wikiurl "https://id.wikipedia.org/wiki/Sebby_Sambom" .

:AlidiusTjardavanStarkenborghStachouwer :image "COLLECTIE TROPENMUSEUM Portret van Gouverneur-Generaal Tjarda van Starkenborgh Stachouwer TMnr 10018816.jpg";
  :wikiurl "https://id.wikipedia.org/wiki/Alidius_Tjarda_van_Starkenborgh_Stachouwer" .

:DaanMogot :image "Daan_Mogot_1.jpg";
  :wikiurl "https://id.wikipedia.org/wiki/Daan_Mogot" .

:LudolphHendrikvanOyen :image "Ludolph_Hendrik_van_Oyen_(1943).jpg";
  :wikiurl "https://id.wikipedia.org/wiki/Ludolph_Hendrik_van_Oyen" .

:TjokordaGdeRakaSoekawati :image "Tjokorda_Gde_Raka_Soekawati,_Volume_I_of_Pendidikan_Politik_Rakjat,_p4.jpg";
  :wikiurl "https://id.wikipedia.org/wiki/Tjokorda_Gde_Raka_Soekawati" .

:Wongsonegoro :image "Wongsonegoro,_Kami_Perkenalkan_(1954),_p17.jpg";
  :wikiurl "https://id.wikipedia.org/wiki/Wongsonegoro" .

:Kariadi :image "https://static.promediateknologi.id/crop/0x0:0x0/750x500/webp/photo/2021/11/09/2160610581.jpg";
  :wikiurl "https://id.wikipedia.org/wiki/Kariadi" .

:GatotSoebroto :image "Col_Gatot_Subroto,_Kenang-Kenangan_Pada_Panglima_Besar_Letnan_Djenderal_Soedirman,_p27.jpg";
  :wikiurl "https://id.wikipedia.org/wiki/Gatot_Soebroto" .

:KellyKwalik :image "Kelly_Kwalik.png";
  :wikiurl "https://id.wikipedia.org/wiki/Kelly_Kwalik" .

:BJHabibie :image "B._J._Habibie,_President_of_Indonesia_portrait.jpg";
  :wikiurl "https://id.wikipedia.org/wiki/B._J._Habibie" .

:ThomasCHart :image "Thomas_C._Hart.jpg";
  :wikiurl "https://id.wikipedia.org/wiki/Thomas_C._Hart" .

:ShojiNishimura :image "ShojiNishimura.jpg";
  :wikiurl "https://id.wikipedia.org/wiki/Shoji_Nishimura" .

:Soedirman :image "Sudirman.jpg";
  :wikiurl "https://id.wikipedia.org/wiki/Soedirman" .

:TakeoTakagi :image "Takagi_Takeo.jpg";
  :wikiurl "https://id.wikipedia.org/wiki/Takeo_Takagi" .

:DirkReinhardAdelbertvanLangen :image "D.R.A._van_Langen.png";
  :wikiurl "https://id.wikipedia.org/wiki/Dirk_Reinhard_Adelbert_van_Langen" .

:BambangSoegeng :image "Djenderal_Major_Bambang_Sugeng.png";
  :wikiurl "https://id.wikipedia.org/wiki/Bambang_Soegeng" .

:OeripSoemohardjo :image "Oerip_Soemohardjo_5_November_1947_KR.JPG";
  :wikiurl "https://id.wikipedia.org/wiki/Oerip_Soemohardjo" .

:AndikaPerkasa :image "Jenderal_TNI_Andika_Perkasa,_Panglima_TNI.jpg";
  :wikiurl "https://id.wikipedia.org/wiki/Andika_Perkasa" .

:ConradHelfrich :image "Conrad_Helfrich_colourized.jpg";
  :wikiurl "https://id.wikipedia.org/wiki/Conrad_Helfrich" .

:ArchibaldWavell1stEarlWavell :image "Archibald Wavell2.jpg";
  :wikiurl "https://id.wikipedia.org/wiki/Archibald_Wavell,_1st_Earl_Wavell" .

:KarelDoorman :image "Karel_Doorman_as_lieutenant-commander.jpg";
  :wikiurl "https://id.wikipedia.org/wiki/Karel_Doorman" .

:HamengkubuwanaIX :image "Hamengkubawono_IX_Official_Portrait.jpg";
  :wikiurl "https://id.wikipedia.org/wiki/Hamengkubuwana_IX" .

:VentjeSumual :image "https://mmc.tirto.id/image/2017/03/02/TIRTO_2106LetkolVentjeSumual_square.JPG";
  :wikiurl "https://id.wikipedia.org/wiki/Ventje_Sumual" .

:Soeharto :image "President_Suharto,_1993.jpg";
  :wikiurl "https://id.wikipedia.org/wiki/Soeharto" .

:LeslieMorshead :image "Morshead_(AWM_009517).jpg";
  :wikiurl "https://id.wikipedia.org/wiki/Leslie_Morshead" .

:SusiloBambangYudhoyono :image "Presiden_Susilo_Bambang_Yudhoyono.png";
  :wikiurl "https://id.wikipedia.org/wiki/Susilo_Bambang_Yudhoyono" .

:SaalahYusufSutanMangkuto :image "SY_Sutan_Mangkuto.jpg";
  :wikiurl "https://id.wikipedia.org/wiki/Saalah_Yusuf_Sutan_Mangkuto" .

:WilhelminadariBelanda :image "Jacob_Merkelbach,_Afb_010164033306.jpg";
  :wikiurl "https://id.wikipedia.org/wiki/Wilhelmina_dari_Belanda" .

:LeonardusBenyaminMoerdani :image "Leonardus Benjamin Moerdani as Commander of the Indonesian National Armed Forces.jpg";
  :wikiurl "https://id.wikipedia.org/wiki/Leonardus_Benyamin_Moerdani" .

:MarufAmin :image "Ma'ruf_Amin_2019_official_portrait.jpg";
  :wikiurl "https://id.wikipedia.org/wiki/Ma%27ruf_Amin" .

:MegawatiSoekarnoputri :image "President_Megawati_Sukarnoputri_-_Indonesia.jpg";
  :wikiurl "https://id.wikipedia.org/wiki/Megawati_Soekarnoputri" .

:TBSimatupang :image "Kolonel_Simatoepang_Chef-staf_van_de_TNI,_uitgever_van_de_order_\"staakt_het_vure,_Bestanddeelnr_344030_010.jpg";
  :wikiurl "https://id.wikipedia.org/wiki/T.B._Simatupang" .

:AdamBB :image "Syekh_Adam_BB.jpg";
  :wikiurl "https://id.wikipedia.org/wiki/Adam_B.B." .

:Wiranto :image "Wiranto2.jpg";
  :wikiurl "https://id.wikipedia.org/wiki/Wiranto" .

:SyarifHamidIIdariPontianak :image "Syarif_Hamid_II_of_Pontianak.jpg";
  :wikiurl "https://id.wikipedia.org/wiki/Syarif_Hamid_II_dari_Pontianak" .

:PhilipChristison :image "https://asset.kompas.com/crops/26NcBHvtwCkAdI8GxsAkg3mMHxM=/0x56:549x422/750x500/data/photo/2021/08/17/611bbaf6c9217.jpeg";
  :wikiurl "https://id.wikipedia.org/wiki/Philip_Christison" .

:BennyWenda :image "Benny_Wenda.png";
  :wikiurl "https://id.wikipedia.org/wiki/Benny_Wenda" .

:AbdulkadirWidjojoatmodjo :image "Voorzitter_van_de_Nederlandse_delegatie_op_de_Renville_Abdoel_Kadir,_Bestanddeelnr_902-5011_(3x4).jpg";
  :wikiurl "https://id.wikipedia.org/wiki/Abdulkadir_Widjojoatmodjo" .

:JacobPrai :image "https://www.ulmwp.org/wp-content/uploads/2022/06/287230120_3152293418408468_6921440470420884462_n-768x541.jpg";
  :wikiurl "https://id.wikipedia.org/wiki/Jacob_Prai" .

:AbdulKaharMuzakkar :image "Kaharmuzakkar.jpg";
  :wikiurl "https://id.wikipedia.org/wiki/Abdul_Kahar_Muzakkar" .

:IsmaelLengah :image "https://asset.kompas.com/crops/dnVXmfGXkoUifmdX37ydnOPlKeY=/0x166:1000x833/750x500/data/photo/2023/03/15/64111c9ba8710.jpeg";
  :wikiurl "https://id.wikipedia.org/wiki/Ismael_Lengah" .

:TrySutrisno :image "Try_Sutrisno_Official_Portrait.jpg";
  :wikiurl "https://id.wikipedia.org/wiki/Try_Sutrisno" .

:PakubuwanaXII :image "SSISKS_Pakubuwono_XII.jpg";
  :wikiurl "https://id.wikipedia.org/wiki/Pakubuwana_XII" .

:MangkunegaraVIII :image "Raden_Mas_Saroso_Notosoeparto,_de_latere_Mangkoe_Nagoro_VIII.jpg";
  :wikiurl "https://id.wikipedia.org/wiki/Mangkunegara_VIII" .

:AchmadiHadisoemarto :image "Achmadi_Hadisumarto.png";
  :wikiurl "https://id.wikipedia.org/wiki/Achmadi_Hadisoemarto" .

:JokoWidodo :image "Joko_Widodo_2019_official_portrait.jpg";
  :wikiurl "https://id.wikipedia.org/wiki/Joko_Widodo" .

:JacobRumbiak :image "https://www.ulmwp.org/wp-content/uploads/2016/04/jacob-rumbiak-foreign-affairs-minister-federated-republic-of-west-papua.jpg";
  :wikiurl "https://id.wikipedia.org/wiki/Jacob_Rumbiak" .

:SekarmadjiMaridjanKartosoewirjo :image "Kartosuwirjo_17_August_1950_KR.jpg";
  :wikiurl "https://id.wikipedia.org/wiki/Sekarmadji_Maridjan_Kartosoewirjo" .

:AmirSjarifoeddin :image "Amir_Sjarifoeddin.jpg";
  :wikiurl "https://id.wikipedia.org/wiki/Amir_Sjarifoeddin" .

:AgustinusAdisoetjipto :image "Potret_Adisucipto.jpg";
  :wikiurl "https://id.wikipedia.org/wiki/Agustinus_Adisoetjipto" .

:AbdurrahmanWahid :image "President_Abdurrahman_Wahid_-_Indonesia.jpg";
  :wikiurl "https://id.wikipedia.org/wiki/Abdurrahman_Wahid" .

:JulianadariBelanda :image "Prinses_Juliana_1981.jpg";
  :wikiurl "https://id.wikipedia.org/wiki/Juliana_dari_Belanda" .

:wikipediaBandungLautanApi :wikiurl "https://id.wikipedia.org/wiki/Bandung_Lautan_Api";
  sem:hasActor :MacDonald, :MuhammadToha, :AbdulHarisNasution, :KerajaanBelanda, :RepublikIndonesia .

:wikipediaPemberontakanDITIIdiAceh :wikiurl "https://id.wikipedia.org/wiki/Pemberontakan_DI/TII_di_Aceh" .

:wikipediaDelapanJamPertempurandiMangkang :wikiurl "https://id.wikipedia.org/wiki/Delapan_Jam_Pertempuran_di_Mangkang" .

:wikipediaPeristiwa19November :wikiurl "https://id.wikipedia.org/wiki/Peristiwa_19_November" .

:PangSuma :wikiurl "https://id.wikipedia.org/wiki/Pang_Suma" .

:LoaSekHie :wikiurl "https://id.wikipedia.org/wiki/Loa_Sek_Hie" .

sem:Actor <http://www.w3.org/2004/02/skos/core#broadMatch> <http://sw.opencyc.org/2009/04/07/concept/en/SomethingExisting>,
    <http://www.loa-cnr.it/ontologies/DOLCE-Lite.owl#endurant>;
  <http://www.w3.org/2004/02/skos/core#closeMatch> <http://purl.org/dc/terms/Agent>,
    <http://purl.org/dc/terms/AgentClass>, <http://sw.opencyc.org/2009/04/07/concept/en/Agent-Generic>,
    <http://www.ontologyportal.org/translations/SUMO.owl.txt#Agent>, <http://www8.informatik.uni-erlangen.de/IMMD8/Services/cidoc-crm/erlangen-crm_090330_5_0_1.owl#E39.Actor>,
    foaf:Agent .

sem:Event <http://www.w3.org/2004/02/skos/core#broadMatch> <http://linkedevents.org/ontology/Event>,
    <http://purl.org/NET/c4dm/event.owl#Event>;
  <http://www.w3.org/2004/02/skos/core#closeMatch> <http://purl.org/dc/dcmitype/Event>,
    <http://sw.opencyc.org/2009/04/07/concept/en/Situation>, <http://www.loa-cnr.it/ontologies/DOLCE-Lite.owl#perdurant>,
    <http://www.ontologyportal.org/translations/SUMO.owl.txt#Process>, <http://www8.informatik.uni-erlangen.de/IMMD8/Services/cidoc-crm/erlangen-crm_090330_5_0_1.owl#E5.Event> .

sem:hasTime <http://www.w3.org/2004/02/skos/core#broadMatch> <http://linkedevents.org/ontology/atTime> .

sem:Time <http://www.w3.org/2004/02/skos/core#broadMatch> <http://www.w3.org/2006/timeTemporalEntity> .

sem:Object <http://www.w3.org/2004/02/skos/core#broadMatch> <http://sw.opencyc.org/2009/04/07/concept/en/SomethingExisting>,
    <http://www.loa-cnr.it/ontologies/DOLCE-Lite.owl#endurant>;
  <http://www.w3.org/2004/02/skos/core#closeMatch> <http://www.ontologyportal.org/translations/SUMO.owl.txt#Object>,
    <http://www8.informatik.uni-erlangen.de/IMMD8/Services/cidoc-crm/erlangen-crm_090330_5_0_1.owl#E19.Physical_Object>,
    <http://www8.informatik.uni-erlangen.de/IMMD8/Services/cidoc-crm/erlangen-crm_090330_5_0_1.owl#E21.Person>;
  <http://www.w3.org/2004/02/skos/core#narrowMatch> <http://purl.org/NET/c4dm/event.owl#Factor>,
    <http://purl.org/NET/c4dm/event.owl#Product>, <http://purl.org/dc/dcmitype/PhysicalObject>,
    <http://purl.org/dc/terms/PhysicalResource> .

sem:type <http://www.w3.org/2004/02/skos/core#closeMatch> dc:type;
  <http://www.w3.org/2004/02/skos/core#relatedMatch> <http://www.kulttuurisampo.fi/ebkr/quality> .

sem:Place <http://www.w3.org/2004/02/skos/core#closeMatch> <http://purl.org/dc/terms/Location>,
    <http://sw.opencyc.org/2009/04/07/concept/en/EnduringThing-Localized>, <http://www.ontologyportal.org/translations/SUMO.owl.txt#GeographicArea>,
    <http://www8.informatik.uni-erlangen.de/IMMD8/Services/cidoc-crm/erlangen-crm_090330_5_0_1.owl#E53.Place>;
  <http://www.w3.org/2004/02/skos/core#narrowMatch> <http://www.loa-cnr.it/ontologies/DOLCE-Lite.owl#PhysicalRegion>,
    wgs:SpatialThing .

sem:Type <http://www.w3.org/2004/02/skos/core#closeMatch> <http://www.loa-cnr.it/ontologies/DOLCE-Lite.owl#AbstractRegion>,
    <http://www8.informatik.uni-erlangen.de/IMMD8/Services/cidoc-crm/erlangen-crm_090330_5_0_1.owl#E55.Type> .

sem:hasTimeStamp <http://www.w3.org/2004/02/skos/core#closeMatch> <http://www.kulttuurisampo.fi/ebkr/time> .

geo:asWKT <http://www.w3.org/2004/02/skos/core#definition> "The WKT serialization of a Geometry"@en;
  <http://www.w3.org/2004/02/skos/core#example> <http://www.opengis.net/spec/geosparql/1.1/specification.html#C.1.2.2>,
    <http://www.opengis.net/spec/geosparql/1.1/specification.html#C.2.1>, <http://www.opengis.net/spec/geosparql/1.1/specification.html#C.1.1.2.4>,
    <http://www.opengis.net/spec/geosparql/1.1/specification.html#C.1.1.2.2>, <http://www.opengis.net/spec/geosparql/1.1/specification.html#C.1.1.2.3>,
    <http://www.opengis.net/spec/geosparql/1.1/specification.html#C.1.1.2.5>, <http://www.opengis.net/spec/geosparql/1.1/specification.html#C.1.1.2.6>,
    <http://www.opengis.net/spec/geosparql/1.1/specification.html#C.1.1.2.8>, <http://www.opengis.net/spec/geosparql/1.1/specification.html#C.1.1.3.2>,
    <http://www.opengis.net/spec/geosparql/1.1/specification.html#C.1.1.3.3>, <http://www.opengis.net/spec/geosparql/1.1/specification.html#C.1.1.3.1>,
    <http://www.opengis.net/spec/geosparql/1.1/specification.html#C.2.2.4>;
  <http://www.w3.org/2004/02/skos/core#prefLabel> "as WKT"@en .

geo:asGML <http://www.w3.org/2004/02/skos/core#definition> "The GML serialization of a Geometry"@en;
  <http://www.w3.org/2004/02/skos/core#example> <http://www.opengis.net/spec/geosparql/1.1/specification.html#C.1.2.4>;
  <http://www.w3.org/2004/02/skos/core#prefLabel> "as GML"@en .

geo:hasDefaultGeometry <http://www.w3.org/2004/02/skos/core#definition> "The default Geometry to be used in spatial calculations. It is usually the most detailed Geometry."@en;
  <http://www.w3.org/2004/02/skos/core#note> "Duplicate properties defaultGeometry and hasDefaultGeometry exist because of an inconsistency between ontology and documentation in GeoSPARQL 1.0. Only hasDefaultGeometry is described in the documention."@en;
  <http://www.w3.org/2004/02/skos/core#prefLabel> "has default geometry"@en .

geo:sfEquals <http://www.w3.org/2004/02/skos/core#definition> "States that the subject SpatialObject spatially equals the object SpatialObject. DE-9IM: TFFFTFFFT"@en;
  <http://www.w3.org/2004/02/skos/core#prefLabel> "equals"@en .

geo:sfDisjoint <http://www.w3.org/2004/02/skos/core#definition> "States that the subject SpatialObject is spatially disjoint from the object SpatialObject. DE-9IM: FF*FF****"@en;
  <http://www.w3.org/2004/02/skos/core#prefLabel> "disjoint"@en .

geo:sfIntersects <http://www.w3.org/2004/02/skos/core#definition> "States that the subject SpatialObject is not spatially disjoint from the object SpatialObject. DE-9IM: T******** ^ *T******* ^ ***T***** ^ ****T****"@en;
  <http://www.w3.org/2004/02/skos/core#prefLabel> "intersects"@en .

geo:sfTouches <http://www.w3.org/2004/02/skos/core#definition> "States that the subject SpatialObject spatially touches the object SpatialObject. DE-9IM: FT******* ^ F**T***** ^ F***T****"@en;
  <http://www.w3.org/2004/02/skos/core#prefLabel> "touches"@en .

geo:sfWithin <http://www.w3.org/2004/02/skos/core#definition> "States that the subject SpatialObject is spatially within the object SpatialObject. DE-9IM: T*F**F***"@en;
  <http://www.w3.org/2004/02/skos/core#prefLabel> "within"@en .

geo:sfContains <http://www.w3.org/2004/02/skos/core#definition> "States that the subject SpatialObject spatially contains the object SpatialObject. DE-9IM: T*****FF*"@en;
  <http://www.w3.org/2004/02/skos/core#prefLabel> "contains"@en .

geo:sfOverlaps <http://www.w3.org/2004/02/skos/core#definition> "States that the subject SpatialObject spatially overlaps the object SpatialObject. DE-9IM: T*T***T**"@en;
  <http://www.w3.org/2004/02/skos/core#prefLabel> "overlaps"@en .

geo:sfCrosses <http://www.w3.org/2004/02/skos/core#definition> "States that the subject SpatialObject spatially crosses the object SpatialObject. DE-9IM: T*T******"@en;
  <http://www.w3.org/2004/02/skos/core#prefLabel> "crosses"@en .

geo:ehEquals <http://www.w3.org/2004/02/skos/core#definition> "States that the subject SpatialObject spatially equals the object SpatialObject. DE-9IM: TFFFTFFFT"@en;
  <http://www.w3.org/2004/02/skos/core#prefLabel> "equals"@en .

geo:ehDisjoint <http://www.w3.org/2004/02/skos/core#definition> "States that the subject SpatialObject is spatially disjoint from the object SpatialObject. DE-9IM: FF*FF****"@en;
  <http://www.w3.org/2004/02/skos/core#prefLabel> "disjoint"@en .

geo:ehMeet <http://www.w3.org/2004/02/skos/core#definition> "States that the subject SpatialObject spatially meets the object SpatialObject. DE-9IM: FT******* ^ F**T***** ^ F***T****"@en;
  <http://www.w3.org/2004/02/skos/core#prefLabel> "meet"@en .

geo:ehOverlap <http://www.w3.org/2004/02/skos/core#definition> "States that the subject SpatialObject spatially overlaps the object SpatialObject. DE-9IM: T*T***T**"@en;
  <http://www.w3.org/2004/02/skos/core#prefLabel> "overlap"@en .

geo:ehCovers <http://www.w3.org/2004/02/skos/core#definition> "States that the subject SpatialObject spatially covers the object SpatialObject. DE-9IM: T*TFT*FF*"@en;
  <http://www.w3.org/2004/02/skos/core#prefLabel> "covers"@en .

geo:ehCoveredBy <http://www.w3.org/2004/02/skos/core#definition> "States that the subject SpatialObject is spatially covered by the object SpatialObject. DE-9IM: TFF*TFT**"@en;
  <http://www.w3.org/2004/02/skos/core#prefLabel> "covered by"@en .

geo:ehInside <http://www.w3.org/2004/02/skos/core#definition> "States that the subject SpatialObject is spatially inside the object SpatialObject. DE-9IM: TFF*FFT**"@en;
  <http://www.w3.org/2004/02/skos/core#prefLabel> "inside"@en .

geo:ehContains <http://www.w3.org/2004/02/skos/core#definition> "States that the subject SpatialObject spatially contains the object SpatialObject. DE-9IM: T*TFF*FF*"@en;
  <http://www.w3.org/2004/02/skos/core#prefLabel> "contains"@en .

geo:rcc8eq <http://www.w3.org/2004/02/skos/core#definition> "States that the subject SpatialObject spatially equals the object SpatialObject. DE-9IM: TFFFTFFFT"@en;
  <http://www.w3.org/2004/02/skos/core#prefLabel> "equals"@en .

geo:rcc8dc <http://www.w3.org/2004/02/skos/core#definition> "States that the subject SpatialObject is spatially disjoint from the object SpatialObject. DE-9IM: FFTFFTTTT"@en;
  <http://www.w3.org/2004/02/skos/core#prefLabel> "disconnected"@en .

geo:rcc8ec <http://www.w3.org/2004/02/skos/core#definition> "States that the subject SpatialObject spatially meets the object SpatialObject. DE-9IM: FFTFTTTTT"@en;
  <http://www.w3.org/2004/02/skos/core#prefLabel> "externally connected"@en .

geo:rcc8po <http://www.w3.org/2004/02/skos/core#definition> "States that the subject SpatialObject spatially overlaps the object SpatialObject. DE-9IM: TTTTTTTTT"@en;
  <http://www.w3.org/2004/02/skos/core#prefLabel> "partially overlapping"@en .

geo:rcc8tppi <http://www.w3.org/2004/02/skos/core#definition> "States that the subject SpatialObject spatially covers the object SpatialObject. DE-9IM: TTTFTTFFT"@en;
  <http://www.w3.org/2004/02/skos/core#prefLabel> "tangential proper part inverse"@en .

geo:rcc8tpp <http://www.w3.org/2004/02/skos/core#definition> "States that the subject SpatialObject is spatially covered by the object SpatialObject. DE-9IM: TFFTTFTTT"@en;
  <http://www.w3.org/2004/02/skos/core#prefLabel> "tangential proper part"@en .

geo:rcc8ntpp <http://www.w3.org/2004/02/skos/core#definition> "States that the subject SpatialObject is spatially inside the object SpatialObject. DE-9IM: TFFTFFTTT"@en;
  <http://www.w3.org/2004/02/skos/core#prefLabel> "non-tangential proper part"@en .

geo:rcc8ntppi <http://www.w3.org/2004/02/skos/core#definition> "States that the subject SpatialObject spatially contains the object SpatialObject. DE-9IM: TTTFFTFFT"@en;
  <http://www.w3.org/2004/02/skos/core#prefLabel> "non-tangential proper part inverse"@en .

geo:dggsLiteral <http://www.w3.org/2004/02/skos/core#definition> "A textual serialization of a Discrete Global Grid (DGGS) Geometry object."@en;
  <http://www.w3.org/2004/02/skos/core#example> <http://www.opengis.net/spec/geosparql/1.1/specification.html#C.1.2.4>,
    " \"<https://w3id.org/dggs/auspix> OrdinateList (R3234)\"^^<http://www.opengis.net/ont/geosparql#dggsLiteral>";
  <http://www.w3.org/2004/02/skos/core#prefLabel> "DGGS Literal"@en;
  <http://www.w3.org/2004/02/skos/core#scopeNote> "This datatype is not expected to be used directly but to serve as an abstract datatype for a series of specific DGGS literal types, for specific DGGS implementations"@en .

geo:geoJSONLiteral <http://www.w3.org/2004/02/skos/core#definition> "A GeoJSON serialization of a Geometry object."@en;
  <http://www.w3.org/2004/02/skos/core#example> <http://www.opengis.net/spec/geosparql/1.1/specification.html#C.1.2.4>;
  <http://www.w3.org/2004/02/skos/core#prefLabel> "GeoJSON Literal"@en .

geo:gmlLiteral <http://www.w3.org/2004/02/skos/core#definition> "A GML serialization of a Geometry object."@en;
  <http://www.w3.org/2004/02/skos/core#example> <http://www.opengis.net/spec/geosparql/1.1/specification.html#C.1.2.4>;
  <http://www.w3.org/2004/02/skos/core#prefLabel> "GML Literal"@en .

geo:kmlLiteral <http://www.w3.org/2004/02/skos/core#definition> "A KML serialization of a Geometry object."@en;
  <http://www.w3.org/2004/02/skos/core#example> <http://www.opengis.net/spec/geosparql/1.1/specification.html#C.1.2.4>;
  <http://www.w3.org/2004/02/skos/core#prefLabel> "KML Literal"@en .

geo:wktLiteral <http://www.w3.org/2004/02/skos/core#definition> "A Well-known Text serialization of a Geometry object."@en;
  <http://www.w3.org/2004/02/skos/core#example> <http://www.opengis.net/spec/geosparql/1.1/specification.html#C.2.2.2>;
  <http://www.w3.org/2004/02/skos/core#prefLabel> "Well-known Text Literal"@en .

time:generalDay <http://www.w3.org/2004/02/skos/core#definition> """Day of month - formulated as a text string with a pattern constraint to reproduce the same lexical form as gDay, except that values up to 99 are permitted, in order to support calendars with more than 31 days in a month. 
Note that the value-space is not defined, so a generic OWL2 processor cannot compute ordering relationships of values of this type."""@en,
    """Da del mes - formulado como una cadena de texto con una restriccin patrn para reproducir la misma forma lxica que gDay, excepto que se permiten valores hasta el 99, con el propsito de proporcionar soporte a calendarios con meses con ms de 31 das.
            Ntese que el espacio de valores no est definido, por tanto, un procesador genrico de OWL2 no puede computar relaciones de orden de valores de este tipo."""@es .

time:generalMonth <http://www.w3.org/2004/02/skos/core#definition> """Mes del ao - formulado como una cadena de texto con una restriccin patrn para reproducir la misma forma lxica que gMonth, excepto que se permiten valores hasta el 20, con el propsito de proporcionar soporte a calendarios con aos con ms de 12 meses.
            Ntese que el espacio de valores no est definido, por tanto, un procesador genrico de OWL2 no puede computar relaciones de orden de valores de este tipo."""@es,
    """Month of year - formulated as a text string with a pattern constraint to reproduce the same lexical form as gMonth, except that values up to 20 are permitted, in order to support calendars with more than 12 months in the year. 
Note that the value-space is not defined, so a generic OWL2 processor cannot compute ordering relationships of values of this type."""@en .

time:generalYear <http://www.w3.org/2004/02/skos/core#definition> """Nmero de ao - formulado como una cadena de texto con una restriccin patrn para reproducir la misma forma lxica que gYear, aunque no est restringido a valores del calendario gregoriano.
            Ntese que el espacio de valores no est definido, por tanto, un procesador genrico de OWL2 no puede computar relaciones de orden de valores de este tipo."""@es,
    """Year number - formulated as a text string with a pattern constraint to reproduce the same lexical form as gYear, but not restricted to values from the Gregorian calendar. 
Note that the value-space is not defined, so a generic OWL2 processor cannot compute ordering relationships of values of this type."""@en .

geo:Feature <http://www.w3.org/2004/02/skos/core#definition> "A discrete spatial phenomenon in a universe of discourse."@en;
  <http://www.w3.org/2004/02/skos/core#example> <http://www.opengis.net/spec/geosparql/1.1/specification.html#C.1.2.4>,
    <http://www.opengis.net/spec/geosparql/1.1/specification.html#C.1.2.2>, <http://www.opengis.net/spec/geosparql/1.1/specification.html#C.1.1.2.4>,
    <http://www.opengis.net/spec/geosparql/1.1/specification.html#C.1.1.2.2>, <http://www.opengis.net/spec/geosparql/1.1/specification.html#C.1.1.2.3>,
    <http://www.opengis.net/spec/geosparql/1.1/specification.html#C.1.1.2.5>, <http://www.opengis.net/spec/geosparql/1.1/specification.html#C.1.1.2.6>,
    <http://www.opengis.net/spec/geosparql/1.1/specification.html#C.1.1.2.8>, <http://www.opengis.net/spec/geosparql/1.1/specification.html#C.1.1.3.2>,
    <http://www.opengis.net/spec/geosparql/1.1/specification.html#C.1.1.3.3>, <http://www.opengis.net/spec/geosparql/1.1/specification.html#C.1.2.3>,
    <http://www.opengis.net/spec/geosparql/1.1/specification.html#C.1.1.2.7>, <http://www.opengis.net/spec/geosparql/1.1/specification.html#C.1.1.2.9>,
    <http://www.opengis.net/spec/geosparql/1.1/specification.html#C.1.1.2.1>;
  <http://www.w3.org/2004/02/skos/core#note> "A Feature represents a uniquely identifiable phenomenon, for example a river or an apple. While such phenomena (and therefore the Features used to represent them) are bounded, their boundaries may be crisp (e.g., the declared boundaries of a state), vague (e.g., the delineation of a valley versus its neighboring mountains), and change with time (e.g., a storm front). While discrete in nature, Features may be created from continuous observations, such as an isochrone that determines the region that can be reached by ambulance within 5 minutes."@en;
  <http://www.w3.org/2004/02/skos/core#prefLabel> "Feature"@en .

time:TemporalEntity <http://www.w3.org/2004/02/skos/core#definition> "A temporal interval or instant."@en,
    "Un intervalo temporal o un instante."@es .

geo:defaultGeometry <http://www.w3.org/2004/02/skos/core#definition> "The default Geometry to be used in spatial calculations. It is usually the most detailed Geometry."@en;
  <http://www.w3.org/2004/02/skos/core#example> <http://www.opengis.net/spec/geosparql/1.1/specification.html#C.1.2.2>,
    <http://www.opengis.net/spec/geosparql/1.1/specification.html#C.2.1>;
  <http://www.w3.org/2004/02/skos/core#note> "Duplicate properties defaultGeometry and hasDefaultGeometry exist because of an inconsistency between ontology and documentation in GeoSPARQL 1.0. Only hasDefaultGeometry is described in the documention."@en;
  <http://www.w3.org/2004/02/skos/core#prefLabel> "default geometry"@en .

geo:hasGeometry <http://www.w3.org/2004/02/skos/core#definition> "A spatial representation for a given Feature."@en;
  <http://www.w3.org/2004/02/skos/core#example> <http://www.opengis.net/spec/geosparql/1.1/specification.html#C.1.2.4>,
    <http://www.opengis.net/spec/geosparql/1.1/specification.html#C.1.2.2>, <http://www.opengis.net/spec/geosparql/1.1/specification.html#C.1.1.2.4>,
    <http://www.opengis.net/spec/geosparql/1.1/specification.html#C.1.1.2.2>, <http://www.opengis.net/spec/geosparql/1.1/specification.html#C.1.1.2.3>,
    <http://www.opengis.net/spec/geosparql/1.1/specification.html#C.1.1.2.5>, <http://www.opengis.net/spec/geosparql/1.1/specification.html#C.1.1.2.6>,
    <http://www.opengis.net/spec/geosparql/1.1/specification.html#C.1.1.2.8>, <http://www.opengis.net/spec/geosparql/1.1/specification.html#C.1.1.3.2>,
    <http://www.opengis.net/spec/geosparql/1.1/specification.html#C.1.1.3.3>, <http://www.opengis.net/spec/geosparql/1.1/specification.html#C.1.2.3>,
    <http://www.opengis.net/spec/geosparql/1.1/specification.html#C.2>;
  <http://www.w3.org/2004/02/skos/core#prefLabel> "has geometry"@en .

geo:Geometry <http://www.w3.org/2004/02/skos/core#definition> "A coherent set of direct positions in space. The positions are held within a Spatial Reference System (SRS)."@en;
  <http://www.w3.org/2004/02/skos/core#example> <http://www.opengis.net/spec/geosparql/1.1/specification.html#C.1.2.4>,
    <http://www.opengis.net/spec/geosparql/1.1/specification.html#C.1.2.2>, <http://www.opengis.net/spec/geosparql/1.1/specification.html#C.1.1.2.4>,
    <http://www.opengis.net/spec/geosparql/1.1/specification.html#C.1.1.2.2>, <http://www.opengis.net/spec/geosparql/1.1/specification.html#C.1.1.2.3>,
    <http://www.opengis.net/spec/geosparql/1.1/specification.html#C.1.1.2.5>, <http://www.opengis.net/spec/geosparql/1.1/specification.html#C.1.1.2.6>,
    <http://www.opengis.net/spec/geosparql/1.1/specification.html#C.1.1.2.8>, <http://www.opengis.net/spec/geosparql/1.1/specification.html#C.1.1.3.2>,
    <http://www.opengis.net/spec/geosparql/1.1/specification.html#C.1.1.3.3>, <http://www.opengis.net/spec/geosparql/1.1/specification.html#C.1.2.3>,
    <http://www.opengis.net/spec/geosparql/1.1/specification.html#C.1.1.3.1>;
  <http://www.w3.org/2004/02/skos/core#note> "Geometry can be used as a representation of the shape, extent or location of a Feature and may exist as a self-contained entity."@en;
  <http://www.w3.org/2004/02/skos/core#prefLabel> "Geometry"@en .

geo:SpatialObject <http://www.w3.org/2004/02/skos/core#definition> "Anything spatial (being or having a shape, position or an extent)."@en;
  <http://www.w3.org/2004/02/skos/core#example> <http://www.opengis.net/spec/geosparql/1.1/specification.html#C.1.1.1.2>,
    <http://www.opengis.net/spec/geosparql/1.1/specification.html#C.1.1.1.1>;
  <http://www.w3.org/2004/02/skos/core#note> "Subclasses of this class are expected to be used for instance data."@en;
  <http://www.w3.org/2004/02/skos/core#prefLabel> "Spatial Object"@en .

geo:hasArea <http://www.w3.org/2004/02/skos/core#definition> "The area of a Spatial Object."@en;
  <http://www.w3.org/2004/02/skos/core#example> <http://www.opengis.net/spec/geosparql/1.1/specification.html#C.1.2.2>,
    <http://www.opengis.net/spec/geosparql/1.1/specification.html#C.1.1.2.4>;
  <http://www.w3.org/2004/02/skos/core#prefLabel> "has area"@en .

geo:hasSize <http://www.w3.org/2004/02/skos/core#definition> "Subproperties of this property are used to indicate the size of a Spatial Object as a measurement or estimate of one or more dimensions of the Spatial Object's spatial presence."@en;
  <http://www.w3.org/2004/02/skos/core#note> "The recommended way to specify size is by using a subproperty of hasMetricSize. Subproperties of hasSize can be used if more complex expressions are necessary, for example if the unit of length can not be converted to meter, or if additional data are needed to describe the measurement or estimate."@en;
  <http://www.w3.org/2004/02/skos/core#prefLabel> "has size"@en .

geo:hasBoundingBox <http://www.w3.org/2004/02/skos/core#definition> "The minimum or smallest bounding or enclosing box of a given Feature."@en;
  <http://www.w3.org/2004/02/skos/core#example> <http://www.opengis.net/spec/geosparql/1.1/specification.html#C.1.2.2>;
  <http://www.w3.org/2004/02/skos/core#prefLabel> "has bounding box"@en;
  <http://www.w3.org/2004/02/skos/core#scopeNote> "The target is a Geometry that defines a rectilinear region whose edges are aligned with the axes of the coordinate reference system, which exactly contains the Feature, for example an instance of http://www.opengis.net/ont/sf#envelope."@en .

geo:hasCentroid <http://www.w3.org/2004/02/skos/core#definition> "The arithmetic mean position of all the Geometry points of a given Feature."@en;
  <http://www.w3.org/2004/02/skos/core#example> <http://www.opengis.net/spec/geosparql/1.1/specification.html#C.1.2.2>;
  <http://www.w3.org/2004/02/skos/core#prefLabel> "has centroid"@en;
  <http://www.w3.org/2004/02/skos/core#scopeNote> "The target Geometry shall describe a point, for example an instance of http://www.opengis.net/ont/sf#Point."@en .

geo:hasLength <http://www.w3.org/2004/02/skos/core#definition> "The length of a Spatial Object."@en;
  <http://www.w3.org/2004/02/skos/core#example> <http://www.opengis.net/spec/geosparql/1.1/specification.html#C.1.2.2>,
    <http://www.opengis.net/spec/geosparql/1.1/specification.html#C.1.1.2.7>;
  <http://www.w3.org/2004/02/skos/core#prefLabel> "has length"@en .

geo:hasPerimeterLength <http://www.w3.org/2004/02/skos/core#definition> "The length of the perimeter of a Spatial Object."@en;
  <http://www.w3.org/2004/02/skos/core#example> <http://www.opengis.net/spec/geosparql/1.1/specification.html#C.1.1.1.2>;
  <http://www.w3.org/2004/02/skos/core#prefLabel> "has perimeter length"@en .

geo:hasSpatialAccuracy <http://www.w3.org/2004/02/skos/core#definition> "The positional accuracy of the coordinates of a Geometry."@en;
  <http://www.w3.org/2004/02/skos/core#example> <http://www.opengis.net/spec/geosparql/1.1/specification.html#C.1.2.3>;
  <http://www.w3.org/2004/02/skos/core#note> "Spatial accuracy is applicable when a Geometry is used to represent a Feature. It is expressed as a distance that indicates the truthfullness of the positions (coordinates) that define the Geometry. In this case accuracy defines a zone surrounding each coordinate within wich the real positions are known to be. The accuracy value defines this zone as a distance from the coordinate(s) in all directions (e.g. a line, a circle or a sphere, depending on spatial dimension)."@en;
  <http://www.w3.org/2004/02/skos/core#prefLabel> "has spatial accuracy"@en .

geo:hasSpatialResolution <http://www.w3.org/2004/02/skos/core#definition> "The spatial resolution of a Geometry."@en;
  <http://www.w3.org/2004/02/skos/core#example> <http://www.opengis.net/spec/geosparql/1.1/specification.html#C.1.2.2>;
  <http://www.w3.org/2004/02/skos/core#note> "Spatial resolution specifies the level of detail of a Geometry. It the smallest distinguishable distance between spatially adjacent coordinates."@en;
  <http://www.w3.org/2004/02/skos/core#prefLabel> "has spatial resolution"@en .

geo:hasVolume <http://www.w3.org/2004/02/skos/core#definition> "The volume of a three-dimensional Spatial Object."@en;
  <http://www.w3.org/2004/02/skos/core#example> <http://www.opengis.net/spec/geosparql/1.1/specification.html#C.1.2.2>;
  <http://www.w3.org/2004/02/skos/core#prefLabel> "has volume"@en .

time:after <http://www.w3.org/2004/02/skos/core#definition> "Asume una direccin en el tiempo. Si una entidad temporal T1 est despus de otra entidad temporal T2, entonces el principio de T1 est despus del final de T2."@es,
    "Gives directionality to time. If a temporal entity T1 is after another temporal entity T2, then the beginning of T1 is after the end of T2."@en .

time:before <http://www.w3.org/2004/02/skos/core#definition> "Asume una direccin en el tiempo. Si una entidad temporal T1 est antes que otra entidad temporal T2, entonces el final de T1 est antes que el principio de T2. As, \"antes\" se puede considerar bsica para instantes y derivada para intervalos."@es,
    "Gives directionality to time. If a temporal entity T1 is before another temporal entity T2, then the end of T1 is before the beginning of T2. Thus, \"before\" can be considered to be basic to instants and derived for intervals."@en .

time:dayOfWeek <http://www.w3.org/2004/02/skos/core#definition> "The day of week, whose value is a member of the class time:DayOfWeek"@en,
    "El da de la semana, cuyo valor es un miembro de la clase 'da de la semana'."@es .

time:GeneralDateTimeDescription <http://www.w3.org/2004/02/skos/core#definition> "Description of date and time structured with separate values for the various elements of a calendar-clock system"@en,
    "Descripcin de fecha y hora estructurada con valores separados para los distintos elementos de un sistema calendario-reloj.";
  <http://www.w3.org/2004/02/skos/core#note> "Algunas combinaciones de propiedades son redundantes - por ejemplo, dentro de un 'ao' especificado si se proporciona 'da del ao' entonces 'da' y 'mes' se pueden computar, y viceversa. Los valores individuales deberan ser consistentes entre ellos y con el calendario, indicado a travs del valor de la propiedad 'tiene TRS'."@es,
    "Some combinations of properties are redundant - for example, within a specified :year if :dayOfYear is provided then :day and :month can be computed, and vice versa. Individual values should be consistent with each other and the calendar, indicated through the value of the :hasTRS property." .

time:DayOfWeek <http://www.w3.org/2004/02/skos/core#definition> "El da de la semana"@es,
    "The day of week"@en;
  <http://www.w3.org/2004/02/skos/core#note> "La pertenencia a la clase 'da de la semana' est abierta, para permitir longitudes de semana alternativas y diferentes nombres de das."@es,
    "Membership of the class :DayOfWeek is open, to allow for alternative week lengths and different day names."@en .

time:hasBeginning <http://www.w3.org/2004/02/skos/core#definition> "Comienzo de una entidad temporal."@es,
    "Beginning of a temporal entity."@en .

time:hasTime <http://www.w3.org/2004/02/skos/core#definition> "Proporciona soporte a la asociacin de una entidad temporal (instante o intervalo) a cualquier cosa."@es,
    "Supports the association of a temporal entity (instant or interval) to any thing"@en .

time:Instant <http://www.w3.org/2004/02/skos/core#definition> "A temporal entity with zero extent or duration"@en,
    "Una entidad temporal con una extensin o duracin cero."@es .

time:hasDateTimeDescription <http://www.w3.org/2004/02/skos/core#definition> "Valor de intervalo de fecha-hora expresado como un valor estructurado. El principio y el final del intervalo coincide con los lmites del elemento ms corto en la descripcin."@es,
    "Value of DateTimeInterval expressed as a structured value. The beginning and end of the interval coincide with the limits of the shortest element in the description."@en .

time:DateTimeInterval <http://www.w3.org/2004/02/skos/core#definition> "'intervalo de fecha-hora' es una subclase de 'intervalo propio', definida utilizando el multi-elemento 'descripcin de fecha-hora'."@es,
    "DateTimeInterval is a subclass of ProperInterval, defined using the multi-element DateTimeDescription."@en;
  <http://www.w3.org/2004/02/skos/core#note> "'intervalo de fecha-hora' se puede utilizar slo para un intervalo cuyos lmites coinciden con un elemento de fecha-hora alineados con el calendario y la zona horaria indicados. Por ejemplo, aunque ambos tienen una duracin de un da, el intervalo de 24 horas que empieza en la media noche del comienzo del 8 mayo en Europa Central se puede expresar como un 'intervalo de fecha-hora', el intervalo de 24 horas que empieza a las 1:30pm no."@es,
    ":DateTimeInterval can only be used for an interval whose limits coincide with a date-time element aligned to the calendar and timezone indicated. For example, while both have a duration of one day, the 24-hour interval beginning at midnight at the beginning of 8 May in Central Europe can be expressed as a :DateTimeInterval, but the 24-hour interval starting at 1:30pm cannot."@en .

time:hasDuration <http://www.w3.org/2004/02/skos/core#definition> "Duracin de una entidad temporal, evento o actividad, o cosa, expresada como un valor escalado."@es,
    "Duration of a temporal entity, event or activity, or thing, expressed as a scaled value"@en .

time:hasTemporalDuration <http://www.w3.org/2004/02/skos/core#definition> "Duracin de una entidad temporal."@es,
    "Duration of a temporal entity."@en .

time:Duration <http://www.w3.org/2004/02/skos/core#definition> "Duracin de una extensin temporal expresada como un nmero escalado por una unidad temporal."@es,
    "Duration of a temporal extent expressed as a number scaled by a temporal unit"@en;
  <http://www.w3.org/2004/02/skos/core#note> "Alternativa a 'descripcin de tiempo' para proporcionar descripcin soporte a una duracin temporal diferente a utilizar un sistema de calendario/reloj."@es,
    "Alternative to time:DurationDescription to support description of a temporal duration other than using a calendar/clock system."@en .

time:hasDurationDescription <http://www.w3.org/2004/02/skos/core#definition> "Duracin de una entidad temporal, expresada utilizando una descripcin estructurada."@es,
    "Duration of a temporal entity, expressed using a structured description"@en .

time:GeneralDurationDescription <http://www.w3.org/2004/02/skos/core#definition> "Descripcin de extensin temporal estructurada con valores separados para los distintos elementos de un sistema de horario-calendario."@es,
    "Description of temporal extent structured with separate values for the various elements of a calendar-clock system."@en;
  <http://www.w3.org/2004/02/skos/core#note> "La extensin de una duracin de tiempo expresada como una 'descripcin de duracin general' depende del Sistema de Referencia Temporal. En algunos calendarios la longitud de la semana o del mes no es constante a lo largo del ao. Por tanto, un valor como \"25 meses\" puede no ser necesariamente ser comparado con un duracin similar expresada en trminos de semanas o das. Cuando se consideran calendarios que no estn basados en el movimiento de la Tierra, se deben tomar incluso ms precauciones en la comparacin de duraciones."@es,
    "The extent of a time duration expressed as a GeneralDurationDescription depends on the Temporal Reference System. In some calendars the length of the week or month is not constant within the year. Therefore, a value like \"2.5 months\" may not necessarily be exactly compared with a similar duration expressed in terms of weeks or days. When non-earth-based calendars are considered even more care must be taken in comparing durations."@en .

time:hasEnd <http://www.w3.org/2004/02/skos/core#definition> "End of a temporal entity."@en,
    "Final de una entidad temporal."@es .

time:hasTRS <http://www.w3.org/2004/02/skos/core#definition> "El sistema de referencia temporal utilizado por una posicin temporal o descripcin de extensin."@es,
    "The temporal reference system used by a temporal position or extent description. "@en .

time:TemporalPosition <http://www.w3.org/2004/02/skos/core#definition> "A position on a time-line"@en,
    "Una posicin sobre una lnea de tiempo."@es .

time:TRS <http://www.w3.org/2004/02/skos/core#definition> """A temporal reference system, such as a temporal coordinate system (with an origin, direction, and scale), a calendar-clock combination, or a (possibly hierarchical) ordinal system. 

This is a stub class, representing the set of all temporal reference systems."""@en,
    """Un sistema de referencia temporal, tal como un sistema de coordenadas temporales (con un origen, una direccin y una escala), una combinacin calendario-reloj, o un sistema ordinal (posiblemente jerrquico).
    Esta clase comodn representa el conjunto de todos los sistemas de referencia temporal."""@es;
  <http://www.w3.org/2004/02/skos/core#note> "A taxonomy of temporal reference systems is provided in ISO 19108:2002 [ISO19108], including (a) calendar + clock systems; (b) temporal coordinate systems (i.e. numeric offset from an epoch); (c) temporal ordinal reference systems (i.e. ordered sequence of named intervals, not necessarily of equal duration)."@en,
    "En el ISO 19108:2002 [ISO19108] se proporciona una taxonoma de sistemas de referencia temporal, incluyendo (a) sistemas de calendario + reloj; (b) sistemas de coordenadas temporales (es decir, desplazamiento numrico a partir de una poca); (c) sistemas de referencia ordinales temporales (es decir, secuencia ordenada de intervalos nombrados, no necesariamente de igual duracin)."@es .

time:TemporalDuration <http://www.w3.org/2004/02/skos/core#definition> "Extensin de tiempo; duracin de un intervalo de tiempo independiente de su posicin de inicio particular."@es,
    "Time extent; duration of a time interval separate from its particular start position"@en .

time:inDateTime <http://www.w3.org/2004/02/skos/core#definition> "Posicin de un instante, expresada utilizando una descripcin estructurada."@es,
    "Position of an instant, expressed using a structured description"@en .

time:inTemporalPosition <http://www.w3.org/2004/02/skos/core#definition> "Posicin de un instante de tiempo."@es,
    "Position of a time instant"@en .

time:inTimePosition <http://www.w3.org/2004/02/skos/core#definition> "Posicin de un instante, expresada como una coordenada temporal o un valor nominal."@es,
    "Position of a time instant expressed as a TimePosition"@en .

time:TimePosition <http://www.w3.org/2004/02/skos/core#definition> "A temporal position described using either a (nominal) value from an ordinal reference system, or a (numeric) value in a temporal coordinate system. "@en,
    "Una posicin temporal descrita utilizando bien un valor (nominal) de un sistema de referencia ordinal, o un valor (numrico) en un sistema de coordenadas temporales."@es .

time:inside <http://www.w3.org/2004/02/skos/core#definition> "An instant that falls inside the interval. It is not intended to include beginnings and ends of intervals."@en,
    "Un instante que cae dentro del intervalo. Se asume que no es ni el principio ni el final de ningn intervalo."@es .

time:Interval <http://www.w3.org/2004/02/skos/core#definition> "A temporal entity with an extent or duration"@en,
    "Una entidad temporal con una extensin o duracin."@es .

time:intervalAfter <http://www.w3.org/2004/02/skos/core#definition> "If a proper interval T1 is intervalAfter another proper interval T2, then the beginning of T1 is after the end of T2."@en,
    "Si un intervalo propio T1 es posterior a otro intervalo propio T2, entonces el principio de T1 est despus que el final de T2."@es .

time:intervalDisjoint <http://www.w3.org/2004/02/skos/core#definition> "If a proper interval T1 is intervalDisjoint another proper interval T2, then the beginning of T1 is after the end of T2, or the end of T1 is before the beginning of T2, i.e. the intervals do not overlap in any way, but their ordering relationship is not known."@en,
    "Si un intervalo propio T1 es disjunto con otro intervalo propio T2, entonces el principio de T1 est despus del final de T2, o el final de T1 est antes que el principio de T2, es decir, los intervalos no se solapan de ninguna forma, aunque su relacin de orden no se conozca."@es;
  <http://www.w3.org/2004/02/skos/core#note> "Esta relacin entre intervalos no estaba incluida en las 13 relaciones bsicas definidas por Allen (1984), pero est definida en T.3 como la unin de 'intervalo anterior' con 'intervalo posterior'. Sin embargo, esto est fuera de la expresividad de OWL2, por tanto, est implementado como una propiedad explcita, con 'intervalo anterior' e 'intervalo posterior' como sub-propiedades."@es,
    "This interval relation is not included in the 13 basic relationships defined in Allen (1984), but is defined in (T.3) as the union of :intervalBefore v :intervalAfter . However, that is outside OWL2 expressivity, so is implemented as an explicit property, with :intervalBefore , :intervalAfter as sub-properties"@en .

time:intervalBefore <http://www.w3.org/2004/02/skos/core#definition> "If a proper interval T1 is intervalBefore another proper interval T2, then the end of T1 is before the beginning of T2."@en,
    "Si un intervalo propio T1 est antes que otro intervalo propio T2, entonces el final de T1 est antes que el principio de T2."@es .

time:ProperInterval <http://www.w3.org/2004/02/skos/core#definition> "A temporal entity with non-zero extent or duration, i.e. for which the value of the beginning and end are different"@en,
    "Una entidad temporal con extensin o duracin distinta de cero, es decir, para la cual los valores de principio y fin del intervalo son diferentes."@es .

time:intervalContains <http://www.w3.org/2004/02/skos/core#definition> "If a proper interval T1 is intervalContains another proper interval T2, then the beginning of T1 is before the beginning of T2, and the end of T1 is after the end of T2."@en,
    "Si un intervalo propio T1 contiene otro intervalo propio T2, entonces el principio de T1 est antes que el principio de T2, y el final de T1 est despus del final de T2."@es .

time:intervalDuring <http://www.w3.org/2004/02/skos/core#definition> "If a proper interval T1 is intervalDuring another proper interval T2, then the beginning of T1 is after the beginning of T2, and the end of T1 is before the end of T2."@en,
    "Si un intervalo propio T1 est durante otro intervalo propio T2, entonces del principio de T1 est despus del principio de T2, y el final de T1 est antes que el final de T2."@es .

time:intervalIn <http://www.w3.org/2004/02/skos/core#definition> "If a proper interval T1 is intervalIn another proper interval T2, then the beginning of T1 is after the beginning of T2 or is coincident with the beginning of T2, and the end of T1 is before the end of T2, or is coincident with the end of T2, except that end of T1 may not be coincident with the end of T2 if the beginning of T1 is coincident with the beginning of T2."@en,
    "Si un intervalo propio T1 es un intervalo interior a otro intervalo propio T2, entonces el principio de T1 est despus del principio de T2 o coincide con el principio de T2, y el final de T1 est antes que el final de T2, o coincide con el final de T2, excepto que el final de T1 puede no coincidir con el final de T2 si el principio de T1 coincide con el principio de T2."@es;
  <http://www.w3.org/2004/02/skos/core#note> "Esta relacin entre intervalos no estaba incluida en las 13 relaciones bsicas definidas por Allen (1984), pero se hace referencia a ella como \"una relacin importante\" en Allen y Ferguson (1997). Es la unin disjunta de 'intervalo empieza', 'intervalo durante' y con 'intervalo termina'. Sin embargo, esto est fuera de la expresividad de OWL2, por tanto, se implementa como una propiedad explcita, con 'intervalo empieza', 'intervalo durante' e 'intervalo termina' como sub-propiedades."@es,
    "This interval relation is not included in the 13 basic relationships defined in Allen (1984), but is referred to as 'an important relationship' in Allen and Ferguson (1997). It is the disjoint union of :intervalStarts v :intervalDuring v :intervalFinishes . However, that is outside OWL2 expressivity, so is implemented as an explicit property, with :intervalStarts , :intervalDuring , :intervalFinishes as sub-properties"@en .

time:intervalEquals <http://www.w3.org/2004/02/skos/core#definition> "If a proper interval T1 is intervalEquals another proper interval T2, then the beginning of T1 is coincident with the beginning of T2, and the end of T1 is coincident with the end of T2."@en,
    "Si un intervalo propio T1 es igual a otro intervalo propio T2, entonces el principio de T1 coincide con el principio de T2, y el final de T1 coincide con el final de T2."@es .

time:intervalFinishedBy <http://www.w3.org/2004/02/skos/core#definition> "If a proper interval T1 is intervalFinishedBy another proper interval T2, then the beginning of T1 is before the beginning of T2, and the end of T1 is coincident with the end of T2."@en,
    "Si un intervalo propio T1 est terminado por otro intervalo propio T2, entonces el principio de T1 est antes que el principio de T2, y el final de T1 coincide con el final de T2."@es .

time:intervalFinishes <http://www.w3.org/2004/02/skos/core#definition> "If a proper interval T1 is intervalFinishes another proper interval T2, then the beginning of T1 is after the beginning of T2, and the end of T1 is coincident with the end of T2."@en,
    "Si un intervalo propio T1 termina otro intervalo propio T2, entonces del principio de T1 est despus del principio de T2, y el final de T1 coincide con el final de T2."@es .

time:intervalMeets <http://www.w3.org/2004/02/skos/core#definition> "If a proper interval T1 is intervalMeets another proper interval T2, then the end of T1 is coincident with the beginning of T2."@en,
    "Si un intervalo propio T1 se encuentra con otro intervalo propio T2, entonces el final de T1 coincide con el principio de T2."@es .

time:intervalMetBy <http://www.w3.org/2004/02/skos/core#definition> "If a proper interval T1 is intervalMetBy another proper interval T2, then the beginning of T1 is coincident with the end of T2."@en,
    "Si un intervalo propio T1 es 'intervalo encontrado por' otro intervalo propio T2, entonces el principio de T1 coincide con el final de T2."@es .

time:intervalOverlappedBy <http://www.w3.org/2004/02/skos/core#definition> "If a proper interval T1 is intervalOverlappedBy another proper interval T2, then the beginning of T1 is after the beginning of T2, the beginning of T1 is before the end of T2, and the end of T1 is after the end of T2."@en,
    "Si un intervalo propio T1 es 'intervalo solapado por' otro intervalo propio T2, entonces el principio de T1 es posterior al principio de T2, y el principio de T1 es anterior al final de T2, y el final de T1 es posterior al final de T2."@es .

time:intervalOverlaps <http://www.w3.org/2004/02/skos/core#definition> "If a proper interval T1 is intervalOverlaps another proper interval T2, then the beginning of T1 is before the beginning of T2, the end of T1 is after the beginning of T2, and the end of T1 is before the end of T2."@en,
    "Si un intervalo propio T1 se solapa con otro intervalo propio T2, entonces el principio de T1 es anterior al principio de T2, el final de T1 es posterior al principio de T2, y el final de T1 es anterior al final de T2."@es .

time:intervalStartedBy <http://www.w3.org/2004/02/skos/core#definition> "If a proper interval T1 is intervalStarted another proper interval T2, then the beginning of T1 is coincident with the beginning of T2, and the end of T1 is after the end of T2."@en,
    "Si un intervalo propio T1 es empezado por otro intervalo propio T2, entonces el principio de T1 coincide con el principio de T2, y el final de T1 es posterior al final de T2."@es .

time:intervalStarts <http://www.w3.org/2004/02/skos/core#definition> "If a proper interval T1 is intervalStarts another proper interval T2, then the beginning of T1 is coincident with the beginning of T2, and the end of T1 is before the end of T2."@en,
    "Si un intervalo propio T1 empieza otro intervalo propio T2, entonces del principio de T1 con el final de T2, y el final de T1 es anterior al final de T2."@es .

time:monthOfYear <http://www.w3.org/2004/02/skos/core#definition> "El mes del ao, cuyo valor es un miembro de la clase 'mes del ao'."@es,
    "The month of the year, whose value is a member of the class time:MonthOfYear"@en .

time:MonthOfYear <http://www.w3.org/2004/02/skos/core#definition> "El mes del ao."@es,
    "The month of the year"@en;
  <http://www.w3.org/2004/02/skos/core#note> "La pertenencia a la clase 'mes del ao' est abierta, a permitir calendarios anuales alternativos y diferentes nombres de meses."@es,
    "Membership of the class :MonthOfYear is open, to allow for alternative annual calendars and different month names."@en .

time:TimeZone <http://www.w3.org/2004/02/skos/core#definition> """A Time Zone specifies the amount by which the local time is offset from UTC. 
	A time zone is usually denoted geographically (e.g. Australian Eastern Daylight Time), with a constant value in a given region. 
The region where it applies and the offset from UTC are specified by a locally recognised governing authority."""@en,
    """Un huso horario especifica la cantidad en que la hora local est desplazada con respecto a UTC.
    Un huso horario normalmente se denota geogrficamente (p.ej. el horario de verano del este de Australia), con un valor constante en una regin dada.
    La regin donde aplica y el desplazamiento desde UTC las especifica una autoridad gubernamental localmente reconocida."""@es;
  <http://www.w3.org/2004/02/skos/core#note> """A designated timezone is associated with a geographic region. However, for a particular region the offset from UTC often varies seasonally, and the dates of the changes may vary from year to year. The timezone designation usually changes for the different seasons (e.g. Australian Eastern Standard Time vs. Australian Eastern Daylight Time). Furthermore, the offset for a timezone may change over longer timescales, though its designation might not.  

Detailed guidance about working with time zones is given in http://www.w3.org/TR/timezone/ ."""@en,
    "An ontology for time zone descriptions was described in [owl-time-20060927] and provided as RDF in a separate namespace tzont:. However, that ontology was incomplete in scope, and the example datasets were selective. Furthermore, since the use of a class from an external ontology as the range of an ObjectProperty in OWL-Time creates a dependency, reference to the time zone class has been replaced with the 'stub' class in the normative part of this version of OWL-Time."@en,
    """Un huso horario designado est asociado con una regin geogrfica. Sin embargo, para una regin particular el desplazamiento desde UTC a menudo vara segn las estaciones, y las fechas de los cambios pueden variar de un ao a otro. La designacin de huso horario  normalmente cambia de una estacin a otra (por ejemplo, el horario estndar frente al horario de verano ambos del este de Australia). Adems, del desplazamiento para un huso horario puede cambiar sobre escalas de tiempo mayores, aunque su designacin no lo haga.
    Se puede encontrar una gua detallada sobre el funcionamiento de husos horarios en http://www.w3.org/TR/timezone/.\"@es , \"En [owl-time-20060927] se describi una ontologa para descripciones de husos horarios, y se proporcion en un espacio de nombres separado tzont:. Sin embargo, dicha ontologa estaba incompleta en su alcance, y el ejemplo de conjuntos de datos (datasets) era selectivo. Adems, puesto que el uso de una clase de una ontologa externa como el rango de una propiedad de objeto en OWL-Time crea una dependencia, la referencia a la clase huso horario se ha reemplazado por una clase que viene a ser un \"cajn de sastre\" en la en la parte normativa de esta versin de OWL-Time."""@es;
  <http://www.w3.org/2004/02/skos/core#scopeNote> "En esta implementacin 'huso horario' no tiene definidas propiedades. Se debera pensar como una superclase \"abstracta\" de todas las implementaciones de huso horario especficas."@es,
    "In this implementation TimeZone has no properties defined. It should be thought of as an 'abstract' superclass of all specific timezone implementations." .

time:TemporalUnit <http://www.w3.org/2004/02/skos/core#definition> "A standard duration, which provides a scale factor for a time extent, or the granularity or precision for a time position."@en,
    "Una duracin estndar, que proporciona un factor de escala para una extensin de tiempo, o la granularidad o precisin para una posicin de tiempo."@es;
  <http://www.w3.org/2004/02/skos/core#note> "La pertenencia de la clase 'unidad de tiempo' est abierta, para permitir otras unidades de tiempo utilizadas en algunas aplicaciones tcnicas (por ejemplo, millones de aos o el mes Baha'i)."@es,
    "Membership of the class TemporalUnit is open, to allow for other temporal units used in some technical applications (e.g. millions of years, Baha'i month)."@en .

geo:asDGGS <http://www.w3.org/2004/02/skos/core#definition> "The Discrete Global Grid System (DGGS) serialization of a Geometry"@en;
  <http://www.w3.org/2004/02/skos/core#example> <http://www.opengis.net/spec/geosparql/1.1/specification.html#C.1.2.4>;
  <http://www.w3.org/2004/02/skos/core#prefLabel> "as DGGS"@en .

geo:hasSerialization <http://www.w3.org/2004/02/skos/core#definition> "Connects a Geometry object with its text-based serialization."@en;
  <http://www.w3.org/2004/02/skos/core#example> <http://www.opengis.net/spec/geosparql/1.1/specification.html#C.1.2.3>;
  <http://www.w3.org/2004/02/skos/core#prefLabel> "has serialization"@en .

geo:asGeoJSON <http://www.w3.org/2004/02/skos/core#definition> "The GeoJSON serialization of a Geometry"@en;
  <http://www.w3.org/2004/02/skos/core#example> <http://www.opengis.net/spec/geosparql/1.1/specification.html#C.1.2.4>;
  <http://www.w3.org/2004/02/skos/core#prefLabel> "as GeoJSON"@en .

geo:asKML <http://www.w3.org/2004/02/skos/core#definition> "The KML serialization of a Geometry"@en;
  <http://www.w3.org/2004/02/skos/core#example> <http://www.opengis.net/spec/geosparql/1.1/specification.html#C.1.2.4>;
  <http://www.w3.org/2004/02/skos/core#prefLabel> "as KML"@en .

geo:coordinateDimension <http://www.w3.org/2004/02/skos/core#definition> "The number of measurements or axes needed to describe the position of this Geometry in a coordinate system."@en;
  <http://www.w3.org/2004/02/skos/core#example> <http://www.opengis.net/spec/geosparql/1.1/specification.html#C.1.2.3>;
  <http://www.w3.org/2004/02/skos/core#prefLabel> "coordinate dimension"@en .

geo:dimension <http://www.w3.org/2004/02/skos/core#definition> "The topological dimension of this geometric object, which must be less than or equal to the coordinate dimension. In non-homogeneous collections, this will return the largest topological dimension of the contained objects."@en;
  <http://www.w3.org/2004/02/skos/core#example> <http://www.opengis.net/spec/geosparql/1.1/specification.html#C.1.2.3>;
  <http://www.w3.org/2004/02/skos/core#prefLabel> "dimension"@en .

geo:hasMetricArea <http://www.w3.org/2004/02/skos/core#definition> "The area of a Spatial Object in square meters."@en;
  <http://www.w3.org/2004/02/skos/core#example> <http://www.opengis.net/spec/geosparql/1.1/specification.html#C.1.2.2>,
    <http://www.opengis.net/spec/geosparql/1.1/specification.html#C.1.1.2.3>, <http://www.opengis.net/spec/geosparql/1.1/specification.html#C.1.1.3.3>,
    <http://www.opengis.net/spec/geosparql/1.1/specification.html#C.1.1.2.9>;
  <http://www.w3.org/2004/02/skos/core#prefLabel> "has area in square meters"@en .

geo:hasMetricSize <http://www.w3.org/2004/02/skos/core#definition> "Subproperties of this property are used to indicate the size of a Spatial Object, as a measurement or estimate of one or more dimensions of the Spatial Object's spatial presence. Units are always metric (meter, square meter or cubic meter)."@en;
  <http://www.w3.org/2004/02/skos/core#prefLabel> "has metric size"@en .

geo:hasMetricLength <http://www.w3.org/2004/02/skos/core#definition> "The length of a Spatial Object in meters."@en;
  <http://www.w3.org/2004/02/skos/core#example> <http://www.opengis.net/spec/geosparql/1.1/specification.html#C.1.2.2>;
  <http://www.w3.org/2004/02/skos/core#prefLabel> "has length in meters"@en .

geo:hasMetricPerimeterLength <http://www.w3.org/2004/02/skos/core#definition> "The length of the perimeter of a Spatial Object in meters."@en;
  <http://www.w3.org/2004/02/skos/core#example> <http://www.opengis.net/spec/geosparql/1.1/specification.html#C.1.1.1.2>;
  <http://www.w3.org/2004/02/skos/core#prefLabel> "has perimeter length in meters"@en .

geo:hasMetricSpatialAccuracy <http://www.w3.org/2004/02/skos/core#definition> "The positional accuracy of the coordinates of a Geometry in meters."@en;
  <http://www.w3.org/2004/02/skos/core#example> <http://www.opengis.net/spec/geosparql/1.1/specification.html#C.1.2.3>;
  <http://www.w3.org/2004/02/skos/core#note> "Spatial accuracy is applicable when a Geometry is used to represent a Feature. It is expressed as a distance that indicates the truthfullness of the positions (coordinates) that define the Geometry. In this case accuracy defines a zone surrounding each coordinate within wich the real positions are known to be. The accuracy value defines this zone as a distance from the coordinate(s) in all directions (e.g. a line, a circle or a sphere, depending on spatial dimension)."@en;
  <http://www.w3.org/2004/02/skos/core#prefLabel> "has spatial accuracy in meters"@en .

geo:hasMetricSpatialResolution <http://www.w3.org/2004/02/skos/core#definition> "The spatial resolution of a Geometry in meters."@en;
  <http://www.w3.org/2004/02/skos/core#example> <http://www.opengis.net/spec/geosparql/1.1/specification.html#C.1.2.2>,
    <http://www.opengis.net/spec/geosparql/1.1/specification.html#C.1.1.2.6>;
  <http://www.w3.org/2004/02/skos/core#note> "Spatial resolution specifies the level of detail of a Geometry. It the smallest dinstinguishable distance between spatially adjacent coordinates."@en;
  <http://www.w3.org/2004/02/skos/core#prefLabel> "has spatial resolution in meters"@en .

geo:hasMetricVolume <http://www.w3.org/2004/02/skos/core#definition> "The volume of a Spatial Object in cubic meters."@en;
  <http://www.w3.org/2004/02/skos/core#example> <http://www.opengis.net/spec/geosparql/1.1/specification.html#C.1.2.2>,
    <http://www.opengis.net/spec/geosparql/1.1/specification.html#C.1.1.2.9>;
  <http://www.w3.org/2004/02/skos/core#prefLabel> "has volume in cubic meters"@en .

geo:isEmpty <http://www.w3.org/2004/02/skos/core#definition> "(true) if this geometric object is the empty Geometry. If true, then this geometric object represents the empty point set for the coordinate space."@en;
  <http://www.w3.org/2004/02/skos/core#example> <http://www.opengis.net/spec/geosparql/1.1/specification.html#C.1.2.3>;
  <http://www.w3.org/2004/02/skos/core#prefLabel> "is empty"@en .

geo:isSimple <http://www.w3.org/2004/02/skos/core#definition> "(true) if this geometric object has no anomalous geometric points, such as self intersection or self tangency."@en;
  <http://www.w3.org/2004/02/skos/core#example> <http://www.opengis.net/spec/geosparql/1.1/specification.html#C.1.2.3>;
  <http://www.w3.org/2004/02/skos/core#prefLabel> "is simple"@en .

geo:spatialDimension <http://www.w3.org/2004/02/skos/core#definition> "The number of measurements or axes needed to describe the spatial position of this Geometry in a coordinate system."@en;
  <http://www.w3.org/2004/02/skos/core#example> <http://www.opengis.net/spec/geosparql/1.1/specification.html#C.1.2.3>;
  <http://www.w3.org/2004/02/skos/core#prefLabel> "spatial dimension"@en .

time:day <http://www.w3.org/2004/02/skos/core#definition> """Day position in a calendar-clock system.

The range of this property is not specified, so can be replaced by any specific representation of a calendar day from any calendar. """@en,
    """Posicin de da en un sistema calendario-reloj.

El rango de esta propiedad no est especificado, por tanto, se puede reemplazar por una representacin especfica de un da de calendario de cualquier calendario."""@es .

time:dayOfYear <http://www.w3.org/2004/02/skos/core#definition> "El nmero de da en el ao."@es,
    "The number of the day within the year"@en .

time:days <http://www.w3.org/2004/02/skos/core#definition> "Longitud de, o elemento de la longitud de, una extensin temporal expresada en das."@es,
    "length of, or element of the length of, a temporal extent expressed in days"@en .

time:hasXSDDuration <http://www.w3.org/2004/02/skos/core#definition> "Extensin de una entidad temporal, expresada utilizando xsd:duration."@es,
    "Extent of a temporal entity, expressed using xsd:duration"@en .

time:hour <http://www.w3.org/2004/02/skos/core#definition> "Hour position in a calendar-clock system."@en,
    "Posicin de hora en un sistema calendario-reloj."@es .

time:hours <http://www.w3.org/2004/02/skos/core#definition> "Longitud de, o elemento de la longitud de, una extensin temporal expresada en horas."@es,
    "length of, or element of the length of, a temporal extent expressed in hours"@en .

time:inXSDDate <http://www.w3.org/2004/02/skos/core#definition> "Posicin de un instante, expresado utilizando xsd:date."@es,
    "Position of an instant, expressed using xsd:date"@en .

time:inXSDDateTime <http://www.w3.org/2004/02/skos/core#definition> "Posicin de un instante, expresado utilizando xsd:dateTime."@es,
    "Position of an instant, expressed using xsd:dateTime"@en;
  <http://www.w3.org/2004/02/skos/core#note> "La propiedad 'en fecha-hora XSD' ha sido reemplazada por 'en fecha-sello de tiempo XSD' que hace obligatorio el campo 'huso horario'."@es,
    "The property :inXSDDateTime is replaced by :inXSDDateTimeStamp which makes the time-zone field mandatory."@en .

time:inXSDDateTimeStamp <http://www.w3.org/2004/02/skos/core#definition> "Posicin de un instante, expresado utilizando xsd:dateTimeStamp."@es,
    "Position of an instant, expressed using xsd:dateTimeStamp"@en .

time:inXSDgYear <http://www.w3.org/2004/02/skos/core#definition> "Posicin de un instante, expresado utilizando xsd:gYear."@es,
    "Position of an instant, expressed using xsd:gYear"@en .

time:inXSDgYearMonth <http://www.w3.org/2004/02/skos/core#definition> "Posicin de un instante, expresado utilizando xsd:gYearMonth."@es,
    "Position of an instant, expressed using xsd:gYearMonth"@en .

time:minute <http://www.w3.org/2004/02/skos/core#definition> "Minute position in a calendar-clock system."@en,
    "Posicin de minuto en un sistema calendario-reloj."@es .

time:minutes <http://www.w3.org/2004/02/skos/core#definition> "Longitud de, o elemento de la longitud de, una extensin temporal expresada en minutos."@es,
    "length, or element of, a temporal extent expressed in minutes"@en .

time:month <http://www.w3.org/2004/02/skos/core#definition> """Month position in a calendar-clock system.

The range of this property is not specified, so can be replaced by any specific representation of a calendar month from any calendar. """@en,
    """Posicin de mes en un sistema calendario-reloj.
            El rango de esta propiedad no est especificado, por tanto, se puede reemplazar por cualquier representacin especfica de un mes de calendario de un calendario cualquiera."""@es .

time:months <http://www.w3.org/2004/02/skos/core#definition> "Longitud de, o elemento de la longitud de, una extensin temporal expresada en meses."@es,
    "length of, or element of the length of, a temporal extent expressed in months"@en .

time:nominalPosition <http://www.w3.org/2004/02/skos/core#definition> "El valor (nominal) que indica posicin temporal en un sistema de referencia ordinal."@es,
    "The (nominal) value indicating temporal position in an ordinal reference system "@en .

time:numericDuration <http://www.w3.org/2004/02/skos/core#definition> "Valor de una extensin temporal expresada como un nmero decimal escalado por una unidad de tiempo."@es,
    "Value of a temporal extent expressed as a decimal number scaled by a temporal unit"@en .

time:numericPosition <http://www.w3.org/2004/02/skos/core#definition> "El valor (numrico) que indica posicin temporal en un sistema de referencia ordinal."@es,
    "The (numeric) value indicating position within a temporal coordinate system "@en .

geo:FeatureCollection <http://www.w3.org/2004/02/skos/core#definition> "A collection of individual Features."@en;
  <http://www.w3.org/2004/02/skos/core#example> <http://www.opengis.net/spec/geosparql/1.1/specification.html#C.1.1.6>;
  <http://www.w3.org/2004/02/skos/core#prefLabel> "Feature Collection"@en .

geo:SpatialObjectCollection <http://www.w3.org/2004/02/skos/core#definition> "A collection of individual Spatial Objects."@en;
  <http://www.w3.org/2004/02/skos/core#note> "This is the superclass of Feature Collection and Geometry Collection."@en;
  <http://www.w3.org/2004/02/skos/core#prefLabel> "Spatial Object Collection"@en .

geo:GeometryCollection <http://www.w3.org/2004/02/skos/core#definition> "A collection of individual Geometries."@en;
  <http://www.w3.org/2004/02/skos/core#example> <http://www.opengis.net/spec/geosparql/1.1/specification.html#C.1.1.7>;
  <http://www.w3.org/2004/02/skos/core#prefLabel> "Geometry Collection"@en .

time:DateTimeDescription <http://www.w3.org/2004/02/skos/core#definition> "Descripcin de fecha y tiempo estructurada con valores separados para los diferentes elementos de un sistema calendario-reloj. El sistema de referencia temporal est fijado al calendario gregoriano, y el rango de las propiedades ao, mes, da restringidas a los correspondientes tipos del XML Schema xsd:gYear, xsd:gMonth y xsd:gDay respectivamente."@es,
    "Description of date and time structured with separate values for the various elements of a calendar-clock system. The temporal reference system is fixed to Gregorian Calendar, and the range of year, month, day properties restricted to corresponding XML Schema types xsd:gYear, xsd:gMonth and xsd:gDay, respectively."@en .

time:DurationDescription <http://www.w3.org/2004/02/skos/core#definition> "Descripcin de extensin temporal estructurada con valores separados para los distintos elementos de un sistema de horario-calendario. El sistema de referencia temporal se fija al calendario gregoriano, y el intervalo de cada una de las propiedades numricas se restringe a xsd:decimal."@es,
    "Description of temporal extent structured with separate values for the various elements of a calendar-clock system. The temporal reference system is fixed to Gregorian Calendar, and the range of each of the numeric properties is restricted to xsd:decimal"@en;
  <http://www.w3.org/2004/02/skos/core#note> "En el calendario gregoriano la longitud de los meses no es fija. Por lo tanto, un valor como \"2,5 meses\" no se puede comparar exactamente con una duracin similar expresada en trminos de semanas o das."@es,
    "In the Gregorian calendar the length of the month is not fixed. Therefore, a value like \"2.5 months\" cannot be exactly compared with a similar duration expressed in terms of weeks or days."@en .

time:Year <http://www.w3.org/2004/02/skos/core#definition> "Year duration";
  <http://www.w3.org/2004/02/skos/core#prefLabel> "Year"@en, "Anno"@it, "Anne (calendrier)"@fr,
    "Ano"@pt, "Ao"@es, "Jaar"@nl, "Jahr"@de, "Rok"@pl, ""@ru, ""@ar, ""@ja, ""@zh .

sem:hasActor <http://www.w3.org/2004/02/skos/core#exactMatch> <http://linkedevents.org/ontology/involved>;
  <http://www.w3.org/2004/02/skos/core#narrowMatch> <http://www.kulttuurisampo.fi/ebkr/agent> .

sem:hasPlace <http://www.w3.org/2004/02/skos/core#exactMatch> <http://www.kulttuurisampo.fi/ebkr/place>;
  <http://www.w3.org/2004/02/skos/core#narrowMatch> <http://linkedevents.org/ontology/inSpace> .

sem:hasSubEvent <http://www.w3.org/2004/02/skos/core#exactMatch> <http://purl.org/NET/c4dm/event.owl#sub_event> .

time:timeZone <http://www.w3.org/2004/02/skos/core#note> """IANA mantiene una base de datos de husos horarios. stas estn bien mantenidas y generalmente se consideran autorizadas, pero los tems individuales no estn disponibles en URIs individuales, por tanto, no se pueden utilizar directamente en datos expresados utilizando OWL-Time.
            La BDPedia proporciona un conjunto de recursos correspondientes a los husos horarios de IANA, con una URI para cada uno (por ejemplo, http://dbpedia.org/resource/Australia/Eucla). El Servicio de Reloj Mundial tambin proporciona una lista de husos horarios con la descripcin de cada uno de los disponibles como una pgina Web individual con una URI adecuada individual (por ejemplo, https://www.timeanddate.com/time/zones/acwst). stos, y otros recursos similares, se puden usar como un valor de la propiedad 'huso horario'."""@es,
    """IANA maintains a database of timezones. These are well maintained and generally considered authoritative, but individual items are not available at individual URIs, so cannot be used directly in data expressed using OWL-Time.

DBPedia provides a set of resources corresponding to the IANA timezones, with a URI for each (e.g. http://dbpedia.org/resource/Australia/Eucla). The World Clock service also provides a list of time zones with the description of each available as an individual webpage with a convenient individual URI (e.g. https://www.timeanddate.com/time/zones/acwst). These or other, similar, resources might be used as a value of the time:timeZone property.""" .

time:week <http://www.w3.org/2004/02/skos/core#note> "Weeks are numbered differently depending on the calendar in use and the local language or cultural conventions (locale). ISO-8601 specifies that the first week of the year includes at least four days, and that Monday is the first day of the week. In that system, week 1 is the week that contains the first Thursday in the year."@en;
  <http://www.w3.org/2004/02/skos/core#scopeNote> "Las semanas estn numeradas de forma diferente dependiendo del calendario en uso y de las convenciones lingsticas y culturales locales (locale en ingls). El ISO-8601 especifica que la primera semana del ao incluye al menos cuatro das, y que el lunes es el primer da de la semana. En ese sistema, la semana 1 es la semana que contiene el primer jueves del ao."@es .

time:xsdDateTime <http://www.w3.org/2004/02/skos/core#note> "Using xsd:dateTime in this place means that the duration of the interval is implicit: it corresponds to the length of the smallest non-zero element of the date-time literal. However, this rule cannot be used for intervals whose duration is more than one rank smaller than the starting time - e.g. the first minute or second of a day, the first hour of a month, or the first day of a year. In these cases the desired interval cannot be distinguished from the interval corresponding to the next rank up. Because of this essential ambiguity, use of this property is not recommended and it is deprecated."@en,
    "Utilizando xsd:dateTime en este lugar significa que la duracin del intervalo est implcita: se corresponde con la longitud del elemento ms pequeo distinto de cero del literal fecha-hora. Sin embargo, esta regla no se puede utilizar para intervalos cuya duracin es mayor que un rango ms pequeo que el tiempo de comienzo - p.ej. el primer minuto o segundo del da, la primera hora del mes, o el primer da del ao. En estos casos el intervalo deseado no se puede distinguir del intervalo correspondiente al prximo rango ms alto. Debido a esta ambigedad esencial, no se recomienda el uso de esta propiedad y est desaprobada." .

time:unitMonth <http://www.w3.org/2004/02/skos/core#prefLabel> "mes"@es, "month"@en,
    "Monat"@de, "maand"@nl, "mese"@it, "miesic"@pl, "mois"@fr, " "@ru, " "@ar,
    ""@ja, ""@zh, ""@kr .

time:Friday <http://www.w3.org/2004/02/skos/core#prefLabel> "Friday"@en, "Freitag"@de,
    "Pitek"@pl, "Sexta-feira"@pt, "Vendredi"@fr, "Venerd"@it, "Viernes"@es, "Vrijdag"@nl,
    ""@ru, ""@ar, ""@zh, ""@ja .

time:Monday <http://www.w3.org/2004/02/skos/core#prefLabel> "Monday"@en, "Lundi"@fr,
    "Luned"@it, "Lunes"@es, "Maandag"@nl, "Montag"@de, "Poniedziaek"@pl, "Segunda-feira"@pt,
    ""@ru, ""@ar, ""@zh, ""@ja .

time:Saturday <http://www.w3.org/2004/02/skos/core#prefLabel> "Saturday"@en, "Sabato"@it,
    "Samedi"@fr, "Samstag"@de, "Sobota"@pl, "Sbado"@es, "Sbado"@pt, "Zaterdag"@nl, ""@ru,
    ""@ar, ""@ja, ""@zh .

time:Sunday <http://www.w3.org/2004/02/skos/core#prefLabel> "Sunday"@en, "Dimanche"@fr,
    "Domenica"@it, "Domingo"@es, "Domingo"@pt, "Niedziela"@pl, "Sonntag"@de, "Zondag"@nl,
    ""@ru, " ()"@ar, ""@ja, ""@zh .

time:Thursday <http://www.w3.org/2004/02/skos/core#prefLabel> "Thursday"@en, "Czwartek"@pl,
    "Donderdag"@nl, "Donnerstag"@de, "Gioved"@it, "Jeudi"@fr, "Jueves"@es, "Quinta-feira"@pt,
    ""@ru, ""@ar, ""@zh, ""@ja .

time:Tuesday <http://www.w3.org/2004/02/skos/core#prefLabel> "Tuesday"@en, "Dienstag"@de,
    "Dinsdag"@nl, "Mardi"@fr, "Marted"@it, "Martes"@es, "Tera-feira"@pt, "Wtorek"@pl,
    ""@ru, ""@ar, ""@zh, ""@ja .

time:Wednesday <http://www.w3.org/2004/02/skos/core#prefLabel> "Wednesday"@en, "Mercoled"@it,
    "Mercredi"@fr, "Mittwoch"@de, "Mircoles"@es, "Quarta-feira"@pt, "Woensdag"@nl, "roda"@pl,
    ""@ru, ""@ar, ""@zh, ""@ja .

time:unitCentury <http://www.w3.org/2004/02/skos/core#prefLabel> "Jahrhundert"@de,
    "century"@en, "eeuw"@nl, "secolo"@it, "siglo"@es, "sicle"@fr, "stulecie"@pl, "sculo"@pt,
    ""@ru, " "@ar, ""@ja, ""@zh, " "@kr .

time:unitDay <http://www.w3.org/2004/02/skos/core#prefLabel> "day"@en, "da"@es, "Tag"@de,
    "dag"@nl, "dia"@pt, "doba"@pl, "giorno"@it, "jour"@fr, " "@ar, ""@ja, ""@zh,
    ""@kr .

time:unitDecade <http://www.w3.org/2004/02/skos/core#prefLabel> "1 "@kr, "10"@ja,
    "Dekade"@de, "decade"@en, "decennio"@it, "decennium"@nl, "dekada"@pl, "dcada"@pt,
    "dcennie"@fr, "una dcada"@es, " "@ru, " "@ar, ""@zh .

time:unitHour <http://www.w3.org/2004/02/skos/core#prefLabel> "hora"@es, "hour"@en,
    "Stunde"@de, "godzina"@pl, "heure"@fr, "hora"@pt, "ora"@it, "uur"@nl, " "@ru,
    " "@ar, ""@zh, ""@ja, " "@kr .

time:unitMillenium <http://www.w3.org/2004/02/skos/core#prefLabel> "Jahrtausend"@de,
    "milenio"@es, "millenium"@en, "millennio"@it, "millennium"@nl, "millnaire"@fr, "milnio"@pt,
    "tysiclecie"@pl, ""@ru, ""@ar, ""@ja, ""@zh, ""@kr .

time:unitMinute <http://www.w3.org/2004/02/skos/core#prefLabel> "minute"@en, "minuto"@es,
    "Minute"@de, "minuta"@pl, "minute"@fr, "minuto"@it, "minuto"@pt, "minuut"@nl, " "@ru,
    " "@ar, ""@ja, ""@zh, ""@kr .

time:unitSecond <http://www.w3.org/2004/02/skos/core#prefLabel> "second"@en, "segundo"@es,
    "Sekunde"@de, "seconde"@fr, "seconde"@nl, "secondo"@it, "segundo"@pt, "sekund"@pl,
    " "@ar, ""@ja, ""@zh, ""@kr .

time:unitWeek <http://www.w3.org/2004/02/skos/core#prefLabel> "semana"@es, "week"@en,
    "Woche"@de, "semaine"@fr, "semana"@pt, "settimana"@it, "tydzie"@pl, "week"@nl, " "@ru,
    " "@ar, ""@zh, ""@ja, ""@kr .

time:unitYear <http://www.w3.org/2004/02/skos/core#prefLabel> "year"@en, "Jahr"@de,
    "1 "@kr, "an"@fr, "anno"@it, "ano"@pt, "jaar"@nl, "rok"@pl, "un ao"@es, " "@ru,
    " "@ar, ""@ja, ""@zh .

sem:Role <http://www.w3.org/2004/02/skos/core#relatedMatch> <http://sw.opencyc.org/2009/04/07/concept/en/Role>,
    <http://www.loa-cnr.it/ontologies/DOLCE-Lite.owl#region>, <http://www.ontologyportal.org/translations/SUMO.owl.txt#IntentionalProcess> .

_:node79 <https://schema.org/affiliation> "Oracle Corporation";
  <https://schema.org/email> "john.herring@oracle.com";
  <https://schema.org/name> "John Herring" .

_:node80 <https://schema.org/affiliation> "Oracle Corporation";
  <https://schema.org/email> "matthew.perry@oracle.com";
  <https://schema.org/name> "Matthew Perry";
  <https://schema.org/url> "https://orcid.org/0000-0003-1988-462X"^^xsd:anyURI .

_:node81 <https://schema.org/affiliation> "Oracle Corporation";
  <https://schema.org/email> "matthew.perry@oracle.com";
  <https://schema.org/name> "Matthew Perry";
  <https://schema.org/url> "https://orcid.org/0000-0003-1988-462X"^^xsd:anyURI .

_:node82 <https://schema.org/affiliation> "Mainz University Of Applied Sciences";
  <https://schema.org/email> "timo.homburg@hs-mainz.de";
  <https://schema.org/name> "Timo Homburg";
  <https://schema.org/url> "https://orcid.org/0000-0002-9499-5840"^^xsd:anyURI .

_:node83 <https://schema.org/affiliation> "KU Leuven", "Neanex Technologies";
  <https://schema.org/email> "mathias.bonduel@neanex.com";
  <https://schema.org/name> "Mathias Bonduel";
  <https://schema.org/url> "https://orcid.org/0000-0002-3313-924X"^^xsd:anyURI .

_:node86 <https://schema.org/affiliation> "Australian National University", "SURROUND Australia Pty Ltd";
  <https://schema.org/email> "nicholas.car@surroundaustralia.com";
  <https://schema.org/name> "Nicholas J. Car";
  <https://schema.org/url> "https://orcid.org/0000-0002-8742-7730"^^xsd:anyURI .

_:node88 <https://schema.org/affiliation> "CSIRO Australia";
  <https://schema.org/email> "simon.cox@csiro.au";
  <https://schema.org/name> "Simon J D Cox";
  <https://schema.org/url> "https://orcid.org/0000-0002-3884-3420"^^xsd:anyURI .

_:node89 <https://schema.org/affiliation> "Australian National University", "SURROUND Australia Pty Ltd";
  <https://schema.org/email> "nicholas.car@surroundaustralia.com";
  <https://schema.org/name> "Nicholas J. Car";
  <https://schema.org/url> "https://orcid.org/0000-0002-8742-7730"^^xsd:anyURI .

_:node90 <https://schema.org/affiliation> "KU Leuven", "Neanex Technologies";
  <https://schema.org/email> "mathias.bonduel@neanex.com";
  <https://schema.org/name> "Mathias Bonduel";
  <https://schema.org/url> "https://orcid.org/0000-0002-3313-924X"^^xsd:anyURI .

_:node91 <https://schema.org/affiliation> "Geoscape Australia";
  <https://schema.org/email> "joseph.abhayaratna@geoscape.com.au";
  <https://schema.org/name> "Joseph Abhayaratna";
  <https://schema.org/url> "https://orcid.org/0000-0001-5075-6234"^^xsd:anyURI .

_:node92 <https://schema.org/affiliation> "Oracle Corporation";
  <https://schema.org/email> "john.herring@oracle.com";
  <https://schema.org/name> "John Herring" .

_:node93 <https://schema.org/affiliation> "CSIRO Australia";
  <https://schema.org/email> "simon.cox@csiro.au";
  <https://schema.org/name> "Simon J D Cox";
  <https://schema.org/url> "https://orcid.org/0000-0002-3884-3420"^^xsd:anyURI .

_:node95 <https://schema.org/affiliation> "Geoscape Australia";
  <https://schema.org/email> "joseph.abhayaratna@geoscape.com.au";
  <https://schema.org/name> "Joseph Abhayaratna";
  <https://schema.org/url> "https://orcid.org/0000-0001-5075-6234"^^xsd:anyURI .

_:node96 <https://schema.org/affiliation> "Mainz University Of Applied Sciences";
  <https://schema.org/email> "timo.homburg@hs-mainz.de";
  <https://schema.org/name> "Timo Homburg";
  <https://schema.org/url> "https://orcid.org/0000-0002-9499-5840"^^xsd:anyURI .

_:node87 <https://schema.org/email> "fjknibbe@gmail.com";
  <https://schema.org/name> "Frans Knibbe";
  <https://schema.org/url> "https://orcid.org/0000-0003-3789-2260"^^xsd:anyURI .

_:node94 <https://schema.org/email> "fjknibbe@gmail.com";
  <https://schema.org/name> "Frans Knibbe";
  <https://schema.org/url> "https://orcid.org/0000-0003-3789-2260"^^xsd:anyURI .

_:node84 <https://schema.org/name> "Open Geospatial Consortium";
  <https://schema.org/url> "https://www.ogc.org"^^xsd:anyURI .

_:node85 <https://schema.org/name> "Open Geospatial Consortium";
  <https://schema.org/url> "https://www.ogc.org"^^xsd:anyURI .

:wikipediaBandungLautanApi sem:hasActor :India, :BritaniaRaya, :HindiaBelanda, :ImperiumBelanda,
    :PemerintahanSipilHindiaBelanda, :KekaisaranBritania;
  sem:accordingTo :wikipedia;
  sem:hasSubEvent :wikipediaRevolusiNasionalIndonesia;
  time:hasTime _:node100 .

:wikipediaPemberontakanDITIIdiAceh sem:hasActor :Soekarno, :DaudBeureueh, :Indonesia,
    :NegaraIslamIndonesia;
  sem:accordingTo :wikipedia;
  sem:hasSubEvent :wikipediaPemberontakanDITII;
  time:hasTime _:node115 .

:wikipediaKampanyeKalimantan1945 sem:hasActor :DouglasMacArthur, :MichiakiKamada,
    :ThomasKinkaid, :BabaMasao, :LeslieMorshead, :Belanda, :KekaisaranJepang, :BritaniaRaya,
    :AmerikaSerikat, :Australia;
  sem:accordingTo :wikipedia;
  sem:hasSubEvent :wikipediaPerangDuniaII;
  time:hasTime _:node120 .

:wikipediaPertempuranBojongKokosan sem:hasActor :AJFDoulton, :EdiSukardi, :Indonesia,
    :BritaniaRaya;
  sem:accordingTo :wikipedia;
  sem:hasSubEvent :wikipediaRevolusiNasionalIndonesia;
  time:hasTime _:node130 .

:wikipediaRevolusiNasionalIndonesia sem:hasActor :MoehammadJasin, :RobertMansergh,
    :AubertinMallaby, :Sutomo, :Soekarno, :RaymondWesterling, :JuliusTahija, :MohammadHatta,
    :REMartadinata, :SutanSjahrir, :AbdulHarisNasution, :HubertusJohannesvanMook, :SimonSpoor,
    :SyafruddinPrawiranegara, :Musso, :TanMalaka, :LouisMountbatten, :DirkCornelisBuurmanvanVreeden,
    :LudolphHendrikvanOyen, :TjokordaGdeRakaSoekawati, :GatotSoebroto, :Soedirman, :DirkReinhardAdelbertvanLangen,
    :BambangSoegeng, :OeripSoemohardjo, :ConradHelfrich, :HamengkubuwanaIX, :Soeharto,
    :WilhelminadariBelanda, :TBSimatupang, :LoaSekHie, :SyarifHamidIIdariPontianak, :PhilipChristison,
    :AbdulkadirWidjojoatmodjo, :AbdulKaharMuzakkar, :PakubuwanaXII, :SekarmadjiMaridjanKartosoewirjo,
    :AmirSjarifoeddin, :AgustinusAdisoetjipto, :JulianadariBelanda, :KNIL, :Belanda, :TNI,
    :RepublikIndonesia, :India, :BritaniaRaya, :DesertirTentaraIndia, :AmerikaSerikat,
    :Australia, :UniSoviet, :KorpsBrigadeMobil, :BKR, :TRI, :PDRI, :KemaharajaanBritania,
    :AngkatanPerangRatuAdil, :PaoAnTui, :HindiaBelanda, :KesultananPontianak, :NICA, :RelawanTentaraKekaisaranJepang,
    :TKR;
  sem:accordingTo :wikipedia;
  sem:hasSubEvent :wikipediaPascaPerangDuniaKedua;
  time:hasTime _:node135 .

:wikipediaPerangCumbok sem:hasActor :TeukuKeumanganUmar, :TeungkuHasanKruengKalee,
    :TeukuDaudCumbok, :TeukuNyakArif, :TeungkuAhmadHasballah, :SyamaunGaharu, :DaudBeureueh,
    :PUSA, :Kaumuleebalang;
  sem:accordingTo :wikipedia;
  sem:hasSubEvent :wikipediaRevolusiNasionalIndonesia;
  time:hasTime _:node170 .

:wikipediaSeranganUmum1Maret1949 sem:hasActor :Meyer, :Soedirman, :DirkReinhardAdelbertvanLangen,
    :BambangSoegeng, :HamengkubuwanaIX, :VentjeSumual, :JMvdBerge, :Soeharto, :Indonesia,
    :Belanda;
  sem:accordingTo :wikipedia;
  sem:hasSubEvent :wikipediaRevolusiNasionalIndonesia;
  time:hasTime _:node185 .

:wikipediaKonflikPapua sem:hasActor :GoliathTabuni, :MathiasWenda, :ListyoSigitPrabowo,
    :AgusSubiyanto, :PrabowoSubianto, :EgianusKogoya, :BudiGunawan, :JoniBotak, :SebbySambom,
    :KellyKwalik, :BJHabibie, :AndikaPerkasa, :Soeharto, :SusiloBambangYudhoyono, :LeonardusBenyaminMoerdani,
    :MarufAmin, :MegawatiSoekarnoputri, :Wiranto, :BennyWenda, :JacobPrai, :TrySutrisno,
    :JokoWidodo, :JacobRumbiak, :AbdurrahmanWahid, :Indonesia, :Tuvalu, :AmerikaSerikat,
    :Samoa, :PapuaNugini, :Tonga, :OrganisasiPapuaMerdeka, :KepulauanSolomon, :Vanuatu,
    :Nauru, :Fiji, :Australia, :UniSoviet, :Libya, :Palau;
  sem:accordingTo :wikipedia;
  sem:hasSubEvent :wikipediaPersengketaanNuginiBaratdanDekolonisasiOseania;
  time:hasTime _:node200 .

:wikipediaPeristiwaTigaMaret sem:hasActor :SaalahYusufSutanMangkuto, :AdamBB, :IsmaelLengah,
    :Indonesia, :MilitanIslam;
  sem:accordingTo :wikipedia;
  sem:hasSubEvent :wikipediaRevolusiNasionalIndonesia;
  time:hasTime _:node205 .

:wikipediaPenyerbuanKotabaruYogyakarta sem:hasActor :HamengkubuwanaIX, :Soeharto,
    :Otzuka, :Indonesia, :Jepang;
  sem:accordingTo :wikipedia;
  sem:hasSubEvent :wikipediaRevolusiNasionalIndonesia;
  time:hasTime _:node210 .

:wikipediaPerangDayakDesa sem:hasActor :PangRati, :Djampi, :PangIyo, :PangSuma, :Nagatani,
    :KekaisaranJepang, :SukuDayakDesa;
  sem:accordingTo :wikipedia;
  sem:hasSubEvent :wikipediaPendudukanJepangdiKalimantanBarat;
  time:hasTime _:node230 .

:wikipediaKampanyeHindiaBelanda sem:hasActor :JisaburoOzawa, :KiyotakeKawaguchi, :NobutakeKond,
    :HeinterPoorten, :HitoshiImamura, :HisaichiTerauchi, :AlidiusTjardavanStarkenborghStachouwer,
    :IbTakahashi, :ThomasCHart, :ShojiNishimura, :TakeoTakagi, :ConradHelfrich, :ArchibaldWavell1stEarlWavell,
    :RichardPeirse, :KarelDoorman, :Belanda, :KekaisaranJepang, :SelandiaBaru, :BritaniaRaya,
    :AmerikaSerikat, :Australia, :ABDACommand, :HindiaBelanda;
  sem:accordingTo :wikipedia;
  sem:hasSubEvent :wikipediaPerangPasifikdariPerangDuniaII;
  time:hasTime _:node240, _:node245 .

:wikipediaPertempuranLengkong sem:hasActor :DaanMogot, :Jepang, :TentaraKeamananRakyat;
  sem:accordingTo :wikipedia;
  time:hasTime _:node250 .

:wikipediaPertempuranMedanArea sem:hasActor :TEDKelly, :JaminGinting, :AbdulKarimMS,
    :AchmadTahir, :Indonesia, :Belanda, :BritaniaRaya, :KemaharajaanBritania, :HindiaBelanda;
  sem:accordingTo :wikipedia;
  sem:hasSubEvent :wikipediaRevolusiNasionalIndonesia;
  time:hasTime _:node260 .

:wikipediaPertempuranKumai sem:hasActor :BarisanUlama, :HindiaBelanda, :LaskarKalimantan,
    :TentaraKeamananRakyat;
  sem:accordingTo :wikipedia;
  sem:hasSubEvent :wikipediaRevolusiNasionalIndonesia;
  time:hasTime _:node265 .

:wikipediaSeranganUmumSurakarta sem:hasActor :SlametRijadi, :Mollinger, :GatotSoebroto,
    :VanVreeden, :PakubuwanaXII, :MangkunegaraVIII, :AchmadiHadisoemarto, :Indonesia,
    :Belanda;
  sem:accordingTo :wikipedia;
  sem:hasSubEvent :wikipediaRevolusiNasionalIndonesia;
  time:hasTime _:node270 .

:wikipediaPuputanMargarana sem:hasActor :JBTKnig, :FMollinger, :IGustiNgurahRai, :Indonesia,
    :Belanda;
  sem:accordingTo :wikipedia;
  sem:hasSubEvent :wikipediaRevolusiNasionalIndonesia;
  time:hasTime _:node280 .

:wikipediaPertempuranLimaHari sem:hasActor :KidoShinichir, :Wongsonegoro, :Kariadi,
    :Indonesia, :Jepang;
  sem:accordingTo :wikipedia;
  sem:hasSubEvent :wikipediaRevolusiNasionalIndonesia;
  time:hasTime _:node285, _:node290 .

:wikipediaPertempuranSurabaya sem:hasActor :MuhammadMangundiprojo, :Soengkono, :HarioJonosewojo,
    :MoehammadJasin, :Moestopo, :RobertMansergh, :AubertinMallaby, :Sutomo, :RepublikIndonesia,
    :India, :BritaniaRaya;
  sem:accordingTo :wikipedia;
  sem:hasSubEvent :wikipediaRevolusiNasionalIndonesia;
  time:hasTime _:node300 .

:wikipediaDelapanJamPertempurandiMangkang sem:hasActor :InfanteriBelanda, :Moekijat,
    :Indonesia, :Belanda;
  sem:accordingTo :wikipedia;
  sem:hasSubEvent :wikipediaPerangKemerdekaanIndonesia;
  time:hasTime _:node325 .

:wikipediaPeristiwa19November sem:hasActor :Indonesia, :Belanda;
  sem:accordingTo :wikipedia;
  sem:hasSubEvent :wikipediaRevolusiNasionalIndonesia;
  time:hasTime _:node335 .

:wikipediaOperasi17Agustus sem:hasActor :Soekarno, :Assaat, :AbdulHarisNasution, :SyafruddinPrawiranegara,
    :MaludinSimbolon, :AhmadYani, :AhmadHusein, :Indonesia, :PRRI;
  sem:accordingTo :wikipedia;
  time:hasTime _:node350 .

:wikipediaGerakan30September sem:accordingTo :wikipedia;
  time:hasTime _:node235 .

_:node100 time:hasBeginning _:node101;
  time:hasEnd _:node103 .

_:node105 time:hasBeginning _:node106;
  time:hasEnd _:node108 .

_:node110 time:hasBeginning _:node111;
  time:hasEnd _:node113 .

_:node115 time:hasBeginning _:node116;
  time:hasEnd _:node118 .

_:node120 time:hasBeginning _:node121;
  time:hasEnd _:node123 .

_:node125 time:hasBeginning _:node126;
  time:hasEnd _:node128 .

_:node130 time:hasBeginning _:node131;
  time:hasEnd _:node133 .

_:node135 time:hasBeginning _:node136;
  time:hasEnd _:node138 .

_:node140 time:hasBeginning _:node141;
  time:hasEnd _:node143 .

_:node145 time:hasBeginning _:node146;
  time:hasEnd _:node148 .

_:node150 time:hasBeginning _:node151;
  time:hasEnd _:node153 .

_:node155 time:hasBeginning _:node156;
  time:hasEnd _:node158 .

_:node160 time:hasBeginning _:node161;
  time:hasEnd _:node163 .

_:node165 time:hasBeginning _:node166;
  time:hasEnd _:node168 .

_:node170 time:hasBeginning _:node171;
  time:hasEnd _:node173 .

_:node175 time:hasBeginning _:node176;
  time:hasEnd _:node178 .

_:node180 time:hasBeginning _:node181;
  time:hasEnd _:node183 .

_:node185 time:hasBeginning _:node186;
  time:hasEnd _:node188 .

_:node190 time:hasBeginning _:node191;
  time:hasEnd _:node193 .

_:node195 time:hasBeginning _:node196;
  time:hasEnd _:node198 .

_:node200 time:hasBeginning _:node201;
  time:hasEnd _:node203 .

_:node205 time:hasBeginning _:node206;
  time:hasEnd _:node208 .

_:node210 time:hasBeginning _:node211;
  time:hasEnd _:node213 .

_:node215 time:hasBeginning _:node216;
  time:hasEnd _:node218 .

_:node220 time:hasBeginning _:node221;
  time:hasEnd _:node223 .

_:node225 time:hasBeginning _:node226;
  time:hasEnd _:node228 .

_:node230 time:hasBeginning _:node231;
  time:hasEnd _:node233 .

_:node235 time:hasBeginning _:node236;
  time:hasEnd _:node238 .

_:node240 time:hasBeginning _:node241;
  time:hasEnd _:node243 .

_:node245 time:hasBeginning _:node246;
  time:hasEnd _:node248 .

_:node250 time:hasBeginning _:node251;
  time:hasEnd _:node253 .

_:node255 time:hasBeginning _:node256;
  time:hasEnd _:node258 .

_:node260 time:hasBeginning _:node261;
  time:hasEnd _:node263 .

_:node265 time:hasBeginning _:node266;
  time:hasEnd _:node268 .

_:node270 time:hasBeginning _:node271;
  time:hasEnd _:node273 .

_:node275 time:hasBeginning _:node276;
  time:hasEnd _:node278 .

_:node280 time:hasBeginning _:node281;
  time:hasEnd _:node283 .

_:node285 time:hasBeginning _:node286;
  time:hasEnd _:node288 .

_:node290 time:hasBeginning _:node291;
  time:hasEnd _:node293 .

_:node295 time:hasBeginning _:node296;
  time:hasEnd _:node298 .

_:node300 time:hasBeginning _:node301;
  time:hasEnd _:node303 .

_:node305 time:hasBeginning _:node306;
  time:hasEnd _:node308 .

_:node310 time:hasBeginning _:node311;
  time:hasEnd _:node313 .

_:node315 time:hasBeginning _:node316;
  time:hasEnd _:node318 .

_:node320 time:hasBeginning _:node321;
  time:hasEnd _:node323 .

_:node325 time:hasBeginning _:node326;
  time:hasEnd _:node328 .

_:node330 time:hasBeginning _:node331;
  time:hasEnd _:node333 .

_:node335 time:hasBeginning _:node336;
  time:hasEnd _:node338 .

_:node340 time:hasBeginning _:node341;
  time:hasEnd _:node343 .

_:node345 time:hasBeginning _:node346;
  time:hasEnd _:node348 .

_:node350 time:hasBeginning _:node351;
  time:hasEnd _:node353 .

_:node355 time:hasBeginning _:node356;
  time:hasEnd _:node358 .

_:node360 time:hasBeginning _:node361;
  time:hasEnd _:node363 .

_:node365 time:hasBeginning _:node366;
  time:hasEnd _:node368 .

_:node370 time:hasBeginning _:node371;
  time:hasEnd _:node373 .

_:node375 time:hasBeginning _:node376;
  time:hasEnd _:node378 .

_:node380 time:hasBeginning _:node381;
  time:hasEnd _:node383 .

_:node385 time:hasBeginning _:node386;
  time:hasEnd _:node388 .

_:node390 time:hasBeginning _:node391;
  time:hasEnd _:node393 .

_:node395 time:hasBeginning _:node396;
  time:hasEnd _:node398 .

_:node400 time:hasBeginning _:node401;
  time:hasEnd _:node403 .

_:node405 time:hasBeginning _:node406;
  time:hasEnd _:node408 .

_:node410 time:hasBeginning _:node411;
  time:hasEnd _:node413 .

_:node415 time:hasBeginning _:node416;
  time:hasEnd _:node418 .

_:node420 time:hasBeginning _:node421;
  time:hasEnd _:node423 .

_:node425 time:hasBeginning _:node426;
  time:hasEnd _:node428 .

_:node430 time:hasBeginning _:node431;
  time:hasEnd _:node433 .

_:node435 time:hasBeginning _:node436;
  time:hasEnd _:node438 .

_:node440 time:hasBeginning _:node441;
  time:hasEnd _:node443 .

_:node445 time:hasBeginning _:node446;
  time:hasEnd _:node448 .

_:node450 time:hasBeginning _:node451;
  time:hasEnd _:node453 .

_:node455 time:hasBeginning _:node456;
  time:hasEnd _:node458 .

_:node460 time:hasBeginning _:node461;
  time:hasEnd _:node463 .

_:node465 time:hasBeginning _:node466;
  time:hasEnd _:node468 .

_:node470 time:hasBeginning _:node471;
  time:hasEnd _:node473 .

_:node475 time:hasBeginning _:node476;
  time:hasEnd _:node478 .

_:node480 time:hasBeginning _:node481;
  time:hasEnd _:node483 .

_:node485 time:hasBeginning _:node486;
  time:hasEnd _:node488 .

_:node490 time:hasBeginning _:node491;
  time:hasEnd _:node493 .

_:node495 time:hasBeginning _:node496;
  time:hasEnd _:node498 .

_:node500 time:hasBeginning _:node501;
  time:hasEnd _:node503 .

_:node505 time:hasBeginning _:node506;
  time:hasEnd _:node508 .

_:node510 time:hasBeginning _:node511;
  time:hasEnd _:node513 .

_:node515 time:hasBeginning _:node516;
  time:hasEnd _:node518 .

_:node520 time:hasBeginning _:node521;
  time:hasEnd _:node523 .

_:node525 time:hasBeginning _:node526;
  time:hasEnd _:node528 .

_:node530 time:hasBeginning _:node531;
  time:hasEnd _:node533 .

_:node535 time:hasBeginning _:node536;
  time:hasEnd _:node538 .

_:node540 time:hasBeginning _:node541;
  time:hasEnd _:node543 .

_:node545 time:hasBeginning _:node546;
  time:hasEnd _:node548 .

_:node550 time:hasBeginning _:node551;
  time:hasEnd _:node553 .

_:node555 time:hasBeginning _:node556;
  time:hasEnd _:node558 .

_:node560 time:hasBeginning _:node561;
  time:hasEnd _:node563 .

_:node565 time:hasBeginning _:node566;
  time:hasEnd _:node568 .

_:node570 time:hasBeginning _:node571;
  time:hasEnd _:node573 .

_:node575 time:hasBeginning _:node576;
  time:hasEnd _:node578 .

_:node580 time:hasBeginning _:node581;
  time:hasEnd _:node583 .

_:node585 time:hasBeginning _:node586;
  time:hasEnd _:node588 .

_:node590 time:hasBeginning _:node591;
  time:hasEnd _:node593 .

_:node595 time:hasBeginning _:node596;
  time:hasEnd _:node598 .

_:node600 time:hasBeginning _:node601;
  time:hasEnd _:node603 .

_:node605 time:hasBeginning _:node606;
  time:hasEnd _:node608 .

_:node610 time:hasBeginning _:node611;
  time:hasEnd _:node613 .

_:node615 time:hasBeginning _:node616;
  time:hasEnd _:node618 .

_:node620 time:hasBeginning _:node621;
  time:hasEnd _:node623 .

_:node625 time:hasBeginning _:node626;
  time:hasEnd _:node628 .

_:node630 time:hasBeginning _:node631;
  time:hasEnd _:node633 .

_:node635 time:hasBeginning _:node636;
  time:hasEnd _:node638 .

_:node640 time:hasBeginning _:node641;
  time:hasEnd _:node643 .

_:node645 time:hasBeginning _:node646;
  time:hasEnd _:node648 .

_:node650 time:hasBeginning _:node651;
  time:hasEnd _:node653 .

_:node655 time:hasBeginning _:node656;
  time:hasEnd _:node658 .

_:node660 time:hasBeginning _:node661;
  time:hasEnd _:node663 .

_:node665 time:hasBeginning _:node666;
  time:hasEnd _:node668 .

_:node670 time:hasBeginning _:node671;
  time:hasEnd _:node673 .

_:node675 time:hasBeginning _:node676;
  time:hasEnd _:node678 .

_:node680 time:hasBeginning _:node681;
  time:hasEnd _:node683 .

_:node685 time:hasBeginning _:node686;
  time:hasEnd _:node688 .

_:node690 time:hasBeginning _:node691;
  time:hasEnd _:node693 .

_:node695 time:hasBeginning _:node696;
  time:hasEnd _:node698 .

_:node700 time:hasBeginning _:node701;
  time:hasEnd _:node703 .

_:node705 time:hasBeginning _:node706;
  time:hasEnd _:node708 .

_:node710 time:hasBeginning _:node711;
  time:hasEnd _:node713 .

_:node715 time:hasBeginning _:node716;
  time:hasEnd _:node718 .

_:node720 time:hasBeginning _:node721;
  time:hasEnd _:node723 .

_:node725 time:hasBeginning _:node726;
  time:hasEnd _:node728 .

_:node730 time:hasBeginning _:node731;
  time:hasEnd _:node733 .

_:node735 time:hasBeginning _:node736;
  time:hasEnd _:node738 .

_:node740 time:hasBeginning _:node741;
  time:hasEnd _:node743 .

_:node745 time:hasBeginning _:node746;
  time:hasEnd _:node748 .

_:node750 time:hasBeginning _:node751;
  time:hasEnd _:node753 .

_:node755 time:hasBeginning _:node756;
  time:hasEnd _:node758 .

_:node760 time:hasBeginning _:node761;
  time:hasEnd _:node763 .

_:node765 time:hasBeginning _:node766;
  time:hasEnd _:node768 .

_:node770 time:hasBeginning _:node771;
  time:hasEnd _:node773 .

_:node775 time:hasBeginning _:node776;
  time:hasEnd _:node778 .

_:node780 time:hasBeginning _:node781;
  time:hasEnd _:node783 .

_:node785 time:hasBeginning _:node786;
  time:hasEnd _:node788 .

_:node790 time:hasBeginning _:node791;
  time:hasEnd _:node793 .

_:node795 time:hasBeginning _:node796;
  time:hasEnd _:node798 .

_:node800 time:hasBeginning _:node801;
  time:hasEnd _:node803 .

_:node805 time:hasBeginning _:node806;
  time:hasEnd _:node808 .

_:node810 time:hasBeginning _:node811;
  time:hasEnd _:node813 .

_:node815 time:hasBeginning _:node816;
  time:hasEnd _:node818 .

_:node820 time:hasBeginning _:node821;
  time:hasEnd _:node823 .

_:node825 time:hasBeginning _:node826;
  time:hasEnd _:node828 .

_:node830 time:hasBeginning _:node831;
  time:hasEnd _:node833 .

_:node835 time:hasBeginning _:node836;
  time:hasEnd _:node838 .

_:node840 time:hasBeginning _:node841;
  time:hasEnd _:node843 .

_:node845 time:hasBeginning _:node846;
  time:hasEnd _:node848 .

_:node850 time:hasBeginning _:node851;
  time:hasEnd _:node853 .

_:node855 time:hasBeginning _:node856;
  time:hasEnd _:node858 .

_:node860 time:hasBeginning _:node861;
  time:hasEnd _:node863 .

_:node865 time:hasBeginning _:node866;
  time:hasEnd _:node868 .

_:node870 time:hasBeginning _:node871;
  time:hasEnd _:node873 .

_:node875 time:hasBeginning _:node876;
  time:hasEnd _:node878 .

_:node880 time:hasBeginning _:node881;
  time:hasEnd _:node883 .

_:node885 time:hasBeginning _:node886;
  time:hasEnd _:node888 .

_:node890 time:hasBeginning _:node891;
  time:hasEnd _:node893 .

_:node895 time:hasBeginning _:node896;
  time:hasEnd _:node898 .

_:node900 time:hasBeginning _:node901;
  time:hasEnd _:node903 .

_:node905 time:hasBeginning _:node906;
  time:hasEnd _:node908 .

_:node910 time:hasBeginning _:node911;
  time:hasEnd _:node913 .

_:node915 time:hasBeginning _:node916;
  time:hasEnd _:node918 .

_:node920 time:hasBeginning _:node921;
  time:hasEnd _:node923 .

_:node925 time:hasBeginning _:node926;
  time:hasEnd _:node928 .

_:node930 time:hasBeginning _:node931;
  time:hasEnd _:node933 .

_:node935 time:hasBeginning _:node936;
  time:hasEnd _:node938 .

_:node940 time:hasBeginning _:node941;
  time:hasEnd _:node943 .

_:node945 time:hasBeginning _:node946;
  time:hasEnd _:node948 .

_:node950 time:hasBeginning _:node951;
  time:hasEnd _:node953 .

_:node955 time:hasBeginning _:node956;
  time:hasEnd _:node958 .

_:node960 time:hasBeginning _:node961;
  time:hasEnd _:node963 .

_:node965 time:hasBeginning _:node966;
  time:hasEnd _:node968 .

_:node970 time:hasBeginning _:node971;
  time:hasEnd _:node973 .

_:node975 time:hasBeginning _:node976;
  time:hasEnd _:node978 .

_:node980 time:hasBeginning _:node981;
  time:hasEnd _:node983 .

_:node985 time:hasBeginning _:node986;
  time:hasEnd _:node988 .

_:node990 time:hasBeginning _:node991;
  time:hasEnd _:node993 .

_:node995 time:hasBeginning _:node996;
  time:hasEnd _:node998 .

_:node1000 time:hasBeginning _:node1001;
  time:hasEnd _:node1003 .

_:node1005 time:hasBeginning _:node1006;
  time:hasEnd _:node1008 .

:wikipediaPerangBelandaPortugal time:hasTime _:node105 .

:wikipediaPeperanganeraNapoleon time:hasTime _:node110 .

:wikipediaPerangPasifik time:hasTime _:node125 .

:wikipediaPerangAceh time:hasTime _:node140, _:node145 .

:wikipediaInvasiCholakeSriwijaya time:hasTime _:node150 .

:wikipediaPerangBelasting time:hasTime _:node155 .

:wikipediaPerangKuning time:hasTime _:node160 .

:wikipediaPerangPadri time:hasTime _:node165 .

:wikipediaPerangJawa17411743 time:hasTime _:node175 .

:wikipediaPerangTakhtaJawaKetiga time:hasTime _:node180 .

:wikipediaPerangTakhtaJawaKedua time:hasTime _:node190 .

:wikipediaIntervensiBelandadiBali1858 time:hasTime _:node195 .

:wikipediaPerangBayu time:hasTime _:node215 .

:wikipediaPerangRegreg time:hasTime _:node220 .

:wikipediaPerangBubat time:hasTime _:node225 .

:wikipediaPertempuranMelaka1641 time:hasTime _:node255 .

:wikipediaPenyerbuanMeesterCornelis time:hasTime _:node275 .

:wikipediaIntervensiBelandadiBali1908 time:hasTime _:node295 .

:wikipediaInvasiMaluku time:hasTime _:node305 .

:wikipediaPerangDiponegoro time:hasTime _:node310 .

:wikipediaEkspedisiPalembangII time:hasTime _:node315 .

:wikipediaSerbuanYuanMongolkeJawa time:hasTime _:node320 .

:wikipediaPemberontakanRadenRonggo time:hasTime _:node330 .

:wikipediaGegerSepehi time:hasTime _:node340 .

:wikipediaPerangTakhtaJawaPertama time:hasTime _:node345 .

:JisaburoOzawa time:hasTime _:node565 .

:MuhammadMangundiprojo time:hasTime _:node820 .

:Soengkono time:hasTime _:node620 .

:HarioJonosewojo time:hasTime _:node440 .

:MoehammadJasin time:hasTime _:node950 .

:Moestopo time:hasTime _:node445 .

:RobertMansergh time:hasTime _:node450 .

:AubertinMallaby time:hasTime _:node555 .

:Sutomo time:hasTime _:node375 .

:GoliathTabuni time:hasTime _:node655 .

:Soekarno time:hasTime _:node810 .

:KiyotakeKawaguchi time:hasTime _:node785 .

:RaymondWesterling time:hasTime _:node890 .

:MathiasWenda time:hasTime _:node845 .

:JuliusTahija time:hasTime _:node840 .

:InfanteriBelanda time:hasTime _:node625 .

:Moekijat time:hasTime _:node760 .

:MohammadHatta time:hasTime _:node580 .

:DouglasMacArthur time:hasTime _:node805 .

:ListyoSigitPrabowo time:hasTime _:node490 .

:REMartadinata time:hasTime _:node500 .

:TeukuKeumanganUmar time:hasTime _:node690 .

:NobutakeKond time:hasTime _:node830 .

:SutanSjahrir time:hasTime _:node720 .

:SlametRijadi time:hasTime _:node585 .

:TEDKelly time:hasTime _:node755 .

:AgusSubiyanto time:hasTime _:node695 .

:Assaat time:hasTime _:node360 .

:PangRati time:hasTime _:node945 .

:MacDonald time:hasTime _:node920 .

:MuhammadToha time:hasTime _:node780 .

:AbdulHarisNasution time:hasTime _:node635 .

:KidoShinichir time:hasTime _:node615 .

:PrabowoSubianto time:hasTime _:node1005 .

:EgianusKogoya time:hasTime _:node685 .

:BudiGunawan time:hasTime _:node700 .

:JaminGinting time:hasTime _:node405 .

:AbdulKarimMS time:hasTime _:node460 .

:AchmadTahir time:hasTime _:node610 .

:HubertusJohannesvanMook time:hasTime _:node605 .

:TeungkuHasanKruengKalee time:hasTime _:node870 .

:TeukuDaudCumbok time:hasTime _:node455 .

:TeukuNyakArif time:hasTime _:node575 .

:TeungkuAhmadHasballah time:hasTime _:node660 .

:SyamaunGaharu time:hasTime _:node985 .

:DaudBeureueh time:hasTime _:node835 .

:MichiakiKamada time:hasTime _:node540 .

:ThomasKinkaid time:hasTime _:node530 .

:HeinterPoorten time:hasTime _:node650 .

:JBTKnig time:hasTime _:node590 .

:FMollinger time:hasTime _:node990 .

:IGustiNgurahRai time:hasTime _:node815 .

:SimonSpoor time:hasTime _:node965 .

:BabaMasao time:hasTime _:node970 .

:SyafruddinPrawiranegara time:hasTime _:node395 .

:MaludinSimbolon time:hasTime _:node640 .

:AhmadYani time:hasTime _:node520 .

:AhmadHusein time:hasTime _:node740 .

:HitoshiImamura time:hasTime _:node665 .

:AJFDoulton time:hasTime _:node1000 .

:EdiSukardi time:hasTime _:node955 .

:Musso time:hasTime _:node670 .

:TanMalaka time:hasTime _:node905 .

:HisaichiTerauchi time:hasTime _:node710 .

:Meyer time:hasTime _:node885 .

:JoniBotak time:hasTime _:node355 .

:LouisMountbatten time:hasTime _:node855 .

:Djampi time:hasTime _:node775 .

:PangIyo time:hasTime _:node910 .

:PangSuma time:hasTime _:node645 .

:Nagatani time:hasTime _:node370 .

:DirkCornelisBuurmanvanVreeden time:hasTime _:node790 .

:SebbySambom time:hasTime _:node415 .

:Mollinger time:hasTime _:node795 .

:AlidiusTjardavanStarkenborghStachouwer time:hasTime _:node410 .

:DaanMogot time:hasTime _:node935 .

:IbTakahashi time:hasTime _:node430 .

:LudolphHendrikvanOyen time:hasTime _:node825 .

:TjokordaGdeRakaSoekawati time:hasTime _:node850 .

:Wongsonegoro time:hasTime _:node535 .

:Kariadi time:hasTime _:node515 .

:GatotSoebroto time:hasTime _:node865 .

:KellyKwalik time:hasTime _:node550 .

:BJHabibie time:hasTime _:node975 .

:VanVreeden time:hasTime _:node745 .

:ThomasCHart time:hasTime _:node510 .

:ShojiNishimura time:hasTime _:node630 .

:Soedirman time:hasTime _:node705 .

:TakeoTakagi time:hasTime _:node800 .

:DirkReinhardAdelbertvanLangen time:hasTime _:node390 .

:BambangSoegeng time:hasTime _:node425 .

:OeripSoemohardjo time:hasTime _:node730 .

:AndikaPerkasa time:hasTime _:node570 .

:ConradHelfrich time:hasTime _:node470 .

:ArchibaldWavell1stEarlWavell time:hasTime _:node900 .

:RichardPeirse time:hasTime _:node980 .

:KarelDoorman time:hasTime _:node400 .

:HamengkubuwanaIX time:hasTime _:node770 .

:VentjeSumual time:hasTime _:node675 .

:JMvdBerge time:hasTime _:node485 .

:Soeharto time:hasTime _:node680 .

:Otzuka time:hasTime _:node465 .

:LeslieMorshead time:hasTime _:node915 .

:SusiloBambangYudhoyono time:hasTime _:node875 .

:SaalahYusufSutanMangkuto time:hasTime _:node930 .

:WilhelminadariBelanda time:hasTime _:node420 .

:LeonardusBenyaminMoerdani time:hasTime _:node600 .

:MarufAmin time:hasTime _:node860 .

:MegawatiSoekarnoputri time:hasTime _:node495 .

:TBSimatupang time:hasTime _:node940 .

:AdamBB time:hasTime _:node750 .

:Wiranto time:hasTime _:node960 .

:LoaSekHie time:hasTime _:node735 .

:SyarifHamidIIdariPontianak time:hasTime _:node560 .

:PhilipChristison time:hasTime _:node365 .

:BennyWenda time:hasTime _:node525 .

:AbdulkadirWidjojoatmodjo time:hasTime _:node765 .

:JacobPrai time:hasTime _:node715 .

:AbdulKaharMuzakkar time:hasTime _:node880 .

:IsmaelLengah time:hasTime _:node380 .

:TrySutrisno time:hasTime _:node545 .

:PakubuwanaXII time:hasTime _:node995 .

:MangkunegaraVIII time:hasTime _:node435 .

:AchmadiHadisoemarto time:hasTime _:node595 .

:JokoWidodo time:hasTime _:node475 .

:JacobRumbiak time:hasTime _:node480 .

:SekarmadjiMaridjanKartosoewirjo time:hasTime _:node725 .

:AmirSjarifoeddin time:hasTime _:node895 .

:AgustinusAdisoetjipto time:hasTime _:node385 .

:AbdurrahmanWahid time:hasTime _:node505 .

:JulianadariBelanda time:hasTime _:node925 .

_:node10 owl:unionOf _:node11 .

_:node13 owl:unionOf _:node14 .

_:node63 owl:unionOf _:node64 .

_:node67 owl:unionOf _:node68 .

time:hasTime <http://www.w3.org/2004/02/skos/core#editorialNote> "Caracterstica arriesgada -aadida en la revisin del 2017 que no ha sido todava utilizada de forma amplia."@es,
    "Feature at risk - added in 2017 revision, and not yet widely used. "@en .

time:monthOfYear <http://www.w3.org/2004/02/skos/core#editorialNote> "Feature at risk - added in 2017 revision, and not yet widely used. "@en,
    "Caracterstica arriesgada - aadida en la revisin de 2017, y todava no ampliamente utilizada."@es .

time:MonthOfYear <http://www.w3.org/2004/02/skos/core#editorialNote> "Feature at risk - added in 2017 revision, and not yet widely used. "@en,
    "Caracterstica en riesgo - aadida en la revisin de 2017, y no utilizada todava de forma amplia."@es .

time:hasXSDDuration <http://www.w3.org/2004/02/skos/core#editorialNote> "Feature at risk - added in 2017 revision, and not yet widely used. "@en,
    "Caracterstica arriesgada - aadida en la revisin de 2017, y todava no ampliamente utilizada."@es .

_:node101 time:inDateTime _:node102 .

_:node103 time:inDateTime _:node104 .

_:node106 time:inDateTime _:node107 .

_:node108 time:inDateTime _:node109 .

_:node111 time:inDateTime _:node112 .

_:node113 time:inDateTime _:node114 .

_:node116 time:inDateTime _:node117 .

_:node118 time:inDateTime _:node119 .

_:node121 time:inDateTime _:node122 .

_:node123 time:inDateTime _:node124 .

_:node126 time:inDateTime _:node127 .

_:node128 time:inDateTime _:node129 .

_:node131 time:inDateTime _:node132 .

_:node133 time:inDateTime _:node134 .

_:node136 time:inDateTime _:node137 .

_:node138 time:inDateTime _:node139 .

_:node141 time:inDateTime _:node142 .

_:node143 time:inDateTime _:node144 .

_:node146 time:inDateTime _:node147 .

_:node148 time:inDateTime _:node149 .

_:node151 time:inDateTime _:node152 .

_:node153 time:inDateTime _:node154 .

_:node156 time:inDateTime _:node157 .

_:node158 time:inDateTime _:node159 .

_:node161 time:inDateTime _:node162 .

_:node163 time:inDateTime _:node164 .

_:node166 time:inDateTime _:node167 .

_:node168 time:inDateTime _:node169 .

_:node171 time:inDateTime _:node172 .

_:node173 time:inDateTime _:node174 .

_:node176 time:inDateTime _:node177 .

_:node178 time:inDateTime _:node179 .

_:node181 time:inDateTime _:node182 .

_:node183 time:inDateTime _:node184 .

_:node186 time:inDateTime _:node187 .

_:node188 time:inDateTime _:node189 .

_:node191 time:inDateTime _:node192 .

_:node193 time:inDateTime _:node194 .

_:node196 time:inDateTime _:node197 .

_:node198 time:inDateTime _:node199 .

_:node201 time:inDateTime _:node202 .

_:node203 time:inDateTime _:node204 .

_:node206 time:inDateTime _:node207 .

_:node208 time:inDateTime _:node209 .

_:node211 time:inDateTime _:node212 .

_:node213 time:inDateTime _:node214 .

_:node216 time:inDateTime _:node217 .

_:node218 time:inDateTime _:node219 .

_:node221 time:inDateTime _:node222 .

_:node223 time:inDateTime _:node224 .

_:node226 time:inDateTime _:node227 .

_:node228 time:inDateTime _:node229 .

_:node231 time:inDateTime _:node232 .

_:node233 time:inDateTime _:node234 .

_:node236 time:inDateTime _:node237 .

_:node238 time:inDateTime _:node239 .

_:node241 time:inDateTime _:node242 .

_:node243 time:inDateTime _:node244 .

_:node246 time:inDateTime _:node247 .

_:node248 time:inDateTime _:node249 .

_:node251 time:inDateTime _:node252 .

_:node253 time:inDateTime _:node254 .

_:node256 time:inDateTime _:node257 .

_:node258 time:inDateTime _:node259 .

_:node261 time:inDateTime _:node262 .

_:node263 time:inDateTime _:node264 .

_:node266 time:inDateTime _:node267 .

_:node268 time:inDateTime _:node269 .

_:node271 time:inDateTime _:node272 .

_:node273 time:inDateTime _:node274 .

_:node276 time:inDateTime _:node277 .

_:node278 time:inDateTime _:node279 .

_:node281 time:inDateTime _:node282 .

_:node283 time:inDateTime _:node284 .

_:node286 time:inDateTime _:node287 .

_:node288 time:inDateTime _:node289 .

_:node291 time:inDateTime _:node292 .

_:node293 time:inDateTime _:node294 .

_:node296 time:inDateTime _:node297 .

_:node298 time:inDateTime _:node299 .

_:node301 time:inDateTime _:node302 .

_:node303 time:inDateTime _:node304 .

_:node306 time:inDateTime _:node307 .

_:node308 time:inDateTime _:node309 .

_:node311 time:inDateTime _:node312 .

_:node313 time:inDateTime _:node314 .

_:node316 time:inDateTime _:node317 .

_:node318 time:inDateTime _:node319 .

_:node321 time:inDateTime _:node322 .

_:node323 time:inDateTime _:node324 .

_:node326 time:inDateTime _:node327 .

_:node328 time:inDateTime _:node329 .

_:node331 time:inDateTime _:node332 .

_:node333 time:inDateTime _:node334 .

_:node336 time:inDateTime _:node337 .

_:node338 time:inDateTime _:node339 .

_:node341 time:inDateTime _:node342 .

_:node343 time:inDateTime _:node344 .

_:node346 time:inDateTime _:node347 .

_:node348 time:inDateTime _:node349 .

_:node351 time:inDateTime _:node352 .

_:node353 time:inDateTime _:node354 .

_:node356 time:inDateTime _:node357 .

_:node358 time:inDateTime _:node359 .

_:node361 time:inDateTime _:node362 .

_:node363 time:inDateTime _:node364 .

_:node366 time:inDateTime _:node367 .

_:node368 time:inDateTime _:node369 .

_:node371 time:inDateTime _:node372 .

_:node373 time:inDateTime _:node374 .

_:node376 time:inDateTime _:node377 .

_:node378 time:inDateTime _:node379 .

_:node381 time:inDateTime _:node382 .

_:node383 time:inDateTime _:node384 .

_:node386 time:inDateTime _:node387 .

_:node388 time:inDateTime _:node389 .

_:node391 time:inDateTime _:node392 .

_:node393 time:inDateTime _:node394 .

_:node396 time:inDateTime _:node397 .

_:node398 time:inDateTime _:node399 .

_:node401 time:inDateTime _:node402 .

_:node403 time:inDateTime _:node404 .

_:node406 time:inDateTime _:node407 .

_:node408 time:inDateTime _:node409 .

_:node411 time:inDateTime _:node412 .

_:node413 time:inDateTime _:node414 .

_:node416 time:inDateTime _:node417 .

_:node418 time:inDateTime _:node419 .

_:node421 time:inDateTime _:node422 .

_:node423 time:inDateTime _:node424 .

_:node426 time:inDateTime _:node427 .

_:node428 time:inDateTime _:node429 .

_:node431 time:inDateTime _:node432 .

_:node433 time:inDateTime _:node434 .

_:node436 time:inDateTime _:node437 .

_:node438 time:inDateTime _:node439 .

_:node441 time:inDateTime _:node442 .

_:node443 time:inDateTime _:node444 .

_:node446 time:inDateTime _:node447 .

_:node448 time:inDateTime _:node449 .

_:node451 time:inDateTime _:node452 .

_:node453 time:inDateTime _:node454 .

_:node456 time:inDateTime _:node457 .

_:node458 time:inDateTime _:node459 .

_:node461 time:inDateTime _:node462 .

_:node463 time:inDateTime _:node464 .

_:node466 time:inDateTime _:node467 .

_:node468 time:inDateTime _:node469 .

_:node471 time:inDateTime _:node472 .

_:node473 time:inDateTime _:node474 .

_:node476 time:inDateTime _:node477 .

_:node478 time:inDateTime _:node479 .

_:node481 time:inDateTime _:node482 .

_:node483 time:inDateTime _:node484 .

_:node486 time:inDateTime _:node487 .

_:node488 time:inDateTime _:node489 .

_:node491 time:inDateTime _:node492 .

_:node493 time:inDateTime _:node494 .

_:node496 time:inDateTime _:node497 .

_:node498 time:inDateTime _:node499 .

_:node501 time:inDateTime _:node502 .

_:node503 time:inDateTime _:node504 .

_:node506 time:inDateTime _:node507 .

_:node508 time:inDateTime _:node509 .

_:node511 time:inDateTime _:node512 .

_:node513 time:inDateTime _:node514 .

_:node516 time:inDateTime _:node517 .

_:node518 time:inDateTime _:node519 .

_:node521 time:inDateTime _:node522 .

_:node523 time:inDateTime _:node524 .

_:node526 time:inDateTime _:node527 .

_:node528 time:inDateTime _:node529 .

_:node531 time:inDateTime _:node532 .

_:node533 time:inDateTime _:node534 .

_:node536 time:inDateTime _:node537 .

_:node538 time:inDateTime _:node539 .

_:node541 time:inDateTime _:node542 .

_:node543 time:inDateTime _:node544 .

_:node546 time:inDateTime _:node547 .

_:node548 time:inDateTime _:node549 .

_:node551 time:inDateTime _:node552 .

_:node553 time:inDateTime _:node554 .

_:node556 time:inDateTime _:node557 .

_:node558 time:inDateTime _:node559 .

_:node561 time:inDateTime _:node562 .

_:node563 time:inDateTime _:node564 .

_:node566 time:inDateTime _:node567 .

_:node568 time:inDateTime _:node569 .

_:node571 time:inDateTime _:node572 .

_:node573 time:inDateTime _:node574 .

_:node576 time:inDateTime _:node577 .

_:node578 time:inDateTime _:node579 .

_:node581 time:inDateTime _:node582 .

_:node583 time:inDateTime _:node584 .

_:node586 time:inDateTime _:node587 .

_:node588 time:inDateTime _:node589 .

_:node591 time:inDateTime _:node592 .

_:node593 time:inDateTime _:node594 .

_:node596 time:inDateTime _:node597 .

_:node598 time:inDateTime _:node599 .

_:node601 time:inDateTime _:node602 .

_:node603 time:inDateTime _:node604 .

_:node606 time:inDateTime _:node607 .

_:node608 time:inDateTime _:node609 .

_:node611 time:inDateTime _:node612 .

_:node613 time:inDateTime _:node614 .

_:node616 time:inDateTime _:node617 .

_:node618 time:inDateTime _:node619 .

_:node621 time:inDateTime _:node622 .

_:node623 time:inDateTime _:node624 .

_:node626 time:inDateTime _:node627 .

_:node628 time:inDateTime _:node629 .

_:node631 time:inDateTime _:node632 .

_:node633 time:inDateTime _:node634 .

_:node636 time:inDateTime _:node637 .

_:node638 time:inDateTime _:node639 .

_:node641 time:inDateTime _:node642 .

_:node643 time:inDateTime _:node644 .

_:node646 time:inDateTime _:node647 .

_:node648 time:inDateTime _:node649 .

_:node651 time:inDateTime _:node652 .

_:node653 time:inDateTime _:node654 .

_:node656 time:inDateTime _:node657 .

_:node658 time:inDateTime _:node659 .

_:node661 time:inDateTime _:node662 .

_:node663 time:inDateTime _:node664 .

_:node666 time:inDateTime _:node667 .

_:node668 time:inDateTime _:node669 .

_:node671 time:inDateTime _:node672 .

_:node673 time:inDateTime _:node674 .

_:node676 time:inDateTime _:node677 .

_:node678 time:inDateTime _:node679 .

_:node681 time:inDateTime _:node682 .

_:node683 time:inDateTime _:node684 .

_:node686 time:inDateTime _:node687 .

_:node688 time:inDateTime _:node689 .

_:node691 time:inDateTime _:node692 .

_:node693 time:inDateTime _:node694 .

_:node696 time:inDateTime _:node697 .

_:node698 time:inDateTime _:node699 .

_:node701 time:inDateTime _:node702 .

_:node703 time:inDateTime _:node704 .

_:node706 time:inDateTime _:node707 .

_:node708 time:inDateTime _:node709 .

_:node711 time:inDateTime _:node712 .

_:node713 time:inDateTime _:node714 .

_:node716 time:inDateTime _:node717 .

_:node718 time:inDateTime _:node719 .

_:node721 time:inDateTime _:node722 .

_:node723 time:inDateTime _:node724 .

_:node726 time:inDateTime _:node727 .

_:node728 time:inDateTime _:node729 .

_:node731 time:inDateTime _:node732 .

_:node733 time:inDateTime _:node734 .

_:node736 time:inDateTime _:node737 .

_:node738 time:inDateTime _:node739 .

_:node741 time:inDateTime _:node742 .

_:node743 time:inDateTime _:node744 .

_:node746 time:inDateTime _:node747 .

_:node748 time:inDateTime _:node749 .

_:node751 time:inDateTime _:node752 .

_:node753 time:inDateTime _:node754 .

_:node756 time:inDateTime _:node757 .

_:node758 time:inDateTime _:node759 .

_:node761 time:inDateTime _:node762 .

_:node763 time:inDateTime _:node764 .

_:node766 time:inDateTime _:node767 .

_:node768 time:inDateTime _:node769 .

_:node771 time:inDateTime _:node772 .

_:node773 time:inDateTime _:node774 .

_:node776 time:inDateTime _:node777 .

_:node778 time:inDateTime _:node779 .

_:node781 time:inDateTime _:node782 .

_:node783 time:inDateTime _:node784 .

_:node786 time:inDateTime _:node787 .

_:node788 time:inDateTime _:node789 .

_:node791 time:inDateTime _:node792 .

_:node793 time:inDateTime _:node794 .

_:node796 time:inDateTime _:node797 .

_:node798 time:inDateTime _:node799 .

_:node801 time:inDateTime _:node802 .

_:node803 time:inDateTime _:node804 .

_:node806 time:inDateTime _:node807 .

_:node808 time:inDateTime _:node809 .

_:node811 time:inDateTime _:node812 .

_:node813 time:inDateTime _:node814 .

_:node816 time:inDateTime _:node817 .

_:node818 time:inDateTime _:node819 .

_:node821 time:inDateTime _:node822 .

_:node823 time:inDateTime _:node824 .

_:node826 time:inDateTime _:node827 .

_:node828 time:inDateTime _:node829 .

_:node831 time:inDateTime _:node832 .

_:node833 time:inDateTime _:node834 .

_:node836 time:inDateTime _:node837 .

_:node838 time:inDateTime _:node839 .

_:node841 time:inDateTime _:node842 .

_:node843 time:inDateTime _:node844 .

_:node846 time:inDateTime _:node847 .

_:node848 time:inDateTime _:node849 .

_:node851 time:inDateTime _:node852 .

_:node853 time:inDateTime _:node854 .

_:node856 time:inDateTime _:node857 .

_:node858 time:inDateTime _:node859 .

_:node861 time:inDateTime _:node862 .

_:node863 time:inDateTime _:node864 .

_:node866 time:inDateTime _:node867 .

_:node868 time:inDateTime _:node869 .

_:node871 time:inDateTime _:node872 .

_:node873 time:inDateTime _:node874 .

_:node876 time:inDateTime _:node877 .

_:node878 time:inDateTime _:node879 .

_:node881 time:inDateTime _:node882 .

_:node883 time:inDateTime _:node884 .

_:node886 time:inDateTime _:node887 .

_:node888 time:inDateTime _:node889 .

_:node891 time:inDateTime _:node892 .

_:node893 time:inDateTime _:node894 .

_:node896 time:inDateTime _:node897 .

_:node898 time:inDateTime _:node899 .

_:node901 time:inDateTime _:node902 .

_:node903 time:inDateTime _:node904 .

_:node906 time:inDateTime _:node907 .

_:node908 time:inDateTime _:node909 .

_:node911 time:inDateTime _:node912 .

_:node913 time:inDateTime _:node914 .

_:node916 time:inDateTime _:node917 .

_:node918 time:inDateTime _:node919 .

_:node921 time:inDateTime _:node922 .

_:node923 time:inDateTime _:node924 .

_:node926 time:inDateTime _:node927 .

_:node928 time:inDateTime _:node929 .

_:node931 time:inDateTime _:node932 .

_:node933 time:inDateTime _:node934 .

_:node936 time:inDateTime _:node937 .

_:node938 time:inDateTime _:node939 .

_:node941 time:inDateTime _:node942 .

_:node943 time:inDateTime _:node944 .

_:node946 time:inDateTime _:node947 .

_:node948 time:inDateTime _:node949 .

_:node951 time:inDateTime _:node952 .

_:node953 time:inDateTime _:node954 .

_:node956 time:inDateTime _:node957 .

_:node958 time:inDateTime _:node959 .

_:node961 time:inDateTime _:node962 .

_:node963 time:inDateTime _:node964 .

_:node966 time:inDateTime _:node967 .

_:node968 time:inDateTime _:node969 .

_:node971 time:inDateTime _:node972 .

_:node973 time:inDateTime _:node974 .

_:node976 time:inDateTime _:node977 .

_:node978 time:inDateTime _:node979 .

_:node981 time:inDateTime _:node982 .

_:node983 time:inDateTime _:node984 .

_:node986 time:inDateTime _:node987 .

_:node988 time:inDateTime _:node989 .

_:node991 time:inDateTime _:node992 .

_:node993 time:inDateTime _:node994 .

_:node996 time:inDateTime _:node997 .

_:node998 time:inDateTime _:node999 .

_:node1001 time:inDateTime _:node1002 .

_:node1003 time:inDateTime _:node1004 .

_:node1006 time:inDateTime _:node1007 .

_:node1008 time:inDateTime _:node1009 .

time:intervalEquals owl:propertyDisjointWith time:intervalIn .

_:node102 time:day "24";
  time:month "3";
  time:year "1946" .

_:node104 time:day "24";
  time:month "4";
  time:year "1946" .

_:node117 time:day "20";
  time:month "9";
  time:year "1953" .

_:node122 time:day "1";
  time:month "5";
  time:year "1945" .

_:node124 time:day "15";
  time:month "8";
  time:year "1945" .

_:node127 time:day "7";
  time:month "12";
  time:year "1941" .

_:node129 time:day "2";
  time:month "9";
  time:year "1945" .

_:node137 time:day "29";
  time:month "9";
  time:year "1945" .

_:node139 time:day "27";
  time:month "12";
  time:year "1949" .

_:node157 time:day "15";
  time:month "6";
  time:year "1908" .

_:node159 time:day "16";
  time:month "6";
  time:year "1908" .

_:node172 time:day "2";
  time:month "12";
  time:year "1945" .

_:node174 time:day "16";
  time:month "1";
  time:year "1946" .

_:node182 time:day "15";
  time:month "12";
  time:year "1749" .

_:node187 time:day "1";
  time:month "3";
  time:year "1949" .

_:node202 time:day "1";
  time:month "10";
  time:year "1962" .

_:node207 time:day "3";
  time:month "3";
  time:year "1947" .

_:node212 time:day "7";
  time:month "10";
  time:year "1945" .

_:node217 time:day "5";
  time:month "7";
  time:year "1771" .

_:node219 time:day "11";
  time:month "10";
  time:year "1772" .

_:node234 time:day "0";
  time:month "6";
  time:year "1945" .

_:node237 time:day "30";
  time:month "9";
  time:year "1965" .

_:node239 time:day "1";
  time:month "10";
  time:year "1965" .

_:node242 time:day "8";
  time:month "12";
  time:year "1941" .

_:node244 time:day "9";
  time:month "3";
  time:year "1942" .

_:node247 time:day "8";
  time:month "12";
  time:year "1941" .

_:node249 time:day "9";
  time:month "3";
  time:year "1942" .

_:node252 time:day "25";
  time:month "1";
  time:year "1946" .

_:node262 time:day "13";
  time:month "10";
  time:year "1945" .

_:node264 time:day "15";
  time:month "4";
  time:year "1946" .

_:node267 time:day "14";
  time:month "1";
  time:year "1946" .

_:node272 time:day "7";
  time:month "8";
  time:year "1949" .

_:node277 time:day "14";
  time:month "8";
  time:year "1811" .

_:node279 time:day "26";
  time:month "8";
  time:year "1811" .

_:node282 time:day "20";
  time:month "11";
  time:year "1946" .

_:node287 time:day "15";
  time:month "10";
  time:year "1945" .

_:node289 time:day "19";
  time:month "10";
  time:year "1945" .

_:node292 time:day "15";
  time:month "10";
  time:year "1945" .

_:node294 time:day "19";
  time:month "10";
  time:year "1945" .

_:node297 time:day "28";
  time:month "4";
  time:year "1908" .

_:node302 time:day "27";
  time:month "10";
  time:year "1945" .

_:node304 time:day "20";
  time:month "11";
  time:year "1945" .

_:node312 time:day "21";
  time:month "6";
  time:year "1825" .

_:node314 time:day "9";
  time:month "2";
  time:year "1830" .

_:node322 time:day "22";
  time:month "1";
  time:year "1293" .

_:node332 time:day "20";
  time:month "11";
  time:year "1810" .

_:node334 time:day "17";
  time:month "12";
  time:year "1810" .

_:node337 time:day "19";
  time:month "11";
  time:year "1945" .

_:node342 time:day "19";
  time:month "6";
  time:year "1812" .

_:node344 time:day "20";
  time:month "6";
  time:year "1812" .

_:node352 time:day "17";
  time:month "4";
  time:year "1958" .

_:node354 time:day "24";
  time:month "5";
  time:year "1958" .

_:node362 time:day "18";
  time:month "09";
  time:year "1904" .

_:node364 time:day "16";
  time:month "06";
  time:year "1976" .

_:node367 time:day "17";
  time:month "11";
  time:year "1893" .

_:node369 time:day "21";
  time:month "12";
  time:year "1993" .

_:node377 time:day "03";
  time:month "10";
  time:year "1920" .

_:node379 time:day "07";
  time:month "10";
  time:year "1981" .

_:node382 time:day "22";
  time:month "09";
  time:year "1914" .

_:node384 time:day "11";
  time:month "01";
  time:year "2005" .

_:node387 time:day "03";
  time:month "07";
  time:year "1916" .

_:node389 time:day "29";
  time:month "07";
  time:year "1947" .

_:node392 time:day "17";
  time:month "05";
  time:year "1898" .

_:node394 time:day "20";
  time:month "01";
  time:year "1983" .

_:node397 time:day "28";
  time:month "02";
  time:year "1911" .

_:node399 time:day "15";
  time:month "02";
  time:year "1989" .

_:node402 time:day "23";
  time:month "04";
  time:year "1889" .

_:node404 time:day "28";
  time:month "02";
  time:year "1942" .

_:node407 time:day "12";
  time:month "01";
  time:year "1921" .

_:node409 time:day "23";
  time:month "10";
  time:year "1974" .

_:node412 time:day "07";
  time:month "03";
  time:year "1888" .

_:node414 time:day "16";
  time:month "08";
  time:year "1978" .

_:node417 time:day "03";
  time:month "01";
  time:year "1975" .

_:node422 time:day "31";
  time:month "08";
  time:year "1880" .

_:node424 time:day "28";
  time:month "11";
  time:year "1962" .

_:node427 time:day "31";
  time:month "10";
  time:year "1913" .

_:node429 time:day "22";
  time:month "06";
  time:year "1977" .

_:node437 time:day "01";
  time:month "01";
  time:year "1920" .

_:node439 time:day "03";
  time:month "09";
  time:year "1987" .

_:node442 time:day "09";
  time:month "06";
  time:year "1920" .

_:node444 time:day "22";
  time:month "03";
  time:year "1994" .

_:node447 time:day "13";
  time:month "06";
  time:year "1913" .

_:node449 time:day "29";
  time:month "09";
  time:year "1986" .

_:node452 time:day "12";
  time:month "05";
  time:year "1900" .

_:node454 time:day "08";
  time:month "11";
  time:year "1970" .

_:node472 time:day "11";
  time:month "10";
  time:year "1886" .

_:node474 time:day "20";
  time:month "09";
  time:year "1962" .

_:node477 time:day "21";
  time:month "06";
  time:year "1961" .

_:node482 time:day "11";
  time:month "03";
  time:year "1958" .

_:node492 time:day "05";
  time:month "05";
  time:year "1969" .

_:node497 time:day "23";
  time:month "01";
  time:year "1947" .

_:node502 time:day "29";
  time:month "03";
  time:year "1921" .

_:node504 time:day "06";
  time:month "10";
  time:year "1966" .

_:node507 time:day "07";
  time:month "09";
  time:year "1940" .

_:node509 time:day "30";
  time:month "12";
  time:year "2009" .

_:node512 time:day "12";
  time:month "06";
  time:year "1877" .

_:node514 time:day "04";
  time:month "07";
  time:year "1971" .

_:node517 time:day "15";
  time:month "09";
  time:year "1905" .

_:node519 time:day "14";
  time:month "10";
  time:year "1945" .

_:node522 time:day "19";
  time:month "06";
  time:year "1922" .

_:node524 time:day "01";
  time:month "10";
  time:year "1965" .

_:node537 time:day "20";
  time:month "04";
  time:year "1897" .

_:node539 time:day "04";
  time:month "03";
  time:year "1978" .

_:node547 time:day "15";
  time:month "11";
  time:year "1935" .

_:node554 time:day "16";
  time:month "12";
  time:year "2009" .

_:node557 time:day "12";
  time:month "12";
  time:year "1899" .

_:node559 time:day "30";
  time:month "10";
  time:year "1945" .

_:node562 time:day "12";
  time:month "07";
  time:year "1913" .

_:node564 time:day "30";
  time:month "03";
  time:year "1978" .

_:node567 time:day "02";
  time:month "10";
  time:year "1886" .

_:node569 time:day "09";
  time:month "11";
  time:year "1966" .

_:node572 time:day "21";
  time:month "12";
  time:year "1964" .

_:node577 time:day "17";
  time:month "07";
  time:year "1899" .

_:node579 time:day "04";
  time:month "05";
  time:year "1946" .

_:node582 time:day "12";
  time:month "08";
  time:year "1902" .

_:node584 time:day "14";
  time:month "03";
  time:year "1980" .

_:node587 time:day "26";
  time:month "07";
  time:year "1927" .

_:node589 time:day "04";
  time:month "11";
  time:year "1950" .

_:node597 time:day "05";
  time:month "06";
  time:year "1927" .

_:node599 time:day "02";
  time:month "01";
  time:year "1984" .

_:node602 time:day "02";
  time:month "10";
  time:year "1932" .

_:node604 time:day "29";
  time:month "08";
  time:year "2004" .

_:node607 time:day "20";
  time:month "05";
  time:year "1894" .

_:node609 time:day "10";
  time:month "05";
  time:year "1965" .

_:node612 time:day "27";
  time:month "06";
  time:year "1924" .

_:node614 time:day "17";
  time:month "08";
  time:year "2002" .

_:node622 time:day "01";
  time:month "01";
  time:year "1911" .

_:node624 time:day "12";
  time:month "09";
  time:year "1977" .

_:node632 time:day "30";
  time:month "11";
  time:year "1889" .

_:node634 time:day "24";
  time:month "10";
  time:year "1944" .

_:node637 time:day "03";
  time:month "12";
  time:year "1918" .

_:node639 time:day "06";
  time:month "09";
  time:year "2000" .

_:node642 time:day "13";
  time:month "04";
  time:year "1916" .

_:node644 time:day "15";
  time:month "04";
  time:year "2000" .

_:node652 time:day "21";
  time:month "11";
  time:year "1887" .

_:node654 time:day "15";
  time:month "01";
  time:year "1968" .

_:node667 time:day "28";
  time:month "06";
  time:year "1886" .

_:node669 time:day "04";
  time:month "10";
  time:year "1968" .

_:node672 time:day "12";
  time:month "08";
  time:year "1897" .

_:node674 time:day "31";
  time:month "10";
  time:year "1948" .

_:node677 time:day "11";
  time:month "06";
  time:year "1923" .

_:node679 time:day "28";
  time:month "03";
  time:year "2010" .

_:node682 time:day "08";
  time:month "06";
  time:year "1921" .

_:node684 time:day "27";
  time:month "01";
  time:year "2008" .

_:node697 time:day "05";
  time:month "08";
  time:year "1967" .

_:node702 time:day "11";
  time:month "12";
  time:year "1959" .

_:node707 time:day "24";
  time:month "01";
  time:year "1916" .

_:node709 time:day "29";
  time:month "01";
  time:year "1950" .

_:node712 time:day "08";
  time:month "08";
  time:year "1879" .

_:node714 time:day "12";
  time:month "06";
  time:year "1946" .

_:node717 time:day "17";
  time:month "07";
  time:year "1942" .

_:node719 time:day "26";
  time:month "05";
  time:year "2022" .

_:node722 time:day "05";
  time:month "03";
  time:year "1909" .

_:node724 time:day "09";
  time:month "04";
  time:year "1966" .

_:node727 time:day "07";
  time:month "01";
  time:year "1905" .

_:node729 time:day "05";
  time:month "09";
  time:year "1962" .

_:node732 time:day "22";
  time:month "02";
  time:year "1893" .

_:node734 time:day "17";
  time:month "11";
  time:year "1948" .

_:node742 time:day "01";
  time:month "04";
  time:year "1925" .

_:node744 time:day "28";
  time:month "11";
  time:year "1998" .

_:node752 time:day "31";
  time:month "08";
  time:year "1889" .

_:node754 time:day "15";
  time:month "07";
  time:year "1953" .

_:node762 time:day "15";
  time:month "12";
  time:year "1927" .

_:node764 time:day "01";
  time:month "11";
  time:year "1985" .

_:node767 time:day "18";
  time:month "12";
  time:year "1904" .

_:node769 time:day "24";
  time:month "12";
  time:year "1992" .

_:node772 time:day "12";
  time:month "04";
  time:year "1912" .

_:node774 time:day "02";
  time:month "10";
  time:year "1988" .

_:node784 time:day "11";
  time:month "07";
  time:year "1946" .

_:node787 time:day "03";
  time:month "12";
  time:year "1892" .

_:node789 time:day "16";
  time:month "05";
  time:year "1961" .

_:node792 time:day "16";
  time:month "06";
  time:year "1902" .

_:node794 time:day "12";
  time:month "06";
  time:year "1964" .

_:node802 time:day "25";
  time:month "01";
  time:year "1892" .

_:node804 time:day "08";
  time:month "07";
  time:year "1944" .

_:node807 time:day "26";
  time:month "01";
  time:year "1880" .

_:node809 time:day "05";
  time:month "04";
  time:year "1964" .

_:node812 time:day "06";
  time:month "06";
  time:year "1901" .

_:node814 time:day "21";
  time:month "06";
  time:year "1970" .

_:node817 time:day "30";
  time:month "01";
  time:year "1917" .

_:node819 time:day "20";
  time:month "11";
  time:year "1946" .

_:node822 time:day "05";
  time:month "01";
  time:year "1905" .

_:node824 time:day "13";
  time:month "12";
  time:year "1988" .

_:node827 time:day "25";
  time:month "04";
  time:year "1889" .

_:node829 time:day "28";
  time:month "07";
  time:year "1953" .

_:node832 time:day "25";
  time:month "09";
  time:year "1886" .

_:node834 time:day "19";
  time:month "02";
  time:year "1953" .

_:node837 time:day "23";
  time:month "09";
  time:year "1896" .

_:node839 time:day "10";
  time:month "06";
  time:year "1987" .

_:node842 time:day "13";
  time:month "07";
  time:year "1916" .

_:node844 time:day "30";
  time:month "07";
  time:year "2002" .

_:node852 time:day "15";
  time:month "01";
  time:year "1899" .

_:node857 time:day "25";
  time:month "06";
  time:year "1900" .

_:node859 time:day "15";
  time:month "08";
  time:year "1979" .

_:node862 time:day "11";
  time:month "03";
  time:year "1943" .

_:node867 time:day "10";
  time:month "10";
  time:year "1907" .

_:node869 time:day "11";
  time:month "06";
  time:year "1962" .

_:node877 time:day "09";
  time:month "09";
  time:year "1949" .

_:node882 time:day "24";
  time:month "03";
  time:year "1921" .

_:node884 time:day "03";
  time:month "02";
  time:year "1965" .

_:node892 time:day "31";
  time:month "08";
  time:year "1919" .

_:node894 time:day "26";
  time:month "11";
  time:year "1987" .

_:node897 time:day "24";
  time:month "04";
  time:year "1907" .

_:node899 time:day "19";
  time:month "12";
  time:year "1948" .

_:node902 time:day "05";
  time:month "05";
  time:year "1883" .

_:node904 time:day "24";
  time:month "05";
  time:year "1950" .

_:node907 time:day "02";
  time:month "06";
  time:year "1897" .

_:node909 time:day "21";
  time:month "02";
  time:year "1949" .

_:node917 time:day "18";
  time:month "09";
  time:year "1889" .

_:node919 time:day "26";
  time:month "09";
  time:year "1959" .

_:node927 time:day "30";
  time:month "04";
  time:year "1909" .

_:node929 time:day "20";
  time:month "03";
  time:year "2004" .

_:node937 time:day "28";
  time:month "12";
  time:year "1927" .

_:node939 time:day "25";
  time:month "01";
  time:year "1946" .

_:node942 time:day "28";
  time:month "01";
  time:year "1920" .

_:node944 time:day "01";
  time:month "01";
  time:year "1990" .

_:node952 time:day "09";
  time:month "06";
  time:year "1920" .

_:node954 time:day "03";
  time:month "05";
  time:year "2012" .

_:node957 time:day "18";
  time:month "02" .

_:node959 time:day "05";
  time:month "09" .

_:node962 time:day "04";
  time:month "04" .

_:node967 time:day "12";
  time:month "01" .

_:node969 time:day "25";
  time:month "05" .

_:node977 time:day "25";
  time:month "06" .

_:node979 time:day "11";
  time:month "09" .

_:node987 time:day "10";
  time:month "11" .

_:node989 time:day "30";
  time:month "09" .

_:node997 time:day "14";
  time:month "04" .

_:node999 time:day "11";
  time:month "06" .

_:node1007 time:day "17";
  time:month "10" .

time:unitMonth time:days 0;
  time:hours 0;
  time:minutes 0;
  time:months 1;
  time:seconds 0;
  time:weeks 0 .

time:unitCentury time:days 0;
  time:hours 0;
  time:minutes 0;
  time:months 0;
  time:seconds 0;
  time:weeks 0 .

time:unitDay time:days 1;
  time:hours 0;
  time:minutes 0;
  time:months 0;
  time:seconds 0;
  time:weeks 0 .

time:unitDecade time:days 0;
  time:hours 0;
  time:minutes 0;
  time:months 0;
  time:seconds 0;
  time:weeks 0 .

time:unitHour time:days 0;
  time:hours 1;
  time:minutes 0;
  time:months 0;
  time:seconds 0;
  time:weeks 0 .

time:unitMillenium time:days 0;
  time:hours 0;
  time:minutes 0;
  time:months 0;
  time:seconds 0;
  time:weeks 0 .

time:unitMinute time:days 0;
  time:hours 0;
  time:minutes 1;
  time:months 0;
  time:seconds 0;
  time:weeks 0 .

time:unitSecond time:days 0;
  time:hours 0;
  time:minutes 0;
  time:months 0;
  time:seconds 1;
  time:weeks 0 .

time:unitWeek time:days 0;
  time:hours 0;
  time:minutes 0;
  time:months 0;
  time:seconds 0;
  time:weeks 1 .

time:unitYear time:days 0;
  time:hours 0;
  time:minutes 0;
  time:months 0;
  time:seconds 0;
  time:weeks 0 .

time:inXSDDateTime owl:deprecated true .

time:xsdDateTime owl:deprecated true .

time:January owl:deprecated true .

time:Year owl:deprecated true .

_:node177 time:month "2";
  time:year "1741" .

_:node184 time:month "2";
  time:year "1757" .

_:node299 time:month "4" .

_:node307 time:month "2";
  time:year "1810" .

_:node309 time:month "8";
  time:year "1810" .

_:node324 time:month "7";
  time:year "1293" .

_:node107 time:year "1602" .

_:node109 time:year "1663" .

_:node112 time:year "1803" .

_:node114 time:year "1815" .

_:node132 time:year "1945" .

_:node142 time:year "1873" .

_:node144 time:year "1904" .

_:node147 time:year "1873" .

_:node149 time:year "1904" .

_:node152 time:year "1025" .

_:node162 time:year "1741" .

_:node164 time:year "1750" .

_:node167 time:year "1803" .

_:node169 time:year "1837" .

_:node179 time:year "1743" .

_:node192 time:year "1719" .

_:node194 time:year "1723" .

_:node197 time:year "1858" .

_:node222 time:year "1404" .

_:node224 time:year "1406" .

_:node227 time:year "1357" .

_:node232 time:year "1944" .

_:node257 time:year "1641" .

_:node317 time:year "1821" .

_:node327 time:year "1946" .

_:node347 time:year "1704" .

_:node349 time:year "1708" .

_:node527 time:year "1975" .

_:node552 time:year "1955" .

_:node657 time:year "1959" .

_:node687 time:year "1999" .

_:node737 time:year "1898" .

_:node739 time:year "1965" .

_:node782 time:year "1927" .

_:node854 time:year "1967" .

_:node932 time:year "1901" .

_:node957 time:year "1916" .

_:node959 time:year "2014" .

_:node962 time:year "1947" .

_:node967 time:year "1902" .

_:node969 time:year "1949" .

_:node977 time:year "1936" .

_:node979 time:year "2019" .

_:node987 time:year "1913" .

_:node989 time:year "2000" .

_:node997 time:year "1925" .

_:node999 time:year "2004" .

_:node1007 time:year "1951" .

time:unitMonth time:years 0 .

time:unitCentury time:years 100 .

time:unitDay time:years 0 .

time:unitDecade time:years 10 .

time:unitHour time:years 0 .

time:unitMillenium time:years 1000 .

time:unitMinute time:years 0 .

time:unitSecond time:years 0 .

time:unitWeek time:years 0 .

time:unitYear time:years 1 .

geo:Feature owl:disjointWith geo:Geometry .

time:Instant owl:disjointWith time:ProperInterval .

_:node16 owl:onProperty rdfs:member;
  owl:allValuesFrom geo:Feature .

_:node17 owl:onProperty rdfs:member;
  owl:allValuesFrom geo:Geometry .

_:node18 owl:onProperty rdfs:member;
  owl:allValuesFrom geo:SpatialObject .

_:node19 owl:onProperty time:hasTRS;
  owl:hasValue <http://www.opengis.net/def/uom/ISO-8601/0/Gregorian> .

_:node20 owl:onProperty time:day;
  owl:allValuesFrom xsd:gDay .

_:node21 owl:onProperty time:month;
  owl:allValuesFrom xsd:gMonth .

_:node22 owl:onProperty time:year;
  owl:allValuesFrom xsd:gYear .

_:node23 owl:onProperty time:unitType;
  owl:cardinality "1"^^xsd:nonNegativeInteger .

_:node24 owl:onProperty time:numericDuration;
  owl:cardinality "1"^^xsd:nonNegativeInteger .

_:node25 owl:onProperty time:hasTRS;
  owl:hasValue <http://www.opengis.net/def/uom/ISO-8601/0/Gregorian> .

_:node26 owl:onProperty time:days;
  owl:allValuesFrom xsd:decimal .

_:node27 owl:onProperty time:hours;
  owl:allValuesFrom xsd:decimal .

_:node28 owl:onProperty time:minutes;
  owl:allValuesFrom xsd:decimal .

_:node29 owl:onProperty time:months;
  owl:allValuesFrom xsd:decimal .

_:node30 owl:onProperty time:seconds;
  owl:allValuesFrom xsd:decimal .

_:node31 owl:onProperty time:weeks;
  owl:allValuesFrom xsd:decimal .

_:node32 owl:onProperty time:years;
  owl:allValuesFrom xsd:decimal .

_:node33 owl:onProperty time:unitType;
  owl:cardinality "1"^^xsd:nonNegativeInteger .

_:node34 owl:onProperty time:dayOfWeek;
  owl:maxCardinality "1"^^xsd:nonNegativeInteger .

_:node35 owl:onProperty time:monthOfYear;
  owl:maxCardinality "1"^^xsd:nonNegativeInteger .

_:node36 owl:onProperty time:timeZone;
  owl:maxCardinality "1"^^xsd:nonNegativeInteger .

_:node37 owl:onProperty time:day;
  owl:maxCardinality "1"^^xsd:nonNegativeInteger .

_:node38 owl:onProperty time:dayOfYear;
  owl:maxCardinality "1"^^xsd:nonNegativeInteger .

_:node39 owl:onProperty time:hour;
  owl:maxCardinality "1"^^xsd:nonNegativeInteger .

_:node40 owl:onProperty time:minute;
  owl:maxCardinality "1"^^xsd:nonNegativeInteger .

_:node41 owl:onProperty time:month;
  owl:maxCardinality "1"^^xsd:nonNegativeInteger .

_:node42 owl:onProperty time:second;
  owl:maxCardinality "1"^^xsd:nonNegativeInteger .

_:node43 owl:onProperty time:week;
  owl:maxCardinality "1"^^xsd:nonNegativeInteger .

_:node44 owl:onProperty time:year;
  owl:maxCardinality "1"^^xsd:nonNegativeInteger .

_:node45 owl:onProperty time:hasTRS;
  owl:cardinality "1"^^xsd:nonNegativeInteger .

_:node46 owl:onProperty time:days;
  owl:maxCardinality "1"^^xsd:nonNegativeInteger .

_:node47 owl:onProperty time:hours;
  owl:maxCardinality "1"^^xsd:nonNegativeInteger .

_:node48 owl:onProperty time:minutes;
  owl:maxCardinality "1"^^xsd:nonNegativeInteger .

_:node49 owl:onProperty time:months;
  owl:maxCardinality "1"^^xsd:nonNegativeInteger .

_:node50 owl:onProperty time:seconds;
  owl:maxCardinality "1"^^xsd:nonNegativeInteger .

_:node51 owl:onProperty time:weeks;
  owl:maxCardinality "1"^^xsd:nonNegativeInteger .

_:node52 owl:onProperty time:years;
  owl:maxCardinality "1"^^xsd:nonNegativeInteger .

_:node53 owl:onProperty time:unitType;
  owl:hasValue time:unitMonth .

_:node54 owl:onProperty time:month;
  owl:hasValue "--01" .

_:node55 owl:onProperty time:unitType;
  owl:hasValue time:unitMonth .

_:node56 owl:onProperty time:day;
  owl:cardinality "0"^^xsd:nonNegativeInteger .

_:node57 owl:onProperty time:hour;
  owl:cardinality "0"^^xsd:nonNegativeInteger .

_:node58 owl:onProperty time:minute;
  owl:cardinality "0"^^xsd:nonNegativeInteger .

_:node59 owl:onProperty time:month;
  owl:cardinality "1"^^xsd:nonNegativeInteger .

_:node60 owl:onProperty time:second;
  owl:cardinality "0"^^xsd:nonNegativeInteger .

_:node61 owl:onProperty time:week;
  owl:cardinality "0"^^xsd:nonNegativeInteger .

_:node62 owl:onProperty time:year;
  owl:cardinality "0"^^xsd:nonNegativeInteger .

_:node66 owl:onProperty time:hasTRS;
  owl:cardinality "1"^^xsd:nonNegativeInteger .

_:node69 owl:onProperty time:nominalPosition;
  owl:cardinality "1"^^xsd:nonNegativeInteger .

_:node71 owl:onProperty time:numericPosition;
  owl:cardinality "1"^^xsd:nonNegativeInteger .

_:node72 owl:onProperty time:days;
  owl:cardinality "0"^^xsd:nonNegativeInteger .

_:node73 owl:onProperty time:hours;
  owl:cardinality "0"^^xsd:nonNegativeInteger .

_:node74 owl:onProperty time:minutes;
  owl:cardinality "0"^^xsd:nonNegativeInteger .

_:node75 owl:onProperty time:months;
  owl:cardinality "0"^^xsd:nonNegativeInteger .

_:node76 owl:onProperty time:seconds;
  owl:cardinality "0"^^xsd:nonNegativeInteger .

_:node77 owl:onProperty time:weeks;
  owl:cardinality "0"^^xsd:nonNegativeInteger .

_:node78 owl:onProperty time:years;
  owl:cardinality "1"^^xsd:nonNegativeInteger .

_:node97 xsd:pattern "--(0[1-9]|1[0-9]|20)(Z|(\\+|-)((0[0-9]|1[0-3]):[0-5][0-9]|14:00))?" .

_:node98 xsd:pattern "---(0[1-9]|[1-9][0-9])(Z|(\\+|-)((0[0-9]|1[0-3]):[0-5][0-9]|14:00))?" .

_:node99 xsd:pattern "-?([1-9][0-9]{3,}|0[0-9]{3})(Z|(\\+|-)((0[0-9]|1[0-3]):[0-5][0-9]|14:00))?" .

:wikipediaBandungLautanApi <https://semanticweb.cs.vu.nl/2009/11/sem/accordingTo>
    :wikipedia;
  dc:description "Peristiwa Bandung Lautan Api adalah peristiwa kebakaran besar yang terjadi di Bandung, provinsi Jawa Barat, Indonesia pada 24 Maret 1946. Sekitar 200.000 penduduk Bandung membakar kediaman mereka sendiri dalam peristiwa tersebut , kemudian meninggalkan kota menuju pegunungan di daerah selatan Bandung. Hal ini dilakukan untuk mencegah tentara Sekutu yang dapat menggunakan kota Bandung sebagai markas strategis militer dalam Perang Kemerdekaan Indonesia." .

:wikipediaPerangBelandaPortugal <https://semanticweb.cs.vu.nl/2009/11/sem/accordingTo>
    :wikipedia .

:wikipediaPeperanganeraNapoleon <https://semanticweb.cs.vu.nl/2009/11/sem/accordingTo>
    :wikipedia .

:wikipediaPemberontakanDITIIdiAceh <https://semanticweb.cs.vu.nl/2009/11/sem/accordingTo>
    :wikipedia;
  dc:description "Pemberontakan DI/TII di Aceh dimulai pada tanggal 20 September 1953. Dimulai dengan pernyataan Proklamasi berdirinya Negara Islam Indonesia oleh Daud Beureueh, proklamasi itu menyatakan diri bahwa Aceh sebagai bagian dari Negara Islam Indonesia (NII) dibawah kepemimpinan Imam Besar NII" .

:wikipediaKampanyeKalimantan1945 <https://semanticweb.cs.vu.nl/2009/11/sem/accordingTo>
    :wikipedia;
  dc:description "Kampanye Kalimantan tahun 1945 atau Kampanye Borneo tahun 1945 adalah kampanye utama terakhir Sekutu di wilayah Pasifik barat laut selama Perang Dunia II. Dalam berbagai serangan amfibi antara 1 Mei hingga 21 Juli 1945, tentara Australia di bawah Jendral Leslie Morshead, menyerang tentara Jepang yang menduduki pulau ini." .

:wikipediaPerangPasifik <https://semanticweb.cs.vu.nl/2009/11/sem/accordingTo> :wikipedia .

:wikipediaPertempuranBojongKokosan <https://semanticweb.cs.vu.nl/2009/11/sem/accordingTo>
    :wikipedia;
  dc:description "Pertempuran Bojong Kokosan adalah pertempuran yang terjadi ketika konvoi tentara Inggris (Sekutu) yang hendak memperkuat pasukannya di Bandung disergap para pejuang Indonesia di Bojong Kokosan, Sukabumi." .

:wikipediaRevolusiNasionalIndonesia <https://semanticweb.cs.vu.nl/2009/11/sem/accordingTo>
    :wikipedia;
  dc:description "Revolusi Nasional Indonesia adalah sebuah konflik bersenjata dan pertentangan diplomasi antara Republik Indonesia yang baru lahir melawan Kerajaan Belanda yang dibantu oleh pihak Sekutu, diwakili oleh Inggris. Rangkaian peristiwa ini terjadi mulai dari mendaratnya pasukan sekutu Inggris pertama kali di Jakarta pada 29 September 1945 yang dipimpin oleh Letnan Jenderal Christinson setelah ditandatanganinya Civil Affairs Agreement. Konflik ini berlangsung selama 4 tahun hingga pengakuan kemerdekaan Indonesia oleh Kerajaan Belanda pada 27 Desember 1949. Meskipun demikian, gerakan revolusi itu sendiri telah dimulai pada tahun 1908, yang saat ini diperingati sebagai tahun dimulainya kebangkitan nasional Indonesia." .

:wikipediaPerangAceh <https://semanticweb.cs.vu.nl/2009/11/sem/accordingTo> :wikipedia .

:wikipediaInvasiCholakeSriwijaya <https://semanticweb.cs.vu.nl/2009/11/sem/accordingTo>
    :wikipedia .

:wikipediaPerangBelasting <https://semanticweb.cs.vu.nl/2009/11/sem/accordingTo> :wikipedia .

:wikipediaPerangKuning <https://semanticweb.cs.vu.nl/2009/11/sem/accordingTo> :wikipedia .

:wikipediaPerangPadri <https://semanticweb.cs.vu.nl/2009/11/sem/accordingTo> :wikipedia .

:wikipediaPerangCumbok <https://semanticweb.cs.vu.nl/2009/11/sem/accordingTo> :wikipedia;
  dc:description "Perang Cumbok (dikenal juga sebagai Peristiwa Cumbok atau Revolusi Sosial) adalah serangkaian pertempuran yang terjadi di Kabupaten Pidie, Aceh mulai 2 Desember 1945 hingga 16 Januari 1946. Perang ini pecah antara kalangan ulama (teungku) para pendukung proklamasi kemerdekaan Indonesia yang tergabung dalam Persatuan Ulama Seluruh Aceh melawan kubu uleebalang (teuku) yang lebih memilih kekuasaan Belanda, sehingga menyebabkan revolusi di tatanan sosial masyarakat Aceh pada saat itu." .

:wikipediaPerangJawa17411743 <https://semanticweb.cs.vu.nl/2009/11/sem/accordingTo>
    :wikipedia .

:wikipediaPerangTakhtaJawaKetiga <https://semanticweb.cs.vu.nl/2009/11/sem/accordingTo>
    :wikipedia .

:wikipediaSeranganUmum1Maret1949 <https://semanticweb.cs.vu.nl/2009/11/sem/accordingTo>
    :wikipedia;
  dc:description "Serangan Umum 1 Maret 1949 adalah serangan yang terjadi pada tanggal 1 Maret 1949 di Yogyakarta. Serangan ini telah dipersiapkan oleh jajaran tertinggi militer di wilayah Divisi III/GM III dengan mengikutsertakan  pimpinan pemerintah sipil setempat berdasarkan instruksi dari Panglima Divisi III, Kol. Bambang Sugeng. Serangan ini bertujuan untuk membuktikan kepada dunia internasional bahwa Tentara Nasional Indonesia (TNI) dan Kepolisian Negara Republik indonesia masih ada dan cukup kuat, dengan harapan dapat memperkuat posisi Indonesia dalam perundingan yang sedang berlangsung di Dewan Keamanan PBB. Perundingan tersebut memiliki tujuan utama untuk mematahkan moral pasukan Belanda serta membuktikan pada dunia internasional bahwa Tentara Nasional Indonesia (TNI) masih mempunyai kekuatan untuk mengadakan perlawanan. Soeharto pada waktu itu menjabat sebagai Komandan Brigade X/Wehrkreis III turut serta sebagai pelaksana lapangan di wilayah Yogyakarta." .

:wikipediaPerangTakhtaJawaKedua <https://semanticweb.cs.vu.nl/2009/11/sem/accordingTo>
    :wikipedia .

:wikipediaIntervensiBelandadiBali1858 <https://semanticweb.cs.vu.nl/2009/11/sem/accordingTo>
    :wikipedia .

:wikipediaKonflikPapua <https://semanticweb.cs.vu.nl/2009/11/sem/accordingTo> :wikipedia;
  dc:description "Konflik Papua adalah konflik militer yang tejadi di wilayah Papua, Indonesia. diawali pada tahun 1961, muncul keinginan Belanda untuk membentuk negara Papua Barat yang terlepas dari Indonesia, Langkah Belanda ini kemudian ditentang oleh Presiden Indonesia, Soekarno dengan mendekatkan diri pada negara komunis terutama Uni Soviet. Sikap Soekarno ini membuat takut Belanda dan Presiden Amerika Serikat, John F. Kennedy. Sebab jika hal itu dibiarkan maka Indonesia kemungkinan menjadi negara komunis terbesar di Asia Tenggara. Ketakutan itu lalu membuat Belanda mengambil sikap untuk menyerahkan masalah Papua ke PBB. Dari dan melalui PBB, Belanda mengambil sikap untuk keluar dari Papua dan tidak jadi mengambil, merebut, dan menjajah Papua lalu Papua diserahkan \"kembali\" ke Indonesia dengan syarat memberi kesempatan pada rakyat Papua untuk menentukan sikap sendiri atau referendum (Penentuan Pendapat Rakyat/PEPERA)." .

:wikipediaPeristiwaTigaMaret <https://semanticweb.cs.vu.nl/2009/11/sem/accordingTo>
    :wikipedia;
  dc:description "Peristiwa Tiga Maret adalah sebuah upaya pemberontakan terhadap pemerintahan Republik Indonesia di Sumatera Barat pada masa Revolusi Nasional Indonesia oleh para militan Islam. Pemberontakan ini gagal dan para pemimpinnya ditangkap." .

:wikipediaPenyerbuanKotabaruYogyakarta <https://semanticweb.cs.vu.nl/2009/11/sem/accordingTo>
    :wikipedia;
  dc:description "Penyerbuan markas Jepang di Kotabaru Yogyakarta (atau lebih dikenal sebagai Penyerbuan Kotabaru Yogyakarta) diawali dengan perundingan antara Jepang dengan pejuang Yogyakarta yang berlangsung pada tanggal 6 Oktober 1945. Perundingan ini tidak mencapai mufakat karena Jepang tidak mau menyerahkan senjatanya pada pejuang Yogyakarta sehingga pada tanggal 7 Oktober 1945 dilakukan penyerbuan ke markas Jepang oleh para pejuang Yogyakarta." .

:wikipediaPerangBayu <https://semanticweb.cs.vu.nl/2009/11/sem/accordingTo> :wikipedia .

:wikipediaPerangRegreg <https://semanticweb.cs.vu.nl/2009/11/sem/accordingTo> :wikipedia .

:wikipediaPerangBubat <https://semanticweb.cs.vu.nl/2009/11/sem/accordingTo> :wikipedia .

:wikipediaPerangDayakDesa <https://semanticweb.cs.vu.nl/2009/11/sem/accordingTo> :wikipedia;
  dc:description "Perang Dayak Desa adalah perang antara Suku Dayak Desa dan pasukan Kekaisaran Jepang pada masa pendudukan Jepang di Kalimantan Barat. Perang yang berlangsung tahun 1944 hingga 1945 di Sanggau, Kalimantan Barat ini dilatarbelakangi oleh perlakuan Jepang yang sewenang-wenang terhadap Suku Dayak Desa." .

:wikipediaGerakan30September <https://semanticweb.cs.vu.nl/2009/11/sem/accordingTo>
    :wikipedia;
  dc:description "Gerakan 30 September (G30S) adalah sebuah peristiwa berlatar belakang kudeta yang terjadi selama satu malam pada tanggal 30 September hingga 1 Oktober 1965 yang mengakibatkan gugurnya enam jenderal serta satu orang perwira pertama militer Indonesia dan jenazahnya dimasukkan ke dalam suatu lubang sumur lama di area Lubang Buaya, Jakarta Timur. Penyebutan peristiwa ini memiliki ragam jenis, Presiden Soekarno menyebut peristiwa ini dengan istilah GESTOK (Gerakan Satu Oktober), sementara Presiden Soeharto menyebutnya dengan istilah GESTAPU (Gerakan September Tiga Puluh), dan pada Orde Baru, Presiden Soeharto mengubah sebutannya menjadi G30S/PKI (Gerakan 30 September PKI) oleh karena tudingan bahwa Partai Komunis Indonesia (PKI) bertanggung jawab atas peristiwa ini. Korban kekejaman tragedi ini berada di Yogyakarta dan Jakarta. Salah satu korban kekejaman tragedi ini di Yogyakarta adalah Katamso Darmokusumo dan Sugiyono Mangunwiyoto." .

:wikipediaKampanyeHindiaBelanda <https://semanticweb.cs.vu.nl/2009/11/sem/accordingTo>
    :wikipedia;
  dc:description "Kampanye Hindia Belanda adalah upaya Sekutu untuk mempertahankan Hindia Belanda dari Jepang selama Perang Dunia II, terutama pada periode tahun 1941 sampai dengan tahun 1942. Sumber minyak bumi Hindia Belanda yang kaya menjadi tujuan utama Jepang selama perang. Kampanye ini menyebabkan pendudukan Jepang selama tiga setengah tahun dan berakhirnya penjajahan Belanda di wilayah Nusantara." .

:wikipediaPertempuranLengkong <https://semanticweb.cs.vu.nl/2009/11/sem/accordingTo>
    :wikipedia;
  dc:description "Pertempuran Lengkong adalah pertempuran Tentara Keamanan Rakyat melawan pasukan Jepang di Desa Lengkong, Serpong, Tangerang Selatan, Banten, Indonesia yang terjadi pada tanggal 25 Januari 1946." .

:wikipediaPertempuranMelaka1641 <https://semanticweb.cs.vu.nl/2009/11/sem/accordingTo>
    :wikipedia .

:wikipediaPertempuranMedanArea <https://semanticweb.cs.vu.nl/2009/11/sem/accordingTo>
    :wikipedia;
  dc:description "Pertempuran Medan Area adalah sebuah peristiwa perlawanan rakyat terhadap Pasukan Sekutu yang terjadi di kawasan Medan, Sumatera Utara." .

:wikipediaPertempuranKumai <https://semanticweb.cs.vu.nl/2009/11/sem/accordingTo>
    :wikipedia;
  dc:description "Pertempuran Kumai atau juga dikenal sebagai Pertempuran 14 Januari adalah sebuah pertikaian antara Pemerintahan Republik Indonesia dan para milisi Indonesia melawan Tentara Kerajaan Hindia Belanda di kota Kumai, Kalimantan Tengah. Milisi Indonesia, kebanyakan terdiri dari pemuda, Tentara Indonesia yang baru dibentuk, dan ulama Islam bersenjata dikenal sebagai Barisan Ulama atau Barisan Berjenggot bertindak melawan konvoi bersenjata Belanda yang berniat untuk mendarat di pelabuhan." .

:wikipediaSeranganUmumSurakarta <https://semanticweb.cs.vu.nl/2009/11/sem/accordingTo>
    :wikipedia;
  dc:description "Serangan Umum Surakarta atau juga disebut Serangan Umum Empat Hari berlangsung pada tanggal 7 -10 Agustus 1949 secara gerilya oleh para pejuang, pelajar, dan mahasiswa. Pelajar dan mahasiswa yang berjuang tersebut kemudian dikenal sebagai tentara pelajar. Mereka berhasil membumihanguskan dan menduduki markas-maskas Belanda di Surakarta dan sekitarnya. Menurut catatan sejarah, serangan itu digagas di kawasan Monumen Banjarsari, Surakarta. Untuk menyusun serangan, para pejuang berkumpul di Desa Wonosido, Kabupaten Sragen dari situlah ide untuk melakukan serangan umum dikobarkan." .

:wikipediaPenyerbuanMeesterCornelis <https://semanticweb.cs.vu.nl/2009/11/sem/accordingTo>
    :wikipedia .

:wikipediaPuputanMargarana <https://semanticweb.cs.vu.nl/2009/11/sem/accordingTo>
    :wikipedia;
  dc:description "Pertempuran Puputan Margarana merupakan salah satu pertempuran antara Indonesia dan Belanda dalam masa Perang kemerdekaan Indonesia yang terjadi pada 20 November 1946. Pertempuran ini dipimpin oleh Kepala Divisi Sunda Kecil Kolonel I Gusti Ngurah Rai. Dimana Pasukan TKR di wilayah ini bertempur dengan habis habisan untuk mengusir Pasukan Belanda yang kembali datang setelah kekalahan Jepang, untuk menguasai kembali wilayahnya yang direbut Jepang pada Perang Dunia II, mengakibatkan gugurnya seluruh pasukan termasuk I Gusti Ngurah Rai yang kemudian dikenang sebagai salah-satu Puputan pada era awal kemerdekaan serta mengakibatkan Belanda sukses mendirikan Negara Indonesia Timur." .

:wikipediaPertempuranLimaHari <https://semanticweb.cs.vu.nl/2009/11/sem/accordingTo>
    :wikipedia;
  dc:description "Pertempuran Lima Hari adalah adalah bentrokan antara pasukan Jepang dari Tentara Keenambelas dan pasukan Indonesia yang terdiri dari personil Badan Keamanan Rakyat dan pemuda pada bulan Oktober 1945 di kota Semarang, Jawa Tengah. Pertempuran ini dianggap sebagai bentrokan besar pertama yang melibatkan militer Indonesia." .

:wikipediaIntervensiBelandadiBali1908 <https://semanticweb.cs.vu.nl/2009/11/sem/accordingTo>
    :wikipedia .

:wikipediaPertempuranSurabaya <https://semanticweb.cs.vu.nl/2009/11/sem/accordingTo>
    :wikipedia;
  dc:description "Pertempuran Surabaya merupakan pertempuran antara pasukan pejuang Indonesia yang diorganisir oleh pasukan anggota eks. Pembela Tanah Air yang dibentuk oleh Pasukan Jepang dan Polisi Istimewa di waktu masa Pendudukan Jepang di Indonesia (yang dulunya Hindia Belanda) pada saat itu, yang bertujuan untuk mencegah pasukan sekutu pasca Jepang menyerah tanpa syarat kepada sekutu  di Perang Pasifik yang mendarat di kota Surabaya yang terdiri dari pasukan Kekaisaran Britania dengan sukarelawan Persemakmuran Britania yakni Angkatan Darat India Britania dengan mendapatkan dukungan khusus oleh tentara Kekaisaran Belanda. Puncaknya terjadi pada tanggal 10 November 1945. Pertempuran ini adalah perang pertama pasukan Indonesia dengan pasukan Sekutu  setelah Proklamasi Kemerdekaan Indonesia dan satu pertempuran terbesar dan terberat dalam sejarah Revolusi Nasional Indonesia yang menjadi simbol nasional atas perlawanan Indonesia terhadap kolonialisme dan Imperialisme. Usai pertempuran ini, dukungan rakyat Indonesia dan dunia internasional terhadap perjuangan kemerdekaan Indonesia semakin kuat. 10 November diperingati setiap tahun sebagai Hari Pahlawan di Indonesia." .

:wikipediaInvasiMaluku <https://semanticweb.cs.vu.nl/2009/11/sem/accordingTo> :wikipedia .

:wikipediaPerangDiponegoro <https://semanticweb.cs.vu.nl/2009/11/sem/accordingTo>
    :wikipedia .

:wikipediaEkspedisiPalembangII <https://semanticweb.cs.vu.nl/2009/11/sem/accordingTo>
    :wikipedia .

:wikipediaSerbuanYuanMongolkeJawa <https://semanticweb.cs.vu.nl/2009/11/sem/accordingTo>
    :wikipedia .

:wikipediaDelapanJamPertempurandiMangkang <https://semanticweb.cs.vu.nl/2009/11/sem/accordingTo>
    :wikipedia;
  dc:description "Delapan Jam Pertempuran di Mangkang adalah sebuah peristiwa perlawanan pasukan Corps Mariners C.A. IV bertugas di daerah Pekalongan, Batang dan Pemalang yang dikenal sebagai Sub Wehrkreise Slamet V (SWKS V) terhadap Sekutu yang terjadi di Mangkang, Semarang, Jawa Tengah. dibawah pimpinan Letnan. Moekijat." .

:wikipediaPemberontakanRadenRonggo <https://semanticweb.cs.vu.nl/2009/11/sem/accordingTo>
    :wikipedia .

:wikipediaPeristiwa19November <https://semanticweb.cs.vu.nl/2009/11/sem/accordingTo>
    :wikipedia;
  dc:description "Peristiwa 19 November merupakan suatu peristiwa di awal Revolusi Nasional Indonesia dimana iring-iringan kendaraan Belanda disergap pemuda Indonesia di Kabupaten Kolaka, Sulawesi Tenggara, tanggal 19 November 1945." .

:wikipediaGegerSepehi <https://semanticweb.cs.vu.nl/2009/11/sem/accordingTo> :wikipedia .

:wikipediaPerangTakhtaJawaPertama <https://semanticweb.cs.vu.nl/2009/11/sem/accordingTo>
    :wikipedia .

:wikipediaOperasi17Agustus <https://semanticweb.cs.vu.nl/2009/11/sem/accordingTo>
    :wikipedia;
  dc:description "Operasi 17 Agustus merupakan operasi militer yang dipimpin oleh Kolonel Ahmad Yani yang bertujuan untuk menumpas gerakan Pemerintahan Revolusioner Republik Indonesia (PRRI) yang berada di Sumatera Barat, tepatnya di Padang. Operasi militer ini merupakan operasi gabungan yang melibatkan TNI Angkatan Laut, Angkatan Darat, dan Angkatan Udara. 17 Agustus merujuk pada sandi yang digunakan oleh Kolonel Ahmad Yani." .

:JisaburoOzawa dc:description "Jisaburo Ozawa (2 Oktober 1886  9 November 1966) adalah laksamana Angkatan Laut Jepang.[2] Pada awal Perang Dunia II ia menjadi komandan satuan yang membantu pendudukan Semenanjung Malaya (Singapura) dan Sumatra (Palembang).[2] Selanjutnya ia juga menaklukan Jawa Barat.[2] Setelah menduduki pulau-pulau di selatan ini, ia mengalami kekalahan di pertempuran Laut Filipina (1944).[2] Ia juga mengambil bagian dalam pertempuran Teluk Leyte (1944).[2]" .

:MuhammadMangundiprojo dc:description "Mayor Jenderal TNI (Purn.) Raden Muhammad Mangoendiprodjo (EYD: Muhammad Mangundiprojo; 5 Januari 1905  13 Desember 1988) adalah seorang pejuang kemerdekaan dan perwira militer Indonesia yang ikut serta dalam Pertempuran Surabaya pada tanggal 10 November 1945. Ia diangkat sebagai Pahlawan Nasional Indonesia oleh Presiden Joko Widodo pada tanggal 7 November 2014." .

:Soengkono dc:description "Mayor Jenderal TNI (Purn.) Soengkono (1 Januari 1911  12 September 1977) adalah seorang tokoh militer Indonesia dan merupakan tokoh dalam Pertempuran Surabaya  10 November 1945 di Surabaya, Jawa Timur. Saat itu ia menjabat komandan BKR (Badan Keamanan Rakyat). Saat ini namanya diabadikan menjadi nama jalan utama di Kota Surabaya yaitu Jalan Mayjen Sungkono." .

:HarioJonosewojo dc:description "Mayor Jenderal TNI (Purn.) Kanjeng Raden Mas Hario Jonosewojo Handajaningrat atau K.R.M. Hario Jonosewojo Handajaningrat (9 Juni 1921  22 Maret 1994) adalah seorang tokoh militer Indonesia. Dan mantan Panglima Divisi VI/Narotama TRI. Ia juga seorang tokoh yang berperan dalam membantu dalam perjuangan kemerdekaan Indonesia dan perkembangan lembaga olahraga di Indonesia. Ia akrab dipanggil mas Piet. Ia merupakan lulusan pendidikan di Command General Staff College Regular Course di Fort Leavenworth Kansas, AS pada tahun 1960-1961, dimana sepulang dari pendidikan tersebut beliau dan keluarga menempati kediaman di jalan Lembang Terusan, Jakarta hingga akhir hayatnya. Sejak remaja ia sering bermain tennis. Ia sering mengikuti berbagai kejuaraan namun belum pernah juara. Ia masuk PELTI (Persatuan Lawn Tennis Indonesia) sejak serikat tennis ini didirikan pada tahun 1948. 15 tahun semenjak ia bergabung dengan PELTI, ia dipercaya menjadi ketua umum PELTI pada tahun 1963. Ia juga pernah menjadi Ajudan Senior Pejabat Presiden Djuanda dan kepala sekuriti BKR (Badan Keamanan Rakyat) Surabaya.[1]" .

:MoehammadJasin dc:description "Komisaris Jenderal Polisi (Purn.) Dr. H. Moehammad Jasin (9 Juni 1920  3 Mei 2012) yang dikenal sebagai \"Bapak Brimob Polri\". Moehammad Jasin menghembuskan nafas terakhir pada hari Kamis tanggal 3 Mei 2012 pukul 15.30 WIB, dalam usia 91 tahun di RS Polri Kramat Jati[1] dan dimakamkan di Taman Makam Pahlawan Kalibata.",
    "Komisaris Jenderal Polisi (Purn.) Dr. H. Moehammad Jasin (9 Juni 1920  3 Mei 2012) yang dikenal sebagai \"Bapak Brimob Polri\". Moehammad Jasin menghembuskan nafas terakhir pada hari Kamis tanggal 3 Mei 2012 pukul 15.30 WIB, dalam usia 91 tahun di RS Polri Kramat Jati dan dimakamkan di Taman Makam Pahlawan Kalibata." .

:Moestopo dc:description "Mayor Jenderal TNI (Purn.) Prof. DR. Moestopo (13 Juni 1913  29 September 1986) adalah seorang dokter gigi Indonesia, pejuang kemerdekaan, dan pendidik. Dia dinyatakan sebagai Pahlawan Nasional pada tanggal 9 November 2007." .

:RobertMansergh dc:description "Jend. Sir Eric Carden Robert Mansergh GCB KBE MC (12 Mei 1900  8 November 1970) adalah jenderal British Army selama dan setelah Perang Dunia II." .

:AubertinMallaby dc:description "Aubertin Walter Sothern Mallaby atau juga dikenal dengan Brigadir Mallaby (12 Desember 1899  30 Oktober 1945) adalah brigadir Britania yang tewas dalam peristiwa baku tembak 30 Oktober di Surabaya dan memicu keluarnya ultimatum Inggris dan meledaknya Pertempuran 10 November." .

:Sutomo dc:description "Sutomo (3 Oktober 1920  7 Oktober 1981) atau lebih dikenal dengan sapaan akrab Bung Tomo adalah pahlawan nasional Indonesia dan pemimpin militer Indonesia pada masa Revolusi Nasional Indonesia yang dikenal karena peranannya dalam Pertempuran 10 November 1945." .

:GoliathTabuni dc:description "Goliath Tabuni adalah panglima tinggi Tentara Pembebasan Nasional Papua Barat. Goliath Tabuni bermarkas di Tingginambut Puncak jaya Papua Pegunungan. Pada tahun 2004 mulai beraksi melawan pemerintah Indonesia di wilayah tersebut. Pada awalnya Gen. Goliath Tabuni berjuang bersama Kelly Kwalik di Timika yang bermarkas di Kali Kabur. Penyaderaan di Mapenduma terjadi Goliath sebagai anggota dari Kelik Kwalik, selanjutnya dia pindah ke Puncakjaya memimpin pasukan dan mulai beraksi pada 2004 sampai saat ini. Goliath Tabuni memimpin perang di puncak jaya dengan sistem strategi gerilya." .

:Soekarno dc:description "Dr. (H.C.) Ir. H. Soekarno[cat.] (Ejaan Republik: Sukarno, Jawa: , pengucapan bahasa Jawa: [sukarn]; 6 Juni 1901  21 Juni 1970) adalah seorang politikus yang berperan penting dalam Revolusi Nasional Indonesia. Ia bersama Mohammad Hatta memproklamasikan Kemerdekaan Indonesia pada tanggal 17 Agustus 1945. Ia orang pertama yang mencetuskan konsep mengenai Pancasila sebagai dasar negara Indonesia dan ia sendiri yang menamainya.Selain sebagai proklamator, Soekarno juga menjabat sebagai Presiden Republik Indonesia pertama sejak 1945 hingga 1967, dengan masa pemerintahannya dikenal juga sebagai Orde Lama.:11, 81:26-32 Pada pertengahan tahun 1960-an, di masa-masa akhir jabatan Soekarno, Indonesia mengalami stagnasi produksi, kemiskinan dan kelaparan yang merajalela, infrastruktur yang tidak terurus, dan hiperinflasi mencapai hampir 600 persen.Pada 11 Maret 1966, Soekarno menandatangani Surat Perintah yang dikenal sebagai Supersemar yang menugaskan Letnan Jenderal Soeharto untuk mengamankan dan menjaga keamanan negara dan institusi kepresidenan. Supersemar menjadi landasan Letnan Jenderal Soeharto untuk membubarkan Partai Komunis Indonesia (PKI) dan mengganti anggota-anggotanya yang duduk di parlemen. Setelah pertanggungjawabannya ditolak Majelis Permusyawaratan Rakyat Sementara (MPRS) pada sidang umum ke empat tahun 1967, Soekarno diberhentikan dari jabatannya sebagai presiden pada Sidang Istimewa MPRS pada tahun yang sama dan Soeharto menggantikannya sebagai pejabat Presiden Republik Indonesia." .

:KiyotakeKawaguchi dc:description "Kiyotake Kawaguchi (  , Kawaguchi Kiyotake, 3 Desember 1892  16 Mei 1961) adalah seorang Jenderal Angkatan Darat Kekaisaran Jepang pada masa Perang Dunia II. Setelah perang berakhir, ia ditangkap oleh otoritas SCAP (Supreme Commander for the Allied Powers) atau Komandan Tertinggi Sekutu dan dituntut sebagai penjahat perang." .

:RaymondWesterling dc:description "Raymond Pierre Paul Westerling (31 Agustus 1919  26 November 1987) adalah komandan pasukan Belanda yang terkenal karena memimpin Pembantaian Westerling (19461947) di Sulawesi Selatan dan percobaan kudeta APRA di Bandung, Jawa Barat. Dia adalah salah satu sosok paling kejam dalam sejarah Indonesia karena pembantaian yang dipimpinnya." .

:JuliusTahija dc:description "Julius Tahija (13 Juli 1916  30 Juli 2002) dulu adalah seorang tentara, politisi, dan pebisnis asal Indonesia. Ia mendapat Orde Militer Willem atas aksinya pada kampanye Hindia Belanda saat bertugas di KNIL dan merupakan satu-satunya orang Indonesia pada masa perang yang menerima penghormatan militer tertinggi dari sebuah negara sekutu selama Perang Dunia II. Ia juga pernah menduduki sejumlah posisi menteri di Negara Indonesia Timur selama Revolusi Nasional Indonesia pada tahun 1947, lalu bekerja dan mendirikan konglomerat Indrapura Group, yang kemudian menjadi salah satu yang terbesar di Indonesia." .

:Moekijat dc:description "Letnan Jenderal KKO (Purn.) Moekijat (EYD: Mukiyat; 15 Desember 1927  1 November 1985) adalah Panglima KKO-AL (sekarang Korps Marinir) dari 16 Oktober 1968 hingga 6 Desember 1971. Ia juga pernah menjadi Kepala KBRI di Kedutaan Besar Republik Indonesia di Pyongyang, Korea Utara (19711975) dan Kedutaan Besar Republik Indonesia di Helsinki, Finlandia (19751980)." .

:MohammadHatta dc:description "Dr. (H.C.) Drs. H. Mohammad Hatta atau dipanggil  Bung Hatta (12 Agustus 1902  14 Maret 1980) adalah seorang tokoh penting dalam perjuangan kemerdekaan Indonesia, negarawan, dan ekonom Indonesia yang menjabat sebagai Wakil Presiden Indonesia pertama. Ia bersama Soekarno adalah Proklamator Kemerdekaan, memainkan peranan sentral dalam perjuangan kemerdekaan Indonesia dari penjajahan Belanda sekaligus memproklamirkannya pada 17 Agustus 1945. Ia pernah menjabat sebagai Perdana Menteri dalam Kabinet Hatta I, Hatta II, dan RIS. Pada 1956, ia mundur dari jabatan wakil presiden." .

:DouglasMacArthur dc:description "Douglas MacArthur (26 Januari 1880  5 April 1964) adalah seorang jenderal bintang lima asal Amerika Serikat dan marsekal lapangan Angkatan Darat Filipina. Ia menjabat sebagai Kepala Staf Angkatan Darat Amerika Serikat pada dasawarsa 1930-an dan memiliki sumbangsih yang besar dalam upaya untuk melawan Kekaisaran Jepang di teater Pasifik selama Perang Dunia II. Ia dianugerahi Medal of Honor berkat jasa-jasanya selama kampanye militer Filipina sehingga dirinya dan ayahnya, Arthur MacArthur, Jr., menjadi pasangan ayah dan anak pertama yang sama-sama mendapatkan medali tersebut. Ia juga merupakan salah satu dari hanya lima orang yang diberikan pangkat Jenderal Besar di Angkatan Darat Amerika Serikat dan satu-satunya orang yang pernah diangkat sebagai marsekal lapangan di Angkatan Darat Filipina." .

:ListyoSigitPrabowo dc:description "Jenderal Polisi Drs. Listyo Sigit Prabowo, M.Si. (lahir 5 Mei 1969) adalah seorang perwira tinggi Polri yang menjabat sebagai Kepala Kepolisian Negara Republik Indonesia (Kapolri) sejak tanggal 27 Januari 2021, menggantikan Jenderal Idham Azis. Ia adalah Kapolri beragama Kristen kedua dalam sejarah setelah Widodo Budidarmo (19741978), dan Kapolri termuda kedua dalam sejarah saat dilantik (51 tahun, 267 hari), hanya kalah dari Tito Karnavian, yang berusia 51 tahun, 261 hari saat dilantik pada 2016. Sigit juga merupakan Alumni SMA Negeri 8 Yogyakarta (1988)." .

:REMartadinata dc:description "Laksamana TNI (Purn.) Raden Eddy Martadinata merupakan tokoh di bidang militer angkatan laut yang lahir di Bandung (29 Maret 1921  6 Oktober 1966), atau yang lebih dikenal dengan nama R. E. Martadinata, adalah tokoh ALRI (Angkatan Laut Republik Indonesia) dan pahlawan nasional Indonesia. Ia meninggal dunia akibat kecelakaan helikopter di Riung Gunung dan dimakamkan di TMP Kalibata, Jakarta." .

:NobutakeKond dc:description "Nobutake Kond ( , Kond Nobutake, 25 September 1886  19 Februari 1953) adalah seorang Laksamana di Angkatan Laut selama Perang Dunia II. Sebagai komandan IJN Armada ke-2, kepala sekolah Angkatan Laut melepaskan diri untuk operasi independen, Kondo dianggap sebagai yang kedua setelah Laksamana  Isoroku Yamamoto." .

:SutanSjahrir dc:description "Sutan Syahrir (ejaan lama: Soetan Sjahrir, 5 Maret 1909  9 April 1966) adalah seorang intelektual, perintis, dan revolusioner kemerdekaan Indonesia. Setelah Indonesia merdeka, ia menjadi politikus dan perdana menteri pertama Indonesia. Ia menjabat sebagai Perdana Menteri Indonesia dari 14 November 1945 hingga 20 Juni 1947. Sjahrir mendirikan Partai Sosialis Indonesia pada tahun 1948. Ia meninggal dalam pengasingan sebagai tawanan politik dan dimakamkan di TMP Kalibata, Jakarta. Sutan Sjahrir ditetapkan sebagai salah seorang Pahlawan Nasional Indonesia pada tanggal 9 April 1966 melalui Keppres nomor 76 tahun 1966." .

:SlametRijadi dc:description "Brigadir Jenderal (Anumerta) TNI Ignatius Slamet Rijadi (EYD: Ignatius Slamet Riyadi; 26 Juli 1927  4 November 1950) adalah seorang tentara Indonesia. Rijadi lahir di Surakarta, Jawa Tengah, putra dari seorang tentara dan penjual buah. \"Dijual\" pada pamannya dan sempat berganti nama saat masih balita demi sembuh dari penyakit, Rijadi tumbuh besar di rumah orangtuanya dan belajar di sekolah milik Belanda. Setelah Jepang menduduki Hindia Belanda, Rijadi menghadiri sekolah pelaut yang dikelola oleh Jepang dan bekerja untuk mereka setelah lulus; ia meninggalkan tentara Jepang menjelang akhir Perang Dunia II dan turut mengobarkan perlawanan selama sisa pendudukan." .

:AgusSubiyanto dc:description "Jenderal TNI H. Agus Subiyanto, S.E., M.Si., (lahir 5 Agustus 1967) adalah seorang perwira tinggi Tentara Nasional Indonesia Angkatan Darat yang menjabat sebagai Panglima Tentara Nasional Indonesia sejak tanggal 22 November 2023, menggantikan Laksamana TNI Yudo Margono. Agus merupakan lulusan Akademi Militer (1991) yang berasal dari kecabangan Infanteri (Kopassus). Sebelumnya, beliau menjabat sebagai Kepala Staf TNI Angkatan Darat. Selain itu juga beliau merupakan putra daerah Jawa Barat yang berasal dari Cijulang, Pangandaran." .

:Assaat dc:description "Mr. Assaat gelar Datuk Mudo (18 September 1904  16 Juni 1976) adalah seorang politisi dan pejuang kemerdekaan Indonesia. Ia merupakan pemangku jabatan Presiden Republik Indonesia pada masa pemerintahan Republik Indonesia di Yogyakarta. Ia juga pernah menjabat sebagai Menteri Dalam Negeri Indonesia." .

:MuhammadToha dc:description "Mohammad Toha atau Mohammad Toha (Bandung, 1927 - Bandung, 11 Juli 1946) adalah seorang komandan Barisan Rakjat Indonesia, sebuah kelompok milisi pejuang yang aktif dalam masa Perang Kemerdekaan Indonesia. Toha gugur dalam kebakaran misi penghancuran gudang amunisi milik Tentara Sekutu bersama rekannya, setelah meledakkan dinamit dalam gudang amunisi tersebut." .

:AbdulHarisNasution dc:description "Jenderal Besar TNI (Purn.) Dr. (H.C.) Abdul Haris Nasution (3 Desember 1918  6 September 2000) adalah seorang jenderal berpangkat tinggi dan politikus Indonesia. Ia bertugas di militer selama Revolusi Nasional Indonesia dan ia tetap di militer selama gejolak berikutnya dari demokrasi Parlementer dan Demokrasi Terpimpin. Setelah jatuhnya Presiden Soekarno dari kekuasaan, ia menjadi Ketua Majelis Permusyawaratan Rakyat Sementara (MPRS) di bawah presiden Soeharto. Lahir dari keluarga Batak Mandailing, di desa Hutapungkut, ia belajar mengajar dan mendaftar di akademi militer di Bandung." .

:PrabowoSubianto dc:description "Jenderal TNI (HOR) (Purn.) Datuk Seri H." .

:EgianusKogoya dc:description "Egianus Kogoya (lahir 1999) adalah Panglima Komando Daerah Perang III Ndugama Tentara Pembebasan Nasional Papua Barat yang merupakan bagian dari kelompok Organisasi Papua Merdeka. Kelompok bersenjata yang dipimpin oleh Egianus Kogoya ini merupakan satu dari tujuh kelompok bersenjata yang masih aktif di Papua. Diperkirakan kelompok ini terdiri dari sekitar 50 orang. Dia merupakan putra dari Daniel Yudas Kogoya yang terlibat dalam penyanderaan tim Ekspedisi Lorentz (1996). " .

:BudiGunawan dc:description "Jenderal Polisi (Purn.) Tan Sri Prof. Dr. Budi Gunawan, S.H., M.Si., Ph.D.,  P.S.M. (lahir 11 Desember 1959) adalah Kepala Badan Intelijen Negara sejak 9 September 2016, dan juga Ketua Umum Pengurus Besar E-Sports Indonesia (PB ESI). Sebelumnya, ia pernah bertugas sebagai Wakapolri mendampingi Kapolri Badrodin Haiti dan Tito Karnavian. Ia adalah unsur Polisi kedua setelah Sutanto yang memimpin Badan Intelijen Negara." .

:JaminGinting dc:description "Letnan Jenderal TNI (Purn.) Drs. Jamin Ginting Suka (disingkat sebagai Jamin Gintings; Ejaan Republik: Djamin Gintings; 12 Januari 1921  23 Oktober 1974) adalah salah satu pejuang kemerdekaan Indonesia yang berasal dari Taneh Karo. Ia diangkat sebagai Pahlawan Nasional Indonesia oleh Joko Widodo pada tanggal 7 November 2014 lalu." .

:AchmadTahir dc:description "Jenderal TNI (HOR) (Purn.) Achmad Tahir (27 Juni 1924  17 Agustus 2002) adalah seorang pejuang kemerdekaan dan tokoh militer Indonesia. Dia pernah mengemban tugas sebagai Panglima Divisi IV/TKR pada zaman revolusi kemerdekaan Indonesia." .

:HubertusJohannesvanMook dc:description "Hubertus Johannes (Huib) van Mook (30 Mei 1894  10 Mei 1965) adalah Gubernur Jenderal Hindia Belanda secara de facto (pangkat sesungguhnya adalah Wakil Gubernur Jenderal) yang terakhir yang menjabat setelah Jepang menguasai Hindia Belanda." .

:TeukuNyakArif dc:description "Teuku Nyak Arif adalah Pahlawan Nasional Indonesia. Ia juga merupakan Residen/gubernur Aceh yang pertama periode 19451946. Pada masa perjuangan kemerdekaan Indonesia, saat Volksraad (parlemen) dibentuk, Teuku Nyak Arif terpilih sebagai wakil pertama dari Aceh." .

:SyamaunGaharu dc:description "Brigjen TNI (Purn.) H. Syamaun Gaharu (10 November 1913  30 September 2000) adalah seorang tokoh pejuang kemerdekaan menentang pemerintahan Hindia Belanda di Aceh." .

:DaudBeureueh dc:description "Teungku Muhammad Daud Beureueh (23 September 1896  10 Juni 1987)  atau bertepatan dengan 10 Zulhijjah 1316 Hijriah, akrab disapa Ayah Daud adalah mantan Gubernur Militer Aceh, Langkat dan Tanah Karo dan pejuang kemerdekaan Indonesia. Ia merupakan tokoh kontroversial yang populer di kalangan masyarakat Aceh. Ia melakukan pemberontakan kepada pemerintah dengan mendirikan NII akibat Soekarno yang melanggar perjanjian dengan rakyat Aceh dan ketidakpuasannya atas pemerintahan Soekarno. Namanya kini diabadikan untuk sebuah jalan di Banda Aceh." .

:HeinterPoorten dc:description "Hein ter Poorten (21 November 1887  15 Januari 1968) ialah komandan KNIL semasa Perang Pasifik." .

:IGustiNgurahRai dc:description "Brigadir Jenderal TNI (Anumerta) I Gusti Ngurah Rai (30 Januari 1917  20 November 1946) adalah seorang tokoh militer Indonesia, yang berjasa dalam Perang Kemerdekaan. Ia merupakan pendiri dan panglima pertama satuan angkatan bersenjata Republik Indonesia di Kepulauan Sunda Kecil, yang memimpin langsung perlawanan bersenjata anti-Belanda di Bali. Ia gugur pada bulan November 1946 dalam pertempuran dengan pasukan Belanda di dekat desa Marga, Bali tengah." .

:SimonSpoor dc:description "Jenderal Simon Hendrik Spoor (12 Januari 1902 - 25 Mei 1949) adalah seorang jenderal Belanda yang terkenal perannya ketika Belanda berusaha merebut kembali Indonesia, dan ia memimpin langsung 2 aksi polisionil Belanda tersebut yaitu Agresi Militer Belanda I dan II." .

:SyafruddinPrawiranegara dc:description "Mr. Sjafruddin Prawiranegara (EYD: Syafruddin Prawiranegara) 28 Februari 1911  15 Februari 1989) adalah seorang negarawan dan ekonom Indonesia. Ia memimpin Indonesia sebagai Ketua Pemerintah Darurat Republik Indonesia (PDRI). Selama masa Demokrasi Liberal, ia menjabat sebagai Menteri Keuangan dan Gubernur Bank Indonesia pertama." .

:MaludinSimbolon dc:description "Kolonel Infanteri Maludin Simbolon (13 September 1916  15 April 2000) adalah seorang pejuang kemerdekaan Indonesia, Panglima Tentara Teritorium I/Bukit Barisan, dan kemudian Menteri Luar Negeri dalam kabinet Pemerintahan Revolusioner Republik Indonesia (PRRI)." .

:AhmadYani dc:description "Jenderal TNI (Anumerta) Ahmad Yani (juga dieja A. Yani, Achmad Yani); (19 Juni 1922  1 Oktober 1965) adalah Menteri/Panglima Angkatan Darat (setingkat KSAD) yang merupakan salah satu Pahlawan Revolusi yang gugur sebagai korban tragedi Gerakan 30 September karena dibunuh dalam Gerakan 30 September saat penculikan dari rumahnya." .

:AhmadHusein dc:description "Kolonel (Purn.) Ahmad Husein (1 April 1925  28 November 1998) adalah seorang pejuang kemerdekaan Indonesia dan pemimpin militer PRRI. Pada tanggal 15 Februari 1958 di Padang dia membentuk Pemerintahan Revolusioner Republik Indonesia (PRRI) di bawah pimpinan Syafruddin Prawiranegara sebagai Perdana Menteri dengan tujuan mengoreksi pemerintahan otoriter Soekarno yang dianggap inkonstitusional dan mengabaikan pembangunan dan kesejahteraan masyarakat di daerah. Tindakan koreksinya itu ternyata mendapat sambutan berupa aksi militer dari pemerintah pusat di Jakarta sehingga menimbulkan perang saudara di Sumatera Barat." .

:HitoshiImamura dc:description "Hitoshi Imamura (Hitosji Imamoera) ( , Imamura Hitoshi, 28 Juni 1886  4 Oktober 1968) adalah seorang jenderal Jepang pada masa Perang Dunia II. Ia pernah menjadi Panglima Tentara ke-16 sekaligus Gubernur Jenderal di Jawa periode Maret - November 1942. Pada bulan November 1942, Letnan Jenderal Imamura menjadi Panglima Tentara ke-8 di Kepulauan Solomon dan Papua Nugini." .

:EdiSukardi dc:description "Kolonel  Inf. (Purn.) Edi Sukardi adalah seorang letnan kolonel Indonesia. Letkol Edi tercatat sebagai pemimpin dalam pertempuran Bojongkokosan yang terjadi di Sukabumi, 9 Desember 1945. Pertempuran Bojongkokosan kemudian diperingati sebagai Hari Juang Siliwangi. Dalam pertempuran Bojongkokosan, Tentara Keamanan Rakyat (TKR) dan berbagai spektrum laskar rakyat, baik kiri maupun kanan, mencegat tentara Inggris. Sebanyak 73 anggota TKR gugur, begitu juga lebih dari 80 orang tentara Inggris tewas. " .

:Musso dc:description "Musso atau Paul Mussotte bernama lengkap Muso Manowar atau Munawar Muso (12 Agustus 1897  31 Oktober 1948) adalah seorang pemimpin Partai Komunis Indonesia (PKI) dan salah satu tokoh kunci dalam pemberontakan Madiun 1948." .

:TanMalaka dc:description "Tan Malaka atau Ibrahim Gelar Datuk Sutan Malaka (2 Juni 1897  21 Februari 1949) adalah pengajar, filsuf, pejuang kemerdekaan Indonesia, pendiri Partai Murba, salah satu Pahlawan Nasional Indonesia, dan penulis Naar de Republiek Indonesia, buku pertama yang ditulis oleh pribumi Hindia Belanda untuk menggambarkan gagasan Hindia Belanda yang merdeka sebagai Indonesia, untuk itu Muhammad Yamin memberikan julukan Tan Malaka sebagai 'Bapak Republik Indonesia'." .

:HisaichiTerauchi dc:description "Hisaichi Terauchi ( , Terauchi Hisaichi) (8 Agustus 1879  12 Juni 1946) adalah seorang Marsekal Medan (Field Marshal) Angkatan Darat Kekaisaran Jepang dan Panglima Grup Angkatan Darat Expedisi Selatan pada masa Perang Dunia Kedua." .

:LouisMountbatten dc:description "Admiral of the Fleet Louis Francis Albert Victor Nicholas Mountbatten (biasa disebut secara informal sebagai Lord Mountbatten) merupakan seorang politisi, negarawan, serta perwira angkatan laut Britania Raya. Lord Mountbatten juga adalah paman dari Pangeran Philip dan sepupu Ratu Elizabeth II. Selama Perang Dunia II, ia bertindak sebagai Panglima Komando Asia Tenggara (1943-1946). Ia merupakan Raja Muda India terakhir sekaligus Gubernur Jenderal India yang pertama. Pada tahun 1950, India berdiri sebagai republik yang merdeka. Berbagai posisi penting dijabat Lord Mountbatten sesudah penugasannya di India baik di Britania Raya maupun di tingkat internasional." .

:PangSuma dc:description "Pang Suma adalah seorang tokoh pejuang kemerdekaan Indonesia yang bergerilya di Kalimantan Barat. Pang Suma dikenal sebagai pejuang melawan penjajah Jepang. Hingga kini, tokoh pahlawan yang bernama Pangsuma, belum ada satu pun yang mengetahui di mana dan kapan ia lahir. Namun menurut penuturan cucu pengawal Pangsuma, Sera, atau lebih dikenal dengan Pang Ronda, menuturkan bahwa Pangsuma berasal dari dusun di Kecamatan Meliau bernama Nek Bindang. Pangsuma merupakan nama panggilan, dalam Bahasa Meliau merupakan penggabungan dua suku kata yakni Pang berarti bapak dan Suma adalah nama anaknya." .

:DirkCornelisBuurmanvanVreeden dc:description "Dirk Cornelis Buurman van Vreeden (16 Juni 1902  12 Juni 1964) adalah komandan KNIL yang terakhir. Ia menjabat antara bulan Mei 1949 hingga Juli 1950. Buurman van Vreeden menempuh pendidikan sekolah dasar di Den Haag dan Kampen. Pada tahun 1921, ia meneruskan ke Koninklijke Militaire Academie di Breda dan kemudian letnan di artileri Koninklijk Nederlandsch-Indisch Leger. Ia belajar di Hogere Krijgsschool antara tahun 1931-1934 dan menduduki berbagai kedudukan militer KNIL di Hindia Belanda (kini Indonesia)." .

:SebbySambom dc:description "Sebby Sambom (lahir 3 Januari 1975) adalah Juru Bicara Tentara Pembebasan Nasional Papua Barat - Organisasi Papua Merdeka (TPNPB-OPM). Dia pernah ditahan pada tanggal 16 Agustus 2008 sehubungan dengan perencanaan atau pidato dalam aksi damai mendukung peluncuran Parlemen Internasional untuk Papua Barat." .

:AlidiusTjardavanStarkenborghStachouwer dc:description "Jonkheer Mr. Alidius Warmoldus Lambertus Tjarda van Starkenborgh-Stachouwer (7 Maret 1888  16 Agustus 1978) adalah seorang bangsawan dan negarawan Belanda, ia dikenal sebagai gubernur jenderal terakhir Hindia Belanda. Ia masuk dalam tahanan Jepang setelah menyerahnya angkatan perang seluruh Hindia Belanda tanpa syarat dalam Kapitulasi Kalijati pada 8 atau 9 Maret 1942. Pada awalnya, ia ditahan di Bandung dan Batavia, kemudian dipindahkan ke Manchuria. Pada saat penandatanganan kapitulasi yang dilakukan oleh Jenderal Hein ter Poorten, Tjarda telah meninggalkan ruangan perundingan. Sebelumnya, pada tanggal 5 Maret 1942, Tjarda telah memisahkan kekuasaan sipil dan militer serta mengalihkan kekuasaan militer kepada Ter Poorten. Ia kemudian tidak menyerahkan kekuasaan sipil atas Hindia Belanda pada Kapitulasi Kalijati. Tindakan tersebut dijadikan dasar bagi Belanda untuk mengalihkan kekuasaan sipil kepada Letnan Gubernur Jenderal Hubertus van Mook yang telah mengasingkan diri ke Australia. Legitimasi inilah yang digunakan untuk membentuk Pemerintahan Sipil Hindia Belanda (NICA) di pengasingan Australia." .

:DaanMogot dc:description "Elias Daniel Mogot, atau lebih dikenal dengan nama Daan Mogot (28 Desember 1927  25 Januari 1946), adalah seorang pejuang kemerdekaan Indonesia dan mantan anggota (dan pelatih) PETA di Bali dan Jakarta pada tahun 1942-1945. Setelah Perang Dunia ke-2 selesai, ia menjadi Komandan TKR di Jakarta dengan pangkat Mayor. Bulan November 1945 mendirikan sekaligus menjadi Direktur Pertama Akademi Militer Tangerang (MAT) dalam usia 18 tahun. Ia gugur di Hutan Lengkong, di selatan Kota Tangerang, bersama 36 orang lainnya dalam pertempuran melawan tentara Jepang saat hendak melucuti senjata mereka di Hutan Lengkong di Tangerang." .

:LudolphHendrikvanOyen dc:description "Ludolph Hendrik van Oyen (juga Oijen; 25 April 1889  28 Juli 1953) adalah seorang letnan jenderal berkebangsaan Belanda dan komandan AU KNIL semasa pecahnya Perang Dunia II. Ludolph Hendrik van Oyen memulai karier militer di Sekolah Taruna Alkmaar sejak tahun 1906 kemudian pada tahun 1911 melanjutkan ke Koninklijke Militaire Academie, Breda. Pada tanggal 4 Agustus 1913, ia menikah dengan Elise Marie Francina Brouwer dan dikaruniai 2 orang anak. Antara tahun 1922-1925, ia menjadi kapiten di Hoogere Krijgsschool, Den Haag dan setelah itu dilantik sebagai mayor dan komandan AU KNIL. Dalam berbagai posisi, ia tetap dalam pangkat itu hingga naik pangkat sebagai mayor jenderal pada tahun 1940." .

:TjokordaGdeRakaSoekawati dc:description "Tjokorda Gde Raka Soekawati (ejaan baru: Cokorda Gde Raka Sukawati), (lahir di Ubud, Gianyar, Bali, 15 Januari 1899 dan meninggal tahun 1967) adalah satu-satunya Presiden Negara Indonesia Timur. Ia menjabat dari tahun 1946 hingga pembubaran Negara Indonesia Timur pada 1950. Gelarnya, Tjokorda Gde, menandai bahwa Soekawati masuk kedalam kasta ksatria. Ia memiliki dua orang istri, yang pertama adalah orang Bali yaitu, Gusti Agung Niang Putu yang memberikan seorang putra yang bernama Tjokorda Ngurah Wim Sukawati. Pada tahun 1933, ia menikahi seorang perempuan Prancis bernama Gilbert Vincent, yang memberikannya dua orang anak." .

:Wongsonegoro dc:description "Mr. Wongsonegoro (20 April 1897  4 Maret 1978) adalah Wakil Perdana Menteri Indonesia Kabinet Ali Sastroamidjojo I pada tahun 1953 hingga tahun 1955 dan Menteri Pendidikan dan Kebudayaan Indonesia pada tahun 1951 hingga tahun 1952. Selain itu pada masa persiapan kemerdekaan Indonesia, ia juga bergabung dengan BPUPKI, mewakili Surakarta, bersama-sama dengan Wuryaningrat, Sosrodiningrat, dan Radjiman Wedyodiningrat." .

:Kariadi dc:description "Untuk nama rumah sakit, lihat: Rumah Sakit Umum Pusat Dr. Kariadi.dr. Kariadi (15 September 1905  14 Oktober 1945) adalah pejuang Indonesia sekaligus dokter, pahlawan nasional yang gugur dalam Pertempuran Lima Hari, Semarang - Jawa Tengah. Namanya kini diabadikan di Rumah Sakit Umum Pusat Dr. Kariadi, Semarang." .

:GatotSoebroto dc:description "Jenderal TNI Gatot Soebroto (10 Oktober 1907  11 Juni 1962) adalah tokoh perjuangan militer Indonesia dalam merebut kemerdekaan dan juga pahlawan nasional Indonesia. Ia dimakamkan di Ungaran, kabupaten Semarang." .

:KellyKwalik dc:description "Kelly Kwalik (lahir di Agimuga, Mimika, Papua, Nugini Belanda, 1955 - meninggal di Timika, Papua, Indonesia, 16 Desember 2009) adalah seorang pemimpin separatis senior dan komandan dari sayap militer Organisasi Papua Merdeka (OPM), sebuah organisasi separatis yang berbasis di Provinsi Papua di Indonesia." .

:BJHabibie dc:description "Prof. Dr.-Ing. Ir. H. Bacharuddin Jusuf Habibie, FREng. (25 Juni 1936  11 September 2019) adalah Presiden Republik Indonesia yang ketiga. Sebelumnya, B.J. Habibie menjabat sebagai Wakil Presiden Republik Indonesia ke-7, menggantikan Try Sutrisno. B. J. Habibie menggantikan Soeharto yang mengundurkan diri dari jabatan presiden pada tanggal 21 Mei 1998. Sebelum memasuki dunia politik, Habibie dikenal luas sebagai seorang profesor dan ilmuwan dalam teknologi aviasi internasional dan satu-satunya presiden Indonesia hingga saat ini yang berlatarbelakang teknokrat." .

:ThomasCHart dc:description "Thomas Charles Hart (12 Juni 1877  4 Juli 1971) adalah seorang laksamana dalam Angkatan Laut Amerika Serikat yang bertugas dari Perang Spanyol-Amerika sampai Perang Dunia II. Setelah ia pensiun dari AL, ia secara singkat menjabat sebagai Senator Amerika Serikat dari Connecticut." .

:ShojiNishimura dc:description "Shji Nishimura ( , Nishimura Shji, 30 November 1889  24 Oktober 1944) adalah seorang Laksamana di Imperial Japanese Navy saat berlangsungnya Perang Dunia II. Ia gugur pada Pertempuran Teluk Leyte." .

:Soedirman dc:description "Jenderal Besar TNI (Anumerta) Raden Soedirman (EYD: Sudirman; 24 Januari 1916  29 Januari 1950) adalah seorang perwira tinggi Indonesia pada masa Revolusi Nasional Indonesia. Sebagai Panglima Besar Tentara Nasional Indonesia pertama, ia adalah sosok yang dihormati di Indonesia. Terlahir dari pasangan rakyat biasa di Purbalingga, Hindia Belanda, Soedirman diadopsi oleh pamannya yang seorang priyayi. Setelah keluarganya pindah ke Cilacap pada tahun 1916, Soedirman tumbuh menjadi seorang siswa rajin; ia sangat aktif dalam kegiatan ekstrakurikuler, termasuk mengikuti program kepanduan yang dijalankan oleh organisasi Islam Muhammadiyah. Saat di sekolah menengah, Soedirman mulai menunjukkan kemampuannya dalam memimpin dan berorganisasi. Soedirman sangat dihormati oleh masyarakat karena ketaatannya pada Islam. Setelah berhenti kuliah keguruan, pada 1936 ia mulai bekerja sebagai seorang guru, dan kemudian menjadi kepala sekolah, di sekolah dasar Muhammadiyah; ia juga aktif dalam kegiatan Muhammadiyah lainnya dan menjadi pemimpin Kelompok Pemuda Muhammadiyah pada tahun 1937. Setelah Jepang menduduki Hindia Belanda pada 1942, Soedirman tetap mengajar. Pada tahun 1944, ia bergabung dengan tentara Pembela Tanah Air (PETA) yang disponsori Jepang, menjabat sebagai komandan batalion di Banyumas. Selama menjabat, Soedirman bersama rekannya sesama prajurit melakukan pemberontakan, hingga kemudian diasingkan ke Bogor." .

:TakeoTakagi dc:description "Takeo Takagi (, Takagi Takeo, 25 Januari 1892  8 Juli 1944) ialah seorang laksamana AL Kekaisaran Jepang pada masa Perang Dunia II." .

:DirkReinhardAdelbertvanLangen dc:description "Mayor-jenderal Dirk Reinhard Adelbert van Langen (17 Mei 1898  20 Januari 1983) adalah seorang anggota Kepala Staf Tentara Kerajaan Hindia Belanda Komandan Teritorial Jawa Timur. Ia juga merupakan panglima brigade T pada Perang Kemerdekaan Indonesia di Hindia Belanda, dari 1946 sampai 1949, pada Revolusi Nasional Indonesia." .

:BambangSoegeng dc:description "Letnan Jenderal TNI (Purn.) Bambang Soegeng (ER: Bambang Sugeng) (31 Oktober 1913  22 Juni 1977) adalah seorang tokoh militer Indonesia dan pernah menjadi Kepala Staf TNI Angkatan Darat ke-3 yang menjabat dari tanggal 22 Desember 1952 hingga 8 Mei 1955.Selain berkarier di dunia militer, Bambang juga pernah menjabat sebagai Duta Besar Indonesia untuk Vatikan, Jepang, dan Brasil." .

:OeripSoemohardjo dc:description "Jenderal TNI (Anumerta) Raden  Oerip Soemohardjo (EYD: Raden Urip Sumoharjo; nama baptis: Benedict Oerip Soemohardjo; 22 Februari 1893  17 November 1948) adalah seorang jenderal dan kepala staf umum Tentara Nasional Indonesia pertama pada masa Revolusi Nasional Indonesia. Lahir di Purworejo, Hindia Belanda, Oerip kecil adalah anak nakal yang sudah memperlihatkan kemampuan memimpin sejak usia dini. Orangtuanya menginginkan dirinya untuk mengikuti jejak kakeknya sebagai bupati, oleh sebab itu, setamat sekolah dasar, ia dikirim ke Sekolah Pendidikan Pegawai Pribumi (OSVIA) di Magelang. Ibunya wafat saat ia menjalani tahun kedua di sekolah, dan Oerip berhenti sekolah untuk mengikuti pelatihan militer di Meester Cornelis, Batavia (kini Jatinegara, Jakarta). Setelah lulus pada tahun 1914, ia menjadi letnan di Koninklijk Nederlands-Indische Leger (KNIL), tentara pemerintah kolonial Belanda. Bertugas selama hampir 25 tahun, ia ditempatkan di tiga pulau berbeda dan dipromosikan beberapa kali, dan akhirnya menjadi perwira pribumi dengan pangkat tertinggi di KNIL." .

:AndikaPerkasa dc:description "Jenderal TNI (Purn.) Muhammad Andika Perkasa, S.E., M.A., M.Sc., M.Phil., Ph.D. (nama lahir: Fransiskus Xaverius Emanuel Andika Perkasa, lahir 21 Desember 1964) adalah seorang purnawirawan TNI yang menjabat Panglima Tentara Nasional Indonesia pada tahun 2021 sampai 2022. Andika merupakan lulusan Akademi Militer tahun 1987. Sebelumnya, dia menjabat sebagai Kepala Staf TNI Angkatan Darat. Pada saat dilantik, ia adalah Panglima TNI tertua sepanjang sejarah, tetapi rekor itu dipecahkan oleh Laksamana Yudo Margono yang dilantik menggantikannya pada tanggal 19 Desember 2022. Selain itu juga berasal dari keluarga campuran Magelang, Jawa Tengah dan Blitar, Jawa Timur." .

:ConradHelfrich dc:description "Luitenant-Admiraal Conrad Emil Lambert Helfrich (KCB) (11 Oktober 1886  20 September 1962) dari Koninklijke Marine adalah tokoh AL utama Belanda dalam Perang Dunia II." .

:ArchibaldWavell1stEarlWavell dc:description "Marsekal Lapangan Archibald Percival Wavell, 1st Earl Wavell,  (5 Mei 1883  24 Mei 1950) adalah seorang perwira senior Angkatan Darat Inggris. Ia bertugas dalam Perang Boer Kedua, Kampanye Bazar Valley dan Perang Besar, di mana ia terluka dalam Pertempuran Ypres Kedua. Ia bertugas dalam Perang Dunia Kedua, awalnya sebagai Ketua Komandan Timur Tengah, di mana ia memimpin pasukan Inggris menuju kemenangan atas Italia di barat Mesir dan timur Libya saat Operasi Compass pada Desember 1940, dan hanya dikalahkan oleh Angkatan Darat erman di Gurun Barat pada April 1941. Ia bertugas sebagai Ketua Komandan India, dari Juli 1941 sampai Juni 1943 (selain melakukan tur sebagai Komandan ABDACOM) dan kemudian menjabat sebagai Viceroy India sampai ia pensiun pada Februari 1947." .

:KarelDoorman dc:description "Karel Willem Frederik Marie Doorman (23 April 1889  28 Februari 1942) ialah laksamana Belanda (bahasa Belanda: schout-bij-nacht) selama Perang Dunia II." .

:HamengkubuwanaIX dc:description "Jenderal TNI (Tit.) (Purn.) H. Sri Sultan Hamengkubuwana IX (Jawa: ; 12 April 1912  2 Oktober 1988, lahir dengan nama Gusti Raden Mas Dorodjatun) adalah Sultan Yogyakarta kesembilan dan Gubernur Daerah Istimewa Yogyakarta yang pertama. Ia merupakan Wakil Presiden Indonesia kedua yang menjabat pada tahun 19731978. Hamengkubuwana IX juga merupakan Ketua Kwartir Nasional Gerakan Pramuka yang pertama dan dikenal sebagai Bapak Pramuka Indonesia." .

:VentjeSumual dc:description "Herman Nicolas Ventje Sumual (11 Juni 1923  28 Maret 2010) adalah salah seorang perwira militer yang berasal dari unsur kelaskaran dan juga tokoh Permesta." .

:Soeharto dc:description "Jenderal Besar TNI (Purn.) H. M. Soeharto, (pelafalan dalam bahasa Indonesia: [/suhrt/]; ER, EYD: Suharto; 8 Juni 1921  27 Januari 2008) adalah Presiden kedua Indonesia yang menjabat dari tahun 1967 hingga 1998. Secara luas dianggap sebagai diktator militer oleh pengamat internasional, Soeharto memimpin Indonesia sebagai rezim otoriter sejak kejatuhan pendahulunya Soekarno pada tahun 1967 hingga pengunduran dirinya pada tahun 1998 menyusul kerusuhan nasional. Kediktatorannya selama 32 tahun dianggap sebagai salah satu kediktatoran paling brutal dan korup di abad ke-20.Sebelum menjadi presiden, Soeharto adalah pemimpin militer pada masa Hindia Belanda dan Kekaisaran Jepang, dengan pangkat terakhir Mayor Jenderal. Setelah Gerakan 30 September 1965, Soeharto kemudian melakukan operasi penertiban dan pengamanan atas perintah dari Presiden Soekarno, salah satu yang dilakukannya adalah dengan menumpas Gerakan 30 September dan menyatakan bahwa PKI sebagai organisasi terlarang. Berbagai kontroversi menyebut operasi ini menewaskan sekitar 100.000 hingga 2 juta jiwa.Soeharto kemudian diberi mandat oleh Majelis Permusyawaratan Rakyat Sementara (MPRS) sebagai Presiden pada 26 Maret 1968 menggantikan Soekarno, dan resmi menjadi presiden pada tahun 1968. Ia dipilih kembali oleh MPR pada tahun 1973, 1978, 1983, 1988, 1993, dan 1998. Pada tahun 1998, masa jabatannya berakhir setelah mengundurkan diri pada tanggal 21 Mei tahun tersebut, menyusul terjadinya kerusuhan Mei 1998 dan pendudukan gedung DPR/MPR oleh ribuan mahasiswa. Ia merupakan orang terlama yang menjabat sebagai presiden Indonesia. Soeharto digantikan oleh B.J. Habibie." .

:LeslieMorshead dc:description "Letnan Jenderal Sir Leslie James Morshead,  (18 September 1889  26 September 1959) adalah seorang prajurit, guru, pengusaha, dan petani asal Australia, yang berkarier militer sepanjang dua perang dunia. Pada Perang Dunia Kedua, ia memimpin pasukan Australia dan Inggris di Pengepungan Tobruk (1941) dan di Pertempuran El Alamein Kedua" .

:SusiloBambangYudhoyono dc:description "Jenderal TNI (HOR) (Purn.) Prof. Dr. H. Susilo Bambang Yudhoyono, M.A. (lahir 9 September 1949), atau lebih dikenal dengan inisialnya SBY, adalah Presiden Indonesia keenam yang menjabat sejak 20 Oktober 2004 sampai 20 Oktober 2014. Ia merupakan Presiden pertama di era Reformasi yang terpilih melalui Pemilihan Umum secara langsung. SBY bersama Wakil Presiden Muhammad Jusuf Kalla, terpilih dalam Pemilu Presiden 2004. Ia berhasil melanjutkan pemerintahannya untuk periode kedua dengan kembali memenangkan Pemilu Presiden 2009, kali ini bersama Wakil Presiden Boediono. Sejak era Reformasi dimulai, Susilo Bambang Yudhoyono merupakan Presiden Indonesia pertama yang menyelesaikan masa jabatan selama 5 tahun dan berhasil terpilih kembali untuk periode kedua." .

:SaalahYusufSutanMangkuto dc:description "Saalah Yusuf Sutan Mangkuto, sering ditulis S.Y. Sutan Mangkuto, (19011974) adalah organisiator dan aktivis Muhammadiyah. Ia merupakan pendiri cabang Muhammadiyah di Padang Panjang pada  1926 dan pernah menjadi Ketua Pimpinan Muhammadiyah Sumatra Tengah periode 19491956." .

:WilhelminadariBelanda dc:description "Ratu Wilhelmina  (Wilhelmina Helena Pauline Marie van Orange-Nassau; (31 Agustus 1880  28 November 1962), Putri Orange-Nassau, adalah Ratu Belanda sejak 1890 - 1948 dan Ibu Suri (dengan sebutan Putri) sejak 1948 - 1962." .

:LeonardusBenyaminMoerdani dc:description "Jenderal TNI (Purn.) Leonardus Benyamin Moerdani, atau L.B. Moerdani, atau kerap disebut Benny Moerdani (2 Oktober 1932  29 Agustus 2004) adalah salah satu tokoh militer Indonesia paling berpengaruh pada era Orde Baru. Benny Moerdani dikenal sebagai perwira TNI yang banyak berkecimpung di dunia intelijen, sehingga sosoknya banyak dianggap misterius. Selain itu, Ia juga memiliki julukan yang merupakan antitesis dari Soeharto yaitu \"Unsmiling General\".Moerdani merupakan perwira yang ikut terjun langsung di operasi militer penanganan pembajakan pesawat Garuda Indonesia Penerbangan 206 di Bandara Don Mueang, Bangkok, Kerajaan Thai pada tanggal 28 Maret 1981, peristiwa yang kemudian dicatat sebagai peristiwa pembajakan pesawat pertama dalam sejarah maskapai penerbangan Republik Indonesia dan terorisme bermotif jihad pertama di Indonesia. Ia juga dianggap banyak kalangan sebagai sosok yang bertanggung jawab terhadap peristiwa Tanjung Priok dan penembakan misterius pada tahun 1980-an ." .

:MarufAmin dc:description "Prof. Dr.  (H.C.) K.H. Ma'ruf Amin (lahir 11 Maret 1943) adalah seorang ulama, dosen, dan politikus Indonesia yang saat ini menjabat sebagai Wakil Presiden Republik Indonesia, terhitung sejak tanggal 20 Oktober 2019. Ma'ruf menyertai politik sejak terpilihnya sebagai anggota DPRD DKI Jakarta pada 1971 hingga menjadi anggota Dewan Perwakilan Rakyat selama dua periode sejak 1997 sampai 2004. Setelahnya, ia aktif di Majelis Ulama Indonesia dan pada akhirnya ditunjuk oleh Joko Widodo untuk mendampinginya pada Pemilu Presiden 2019 dengan didukung oleh Koalisi Indonesia Kerja. Selain itu ia juga merupakan tokoh senior organisasi Nahdlatul Ulama sebagai Rais 'Aam sejak 2015, dan menjadi Mustasyar Pengurus Besar Nahdlatul Ulama sejak ia mencalonkan diri sebagai Wakil Presiden 2019." .

:MegawatiSoekarnoputri dc:description "Prof. Dr. (H.C.) Hj. Diah Permata Megawati Setiawati Soekarnoputri (lahir 23 Januari 1947) adalah Presiden Indonesia yang kelima yang menjabat sejak 23 Juli 2001 sampai 20 Oktober 2004. Ia merupakan presiden wanita Indonesia pertama dan putri dari presiden Indonesia pertama, Soekarno, yang kemudian mengikuti jejak ayahnya menjadi Presiden Indonesia. Pada 20 September 2004, ia kalah suara dari Susilo Bambang Yudhoyono dalam Pemilu Presiden 2004 putaran yang kedua." .

:TBSimatupang dc:description "Letnan Jenderal TNI (Purn.) Tahi Bonar Simatupang (disingkat sebagai T.B. Simatupang; 28 Januari 1920  1 Januari 1990) adalah seorang tokoh militer dan tokoh Gereja di Indonesia." .

:AdamBB dc:description "Syekh Haji Adam B.B. atau Syekh Adam Balai-Balai (31 Agustus 1889  15 Juli 1953) adalah salah seorang Ulama Minangkabau terkemuka yang tercatat sampai pertengahan abad ke-20. Adam B.B. yang sebelumnya adalah seorang pendekar dan parewa gadang (jagoan besar) juga dikenal sebagai ulama dan guru yang menginginkan lulusan surau yang ideal, yaitu kombinasi ulama, pandeka (pendekar) dan jiwa seni yang mandiri dan terampil, seperti sosok pribadinya. Ia merupakan pendiri Surau Pasar Baru (SPB) di Padang Panjang yang kemudian hari menjadi Madrasah Irsyadin Naas (MIN)." .

:Wiranto dc:description "Jenderal TNI (Purn.) Dr. H. Wiranto S.H. S.I.P. M.M. (lahir 4 April 1947) adalah seorang mantan perwira tinggi militer dan politikus senior berkebangsaan Indonesia. Saat ini, ia diberi mandat oleh Presiden Joko Widodo untuk menjabat sebagai Ketua Dewan Pertimbangan Presiden pada akhir 2019. Kiprahnya di politik di awali ketika dirinya ditunjuk menjadi Menteri Pertahanan dan Keamanan menjelang berakhirnya masa Orde Baru. Saat itu, Wiranto tergabung dalam Golongan Karya hingga akhirnya ia membentuk partai baru bernama Partai Hati Nurani Rakyat pada tahun 2006.Wiranto merupakan lulusan Akademi Militer Nasional 1968 berhasil meniti karir militer sampai puncak jabatan di ABRI (sekarang TNI) sebagai Panglima merangkap Menhankam.Jabatan rangkap sebagai Menhankam/Pangab, kecuali Wiranto juga pernah dijabat oleh Jenderal TNI (Purn.) M. Jusuf. Pada pergantian Orde Baru ke Orde Reformasi tahun 1998/1999, Wiranto sebagai Menhankam/Pangab memiliki peran yang sangat menentukan dalam mengawal proses pergantian tersebut." .

:LoaSekHie dc:description "Loa Sek Hie Sia (lahir di Batavia pada tahun 1898 - meninggal di Den Haag pada tahun 1965) dulu adalah seorang politisi dan anggota parlemen di Hindia Belanda. Ia adalah voorzitter atau chairman pertama dari pasukan bela diri etnis Tionghoa, Pao An Tui (1946 - 1949). Ia adalah Peranakan keturunan Tionghoa-Indonesia, Austria, dan Jawa. Dalam karir politiknya, ia mengkampanyekan perlawanan terhadap diskriminasi rasial serta memperjuangkan pelayanan kesehatan dan pendidikan yang lebih baik bagi etnis Tionghoa di Hindia Belanda." .

:SyarifHamidIIdariPontianak dc:description "Sultan Hamid II, lahir dengan nama Syarif Abdul Hamid Alkadrie, (12 Juli 1913  30 Maret 1978) adalah putra sulung Sultan Pontianak ke-6, Sultan Syarif Muhammad Alkadrie, adalah perancang Lambang Negara Indonesia, Garuda Pancasila. Ia memiliki darah keturunan Arab-Indonesia. Semasa hidupnya, Hamid II beristrikan seorang perempuan Belanda kelahiran Surabaya, yang memberikannya dua anak yang sekarang tinggal di Belanda." .

:PhilipChristison dc:description "Jend. Sir (Alexander Frank) Philip Christison, 4th Baronet GBE CB DSO MC (17 November 1893  21 Desember 1993) adalah komandan militer Britania Raya selama Perang Dunia II." .

:BennyWenda dc:description "Benny Wenda (lahir di Lembah Baliem, Irian Jaya) adalah pemimpin kemerdekaan Papua Barat dan Ketua Persatuan Gerakan Pembebasan Papua Barat (Inggris: United Liberation Movement for West Papua (ULMWP)).  Dia adalah pelobi internasional untuk kemerdekaan Papua Barat dari Indonesia. Dia tinggal di pengasingan di Inggris Raya. Pada tahun 2003 dia diberikan suaka politik oleh pemerintah Inggris setelah dia melarikan diri dari tahanan saat diadili." .

:AbdulkadirWidjojoatmodjo dc:description "Raden Abdulkadir Widjojoatmodjo (18 Desember 1904  24 Desember 1992) adalah seorang perwira militer, diplomat, dan pejabat tinggi Hindia Belanda" .

:JacobPrai dc:description "Jacob Prai  (17 Juli 1942  26 Mei 2022) adalah ketua pimpinan Organisasi Papua Merdeka (OPM) yang sebelumnya ia telah menjabat sebagai Kepala Senat Pemerintahan Sementara Papua Barat. Dinyatakan di Great Waris, daerah perbatasan antara Papua Nugini dan Papua Barat, tanah air Prai ini Mr Prai diberi suaka di Swedia dengan Dr John Otto Ondawame dan pernah memimpin Gerakan Papua Kantor Internasional di Malm, Swedia." .

:AbdulKaharMuzakkar dc:description "Abdul Kahar Muzakkar atau Abdul Qahhar Mudzakkar, (24 Maret 1921  3 Februari 1965) (nama kecilnya La Domeng), adalah pendiri Tentara Islam Indonesia di Sulawesi." .

:IsmaelLengah dc:description "Kolonel Ismael Lengah (22 September 1914  11 Januari 2005) adalah seorang tokoh militer dan pejuang kemerdekaan Indonesia. Pada tahun 1956 Ismael Lengah menjabat sebagai Panglima Komando Divisi IX Banteng sebelum meletusnya peristiwa PRRI. Komando Divisi IX Banteng adalah salah satu divisi dalam Angkatan Perang Republik Indonesia (APRI) dengan teritorial Sumatra Tengah yang meliputi provinsi Sumatera Barat, Riau, Kepulauan Riau dan Jambi sekarang. Ismael Lengah menjabat posisi panglima dengan pangkat Kolonel ketika itu.Sebelum dan sesudah kemerdekaan Ismael Lengah selalu aktif dalam perjuangan mengusir penjajah. Ia juga pernah memimpin suatu rapat rahasia di Padang yang dilangsungkan pada tanggal 18 Agustus 1945 yang kemudian berlanjut pada tanggal 25 Agustus 1945 dengan mendirikan Balai Penerangan Pemuda Indonesia (BPPI) yang diketuai langsung olehnya. Kelanjutan dari itu pada tanggal 31 Agustus, terbentuklah Komite Nasional Indonesia (KNI) Daerah Sumatra Tengah yang diketuai oleh Muhammad Sjafei." .

:TrySutrisno dc:description "Jenderal TNI (Purn.) H. Try Sutrisno (lahir 15 November 1935) adalah Wakil Presiden Indonesia ke-6 periode 19931998. Sebelum diangkat sebagai Wakil Presiden Indonesia, Try menjabat sebagai Panglima Angkatan Bersenjata Republik Indonesia (ABRI)." .

:PakubuwanaXII dc:description "Letnan Jenderal TNI (Tit.) Sri Susuhunan Pakubuwana XII (disingkat sebagai PB XII, Jawa:  XII; 14 April 1925  11 Juni 2004) adalah susuhunan Surakarta yang masa pemerintahannya paling lama di antara raja-raja Jawa, yaitu selama 59 tahun, tepatnya mulai tahun 1945 hingga 2004." .

:MangkunegaraVIII dc:description "Kanjeng Gusti Pangeran Adipati Arya Mangkunegara VIII (1 Januari 1920  3 September 1987) adalah Adipati kedelapan Mangkunagaran yang merupakan penguasa dari Kadipaten Praja Mangkunegaraan kenaikan takhta tepat pada tanggal 19 Juli 1944 (masa pemerintahaan Jepang) dan bertepatan pada wafat ayahnya yaitu Mangkunegara VII. Mangkunegara VIII memiliki nama B.R.M Natosoeparto dipilih atas dasar karena merupakan anak laki-laki yang tertua dan mempunyai sebuah pengalaman di luar istana." .

:AchmadiHadisoemarto dc:description "Mayor Jenderal TNI (Purn.) Achmadi Hadisoemarto (EYD: Akhmadi Hadisumarto; 5 Juni 1927  2 Januari 1984)  adalah seorang tentara Indonesia." .

:JokoWidodo dc:description "Ir. H. Joko Widodo (Indonesia: [dk widd]; lahir 21 Juni 1961), lebih dikenal sebagai Jokowi, adalah presiden Indonesia ke-7 yang mulai menjabat sejak terpilih dalam pemilihan umum tahun 2014. Jokowi menjadi presiden Indonesia pertama yang bukan berasal dari elit politik atau militer Indonesia. Ia terpilih bersama Wakil Presiden Jusuf Kalla dan kembali terpilih bersama Wakil Presiden Ma'ruf Amin pada tahun 2019. Sebelumnya ia menjabat sebagai Wali Kota Surakarta dan Gubernur DKI Jakarta." .

:JacobRumbiak dc:description "Drs. Jacob Rumbiak (lahir 11 Maret 1958) adalah akademisi dan pemimpin politik Papua Barat yang telah mengasingkan diri di Australia setelah melarikan diri dari penahanan sebagai tahanan politik selama sepuluh tahun di penjara Indonesia. Rumbiak adalah perwakilan Urusan Luar Negeri dari Republik Federasi Papua Barat yang dideklarasikan pada akhir Kongres Rakyat Papua Ketiga pada 19 Oktober 2011. Nasihat Rumbiak dari dalam Papua Barat untuk tidak menghadiri Kongres karena alasan keamanan dibenarkan dalam penumpasan yang  menyebabkan enam kematian, ratusan penangkapan dan hukuman lima tokoh utama masing-masing penjara tiga tahun karena pengkhianatan." .

:SekarmadjiMaridjanKartosoewirjo dc:description "Sekarmadji Maridjan Kartosoewirjo (7 Januari 1905  5 September 1962) adalah seorang tokoh Islam Indonesia yang mendirikan gerakan Darul Islam dari tahun 1949 hingga tahun 1962, dengan tujuan mendirikan Negara Islam Indonesia berdasarkan hukum syariah." .

:AmirSjarifoeddin dc:description "Mr. Amir Sjarifoeddin Harahap (ER, EYD: Amir Syarifuddin Harahap; 27 April 1907  19 Desember 1948) adalah seorang politikus dan jurnalis Indonesia. Ia menjabat sebagai Perdana Menteri Indonesia ketika Revolusi Nasional Indonesia sedang berlangsung. Amir adalah pemimpin sayap kiri terdepan pada masa Revolusi. Pada tahun 1948. Sebagai pemimpin pemberontakan  PKI Madiun bersama Musso, Amir dieksekusi mati bersama beberapa tokoh PKI lainnya yang terlibat dalam Peristiwa Madiun." .

:AgustinusAdisoetjipto dc:description "Komodor Muda Udara (Anumerta) dr. Agustinus Adisoetjipto (Hanacaraka: ) (3 Juli 1916  29 Juli 1947) adalah seorang pahlawan nasional beragama Katolik Roma dan seorang komodor udara Indonesia. Ia merupakan Bapak Penerbang Indonesia." .

:AbdurrahmanWahid dc:description "Dr. (H.C.) K.H. Abdurrahman Wahid, Lc. ( ; dilahirkan dengan nama Abdurrahman ad-Dakhil; 7 September 1940  30 Desember 2009), atau lebih dikenal dengan nama Gus Dur (), adalah seorang politikus Indonesia dan pemimpin agama Islam yang menjabat sebagai presiden Indonesia ke-4, dari pemilu tahun 1999 hingga pemakzulannya pada tahun 2001. Selain sebagai pemimpin organisasi Nahdlatul Ulama, ia juga merupakan pendiri Partai Kebangkitan Bangsa (PKB). Ia adalah putra Menteri Agama Wahid Hasyim, dan cucu dari pendiri Nahdlatul Ulama, Hasyim Asy'ari. Ia menderita gangguan penglihatan yang disebabkan oleh glaukoma; Ia mengalami kebutaan total pada mata kirinya dan mata kanannya buta sebagian. Ia merupakan presiden Indonesia pertama dan satu-satunya (sejauh ini) yang memiliki disabilitas fisik." .

:JulianadariBelanda dc:description "Juliana Louise Marie Wilhelmina van Oranje-Nassau (30 April 1909  20 Maret 2004) adalah Ratu Kerajaan Belanda dari 6 September 1948, sampai tanggal 30 April 1980, ulang tahunnya ke-71, ketika putrinya, Beatrix naik takhta. Juliana menikah dengan Bernhard dari Lippe Biesterfeld, seorang bangsawan Jerman, pada tanggal 7 Januari 1937 dan mendapatkan empat anak Beatrix (1938), Irene (1939), Putri Margriet (1943), dan Marijke (1947) yang namanya kemudian diganti menjadi Christina." .
